@prefix ci: <https://vocab.methodandstructure.com/content-inventory#> .
@prefix dct: <http://purl.org/dc/terms/> .
@prefix owl: <http://www.w3.org/2002/07/owl#> .
@prefix rdf: <http://www.w3.org/1999/02/22-rdf-syntax-ns#> .
@prefix rdfs: <http://www.w3.org/2000/01/rdf-schema#> .
@prefix skos: <http://www.w3.org/2004/02/skos/core#> .
@prefix xsd: <http://www.w3.org/2001/XMLSchema#> .

<urn:uuid:020f0ba1-d754-4b6b-a536-999616e76db6> a skos:Concept;
  dct:created "2021-12-14T20:56:50Z"^^xsd:dateTime;
  dct:creator <urn:uuid:ca637d4b-c11b-4152-be98-bde602e7abd4>;
  skos:broader <urn:uuid:1ae8c127-f674-44cf-af3d-9382f7c7c1ee>,
    <urn:uuid:081b467a-a40d-4028-9b8c-f2adc43eaefb>,
    <urn:uuid:e162d03b-bfec-4f01-ab7e-56da309550f6>;
  skos:definition "In URLs, path segments are the individual slugs that appear between the slash (/) characters. They are intended to (and sometimes do) represent directory paths, though on the Web their relationship is certainly more tenuous."@en;
  skos:hiddenLabel "path segments"@en;
  skos:inScheme <urn:uuid:bbe073ad-f449-4b25-91ac-7d919613ca51>,
    <urn:uuid:797e83d7-a86f-4838-b5c5-0ec20855197d>,
    <urn:uuid:1b457bed-8a80-4135-92b8-fdea12b4eea3>,
    <urn:uuid:2153d83b-8555-44a3-96e0-821b6663a188>,
    <urn:uuid:2df6fac6-3122-44dc-9f92-5caab7f9b10b>,
    <urn:uuid:4bbcdde6-ed53-4f8d-b3f8-43f800fd05d5>;
  skos:prefLabel "path segment"@en;
  skos:related <urn:uuid:cd9605ea-abe2-425e-904a-5dd35acdec8f> .

<urn:uuid:03ab17be-c88e-40da-94af-ae8a365cbadc> a skos:Concept;
  dct:created "2021-12-14T18:02:28Z"^^xsd:dateTime;
  dct:creator <urn:uuid:ca637d4b-c11b-4152-be98-bde602e7abd4>;
  skos:altLabel "DOAP"@en;
  skos:broader <urn:uuid:91472a37-bea8-4c9c-8f38-836d63510bff>,
    <urn:uuid:86c65d14-2d23-4350-8004-233b2f3e873f>;
  skos:definition "DOAP is an RDF vocabulary for expressing mainly open-source software projects."@en;
  skos:hiddenLabel "description of a project"@en;
  skos:inScheme <urn:uuid:bbe073ad-f449-4b25-91ac-7d919613ca51>,
    <urn:uuid:1b457bed-8a80-4135-92b8-fdea12b4eea3>,
    <urn:uuid:2153d83b-8555-44a3-96e0-821b6663a188>,
    <urn:uuid:797e83d7-a86f-4838-b5c5-0ec20855197d>,
    <urn:uuid:2df6fac6-3122-44dc-9f92-5caab7f9b10b>,
    <urn:uuid:4bbcdde6-ed53-4f8d-b3f8-43f800fd05d5>;
  skos:prefLabel "Description of a Project"@en .

<urn:uuid:046690c9-6341-4109-a9d3-b07b64dc7ba5> a skos:Concept;
  dct:created "2017-02-21T20:10:36Z"^^xsd:dateTime;
  dct:creator <urn:uuid:ca637d4b-c11b-4152-be98-bde602e7abd4>;
  skos:broader <urn:uuid:afd1338d-86da-4c2e-a1cc-9b07679bed1b>,
    <urn:uuid:c0e969c3-4528-4968-8418-d5fe609c2a62>;
  skos:definition "A privilege, in the context of access control, is the ability to access or manipulate a particular information resource. Privileges are granted to accounts, or to security groups."@en;
  skos:inScheme <urn:uuid:49ac68c4-922c-4d9e-88fa-b318fc54d36f>,
    <urn:uuid:bbe073ad-f449-4b25-91ac-7d919613ca51>,
    <urn:uuid:2df6fac6-3122-44dc-9f92-5caab7f9b10b>,
    <urn:uuid:1b457bed-8a80-4135-92b8-fdea12b4eea3>,
    <urn:uuid:2153d83b-8555-44a3-96e0-821b6663a188>,
    <urn:uuid:4bbcdde6-ed53-4f8d-b3f8-43f800fd05d5>;
  skos:prefLabel "privilege"@en;
  skos:related <urn:uuid:e261b25d-32c5-4736-bc32-c613f81f887d>,
    <urn:uuid:4039a99d-c14b-40f2-84d5-4ec72e2217e1>,
    <urn:uuid:d85e3c52-cc94-48a4-8dc5-591de86be52f> .

<urn:uuid:046bcd35-73f1-442e-a48c-53d14dfa99b7> a skos:Concept;
  dct:created "2019-03-02T02:41:22Z"^^xsd:dateTime;
  dct:creator <urn:uuid:ca637d4b-c11b-4152-be98-bde602e7abd4>;
  skos:broader <urn:uuid:f5a254ac-4a2b-405e-91be-7de9fbf7174d>;
  skos:definition "Machine learning refers to the use of statistical methods to program computers. It is typically what people mean by the term \"artificial intelligence\"."@en;
  skos:inScheme <urn:uuid:75f35368-e228-47fe-8efd-7251a2bde816>,
    <urn:uuid:bbe073ad-f449-4b25-91ac-7d919613ca51>,
    <urn:uuid:1b457bed-8a80-4135-92b8-fdea12b4eea3>,
    <urn:uuid:2153d83b-8555-44a3-96e0-821b6663a188>,
    <urn:uuid:4ec7530b-5536-4fb7-bb5a-45a3f5fddc22>,
    <urn:uuid:2df6fac6-3122-44dc-9f92-5caab7f9b10b>,
    <urn:uuid:4bbcdde6-ed53-4f8d-b3f8-43f800fd05d5>;
  skos:prefLabel "machine learning"@en .

<urn:uuid:04f550ab-8eb3-4aa1-b823-b8a3a3e6cd9a> a skos:Concept;
  dct:created "2021-12-14T21:11:45Z"^^xsd:dateTime;
  dct:creator <urn:uuid:ca637d4b-c11b-4152-be98-bde602e7abd4>;
  skos:broader <urn:uuid:aa5f9563-e527-4df2-8518-ce325819f1e6>,
    <urn:uuid:fdb43f70-cb11-49dd-aba6-7011b05ad61a>;
  skos:definition "Code profiling is the technique of attaching sensors to running code to determine which parts are running at suboptimal efficiency. Profiling, among other things, consumes AST and produces a call graph."@en;
  skos:hiddenLabel "profile"@en,
    "profiling"@en;
  skos:inScheme <urn:uuid:bbe073ad-f449-4b25-91ac-7d919613ca51>,
    <urn:uuid:1b457bed-8a80-4135-92b8-fdea12b4eea3>,
    <urn:uuid:2153d83b-8555-44a3-96e0-821b6663a188>,
    <urn:uuid:797e83d7-a86f-4838-b5c5-0ec20855197d>,
    <urn:uuid:2df6fac6-3122-44dc-9f92-5caab7f9b10b>,
    <urn:uuid:4bbcdde6-ed53-4f8d-b3f8-43f800fd05d5>;
  skos:prefLabel "profiling (technique)"@en;
  skos:related <urn:uuid:5495f814-fd98-4b43-aba3-9e63a2063fd5>,
    <urn:uuid:8cb5c042-8ce4-4d8d-a4c0-dd47d90e4bf5> .

<urn:uuid:09021bd6-b97f-42c3-a6ef-83fc72ce8998> a skos:Concept;
  dct:created "2022-12-14T11:19:38Z"^^xsd:dateTime;
  dct:creator <urn:uuid:ca637d4b-c11b-4152-be98-bde602e7abd4>;
  skos:altLabel "DAM"@en,
    "asset store"@en;
  skos:broader <urn:uuid:13385ea1-1f87-4612-b86b-27bc4e339be6>;
  skos:definition "A digital asset management system aggregates the assets (such as images) within an organization's content ecosystem and provides an authoritative repository and tools to facilitate the indexing and retrieval of said assets, with considerable advantages over an ordinary file system."@en;
  skos:hiddenLabel "asset storage"@en;
  skos:inScheme <urn:uuid:bbe073ad-f449-4b25-91ac-7d919613ca51>,
    <urn:uuid:1b457bed-8a80-4135-92b8-fdea12b4eea3>,
    <urn:uuid:2153d83b-8555-44a3-96e0-821b6663a188>,
    <urn:uuid:0c7028f0-8226-47b3-acff-a4e83e6a60fd>,
    <urn:uuid:4bbcdde6-ed53-4f8d-b3f8-43f800fd05d5>;
  skos:narrower <urn:uuid:06f86a10-1b5f-4711-b2fc-3bb5ce14a26e>;
  skos:prefLabel "digital asset management system"@en;
  skos:related <urn:uuid:61c0c9c3-4d91-4509-902a-db09c4188ae5>,
    <urn:uuid:9adc8b42-bbd1-4065-bb57-9a789253c4e4> .

<urn:uuid:09be5d2a-38f3-45d9-bea5-a4413c4fc7f2> a skos:Concept;
  dct:created "2024-02-16T15:24:23Z"^^xsd:dateTime,
    "2024-07-03T21:27:51Z"^^xsd:dateTime;
  dct:creator <urn:uuid:ca637d4b-c11b-4152-be98-bde602e7abd4>;
  skos:altLabel "schema"@en;
  skos:broader <urn:uuid:51a7c4b2-ef0c-4dc1-a538-553622131f09>;
  skos:definition "A data vocabulary (or schema) is a controlled vocabulary with additional rigor, such that is strict enough to define a formal data structure. The scope includes the names (identifiers) of members and valid sequences, cardinality constraints, valid data types, and so on. A data vocabulary can be a conventional document, but the more sophisticated ones can be fed directly into a computer."@en;
  skos:hiddenLabel "schemata"@en;
  skos:inScheme <urn:uuid:bbe073ad-f449-4b25-91ac-7d919613ca51>,
    <urn:uuid:0c7028f0-8226-47b3-acff-a4e83e6a60fd>,
    <urn:uuid:1b457bed-8a80-4135-92b8-fdea12b4eea3>,
    <urn:uuid:2153d83b-8555-44a3-96e0-821b6663a188>,
    <urn:uuid:4bbcdde6-ed53-4f8d-b3f8-43f800fd05d5>;
  skos:prefLabel "data vocabulary"@en .

<urn:uuid:0b758f46-c799-495b-b382-93212d47071c> a skos:Concept;
  dct:created "2022-11-24T01:03:05Z"^^xsd:dateTime;
  dct:creator <urn:uuid:ca637d4b-c11b-4152-be98-bde602e7abd4>;
  skos:altLabel "dev"@en,
    "dev team"@en,
    "development team"@en,
    "software engineering team"@en;
  skos:definition "The dev team is the group (or potentially one of many) within an organization who is principally responsible for creating software."@en;
  skos:hiddenLabel "software engineering (team)"@en;
  skos:inScheme <urn:uuid:bbe073ad-f449-4b25-91ac-7d919613ca51>,
    <urn:uuid:0c7028f0-8226-47b3-acff-a4e83e6a60fd>,
    <urn:uuid:1b457bed-8a80-4135-92b8-fdea12b4eea3>,
    <urn:uuid:2153d83b-8555-44a3-96e0-821b6663a188>,
    <urn:uuid:4bbcdde6-ed53-4f8d-b3f8-43f800fd05d5>;
  skos:prefLabel "(software) development team"@en;
  skos:related <urn:uuid:22c5c553-d574-4bf7-9a4d-13e70afa7f1c> .

<urn:uuid:0e3fc8ff-9903-4c63-8558-4ca69bede9b4> a skos:Concept;
  dct:created "2022-11-23T21:22:41Z"^^xsd:dateTime;
  dct:creator <urn:uuid:ca637d4b-c11b-4152-be98-bde602e7abd4>;
  dct:references <https://doriantaylor.com/intelligent-heterogeneity>;
  rdfs:seeAlso <https://doriantaylor.com/intelligent-heterogeneity>;
  skos:broader <urn:uuid:e7ccb716-f967-439f-9682-dad225efc0b6>;
  skos:definition "Intelligent heterogeneity is the principle that begins with a standing assumption that an information system is always going to drive toward a heterogeneous state, and therefore this should be accommodated and planned for."@en;
  skos:inScheme <urn:uuid:bbe073ad-f449-4b25-91ac-7d919613ca51>,
    <urn:uuid:0c7028f0-8226-47b3-acff-a4e83e6a60fd>,
    <urn:uuid:1b457bed-8a80-4135-92b8-fdea12b4eea3>,
    <urn:uuid:2153d83b-8555-44a3-96e0-821b6663a188>,
    <urn:uuid:4bbcdde6-ed53-4f8d-b3f8-43f800fd05d5>;
  skos:prefLabel "intelligent heterogeneity"@en .

<urn:uuid:1a34027e-4ee7-4bf3-bd4f-c68930c3e435> a skos:Concept;
  dct:created "2021-12-14T19:59:08Z"^^xsd:dateTime;
  dct:creator <urn:uuid:ca637d4b-c11b-4152-be98-bde602e7abd4>;
  skos:altLabel "ISBN"@en;
  skos:broader <urn:uuid:6c18acc3-3119-4f0b-8d24-0ca0ea9449d3>;
  skos:definition "The ISBN is the quintessential identifier for books."@en;
  skos:hiddenLabel "ISBNs"@en,
    "international standard book number"@en;
  skos:inScheme <urn:uuid:1b457bed-8a80-4135-92b8-fdea12b4eea3>,
    <urn:uuid:2153d83b-8555-44a3-96e0-821b6663a188>,
    <urn:uuid:797e83d7-a86f-4838-b5c5-0ec20855197d>,
    <urn:uuid:2df6fac6-3122-44dc-9f92-5caab7f9b10b>,
    <urn:uuid:bbe073ad-f449-4b25-91ac-7d919613ca51>,
    <urn:uuid:4bbcdde6-ed53-4f8d-b3f8-43f800fd05d5>;
  skos:prefLabel "International Standard Book Number"@en .

<urn:uuid:1cadae87-b6e4-4348-a38a-4b8956edc160> a skos:Concept;
  dct:created "2017-06-07T20:29:57Z"^^xsd:dateTime;
  dct:creator <urn:uuid:ca637d4b-c11b-4152-be98-bde602e7abd4>;
  skos:broader <urn:uuid:87cc031a-dab5-41cb-8c86-5225565a0534>;
  skos:definition "Cascading stylesheets is a standardized, declarative, rule-based, domain-specific language for describing presentational parameters of HTML and XML documents."@en;
  skos:inScheme <urn:uuid:49ac68c4-922c-4d9e-88fa-b318fc54d36f>,
    <urn:uuid:1b457bed-8a80-4135-92b8-fdea12b4eea3>,
    <urn:uuid:2153d83b-8555-44a3-96e0-821b6663a188>,
    <urn:uuid:2df6fac6-3122-44dc-9f92-5caab7f9b10b>,
    <urn:uuid:bbe073ad-f449-4b25-91ac-7d919613ca51>,
    <urn:uuid:4bbcdde6-ed53-4f8d-b3f8-43f800fd05d5>;
  skos:prefLabel "Cascading Style Sheets (CSS)"@en .

<urn:uuid:1ecbaef2-f501-4133-bbaa-a436416a182a> a skos:Concept;
  dct:created "2019-03-02T05:45:45Z"^^xsd:dateTime;
  dct:creator <urn:uuid:ca637d4b-c11b-4152-be98-bde602e7abd4>;
  skos:broader <urn:uuid:4eab5a63-adc6-4efd-b49e-402131b519fa>,
    <urn:uuid:86c65d14-2d23-4350-8004-233b2f3e873f>;
  skos:definition "The Dublin Core Metadata Initiative is an early and established vocabulary for modeling various aspects of document metadata."@en;
  skos:inScheme <urn:uuid:75f35368-e228-47fe-8efd-7251a2bde816>,
    <urn:uuid:1b457bed-8a80-4135-92b8-fdea12b4eea3>,
    <urn:uuid:2153d83b-8555-44a3-96e0-821b6663a188>,
    <urn:uuid:2df6fac6-3122-44dc-9f92-5caab7f9b10b>,
    <urn:uuid:bbe073ad-f449-4b25-91ac-7d919613ca51>,
    <urn:uuid:4bbcdde6-ed53-4f8d-b3f8-43f800fd05d5>;
  skos:prefLabel "Dublin Core"@en .

<urn:uuid:1f848da0-5513-4465-bf86-2a6bfb05da23> a skos:Concept;
  dct:created "2019-02-19T21:26:06Z"^^xsd:dateTime;
  dct:creator <urn:uuid:ca637d4b-c11b-4152-be98-bde602e7abd4>;
  skos:broader <urn:uuid:f352a521-b78e-478e-b01d-3a68638025a4>;
  skos:inScheme <urn:uuid:1b457bed-8a80-4135-92b8-fdea12b4eea3>,
    <urn:uuid:2153d83b-8555-44a3-96e0-821b6663a188>,
    <urn:uuid:2df6fac6-3122-44dc-9f92-5caab7f9b10b>,
    <urn:uuid:75f35368-e228-47fe-8efd-7251a2bde816>,
    <urn:uuid:bbe073ad-f449-4b25-91ac-7d919613ca51>,
    <urn:uuid:4bbcdde6-ed53-4f8d-b3f8-43f800fd05d5>;
  skos:prefLabel "DITA"@en .

<urn:uuid:232b5bf9-308b-4a44-bb34-3da310ec586d> a skos:Concept;
  dct:created "2021-12-14T22:45:07Z"^^xsd:dateTime;
  dct:creator <urn:uuid:ca637d4b-c11b-4152-be98-bde602e7abd4>;
  skos:broader <urn:uuid:aa5f9563-e527-4df2-8518-ce325819f1e6>,
    <urn:uuid:fdb43f70-cb11-49dd-aba6-7011b05ad61a>;
  skos:definition "A single source of truth is an idiom in information system design, whereby a single logical system is deemed authoritative over a set of information, and measures are taken to ensure this remains the case."@en;
  skos:inScheme <urn:uuid:1b457bed-8a80-4135-92b8-fdea12b4eea3>,
    <urn:uuid:2153d83b-8555-44a3-96e0-821b6663a188>,
    <urn:uuid:2df6fac6-3122-44dc-9f92-5caab7f9b10b>,
    <urn:uuid:bbe073ad-f449-4b25-91ac-7d919613ca51>,
    <urn:uuid:797e83d7-a86f-4838-b5c5-0ec20855197d>,
    <urn:uuid:4bbcdde6-ed53-4f8d-b3f8-43f800fd05d5>;
  skos:prefLabel "single source of truth"@en .

<urn:uuid:26f190fd-79e0-418c-88d0-8efc13b1b8ac> a skos:Concept;
  dct:created "2021-12-14T03:02:34Z"^^xsd:dateTime;
  dct:creator <urn:uuid:ca637d4b-c11b-4152-be98-bde602e7abd4>;
  skos:broader <urn:uuid:ee2371bb-d9a0-4ee8-a35b-f4e0d9458f02>;
  skos:definition "Client-side JavaScript refers specifically to the language JavaScript executed in a Web browser, versus in some other execution context, such as Node.JS. Client-side JavaScript is the source of most interactive behavior in Web applications."@en;
  skos:hiddenLabel "client-side javascript"@en;
  skos:inScheme <urn:uuid:2df6fac6-3122-44dc-9f92-5caab7f9b10b>,
    <urn:uuid:1b457bed-8a80-4135-92b8-fdea12b4eea3>,
    <urn:uuid:2153d83b-8555-44a3-96e0-821b6663a188>,
    <urn:uuid:bbe073ad-f449-4b25-91ac-7d919613ca51>,
    <urn:uuid:797e83d7-a86f-4838-b5c5-0ec20855197d>,
    <urn:uuid:4bbcdde6-ed53-4f8d-b3f8-43f800fd05d5>;
  skos:prefLabel "client-side JavaScript"@en .

<urn:uuid:27ff1117-f414-4349-9cb0-8347a39ebe69> a skos:Concept;
  dct:created "2017-02-22T14:58:35Z"^^xsd:dateTime;
  dct:creator <urn:uuid:ca637d4b-c11b-4152-be98-bde602e7abd4>;
  skos:definition "Responsive design is a Web design technique that focuses on visual elements which can be stretched, squashed and resized."@en;
  skos:inScheme <urn:uuid:49ac68c4-922c-4d9e-88fa-b318fc54d36f>,
    <urn:uuid:1b457bed-8a80-4135-92b8-fdea12b4eea3>,
    <urn:uuid:2153d83b-8555-44a3-96e0-821b6663a188>,
    <urn:uuid:2df6fac6-3122-44dc-9f92-5caab7f9b10b>,
    <urn:uuid:bbe073ad-f449-4b25-91ac-7d919613ca51>,
    <urn:uuid:4bbcdde6-ed53-4f8d-b3f8-43f800fd05d5>;
  skos:prefLabel "Responsive Design"@en;
  skos:related <urn:uuid:ad6b1b9b-fec4-4378-b8dd-7bbc07a3d706>,
    <urn:uuid:3a2c72e0-4fa5-4477-a51b-d7f073cc1155>,
    <urn:uuid:be93cce1-f21f-4e85-bd34-e005dea3532f> .

<urn:uuid:2a636e04-5882-41ef-a0ad-019c2cbaa3a4> a skos:Concept;
  dct:created "2019-03-03T01:15:10Z"^^xsd:dateTime;
  dct:creator <urn:uuid:ca637d4b-c11b-4152-be98-bde602e7abd4>;
  skos:broader <urn:uuid:86c65d14-2d23-4350-8004-233b2f3e873f>,
    <urn:uuid:4eab5a63-adc6-4efd-b49e-402131b519fa>;
  skos:definition "R2RML is an RDF vocabulary that maps between RDF and relational (SQL) databases."@en;
  skos:inScheme <urn:uuid:75f35368-e228-47fe-8efd-7251a2bde816>,
    <urn:uuid:2df6fac6-3122-44dc-9f92-5caab7f9b10b>,
    <urn:uuid:1b457bed-8a80-4135-92b8-fdea12b4eea3>,
    <urn:uuid:2153d83b-8555-44a3-96e0-821b6663a188>,
    <urn:uuid:bbe073ad-f449-4b25-91ac-7d919613ca51>,
    <urn:uuid:4bbcdde6-ed53-4f8d-b3f8-43f800fd05d5>;
  skos:prefLabel "R2RML"@en;
  skos:related <urn:uuid:2717d0b5-cb79-4d1a-82c0-69cdc1e590a1> .

<urn:uuid:2ca75b6c-2356-4c0b-8068-aa7ad6706536> a skos:Concept;
  dct:created "2021-12-14T19:13:47Z"^^xsd:dateTime;
  dct:creator <urn:uuid:ca637d4b-c11b-4152-be98-bde602e7abd4>;
  skos:broader <urn:uuid:7ddb6eed-d37d-4412-9c10-eff42447eddf>;
  skos:definition "Freemium is the neologism given to the business model whereby a restricted set of functionality in (typically) some software-as-a-service product is given to users free of charge with the anticipation that they will convert into paid customers."@en;
  skos:inScheme <urn:uuid:797e83d7-a86f-4838-b5c5-0ec20855197d>,
    <urn:uuid:1b457bed-8a80-4135-92b8-fdea12b4eea3>,
    <urn:uuid:2153d83b-8555-44a3-96e0-821b6663a188>,
    <urn:uuid:2df6fac6-3122-44dc-9f92-5caab7f9b10b>,
    <urn:uuid:bbe073ad-f449-4b25-91ac-7d919613ca51>,
    <urn:uuid:4bbcdde6-ed53-4f8d-b3f8-43f800fd05d5>;
  skos:prefLabel "freemium"@en .

<urn:uuid:2d5dd0e8-2659-4395-a430-64f024305c17> a skos:Concept;
  dct:created "2022-10-07T12:44:22Z"^^xsd:dateTime;
  dct:creator <urn:uuid:ca637d4b-c11b-4152-be98-bde602e7abd4>;
  skos:broader <urn:uuid:2575586a-6ce1-4527-bb67-7ed7c11f52f7>;
  skos:inScheme <urn:uuid:1b457bed-8a80-4135-92b8-fdea12b4eea3>,
    <urn:uuid:2153d83b-8555-44a3-96e0-821b6663a188>,
    <urn:uuid:2df6fac6-3122-44dc-9f92-5caab7f9b10b>,
    <urn:uuid:bbe073ad-f449-4b25-91ac-7d919613ca51>,
    <urn:uuid:4bbcdde6-ed53-4f8d-b3f8-43f800fd05d5>;
  skos:prefLabel "telemetry"@en .

<urn:uuid:323613c1-005b-44f1-8f9b-ce7313637299> a skos:Concept;
  dct:created "2021-12-14T23:48:28Z"^^xsd:dateTime;
  dct:creator <urn:uuid:ca637d4b-c11b-4152-be98-bde602e7abd4>;
  skos:broader <urn:uuid:c2f6ce23-c916-448d-8e18-c122d347cf17>,
    <urn:uuid:5f47abfe-ba22-4003-a681-24dff12400ac>,
    <urn:uuid:5bdd2fb7-d84d-4583-998b-7d3f2803307e>,
    <urn:uuid:68e38d88-1afd-4443-a1a4-f28abd9dc77d>;
  skos:definition "A variant, in the context of content negotiation, is a particular representation of a resource that occupies a region in the space of all its available dimensions."@en;
  skos:hiddenLabel "variants"@en;
  skos:inScheme <urn:uuid:0c7028f0-8226-47b3-acff-a4e83e6a60fd>,
    <urn:uuid:797e83d7-a86f-4838-b5c5-0ec20855197d>,
    <urn:uuid:bbe073ad-f449-4b25-91ac-7d919613ca51>,
    <urn:uuid:1b457bed-8a80-4135-92b8-fdea12b4eea3>,
    <urn:uuid:2153d83b-8555-44a3-96e0-821b6663a188>,
    <urn:uuid:2df6fac6-3122-44dc-9f92-5caab7f9b10b>,
    <urn:uuid:4bbcdde6-ed53-4f8d-b3f8-43f800fd05d5>;
  skos:prefLabel "variant"@en .

<urn:uuid:3ba16db6-3d69-4bba-8543-5bd62dfec0b6> a skos:Concept;
  dct:created "2021-12-14T16:50:25Z"^^xsd:dateTime;
  dct:creator <urn:uuid:ca637d4b-c11b-4152-be98-bde602e7abd4>;
  skos:altLabel "CI"@en;
  skos:broader <urn:uuid:aa5f9563-e527-4df2-8518-ce325819f1e6>,
    <urn:uuid:fdb43f70-cb11-49dd-aba6-7011b05ad61a>;
  skos:definition "In software development, continuous integration refers to both a process and its concomitant infrastructure for deploying software that itself typically runs a networked information service. A continuous integration system can be configured to automatically package and deploy software directly from version control to its target, upon confirmation of a passing test suite."@en;
  skos:inScheme <urn:uuid:0c7028f0-8226-47b3-acff-a4e83e6a60fd>,
    <urn:uuid:2df6fac6-3122-44dc-9f92-5caab7f9b10b>,
    <urn:uuid:1b457bed-8a80-4135-92b8-fdea12b4eea3>,
    <urn:uuid:2153d83b-8555-44a3-96e0-821b6663a188>,
    <urn:uuid:797e83d7-a86f-4838-b5c5-0ec20855197d>,
    <urn:uuid:bbe073ad-f449-4b25-91ac-7d919613ca51>,
    <urn:uuid:4bbcdde6-ed53-4f8d-b3f8-43f800fd05d5>;
  skos:prefLabel "continuous integration"@en .

<urn:uuid:3fd9fdb1-0f28-463e-9d3e-aaebf18d0a3d> a skos:Concept;
  dct:created "2022-11-24T00:20:25Z"^^xsd:dateTime;
  dct:creator <urn:uuid:ca637d4b-c11b-4152-be98-bde602e7abd4>;
  skos:altLabel "machine-readability"@en;
  skos:definition "All digital data segments are in principle machine-readable, the question is to what extent can the machine do anything meaningful with it? A CSV file, for example, is machine-readable such that it can be read into a spreadsheet program, but contains no embedded semantics beyond the fact that the lines signify rows in a grid, and the commas signify columns. In other words, it can be displayed, but the actual contents of the CSV are meaningless without some outside cue."@en,
    "All digital data segments are in principle machine-readable, the question is to what extent can the machine do anything meaningful with it. A CSV file, for example, is machine-readable such that it can be read into a spreadsheet program, but contains no embedded semantics beyond the fact that the lines signify rows in a grid, and the commas signify columns. In other words, it can be displayed, but the actual contents of the CSV are meaningless without some outside cue."@en;
  skos:inScheme <urn:uuid:bbe073ad-f449-4b25-91ac-7d919613ca51>,
    <urn:uuid:1b457bed-8a80-4135-92b8-fdea12b4eea3>,
    <urn:uuid:2153d83b-8555-44a3-96e0-821b6663a188>,
    <urn:uuid:a1a01f1c-7162-439c-94f1-3e28b99ae8ab>,
    <urn:uuid:ddfaaacc-9dcb-451b-afa6-477e6e787a5c>,
    <urn:uuid:4bbcdde6-ed53-4f8d-b3f8-43f800fd05d5>;
  skos:narrower <urn:uuid:1709ffb5-bbee-40cf-86c3-030f47ff1be7>;
  skos:prefLabel "machine-readable"@en .

<urn:uuid:41d407cf-25e3-4005-83d5-ef62b4ef52f0> a skos:Concept;
  dct:created "2022-11-23T21:33:53Z"^^xsd:dateTime;
  dct:creator <urn:uuid:ca637d4b-c11b-4152-be98-bde602e7abd4>;
  skos:altLabel "business logic"@en;
  skos:broader <urn:uuid:0cf51602-4fc1-4a38-9663-d47aff228b2d>;
  skos:definition "Application logic can be understood as a special case of content, to the extent that it is software behavior that does something directly germane to a specific application, in contrast to being one or more degrees removed from it, such as with infrastructure or other more broadly-applicable code."@en,
    "Application logic can be understood as a special case of content, to the extent that it is software behavior that does something directly germane to a specific application, in contrast to infrastructure or other generic code."@en;
  skos:inScheme <urn:uuid:1b457bed-8a80-4135-92b8-fdea12b4eea3>,
    <urn:uuid:2153d83b-8555-44a3-96e0-821b6663a188>,
    <urn:uuid:0c7028f0-8226-47b3-acff-a4e83e6a60fd>,
    <urn:uuid:bbe073ad-f449-4b25-91ac-7d919613ca51>,
    <urn:uuid:4bbcdde6-ed53-4f8d-b3f8-43f800fd05d5>;
  skos:prefLabel "application logic"@en .

<urn:uuid:428020f0-e8d5-4dbf-a232-7b66b35b1c63> a skos:Concept;
  dct:created "2019-03-02T02:37:33Z"^^xsd:dateTime;
  dct:creator <urn:uuid:ca637d4b-c11b-4152-be98-bde602e7abd4>;
  skos:definition "A virtual machine is a computer within a computer. It serves two main purposes: one is to unify the underlying hardware interface from the point of view of the software, such as with Java, and another is to run as a \"guest\" on top of one, or possibly many, \"host\" computers."@en;
  skos:inScheme <urn:uuid:bbe073ad-f449-4b25-91ac-7d919613ca51>,
    <urn:uuid:1b457bed-8a80-4135-92b8-fdea12b4eea3>,
    <urn:uuid:2153d83b-8555-44a3-96e0-821b6663a188>,
    <urn:uuid:2df6fac6-3122-44dc-9f92-5caab7f9b10b>,
    <urn:uuid:75f35368-e228-47fe-8efd-7251a2bde816>,
    <urn:uuid:4bbcdde6-ed53-4f8d-b3f8-43f800fd05d5>;
  skos:narrower <urn:uuid:1d5cbcc6-63b1-4817-97fa-c979859cf41a>;
  skos:prefLabel "virtual machine"@en;
  skos:related <urn:uuid:855fce21-5560-4ff3-87bf-ef26a28958c4> .

<urn:uuid:43c06230-2371-4974-bb76-d64cf229636c> a skos:Concept;
  dct:created "2022-11-23T23:37:59Z"^^xsd:dateTime;
  dct:creator <urn:uuid:ca637d4b-c11b-4152-be98-bde602e7abd4>;
  rdfs:seeAlso <https://en.wikipedia.org/wiki/The_Mythical_Man-Month>,
    <https://www.pearson.com/en-us/subject-catalog/p/mythical-man-month-the-essays-on-software-engineering-anniversary-edition/P200000000149/9780201835953>;
  skos:definition "Conceptual integrity (Brooks 1975) is the state of affairs wherein a project or its ultimate product(s), and everybody involved, has a unified mental model of what it is and what it's for. Achieving conceptual integrity means decisions come easier and outcomes are more coherent, because there is little to no ambiguity around an optimal course of action."@en;
  skos:inScheme <urn:uuid:1b457bed-8a80-4135-92b8-fdea12b4eea3>,
    <urn:uuid:2153d83b-8555-44a3-96e0-821b6663a188>,
    <urn:uuid:0c7028f0-8226-47b3-acff-a4e83e6a60fd>,
    <urn:uuid:4ec7530b-5536-4fb7-bb5a-45a3f5fddc22>,
    <urn:uuid:bbe073ad-f449-4b25-91ac-7d919613ca51>,
    <urn:uuid:4bbcdde6-ed53-4f8d-b3f8-43f800fd05d5>;
  skos:prefLabel "conceptual integrity"@en;
  skos:related <urn:uuid:775a0b24-a8b3-4e74-989a-ed6f438122d3> .

<urn:uuid:4fbfbd72-47b6-4546-974b-6e420588a64b> a skos:Concept;
  dct:created "2021-12-14T18:17:15Z"^^xsd:dateTime;
  dct:creator <urn:uuid:ca637d4b-c11b-4152-be98-bde602e7abd4>;
  skos:definition "The document root of a Web server is the directory (folder) associated with the root address of a given website's URL."@en;
  skos:inScheme <urn:uuid:bbe073ad-f449-4b25-91ac-7d919613ca51>,
    <urn:uuid:2df6fac6-3122-44dc-9f92-5caab7f9b10b>,
    <urn:uuid:1b457bed-8a80-4135-92b8-fdea12b4eea3>,
    <urn:uuid:2153d83b-8555-44a3-96e0-821b6663a188>,
    <urn:uuid:797e83d7-a86f-4838-b5c5-0ec20855197d>,
    <urn:uuid:4bbcdde6-ed53-4f8d-b3f8-43f800fd05d5>;
  skos:prefLabel "document root"@en;
  skos:related <urn:uuid:1ae8c127-f674-44cf-af3d-9382f7c7c1ee>,
    <urn:uuid:e162d03b-bfec-4f01-ab7e-56da309550f6> .

<urn:uuid:51f44aca-bac0-4dbb-92e5-5b5fc3026b32> a skos:Concept;
  dct:created "2017-06-23T01:50:02Z"^^xsd:dateTime;
  dct:creator <urn:uuid:ca637d4b-c11b-4152-be98-bde602e7abd4>;
  skos:definition "An aggregate value is a quantity which is the result of some operation over some other data, such as a count of entities. Data which is already quantitative can have aggregates in the form of descriptive statistics."@en;
  skos:inScheme <urn:uuid:bbe073ad-f449-4b25-91ac-7d919613ca51>,
    <urn:uuid:49ac68c4-922c-4d9e-88fa-b318fc54d36f>,
    <urn:uuid:2df6fac6-3122-44dc-9f92-5caab7f9b10b>,
    <urn:uuid:1b457bed-8a80-4135-92b8-fdea12b4eea3>,
    <urn:uuid:2153d83b-8555-44a3-96e0-821b6663a188>,
    <urn:uuid:4bbcdde6-ed53-4f8d-b3f8-43f800fd05d5>;
  skos:narrower <urn:uuid:43649147-ce57-43fe-a960-3b4e71b8686f>;
  skos:prefLabel "aggregate value"@en .

<urn:uuid:55c35a7f-8f5d-4fdb-9f39-b77ea3db862c> a skos:Concept;
  dct:created "2022-10-06T03:19:18Z"^^xsd:dateTime;
  dct:creator <urn:uuid:ca637d4b-c11b-4152-be98-bde602e7abd4>;
  skos:definition "A document can be understood as an ordered tree of content."@en;
  skos:inScheme <urn:uuid:bbe073ad-f449-4b25-91ac-7d919613ca51>,
    <urn:uuid:2df6fac6-3122-44dc-9f92-5caab7f9b10b>,
    <urn:uuid:1b457bed-8a80-4135-92b8-fdea12b4eea3>,
    <urn:uuid:2153d83b-8555-44a3-96e0-821b6663a188>,
    <urn:uuid:4bbcdde6-ed53-4f8d-b3f8-43f800fd05d5>;
  skos:prefLabel "document"@en;
  skos:related <urn:uuid:4f4aa0ac-c1b4-4a15-a6f3-518419d5b771> .

<urn:uuid:57cce227-5bbd-4d2c-90ae-49b1cdc48f48> a skos:Concept;
  dct:created "2021-12-14T22:20:38Z"^^xsd:dateTime;
  dct:creator <urn:uuid:ca637d4b-c11b-4152-be98-bde602e7abd4>;
  skos:broader <urn:uuid:02b3d282-d134-487b-8226-80141b5a4338>,
    <urn:uuid:e162d03b-bfec-4f01-ab7e-56da309550f6>,
    <urn:uuid:1ae8c127-f674-44cf-af3d-9382f7c7c1ee>,
    <urn:uuid:23448a6d-3dcc-470f-ae99-e146e2e3f00b>;
  skos:definition "A request-URI, in HTTP parlance, is specifically the part of an HTTP URL after the authority and before the fragment, constituting only the path and the query components. The request-URI is sent to the server as part of the resource request."@en;
  skos:inScheme <urn:uuid:bbe073ad-f449-4b25-91ac-7d919613ca51>,
    <urn:uuid:2df6fac6-3122-44dc-9f92-5caab7f9b10b>,
    <urn:uuid:1b457bed-8a80-4135-92b8-fdea12b4eea3>,
    <urn:uuid:2153d83b-8555-44a3-96e0-821b6663a188>,
    <urn:uuid:797e83d7-a86f-4838-b5c5-0ec20855197d>,
    <urn:uuid:4bbcdde6-ed53-4f8d-b3f8-43f800fd05d5>;
  skos:prefLabel "request-URI"@en .

<urn:uuid:5a09215d-8e0f-4ca1-85b2-1180fbf9a69c> a skos:Concept;
  dct:created "2022-11-23T21:30:15Z"^^xsd:dateTime,
    "2008-09-01T19:09:52+00:00"^^xsd:dateTime;
  dct:creator <urn:uuid:ca637d4b-c11b-4152-be98-bde602e7abd4>;
  dct:modified "2008-10-09T02:02:01+00:00"^^xsd:dateTime,
    "2008-10-10T16:02:45+00:00"^^xsd:dateTime,
    "2008-10-10T21:28:23+00:00"^^xsd:dateTime,
    "2009-03-04T00:43:00+00:00"^^xsd:dateTime,
    "2022-05-31T04:18:52+00:00"^^xsd:dateTime,
    "2022-11-23T21:30:15Z"^^xsd:dateTime;
  owl:sameAs <https://doriantaylor.com/lexicon/cookie>;
  skos:altLabel "cookie"@en;
  skos:broader <urn:uuid:02b3d282-d134-487b-8226-80141b5a4338>;
  skos:definition "A cookie is a state mechanism for HTTP, consisting of a key and an arbitrary value (with some additional metadata), sent from the server to the client. The client then sends this information back to the server with each request."@en;
  skos:inScheme <urn:uuid:0c7028f0-8226-47b3-acff-a4e83e6a60fd>,
    <urn:uuid:1b457bed-8a80-4135-92b8-fdea12b4eea3>,
    <urn:uuid:2153d83b-8555-44a3-96e0-821b6663a188>,
    <urn:uuid:4ec7530b-5536-4fb7-bb5a-45a3f5fddc22>,
    <urn:uuid:bbe073ad-f449-4b25-91ac-7d919613ca51>,
    <urn:uuid:4bbcdde6-ed53-4f8d-b3f8-43f800fd05d5>;
  skos:prefLabel "cookie"@en;
  ci:canonical-slug "http-cookie"^^xsd:token;
  ci:slug "cookie"^^xsd:token .

<urn:uuid:5ec7b7fb-4644-4723-ad08-895a597d96b9> a skos:Concept;
  dct:created "2019-03-04T06:52:50Z"^^xsd:dateTime;
  dct:creator <urn:uuid:ca637d4b-c11b-4152-be98-bde602e7abd4>;
  skos:altLabel "IT"@en;
  skos:definition "Information technology refers to any technology whatsoever that is made to deal with information. The current state of the art of information technology is computers and related electronic hardware. \"IT\" can also refer to a department in an organization charged with managing said hardware (and its related software)."@en;
  skos:inScheme <urn:uuid:bbe073ad-f449-4b25-91ac-7d919613ca51>,
    <urn:uuid:0c7028f0-8226-47b3-acff-a4e83e6a60fd>,
    <urn:uuid:2df6fac6-3122-44dc-9f92-5caab7f9b10b>,
    <urn:uuid:75f35368-e228-47fe-8efd-7251a2bde816>,
    <urn:uuid:1b457bed-8a80-4135-92b8-fdea12b4eea3>,
    <urn:uuid:2153d83b-8555-44a3-96e0-821b6663a188>,
    <urn:uuid:4bbcdde6-ed53-4f8d-b3f8-43f800fd05d5>;
  skos:prefLabel "information technology"@en;
  skos:related <urn:uuid:7284c136-288b-49aa-b129-a56e2be938d2>,
    <urn:uuid:a718d483-af90-4eaf-a59f-31d8897d6e8e>,
    <urn:uuid:b39c1f53-b8ed-49fb-ba57-24dfe7dc2d9f>,
    <urn:uuid:447cbc26-1fb8-4ffe-95f4-1f83b3bc3d21> .

<urn:uuid:5f96d659-2e85-44bd-bdd5-64f96c4fa97b> a skos:Concept;
  dct:created "2021-12-14T23:04:17Z"^^xsd:dateTime;
  dct:creator <urn:uuid:ca637d4b-c11b-4152-be98-bde602e7abd4>;
  skos:definition "Term reconciliation is a process conceived in RDF circles, but not limited to them. It is the act of identifying terms (think keys in map-like data structures) from one information system to another."@en;
  skos:inScheme <urn:uuid:797e83d7-a86f-4838-b5c5-0ec20855197d>,
    <urn:uuid:bbe073ad-f449-4b25-91ac-7d919613ca51>,
    <urn:uuid:2df6fac6-3122-44dc-9f92-5caab7f9b10b>,
    <urn:uuid:1b457bed-8a80-4135-92b8-fdea12b4eea3>,
    <urn:uuid:2153d83b-8555-44a3-96e0-821b6663a188>,
    <urn:uuid:4bbcdde6-ed53-4f8d-b3f8-43f800fd05d5>;
  skos:prefLabel "term reconciliation"@en;
  skos:related <urn:uuid:97edd9ad-7cfd-45fa-91cb-9e2e552e78a1>,
    <urn:uuid:fe500c7a-b458-4d2c-8b3a-efd1bb47d106> .

<urn:uuid:6153aa34-a4eb-4ad1-b197-e6156b453307> a skos:Concept;
  dct:created "2021-12-14T21:15:51Z"^^xsd:dateTime;
  dct:creator <urn:uuid:ca637d4b-c11b-4152-be98-bde602e7abd4>;
  skos:altLabel "PR"@en;
  skos:definition "PR is the business you get into when you get let go from your journalism job. Not to be confused with pull requests."@en;
  skos:inScheme <urn:uuid:797e83d7-a86f-4838-b5c5-0ec20855197d>,
    <urn:uuid:bbe073ad-f449-4b25-91ac-7d919613ca51>,
    <urn:uuid:2df6fac6-3122-44dc-9f92-5caab7f9b10b>,
    <urn:uuid:1b457bed-8a80-4135-92b8-fdea12b4eea3>,
    <urn:uuid:2153d83b-8555-44a3-96e0-821b6663a188>,
    <urn:uuid:4bbcdde6-ed53-4f8d-b3f8-43f800fd05d5>;
  skos:prefLabel "public relations"@en;
  skos:related <urn:uuid:4333e98e-4565-4d4e-b600-d7cc9e95a972> .

<urn:uuid:63e17424-63fb-43ad-81ad-9c990c9938ce> a skos:Concept;
  dct:created "2021-12-14T17:54:16Z"^^xsd:dateTime;
  dct:creator <urn:uuid:ca637d4b-c11b-4152-be98-bde602e7abd4>;
  skos:definition "Crawling is the act of an automated agent mapping out the Web by following links. Google famously crawls the Web for its search engine. Web crawling software can be quite complex and sophisticated in order to deal with copious confounding factors on the open Internet.  Under ideal conditions, content inventories can be generated by crawling."@en;
  skos:hiddenLabel "crawling"@en;
  skos:inScheme <urn:uuid:bbe073ad-f449-4b25-91ac-7d919613ca51>,
    <urn:uuid:797e83d7-a86f-4838-b5c5-0ec20855197d>,
    <urn:uuid:2df6fac6-3122-44dc-9f92-5caab7f9b10b>,
    <urn:uuid:1b457bed-8a80-4135-92b8-fdea12b4eea3>,
    <urn:uuid:2153d83b-8555-44a3-96e0-821b6663a188>,
    <urn:uuid:4bbcdde6-ed53-4f8d-b3f8-43f800fd05d5>;
  skos:prefLabel "Web crawling"@en;
  skos:related <urn:uuid:01dc6e60-8e23-4c4c-a63d-f149cb104f84>,
    <urn:uuid:25e0f651-e8c8-4cce-9126-fbe1f5280cb5> .

<urn:uuid:64020bd3-d3d7-4e5f-980b-95116b19eb0e> a skos:Concept;
  dct:created "2021-12-14T23:50:47Z"^^xsd:dateTime;
  dct:creator <urn:uuid:ca637d4b-c11b-4152-be98-bde602e7abd4>;
  skos:broader <urn:uuid:91bffd8d-1f18-4604-844e-6a5557947a67>;
  skos:definition "A Web hook is a target for remote information systems, identified by URL, for accepting event notifications."@en;
  skos:hiddenLabel "Webhook"@en,
    "web hooks"@en,
    "webhooks"@en;
  skos:inScheme <urn:uuid:bbe073ad-f449-4b25-91ac-7d919613ca51>,
    <urn:uuid:797e83d7-a86f-4838-b5c5-0ec20855197d>,
    <urn:uuid:2df6fac6-3122-44dc-9f92-5caab7f9b10b>,
    <urn:uuid:1b457bed-8a80-4135-92b8-fdea12b4eea3>,
    <urn:uuid:2153d83b-8555-44a3-96e0-821b6663a188>,
    <urn:uuid:4bbcdde6-ed53-4f8d-b3f8-43f800fd05d5>;
  skos:prefLabel "Web hook"@en;
  skos:related <urn:uuid:696cc8e6-8cc0-4e91-b410-97942abf883c> .

<urn:uuid:685c3853-4389-424c-948c-8ad3b60a48c2> a skos:Concept;
  dct:created "2021-12-14T23:43:13Z"^^xsd:dateTime;
  dct:creator <urn:uuid:ca637d4b-c11b-4152-be98-bde602e7abd4>;
  skos:altLabel "UGC"@en;
  skos:definition "User-generated content is exactly what it sounds like: content on a networked information service platform generated or sourced by that platform's users, as opposed to the platform's operators."@en;
  skos:hiddenLabel "ugc"@en;
  skos:inScheme <urn:uuid:bbe073ad-f449-4b25-91ac-7d919613ca51>,
    <urn:uuid:2df6fac6-3122-44dc-9f92-5caab7f9b10b>,
    <urn:uuid:797e83d7-a86f-4838-b5c5-0ec20855197d>,
    <urn:uuid:1b457bed-8a80-4135-92b8-fdea12b4eea3>,
    <urn:uuid:2153d83b-8555-44a3-96e0-821b6663a188>,
    <urn:uuid:4bbcdde6-ed53-4f8d-b3f8-43f800fd05d5>;
  skos:prefLabel "user-generated content"@en;
  skos:related <urn:uuid:c8544100-23fa-466e-8bd0-f8eb001a9e83>,
    <urn:uuid:42747b64-a41c-4321-96cf-c49e711733e6> .

<urn:uuid:6948b692-bc60-4625-9861-9934379f36b5> a skos:Concept;
  dct:created "2021-12-14T20:12:49Z"^^xsd:dateTime;
  dct:creator <urn:uuid:ca637d4b-c11b-4152-be98-bde602e7abd4>;
  skos:altLabel "KLOC"@en,
    "thousand lines of code"@en;
  skos:broader <urn:uuid:fdb43f70-cb11-49dd-aba6-7011b05ad61a>,
    <urn:uuid:aa5f9563-e527-4df2-8518-ce325819f1e6>;
  skos:definition "A thousand lines of code very roughly correlates to (at least no less than) a certain quantity of software development effort, which will nevertheless depend on many other factors to yield an intelligible number."@en;
  skos:inScheme <urn:uuid:bbe073ad-f449-4b25-91ac-7d919613ca51>,
    <urn:uuid:2df6fac6-3122-44dc-9f92-5caab7f9b10b>,
    <urn:uuid:797e83d7-a86f-4838-b5c5-0ec20855197d>,
    <urn:uuid:1b457bed-8a80-4135-92b8-fdea12b4eea3>,
    <urn:uuid:2153d83b-8555-44a3-96e0-821b6663a188>,
    <urn:uuid:4bbcdde6-ed53-4f8d-b3f8-43f800fd05d5>;
  skos:prefLabel "kilo-lines of code"@en .

<urn:uuid:6dddf461-39ab-4037-9f49-2c217f09d289> a skos:Concept;
  dct:created "2021-12-14T21:20:49Z"^^xsd:dateTime;
  dct:creator <urn:uuid:ca637d4b-c11b-4152-be98-bde602e7abd4>;
  skos:broader <urn:uuid:9e506ca3-8be1-431d-9075-548141d9f8c1>,
    <urn:uuid:349633ba-03b8-4126-8e55-1ed9a7c7e4ec>;
  skos:definition "The query component of a URI (everything after the first question mark) is by convention ascribed additional semantics in some contexts, whereby it is taken to represent a set of key-value pairs. A query parameter (key=value) is one of those pairs."@en;
  skos:hiddenLabel "query parameters"@en;
  skos:inScheme <urn:uuid:1b457bed-8a80-4135-92b8-fdea12b4eea3>,
    <urn:uuid:2153d83b-8555-44a3-96e0-821b6663a188>,
    <urn:uuid:797e83d7-a86f-4838-b5c5-0ec20855197d>,
    <urn:uuid:bbe073ad-f449-4b25-91ac-7d919613ca51>,
    <urn:uuid:2df6fac6-3122-44dc-9f92-5caab7f9b10b>,
    <urn:uuid:4bbcdde6-ed53-4f8d-b3f8-43f800fd05d5>;
  skos:prefLabel "query parameter"@en .

<urn:uuid:721ae2be-bf89-42bd-bd8d-3b567fbba55e> a skos:Concept;
  dct:created "2021-12-14T02:59:05Z"^^xsd:dateTime;
  dct:creator <urn:uuid:ca637d4b-c11b-4152-be98-bde602e7abd4>;
  skos:altLabel "canonical form"@en;
  skos:broader <urn:uuid:5bdd2fb7-d84d-4583-998b-7d3f2803307e>,
    <urn:uuid:c2f6ce23-c916-448d-8e18-c122d347cf17>;
  skos:definition "To call a representation of any information resource \"canonical\" implies that said representation at least encapsulates all available information about the resource, and moreover is in some form that is most desirable for, if not storage, then at least exchange."@en;
  skos:inScheme <urn:uuid:1b457bed-8a80-4135-92b8-fdea12b4eea3>,
    <urn:uuid:2153d83b-8555-44a3-96e0-821b6663a188>,
    <urn:uuid:797e83d7-a86f-4838-b5c5-0ec20855197d>,
    <urn:uuid:2df6fac6-3122-44dc-9f92-5caab7f9b10b>,
    <urn:uuid:bbe073ad-f449-4b25-91ac-7d919613ca51>,
    <urn:uuid:4bbcdde6-ed53-4f8d-b3f8-43f800fd05d5>;
  skos:prefLabel "canonical representation"@en;
  skos:related <urn:uuid:332a68b3-06d6-4ac2-8897-4212ba0f3a94> .

<urn:uuid:74279862-8c3e-47b3-8522-07a88fbfd5e8> a skos:Concept;
  dct:created "2021-12-14T20:00:39Z"^^xsd:dateTime;
  dct:creator <urn:uuid:ca637d4b-c11b-4152-be98-bde602e7abd4>;
  skos:definition "In programming, an interpolated (concatenated) string is a string of text that has been composed from multiple parts."@en;
  skos:hiddenLabel "interpolated strings"@en;
  skos:inScheme <urn:uuid:2df6fac6-3122-44dc-9f92-5caab7f9b10b>,
    <urn:uuid:1b457bed-8a80-4135-92b8-fdea12b4eea3>,
    <urn:uuid:2153d83b-8555-44a3-96e0-821b6663a188>,
    <urn:uuid:797e83d7-a86f-4838-b5c5-0ec20855197d>,
    <urn:uuid:bbe073ad-f449-4b25-91ac-7d919613ca51>,
    <urn:uuid:4bbcdde6-ed53-4f8d-b3f8-43f800fd05d5>;
  skos:prefLabel "interpolated string"@en;
  skos:related <urn:uuid:61a28be0-4688-4591-b633-b00ea2053b38> .

<urn:uuid:7767027c-2f40-40fc-9130-1736a47a85de> a skos:Concept;
  dct:created "2017-02-22T01:26:19Z"^^xsd:dateTime;
  dct:creator <urn:uuid:ca637d4b-c11b-4152-be98-bde602e7abd4>;
  skos:definition "A local network is a computer network contained within a house, office, or organization."@en;
  skos:inScheme <urn:uuid:2df6fac6-3122-44dc-9f92-5caab7f9b10b>,
    <urn:uuid:49ac68c4-922c-4d9e-88fa-b318fc54d36f>,
    <urn:uuid:1b457bed-8a80-4135-92b8-fdea12b4eea3>,
    <urn:uuid:2153d83b-8555-44a3-96e0-821b6663a188>,
    <urn:uuid:bbe073ad-f449-4b25-91ac-7d919613ca51>,
    <urn:uuid:4bbcdde6-ed53-4f8d-b3f8-43f800fd05d5>;
  skos:narrower <urn:uuid:b20221c0-4949-471a-adb1-45dfccfbdf1c>;
  skos:prefLabel "local network"@en .

<urn:uuid:78f31a9a-95eb-4daf-965f-de0184f697f7> a skos:Concept;
  dct:created "2022-11-23T22:32:28Z"^^xsd:dateTime;
  dct:creator <urn:uuid:ca637d4b-c11b-4152-be98-bde602e7abd4>;
  skos:broader <urn:uuid:525f262f-32e3-4c35-96d4-e9eb11e19370>;
  skos:definition "An asset transform is one that focuses on transforming files, either in ways that can be round-tripped or ways that are lossy. An example would be converting images from one format to another, or cropping and resizing them."@en;
  skos:inScheme <urn:uuid:1b457bed-8a80-4135-92b8-fdea12b4eea3>,
    <urn:uuid:2153d83b-8555-44a3-96e0-821b6663a188>,
    <urn:uuid:0c7028f0-8226-47b3-acff-a4e83e6a60fd>,
    <urn:uuid:bbe073ad-f449-4b25-91ac-7d919613ca51>,
    <urn:uuid:4bbcdde6-ed53-4f8d-b3f8-43f800fd05d5>;
  skos:prefLabel "asset transform"@en;
  skos:related <urn:uuid:13385ea1-1f87-4612-b86b-27bc4e339be6> .

<urn:uuid:79c4d922-3660-46ce-bdf8-67ffba7116f5> a skos:Concept;
  dct:created "2019-02-28T18:59:31Z"^^xsd:dateTime;
  dct:creator <urn:uuid:ca637d4b-c11b-4152-be98-bde602e7abd4>;
  skos:definition "A syndication feed is a list of Web resources which is polled for updates."@en;
  skos:inScheme <urn:uuid:2df6fac6-3122-44dc-9f92-5caab7f9b10b>,
    <urn:uuid:1b457bed-8a80-4135-92b8-fdea12b4eea3>,
    <urn:uuid:2153d83b-8555-44a3-96e0-821b6663a188>,
    <urn:uuid:bbe073ad-f449-4b25-91ac-7d919613ca51>,
    <urn:uuid:75f35368-e228-47fe-8efd-7251a2bde816>,
    <urn:uuid:4bbcdde6-ed53-4f8d-b3f8-43f800fd05d5>;
  skos:narrower <urn:uuid:4c034864-ee75-4ca7-b93f-119152b11796>,
    <urn:uuid:9ed8a948-df9f-4ee3-95d1-47b28174b6a8>,
    <urn:uuid:ba2258e3-efca-4461-82cc-f6ebbf980b36>;
  skos:prefLabel "syndication feed"@en .

<urn:uuid:7a46613a-70f8-4d1d-ad8f-f23b6f1a9e06> a skos:Concept;
  dct:created "2022-11-23T23:24:52Z"^^xsd:dateTime;
  dct:creator <urn:uuid:ca637d4b-c11b-4152-be98-bde602e7abd4>;
  skos:broader <urn:uuid:a718d483-af90-4eaf-a59f-31d8897d6e8e>;
  skos:definition "An attack surface is an imaginary space that a hypothetical adversary can target. There is likewise an imaginary metric to this space, so the attack surface of a particular system can be thought of as \"larger\" or \"smaller\" than some other system."@en;
  skos:inScheme <urn:uuid:1b457bed-8a80-4135-92b8-fdea12b4eea3>,
    <urn:uuid:2153d83b-8555-44a3-96e0-821b6663a188>,
    <urn:uuid:bbe073ad-f449-4b25-91ac-7d919613ca51>,
    <urn:uuid:4bbcdde6-ed53-4f8d-b3f8-43f800fd05d5>;
  skos:prefLabel "attack surface"@en;
  skos:related <urn:uuid:d5b402b1-92b0-47c2-9063-3b0358b616ee> .

<urn:uuid:7bc6cba9-9c8b-4479-95d0-7c475f95f532> a skos:Concept;
  dct:created "2024-07-03T21:27:51Z"^^xsd:dateTime,
    "2024-02-16T15:24:23Z"^^xsd:dateTime;
  dct:creator <urn:uuid:ca637d4b-c11b-4152-be98-bde602e7abd4>;
  skos:definition "“Eating one's own dog food” is a quality assurance tactic which means to use one's own products and services. It is attributed to Clement Hirsch, the eccentric erstwhile president of Kal Kan Incorporated, who (apocryphally) would pull the stunt of eating from a can of his company's dog food at shareholder meetings."@en;
  skos:hiddenLabel "dog food"@en,
    "dog fooding"@en,
    "dog-food"@en,
    "dogfood"@en,
    "dogfooding"@en;
  skos:inScheme <urn:uuid:bbe073ad-f449-4b25-91ac-7d919613ca51>,
    <urn:uuid:0c7028f0-8226-47b3-acff-a4e83e6a60fd>,
    <urn:uuid:1b457bed-8a80-4135-92b8-fdea12b4eea3>,
    <urn:uuid:2153d83b-8555-44a3-96e0-821b6663a188>,
    <urn:uuid:4bbcdde6-ed53-4f8d-b3f8-43f800fd05d5>;
  skos:prefLabel "dog-fooding"@en .

<urn:uuid:7d6928c9-801e-4205-a00b-8a2b2b1dc9b0> a skos:Concept;
  dct:created "2022-11-24T02:16:22Z"^^xsd:dateTime;
  dct:creator <urn:uuid:ca637d4b-c11b-4152-be98-bde602e7abd4>;
  skos:definition "Metadata is data about data, or in the context of Web content, could be any structured data associated with a webpage."@en;
  skos:hiddenLabel "meta data"@en,
    "meta-data"@en;
  skos:inScheme <urn:uuid:bbe073ad-f449-4b25-91ac-7d919613ca51>,
    <urn:uuid:a1a01f1c-7162-439c-94f1-3e28b99ae8ab>,
    <urn:uuid:ddfaaacc-9dcb-451b-afa6-477e6e787a5c>,
    <urn:uuid:1b457bed-8a80-4135-92b8-fdea12b4eea3>,
    <urn:uuid:2153d83b-8555-44a3-96e0-821b6663a188>,
    <urn:uuid:0c7028f0-8226-47b3-acff-a4e83e6a60fd>,
    <urn:uuid:4bbcdde6-ed53-4f8d-b3f8-43f800fd05d5>;
  skos:prefLabel "metadata"@en;
  skos:related <urn:uuid:c757c1ac-1ec6-4bdd-a35d-85f1d85728bb> .

<urn:uuid:823a4be6-cd1a-4b45-b645-92a03d1c41e8> a skos:Concept;
  dct:created "2019-02-19T04:25:24Z"^^xsd:dateTime;
  dct:creator <urn:uuid:ca637d4b-c11b-4152-be98-bde602e7abd4>;
  skos:broader <urn:uuid:f352a521-b78e-478e-b01d-3a68638025a4>;
  skos:inScheme <urn:uuid:2df6fac6-3122-44dc-9f92-5caab7f9b10b>,
    <urn:uuid:1b457bed-8a80-4135-92b8-fdea12b4eea3>,
    <urn:uuid:2153d83b-8555-44a3-96e0-821b6663a188>,
    <urn:uuid:bbe073ad-f449-4b25-91ac-7d919613ca51>,
    <urn:uuid:75f35368-e228-47fe-8efd-7251a2bde816>,
    <urn:uuid:4bbcdde6-ed53-4f8d-b3f8-43f800fd05d5>;
  skos:prefLabel "DocBook"@en .

<urn:uuid:82a64468-dbd4-4cb2-a526-5ae5482f5957> a skos:Concept;
  dct:created "2019-03-02T07:04:46Z"^^xsd:dateTime;
  dct:creator <urn:uuid:ca637d4b-c11b-4152-be98-bde602e7abd4>;
  skos:definition "Protégé is the go-to editor for OWL ontologies."@en;
  skos:inScheme <urn:uuid:2df6fac6-3122-44dc-9f92-5caab7f9b10b>,
    <urn:uuid:1b457bed-8a80-4135-92b8-fdea12b4eea3>,
    <urn:uuid:2153d83b-8555-44a3-96e0-821b6663a188>,
    <urn:uuid:bbe073ad-f449-4b25-91ac-7d919613ca51>,
    <urn:uuid:75f35368-e228-47fe-8efd-7251a2bde816>,
    <urn:uuid:4bbcdde6-ed53-4f8d-b3f8-43f800fd05d5>;
  skos:prefLabel "Protégé"@en;
  skos:related <urn:uuid:384f764c-9d71-46a3-9865-0af7068c0703>,
    <urn:uuid:ed4d30d7-d3cf-4b21-bcb4-5f2525027be7> .

<urn:uuid:86f1193f-7e4f-4948-86d2-537d9d1ecd4e> a skos:Concept;
  dct:created "2021-12-14T01:09:54Z"^^xsd:dateTime;
  dct:creator <urn:uuid:ca637d4b-c11b-4152-be98-bde602e7abd4>;
  skos:definition "Caching is the process of storing the outcome of a computation or retrieval of information from a remote or computationally expensive source, typically carried out to increase the efficiency and durability of the overall process. A cache is a region in data storage with additional directives to periodically remove elements that are judged by some mechanism to be stale."@en;
  skos:hiddenLabel "caching"@en;
  skos:inScheme <urn:uuid:2df6fac6-3122-44dc-9f92-5caab7f9b10b>,
    <urn:uuid:0c7028f0-8226-47b3-acff-a4e83e6a60fd>,
    <urn:uuid:1b457bed-8a80-4135-92b8-fdea12b4eea3>,
    <urn:uuid:2153d83b-8555-44a3-96e0-821b6663a188>,
    <urn:uuid:797e83d7-a86f-4838-b5c5-0ec20855197d>,
    <urn:uuid:bbe073ad-f449-4b25-91ac-7d919613ca51>,
    <urn:uuid:4bbcdde6-ed53-4f8d-b3f8-43f800fd05d5>;
  skos:narrower <urn:uuid:53819af5-c2d0-4edc-9add-ab79829ace96>;
  skos:prefLabel "cache"@en .

<urn:uuid:8ab18c57-c95b-4c41-9537-8b90434a11bf> a skos:Concept;
  dct:created "2017-02-09T17:38:22Z"^^xsd:dateTime;
  dct:creator <urn:uuid:ca637d4b-c11b-4152-be98-bde602e7abd4>;
  dct:references <https://www.microsoft.com/en-us/cloud-platform/server-virtualization>,
    <https://en.wikipedia.org/wiki/Hyper-V>;
  skos:broader <urn:uuid:81abc2b5-5ead-4549-bff2-f326c38f535c>;
  skos:definition "A virtual server is a computer that runs inside another computer, meaning no additional hardware is necessary."@en ;
  skos:inScheme <urn:uuid:49ac68c4-922c-4d9e-88fa-b318fc54d36f>,
    <urn:uuid:2df6fac6-3122-44dc-9f92-5caab7f9b10b>,
    <urn:uuid:1b457bed-8a80-4135-92b8-fdea12b4eea3>,
    <urn:uuid:2153d83b-8555-44a3-96e0-821b6663a188>,
    <urn:uuid:bbe073ad-f449-4b25-91ac-7d919613ca51>,
    <urn:uuid:4bbcdde6-ed53-4f8d-b3f8-43f800fd05d5>;
  skos:prefLabel "virtual server"@en .

<urn:uuid:8c2c631e-7332-419f-bc5d-2df5dcb6d356> a skos:Concept;
  dct:created "2021-12-14T22:54:44Z"^^xsd:dateTime;
  dct:creator <urn:uuid:ca637d4b-c11b-4152-be98-bde602e7abd4>;
  skos:altLabel "SKU"@en;
  skos:broader <urn:uuid:6c18acc3-3119-4f0b-8d24-0ca0ea9449d3>;
  skos:definition "An SKU is an identifier for a particular product in a company's inventory."@en;
  skos:hiddenLabel "SKUs"@en;
  skos:inScheme <urn:uuid:797e83d7-a86f-4838-b5c5-0ec20855197d>,
    <urn:uuid:2df6fac6-3122-44dc-9f92-5caab7f9b10b>,
    <urn:uuid:1b457bed-8a80-4135-92b8-fdea12b4eea3>,
    <urn:uuid:2153d83b-8555-44a3-96e0-821b6663a188>,
    <urn:uuid:bbe073ad-f449-4b25-91ac-7d919613ca51>,
    <urn:uuid:4bbcdde6-ed53-4f8d-b3f8-43f800fd05d5>;
  skos:prefLabel "stock keeping unit"@en .

<urn:uuid:8cfe9c84-4773-4717-b601-6a6dd5bccc5c> a skos:Concept;
  dct:created "2017-07-12T03:03:57Z"^^xsd:dateTime;
  dct:creator <urn:uuid:ca637d4b-c11b-4152-be98-bde602e7abd4>;
  dct:references <https://www.w3.org/TR/skos-primer/>;
  skos:broader <urn:uuid:86c65d14-2d23-4350-8004-233b2f3e873f>,
    <urn:uuid:4eab5a63-adc6-4efd-b49e-402131b519fa>;
  skos:definition "SKOS (Simple Knowledge Organization System) is an OWL ontology for representing concept schemes and/or thesauri, which are particular kinds of taxonomies."@en;
  skos:inScheme <urn:uuid:91684d49-7b99-4b2e-9641-ea0b8e22f66c>,
    <urn:uuid:2df6fac6-3122-44dc-9f92-5caab7f9b10b>,
    <urn:uuid:1b457bed-8a80-4135-92b8-fdea12b4eea3>,
    <urn:uuid:2153d83b-8555-44a3-96e0-821b6663a188>,
    <urn:uuid:bbe073ad-f449-4b25-91ac-7d919613ca51>,
    <urn:uuid:75f35368-e228-47fe-8efd-7251a2bde816>,
    <urn:uuid:4bbcdde6-ed53-4f8d-b3f8-43f800fd05d5>;
  skos:prefLabel "SKOS"@en;
  skos:related <urn:uuid:0f872daf-97f4-445e-b5d9-0de0087dd129>,
    <urn:uuid:45b6c768-da32-4e5f-9c87-a18d5ec94635>,
    <urn:uuid:ed4d30d7-d3cf-4b21-bcb4-5f2525027be7>,
    <urn:uuid:fe14fe9c-8794-440a-86ad-0e245c3cbb7b> .

<urn:uuid:8e009d49-3661-49be-8ad5-57f5fe59d7e2> a skos:Concept;
  dct:created "2017-08-22T23:33:26Z"^^xsd:dateTime;
  dct:creator <urn:uuid:ca637d4b-c11b-4152-be98-bde602e7abd4>;
  skos:broader <urn:uuid:9767147a-1b6a-440c-949f-7f6056e28411>;
  skos:definition "A coded property is one which takes a finite set of predefined values."@en;
  skos:inScheme <urn:uuid:49ac68c4-922c-4d9e-88fa-b318fc54d36f>,
    <urn:uuid:2df6fac6-3122-44dc-9f92-5caab7f9b10b>,
    <urn:uuid:bbe073ad-f449-4b25-91ac-7d919613ca51>,
    <urn:uuid:1b457bed-8a80-4135-92b8-fdea12b4eea3>,
    <urn:uuid:2153d83b-8555-44a3-96e0-821b6663a188>,
    <urn:uuid:4bbcdde6-ed53-4f8d-b3f8-43f800fd05d5>;
  skos:prefLabel "coded property"@en .

<urn:uuid:92e58bd6-446c-46eb-bacb-d5f098c57ca7> a skos:Concept;
  dct:created "2022-12-02T14:18:28Z"^^xsd:dateTime;
  dct:creator <urn:uuid:ca637d4b-c11b-4152-be98-bde602e7abd4>;
  skos:altLabel "representational state"@en,
    "state"@en;
  skos:definition "In computing, state can be understood as the sum total of all the information needed to reconstruct a process at a particular instant. This in principle makes state an observable, describable, quantifiable object, and potentially an addressable information resource in its own right."@en;
  skos:inScheme <urn:uuid:1b457bed-8a80-4135-92b8-fdea12b4eea3>,
    <urn:uuid:2153d83b-8555-44a3-96e0-821b6663a188>,
    <urn:uuid:0c7028f0-8226-47b3-acff-a4e83e6a60fd>,
    <urn:uuid:4ec7530b-5536-4fb7-bb5a-45a3f5fddc22>,
    <urn:uuid:bbe073ad-f449-4b25-91ac-7d919613ca51>,
    <urn:uuid:4bbcdde6-ed53-4f8d-b3f8-43f800fd05d5>;
  skos:narrower <urn:uuid:288e85ab-887f-437c-9caa-c109cb9d478d>;
  skos:prefLabel "state (computing)"@en .

<urn:uuid:94e05d9c-177d-4e41-9097-7aaf1f39db78> a skos:Concept;
  dct:created "2019-03-07T00:50:33Z"^^xsd:dateTime;
  dct:creator <urn:uuid:ca637d4b-c11b-4152-be98-bde602e7abd4>;
  skos:broader <urn:uuid:f0e4c33f-8930-454a-9a7e-dd2b6cc79dce>,
    <urn:uuid:4694ebe0-589f-40a7-9ef9-67872edb6214>;
  skos:inScheme <urn:uuid:1b457bed-8a80-4135-92b8-fdea12b4eea3>,
    <urn:uuid:2153d83b-8555-44a3-96e0-821b6663a188>,
    <urn:uuid:75f35368-e228-47fe-8efd-7251a2bde816>,
    <urn:uuid:2df6fac6-3122-44dc-9f92-5caab7f9b10b>,
    <urn:uuid:bbe073ad-f449-4b25-91ac-7d919613ca51>,
    <urn:uuid:4bbcdde6-ed53-4f8d-b3f8-43f800fd05d5>;
  skos:prefLabel "SQLite"@en;
  skos:related <urn:uuid:2717d0b5-cb79-4d1a-82c0-69cdc1e590a1> .

<urn:uuid:9bca42c4-969e-4904-933e-ac23b24de656> a skos:Concept;
  dct:created "2022-11-23T21:20:45Z"^^xsd:dateTime;
  dct:creator <urn:uuid:ca637d4b-c11b-4152-be98-bde602e7abd4>;
  skos:altLabel "bijective function"@en,
    "isomorphic"@en,
    "lossless transformation"@en,
    "structure-preserving transformation"@en;
  skos:definition "An isomorphism can be understood as a perfect, 1:1 relation between two sets, such that every element in one set has exactly one counterpart in the other. In computing, an isomorphism is the pair of operations that transform the elements from one set to the other. For example, the \"zip\" and \"unzip\" algorithms, together, form an isomorphism."@en;
  skos:inScheme <urn:uuid:4ec7530b-5536-4fb7-bb5a-45a3f5fddc22>,
    <urn:uuid:bbe073ad-f449-4b25-91ac-7d919613ca51>,
    <urn:uuid:1b457bed-8a80-4135-92b8-fdea12b4eea3>,
    <urn:uuid:2153d83b-8555-44a3-96e0-821b6663a188>,
    <urn:uuid:0c7028f0-8226-47b3-acff-a4e83e6a60fd>,
    <urn:uuid:4bbcdde6-ed53-4f8d-b3f8-43f800fd05d5>;
  skos:prefLabel "isomorphism"@en;
  skos:related <urn:uuid:cc74f8e0-34cc-4a69-b9d5-87b990aca6b6> .

<urn:uuid:9db33933-20e6-4a93-8195-7ee46b013593> a skos:Concept;
  dct:created "2022-11-23T21:41:38Z"^^xsd:dateTime;
  dct:creator <urn:uuid:ca637d4b-c11b-4152-be98-bde602e7abd4>;
  skos:definition "Link rot is the colloquial term used to refer to the tendency for URLs to become decoupled from the information resources they reference."@en;
  skos:inScheme <urn:uuid:0c7028f0-8226-47b3-acff-a4e83e6a60fd>,
    <urn:uuid:bbe073ad-f449-4b25-91ac-7d919613ca51>,
    <urn:uuid:1b457bed-8a80-4135-92b8-fdea12b4eea3>,
    <urn:uuid:2153d83b-8555-44a3-96e0-821b6663a188>,
    <urn:uuid:4bbcdde6-ed53-4f8d-b3f8-43f800fd05d5>;
  skos:prefLabel "link rot"@en;
  skos:related <urn:uuid:4039a99d-c14b-40f2-84d5-4ec72e2217e1>,
    <urn:uuid:e162d03b-bfec-4f01-ab7e-56da309550f6> .

<urn:uuid:b0af57aa-7341-4f23-b179-d9057d37c1e3> a skos:Concept;
  dct:created "2021-12-14T21:28:08Z"^^xsd:dateTime;
  dct:creator <urn:uuid:ca637d4b-c11b-4152-be98-bde602e7abd4>;
  skos:broader <urn:uuid:02b3d282-d134-487b-8226-80141b5a4338>;
  skos:definition "An HTTP redirect instructs a client who has requested one URL to request a different one instead."@en;
  skos:hiddenLabel "redirects"@en;
  skos:inScheme <urn:uuid:bbe073ad-f449-4b25-91ac-7d919613ca51>,
    <urn:uuid:797e83d7-a86f-4838-b5c5-0ec20855197d>,
    <urn:uuid:2df6fac6-3122-44dc-9f92-5caab7f9b10b>,
    <urn:uuid:1b457bed-8a80-4135-92b8-fdea12b4eea3>,
    <urn:uuid:2153d83b-8555-44a3-96e0-821b6663a188>,
    <urn:uuid:4bbcdde6-ed53-4f8d-b3f8-43f800fd05d5>;
  skos:prefLabel "HTTP redirect"@en .

<urn:uuid:b53ed460-4712-4f74-bb92-50692627a0e1> a skos:Concept;
  dct:created "2021-12-14T22:48:51Z"^^xsd:dateTime;
  dct:creator <urn:uuid:ca637d4b-c11b-4152-be98-bde602e7abd4>;
  skos:altLabel "SDK"@en;
  skos:broader <urn:uuid:23ae24d6-80b8-4f31-8510-562c45871694>;
  skos:definition "An SDK is a framework and attendant tooling and other resources for creating software for a given platform."@en;
  skos:hiddenLabel "SDKs"@en,
    "sdk"@en;
  skos:inScheme <urn:uuid:1b457bed-8a80-4135-92b8-fdea12b4eea3>,
    <urn:uuid:2153d83b-8555-44a3-96e0-821b6663a188>,
    <urn:uuid:bbe073ad-f449-4b25-91ac-7d919613ca51>,
    <urn:uuid:2df6fac6-3122-44dc-9f92-5caab7f9b10b>,
    <urn:uuid:797e83d7-a86f-4838-b5c5-0ec20855197d>,
    <urn:uuid:4bbcdde6-ed53-4f8d-b3f8-43f800fd05d5>;
  skos:prefLabel "software development kit"@en;
  skos:related <urn:uuid:fdb43f70-cb11-49dd-aba6-7011b05ad61a> .

<urn:uuid:bccac162-3684-40a3-a5e5-564c51d6b7c3> a skos:Concept;
  dct:created "2021-12-14T18:41:19Z"^^xsd:dateTime;
  dct:creator <urn:uuid:ca637d4b-c11b-4152-be98-bde602e7abd4>;
  skos:definition "A DNS domain name is a mapping of, among other things, IP addresses to (ideally) human-readable words. Domain names are delegated through a hierarchy in the form delegate.principal.top. Domain names form the authority component of a URL, and from which root URLs to websites can be programmatically inferred, which causes some to say URL when they mean domain name."@en;
  skos:inScheme <urn:uuid:797e83d7-a86f-4838-b5c5-0ec20855197d>,
    <urn:uuid:1b457bed-8a80-4135-92b8-fdea12b4eea3>,
    <urn:uuid:2153d83b-8555-44a3-96e0-821b6663a188>,
    <urn:uuid:bbe073ad-f449-4b25-91ac-7d919613ca51>,
    <urn:uuid:2df6fac6-3122-44dc-9f92-5caab7f9b10b>,
    <urn:uuid:4bbcdde6-ed53-4f8d-b3f8-43f800fd05d5>;
  skos:narrower <urn:uuid:97fb551f-c68a-43bb-8153-9c88f916e70b>;
  skos:prefLabel "domain name"@en;
  skos:related <urn:uuid:9e506ca3-8be1-431d-9075-548141d9f8c1> .

<urn:uuid:c133de82-8e10-4303-a97c-6fef4397aa5d> a skos:Concept;
  dct:created "2021-12-14T20:35:01Z"^^xsd:dateTime;
  dct:creator <urn:uuid:ca637d4b-c11b-4152-be98-bde602e7abd4>;
  skos:broader <urn:uuid:42747b64-a41c-4321-96cf-c49e711733e6>;
  skos:definition "Microcontent refers to the text in software systems on e.g., buttons, labels, tool tips, and error messages."@en;
  skos:hiddenLabel "micro-content"@en;
  skos:inScheme <urn:uuid:0c7028f0-8226-47b3-acff-a4e83e6a60fd>,
    <urn:uuid:1b457bed-8a80-4135-92b8-fdea12b4eea3>,
    <urn:uuid:2153d83b-8555-44a3-96e0-821b6663a188>,
    <urn:uuid:797e83d7-a86f-4838-b5c5-0ec20855197d>,
    <urn:uuid:bbe073ad-f449-4b25-91ac-7d919613ca51>,
    <urn:uuid:2df6fac6-3122-44dc-9f92-5caab7f9b10b>,
    <urn:uuid:4bbcdde6-ed53-4f8d-b3f8-43f800fd05d5>;
  skos:prefLabel "microcontent"@en .

<urn:uuid:c3d00465-8d3c-4a0c-9a75-cbf21c53ca2f> a skos:Concept;
  dct:created "2021-12-14T19:53:51Z"^^xsd:dateTime;
  dct:creator <urn:uuid:ca637d4b-c11b-4152-be98-bde602e7abd4>;
  skos:altLabel "I/O"@en;
  skos:broader <urn:uuid:fdb43f70-cb11-49dd-aba6-7011b05ad61a>;
  skos:definition "In software development, I/O is a first-order physical resource constraint, along with CPU, memory, and storage."@en;
  skos:inScheme <urn:uuid:1b457bed-8a80-4135-92b8-fdea12b4eea3>,
    <urn:uuid:2153d83b-8555-44a3-96e0-821b6663a188>,
    <urn:uuid:bbe073ad-f449-4b25-91ac-7d919613ca51>,
    <urn:uuid:797e83d7-a86f-4838-b5c5-0ec20855197d>,
    <urn:uuid:2df6fac6-3122-44dc-9f92-5caab7f9b10b>,
    <urn:uuid:4bbcdde6-ed53-4f8d-b3f8-43f800fd05d5>;
  skos:prefLabel "input/output"@en .

<urn:uuid:ca5c533b-5432-4efb-b5e5-4a5454868176> a skos:Concept;
  dct:created "2021-12-13T22:52:13Z"^^xsd:dateTime;
  dct:creator <urn:uuid:ca637d4b-c11b-4152-be98-bde602e7abd4>;
  skos:definition "An adapter, in the generic sense, is anything that connects one system to another."@en;
  skos:hiddenLabel "adapters"@en;
  skos:inScheme <urn:uuid:797e83d7-a86f-4838-b5c5-0ec20855197d>,
    <urn:uuid:bbe073ad-f449-4b25-91ac-7d919613ca51>,
    <urn:uuid:1b457bed-8a80-4135-92b8-fdea12b4eea3>,
    <urn:uuid:2153d83b-8555-44a3-96e0-821b6663a188>,
    <urn:uuid:2df6fac6-3122-44dc-9f92-5caab7f9b10b>,
    <urn:uuid:4bbcdde6-ed53-4f8d-b3f8-43f800fd05d5>;
  skos:narrower <urn:uuid:3cdd469a-195b-4040-8d74-fd27bc71f12d>,
    <urn:uuid:db972323-c096-4ddf-80ce-0e98f6b7c7c7>;
  skos:prefLabel "adapter"@en .

<urn:uuid:d3b55627-8e74-48b2-b5ac-79545ac83235> a skos:Concept;
  dct:created "2017-06-23T12:47:34Z"^^xsd:dateTime;
  dct:creator <urn:uuid:ca637d4b-c11b-4152-be98-bde602e7abd4>;
  skos:broader <urn:uuid:3a2c72e0-4fa5-4477-a51b-d7f073cc1155>;
  skos:definition "The colour palette assigns a particular colour to a particular mapping of data dimensions and values. This tools has tens of thousands of such mappings, and thus the colour palette is generated programmatically."@en;
  skos:inScheme <urn:uuid:2df6fac6-3122-44dc-9f92-5caab7f9b10b>,
    <urn:uuid:bbe073ad-f449-4b25-91ac-7d919613ca51>,
    <urn:uuid:1b457bed-8a80-4135-92b8-fdea12b4eea3>,
    <urn:uuid:2153d83b-8555-44a3-96e0-821b6663a188>,
    <urn:uuid:49ac68c4-922c-4d9e-88fa-b318fc54d36f>,
    <urn:uuid:4bbcdde6-ed53-4f8d-b3f8-43f800fd05d5>;
  skos:prefLabel "colour palette"@en;
  skos:related <urn:uuid:b8565dd1-8c4d-4699-a240-56898fc32ac8> .

<urn:uuid:d699bb4d-d9ea-4bb4-a411-a88caf6c908c> a skos:Concept;
  dct:created "2019-02-19T21:07:19Z"^^xsd:dateTime;
  dct:creator <urn:uuid:ca637d4b-c11b-4152-be98-bde602e7abd4>;
  skos:broader <urn:uuid:f352a521-b78e-478e-b01d-3a68638025a4>,
    <urn:uuid:fe500c7a-b458-4d2c-8b3a-efd1bb47d106>;
  skos:definition "The XML (and first) concrete syntax for RDF."@en;
  skos:inScheme <urn:uuid:2df6fac6-3122-44dc-9f92-5caab7f9b10b>,
    <urn:uuid:bbe073ad-f449-4b25-91ac-7d919613ca51>,
    <urn:uuid:1b457bed-8a80-4135-92b8-fdea12b4eea3>,
    <urn:uuid:2153d83b-8555-44a3-96e0-821b6663a188>,
    <urn:uuid:75f35368-e228-47fe-8efd-7251a2bde816>,
    <urn:uuid:4bbcdde6-ed53-4f8d-b3f8-43f800fd05d5>;
  skos:prefLabel "RDF/XML"@en .

<urn:uuid:de9fc67d-9b45-49e1-ae41-a7d3a3fc3a0b> a skos:Concept;
  dct:created "2022-11-24T02:18:42Z"^^xsd:dateTime;
  dct:creator <urn:uuid:ca637d4b-c11b-4152-be98-bde602e7abd4>;
  skos:broader <urn:uuid:87cc031a-dab5-41cb-8c86-5225565a0534>;
  skos:definition "A Web template is typically some kind of domain-specific language (and instances thereof) that provides instructions for attaching presentation markup to structural markup."@en;
  skos:inScheme <urn:uuid:1b457bed-8a80-4135-92b8-fdea12b4eea3>,
    <urn:uuid:2153d83b-8555-44a3-96e0-821b6663a188>,
    <urn:uuid:bbe073ad-f449-4b25-91ac-7d919613ca51>,
    <urn:uuid:0c7028f0-8226-47b3-acff-a4e83e6a60fd>,
    <urn:uuid:4bbcdde6-ed53-4f8d-b3f8-43f800fd05d5>;
  skos:prefLabel "Web template"@en;
  skos:related <urn:uuid:b99ffccd-0042-4e5a-a4ce-b58cbdcf3ef9>,
    <urn:uuid:df3de73d-3cb1-4b82-8773-415f1f16cbda> .

<urn:uuid:dfa100f0-2633-400f-911f-b8c3d46d8afa> a skos:Concept;
  dct:created "2019-02-28T21:09:41Z"^^xsd:dateTime;
  dct:creator <urn:uuid:ca637d4b-c11b-4152-be98-bde602e7abd4>;
  skos:broader <urn:uuid:56742b17-2be3-4fbe-bd6f-a1ff1c884fc4>,
    <urn:uuid:fe500c7a-b458-4d2c-8b3a-efd1bb47d106>;
  skos:definition "Notation 3 is a terse, easy-to-type RDF syntax with an additional facility for expressing inference rules. N3 is a superset of  Turtle."@en;
  skos:inScheme <urn:uuid:75f35368-e228-47fe-8efd-7251a2bde816>,
    <urn:uuid:1b457bed-8a80-4135-92b8-fdea12b4eea3>,
    <urn:uuid:2153d83b-8555-44a3-96e0-821b6663a188>,
    <urn:uuid:2df6fac6-3122-44dc-9f92-5caab7f9b10b>,
    <urn:uuid:bbe073ad-f449-4b25-91ac-7d919613ca51>,
    <urn:uuid:4bbcdde6-ed53-4f8d-b3f8-43f800fd05d5>;
  skos:prefLabel "N3"@en .

<urn:uuid:e4aa3ece-2759-4abc-acf5-3cd79d3cffe4> a skos:Concept;
  dct:created "2022-10-27T04:47:06Z"^^xsd:dateTime;
  dct:creator <urn:uuid:ca637d4b-c11b-4152-be98-bde602e7abd4>;
  skos:inScheme <urn:uuid:1b457bed-8a80-4135-92b8-fdea12b4eea3>,
    <urn:uuid:2153d83b-8555-44a3-96e0-821b6663a188>,
    <urn:uuid:2df6fac6-3122-44dc-9f92-5caab7f9b10b>,
    <urn:uuid:bbe073ad-f449-4b25-91ac-7d919613ca51>,
    <urn:uuid:4bbcdde6-ed53-4f8d-b3f8-43f800fd05d5>;
  skos:prefLabel "file system"@en;
  skos:related <urn:uuid:4f4aa0ac-c1b4-4a15-a6f3-518419d5b771> .

<urn:uuid:e4f3ac1e-7ece-4b85-a6df-6a8dc75bf359> a skos:Concept;
  dct:created "2024-07-25T15:19:18Z"^^xsd:dateTime,
    "2020-04-26T15:10:48Z"^^xsd:dateTime,
    "2024-02-16T15:24:23Z"^^xsd:dateTime,
    "2024-07-03T21:27:51Z"^^xsd:dateTime,
    "2022-11-03T14:13:13Z"^^xsd:dateTime;
  dct:creator <urn:uuid:ca637d4b-c11b-4152-be98-bde602e7abd4>;
  skos:definition "Structured argumentation is a form of (potentially collaborative) reasoning and persuasion that takes place in a formal system with a constrained repertoire of operations."@en;
  skos:inScheme <urn:uuid:a1a01f1c-7162-439c-94f1-3e28b99ae8ab>,
    <urn:uuid:ddfaaacc-9dcb-451b-afa6-477e6e787a5c>,
    <urn:uuid:1b457bed-8a80-4135-92b8-fdea12b4eea3>,
    <urn:uuid:2153d83b-8555-44a3-96e0-821b6663a188>,
    <urn:uuid:d4317ece-d4aa-40cb-9df1-1b058cbc24d8>,
    <urn:uuid:bbe073ad-f449-4b25-91ac-7d919613ca51>,
    <urn:uuid:0c7028f0-8226-47b3-acff-a4e83e6a60fd>,
    <urn:uuid:2df6fac6-3122-44dc-9f92-5caab7f9b10b>,
    <urn:uuid:4bbcdde6-ed53-4f8d-b3f8-43f800fd05d5>;
  skos:narrower <urn:uuid:d360bc19-f1e8-4550-aef4-9f84cc236cc5>,
    <urn:uuid:b95d0656-3b14-4e38-8fe2-75401ff7ee31>;
  skos:prefLabel "structured argumentation"@en .

<urn:uuid:e5f494f7-d0ae-486a-aa3c-f718a4041aa6> a skos:Concept;
  dct:created "2017-02-20T02:44:39Z"^^xsd:dateTime;
  dct:creator <urn:uuid:ca637d4b-c11b-4152-be98-bde602e7abd4>;
  skos:broader <urn:uuid:3a2c72e0-4fa5-4477-a51b-d7f073cc1155>;
  skos:definition "A legend is a mapping between a set of entities and a set of features in a map or data visualization. Often the legend relates the entities to a set of colours."@en;
  skos:inScheme <urn:uuid:1b457bed-8a80-4135-92b8-fdea12b4eea3>,
    <urn:uuid:2153d83b-8555-44a3-96e0-821b6663a188>,
    <urn:uuid:49ac68c4-922c-4d9e-88fa-b318fc54d36f>,
    <urn:uuid:bbe073ad-f449-4b25-91ac-7d919613ca51>,
    <urn:uuid:2df6fac6-3122-44dc-9f92-5caab7f9b10b>,
    <urn:uuid:4bbcdde6-ed53-4f8d-b3f8-43f800fd05d5>;
  skos:prefLabel "legend"@en .

<urn:uuid:eb4a3743-44e7-467b-88e0-24946953ce0f> a skos:Concept;
  dct:created "2022-11-24T01:06:42Z"^^xsd:dateTime;
  dct:creator <urn:uuid:ca637d4b-c11b-4152-be98-bde602e7abd4>;
  skos:definition "SRE is the (often dedicated) function of keeping large sites online."@en;
  skos:inScheme <urn:uuid:1b457bed-8a80-4135-92b8-fdea12b4eea3>,
    <urn:uuid:2153d83b-8555-44a3-96e0-821b6663a188>,
    <urn:uuid:bbe073ad-f449-4b25-91ac-7d919613ca51>,
    <urn:uuid:4bbcdde6-ed53-4f8d-b3f8-43f800fd05d5>;
  skos:prefLabel "site reliability engineering"@en;
  skos:related <urn:uuid:22c5c553-d574-4bf7-9a4d-13e70afa7f1c> .

<urn:uuid:ee5f9189-0ef2-461a-9557-ffe2fc095231> a skos:Concept;
  dct:created "2021-12-14T22:52:45Z"^^xsd:dateTime;
  dct:creator <urn:uuid:ca637d4b-c11b-4152-be98-bde602e7abd4>;
  skos:broader <urn:uuid:fdb43f70-cb11-49dd-aba6-7011b05ad61a>;
  skos:definition "Static code analysis involves parsing software code out to AST and tracing the various references throughout. It less resource-intensive and less dangerous (when the code is not trusted) but ultimately less powerful than generating a call graph, because it only identifies code that may be run (and even then potentially not even all of it), instead of code that actually is run."@en;
  skos:inScheme <urn:uuid:797e83d7-a86f-4838-b5c5-0ec20855197d>,
    <urn:uuid:1b457bed-8a80-4135-92b8-fdea12b4eea3>,
    <urn:uuid:2153d83b-8555-44a3-96e0-821b6663a188>,
    <urn:uuid:bbe073ad-f449-4b25-91ac-7d919613ca51>,
    <urn:uuid:2df6fac6-3122-44dc-9f92-5caab7f9b10b>,
    <urn:uuid:4bbcdde6-ed53-4f8d-b3f8-43f800fd05d5>;
  skos:prefLabel "static analysis"@en;
  skos:related <urn:uuid:5495f814-fd98-4b43-aba3-9e63a2063fd5> .

<urn:uuid:00ae5130-bb3f-478b-b97a-e868c8bb17d8> a skos:Concept;
  dct:created "2019-03-04T06:05:29Z"^^xsd:dateTime;
  dct:creator <urn:uuid:ca637d4b-c11b-4152-be98-bde602e7abd4>;
  skos:definition "As the saying goes, a monad is a monoid in the category of endofunctors."@en;
  skos:inScheme <urn:uuid:bbe073ad-f449-4b25-91ac-7d919613ca51>,
    <urn:uuid:75f35368-e228-47fe-8efd-7251a2bde816>,
    <urn:uuid:2df6fac6-3122-44dc-9f92-5caab7f9b10b>,
    <urn:uuid:1b457bed-8a80-4135-92b8-fdea12b4eea3>,
    <urn:uuid:2153d83b-8555-44a3-96e0-821b6663a188>,
    <urn:uuid:4bbcdde6-ed53-4f8d-b3f8-43f800fd05d5>;
  skos:prefLabel "monad"@en .

<urn:uuid:0112333a-e647-4f8a-9b23-2f3861ed079d> a skos:Concept;
  dct:created "2022-06-02T02:18:47Z"^^xsd:dateTime;
  dct:creator <urn:uuid:ca637d4b-c11b-4152-be98-bde602e7abd4>;
  rdfs:seeAlso <https://doriantaylor.com/the-specificity-gradient>;
  skos:definition "A specificity gradient is a conceptual framework that organizes the concerns of an endeavour from an \"outside-in\" perspective, and from coarser to finer detail, which has the side effect of also being largely organized in terms of its sensitivity to time."@en,
    "A specificity gradient is the idea that a conceptual structure can be organized by increasing detail and specificity, from plain language to highly specialized concepts, until they can ultimately be operated over by a computer."@en;
  skos:inScheme <urn:uuid:2df6fac6-3122-44dc-9f92-5caab7f9b10b>,
    <urn:uuid:bbe073ad-f449-4b25-91ac-7d919613ca51>,
    <urn:uuid:a1a01f1c-7162-439c-94f1-3e28b99ae8ab>,
    <urn:uuid:ddfaaacc-9dcb-451b-afa6-477e6e787a5c>,
    <urn:uuid:1b457bed-8a80-4135-92b8-fdea12b4eea3>,
    <urn:uuid:2153d83b-8555-44a3-96e0-821b6663a188>,
    <urn:uuid:abcac1e5-2fe0-4b40-9418-5bc3b62e7d04>,
    <urn:uuid:0c7028f0-8226-47b3-acff-a4e83e6a60fd>,
    <urn:uuid:4bbcdde6-ed53-4f8d-b3f8-43f800fd05d5>;
  skos:prefLabel "specificity gradient"@en;
  skos:related <urn:uuid:c757c1ac-1ec6-4bdd-a35d-85f1d85728bb>,
    <urn:uuid:b097ff77-48cb-4b65-a433-a4aac8abe2ee> .

<urn:uuid:03618f78-d09e-44d1-9149-c6cbebadd9b2> a skos:Concept;
  dct:created "2017-07-10T00:31:46Z"^^xsd:dateTime;
  dct:creator <urn:uuid:ca637d4b-c11b-4152-be98-bde602e7abd4>;
  skos:definition "Enterprise taxonomy software is purpose-made for designing and managing categories of (e.g.) products within an organization."@en;
  skos:inScheme <urn:uuid:75f35368-e228-47fe-8efd-7251a2bde816>,
    <urn:uuid:bbe073ad-f449-4b25-91ac-7d919613ca51>,
    <urn:uuid:2df6fac6-3122-44dc-9f92-5caab7f9b10b>,
    <urn:uuid:91684d49-7b99-4b2e-9641-ea0b8e22f66c>,
    <urn:uuid:1b457bed-8a80-4135-92b8-fdea12b4eea3>,
    <urn:uuid:2153d83b-8555-44a3-96e0-821b6663a188>,
    <urn:uuid:4bbcdde6-ed53-4f8d-b3f8-43f800fd05d5>;
  skos:prefLabel "taxonomy software"@en;
  skos:related <urn:uuid:a382bb78-d3d3-4b6a-b37b-0215c580e55a>,
    <urn:uuid:45b6c768-da32-4e5f-9c87-a18d5ec94635>,
    <urn:uuid:61c0c9c3-4d91-4509-902a-db09c4188ae5> .

<urn:uuid:06f69b4c-ce8b-42ea-b0cb-7f52f233b592> a skos:Concept;
  dct:created "2019-03-02T00:46:23Z"^^xsd:dateTime;
  dct:creator <urn:uuid:ca637d4b-c11b-4152-be98-bde602e7abd4>;
  skos:definition "Sandboxing is the act of creating a hermetic execution environment for a software program, with the aim of limiting its access to resources, or otherwise controlling its behaviour. Sandboxing is a necessary step for handling Turing-complete languages whose behaviour is unknown and potentially untrustworthy, such as any JavaScript downloaded from the internet."@en;
  skos:inScheme <urn:uuid:bbe073ad-f449-4b25-91ac-7d919613ca51>,
    <urn:uuid:75f35368-e228-47fe-8efd-7251a2bde816>,
    <urn:uuid:2df6fac6-3122-44dc-9f92-5caab7f9b10b>,
    <urn:uuid:1b457bed-8a80-4135-92b8-fdea12b4eea3>,
    <urn:uuid:2153d83b-8555-44a3-96e0-821b6663a188>,
    <urn:uuid:4bbcdde6-ed53-4f8d-b3f8-43f800fd05d5>;
  skos:prefLabel "sandboxing"@en;
  skos:related <urn:uuid:4e296fcb-0a17-4397-970b-11e8813f7883> .

<urn:uuid:081b467a-a40d-4028-9b8c-f2adc43eaefb> a skos:Concept;
  dct:created "2021-12-14T20:59:42Z"^^xsd:dateTime;
  dct:creator <urn:uuid:ca637d4b-c11b-4152-be98-bde602e7abd4>;
  skos:broader <urn:uuid:6c18acc3-3119-4f0b-8d24-0ca0ea9449d3>;
  skos:definition "A slug is a string of text used as an identifier, typically without any whitespace. The term is derived from hot metal typesetting."@en;
  skos:hiddenLabel "slugs"@en;
  skos:inScheme <urn:uuid:797e83d7-a86f-4838-b5c5-0ec20855197d>,
    <urn:uuid:bbe073ad-f449-4b25-91ac-7d919613ca51>,
    <urn:uuid:2df6fac6-3122-44dc-9f92-5caab7f9b10b>,
    <urn:uuid:1b457bed-8a80-4135-92b8-fdea12b4eea3>,
    <urn:uuid:2153d83b-8555-44a3-96e0-821b6663a188>,
    <urn:uuid:4bbcdde6-ed53-4f8d-b3f8-43f800fd05d5>;
  skos:prefLabel "slug"@en;
  skos:related <urn:uuid:648c3266-e8a9-4d4b-9c3d-25b6611a93b4>,
    <urn:uuid:ea81d3fd-8cd6-4321-81c0-c4c5299f5844> .

<urn:uuid:0a78b646-9c66-479f-a327-25e670be8c72> a skos:Concept;
  dct:created "2021-12-14T23:40:08Z"^^xsd:dateTime;
  dct:creator <urn:uuid:ca637d4b-c11b-4152-be98-bde602e7abd4>;
  skos:broader <urn:uuid:d2089ee2-d605-43ac-af18-ffbb7151a32d>;
  skos:definition "A user flow is one discrete process undertaken by a user, mediated by a product, to achieve a particular goal."@en;
  skos:hiddenLabel "user flows"@en;
  skos:inScheme <urn:uuid:bbe073ad-f449-4b25-91ac-7d919613ca51>,
    <urn:uuid:797e83d7-a86f-4838-b5c5-0ec20855197d>,
    <urn:uuid:2df6fac6-3122-44dc-9f92-5caab7f9b10b>,
    <urn:uuid:1b457bed-8a80-4135-92b8-fdea12b4eea3>,
    <urn:uuid:2153d83b-8555-44a3-96e0-821b6663a188>,
    <urn:uuid:4bbcdde6-ed53-4f8d-b3f8-43f800fd05d5>;
  skos:prefLabel "user flow"@en;
  skos:related <urn:uuid:0a78b646-9c66-479f-a327-25e670be8c72> .

<urn:uuid:0b356e36-b115-4c86-890b-8b05850a125b> a skos:Concept;
  dct:created "2019-03-02T05:11:19Z"^^xsd:dateTime;
  dct:creator <urn:uuid:ca637d4b-c11b-4152-be98-bde602e7abd4>;
  skos:altLabel "Scalable Vector Graphics"@en;
  skos:definition "Scalable Vector Graphics is an XML vocabulary for doing what it says on the tin."@en;
  skos:inScheme <urn:uuid:bbe073ad-f449-4b25-91ac-7d919613ca51>,
    <urn:uuid:75f35368-e228-47fe-8efd-7251a2bde816>,
    <urn:uuid:2df6fac6-3122-44dc-9f92-5caab7f9b10b>,
    <urn:uuid:1b457bed-8a80-4135-92b8-fdea12b4eea3>,
    <urn:uuid:2153d83b-8555-44a3-96e0-821b6663a188>,
    <urn:uuid:4bbcdde6-ed53-4f8d-b3f8-43f800fd05d5>;
  skos:prefLabel "SVG"@en .

<urn:uuid:0f6e28e8-8a36-49f8-94d4-c681609d448f> a skos:Concept;
  dct:created "2021-12-14T16:32:16Z"^^xsd:dateTime;
  dct:creator <urn:uuid:ca637d4b-c11b-4152-be98-bde602e7abd4>;
  skos:altLabel "CDN"@en;
  skos:broader <urn:uuid:0cf51602-4fc1-4a38-9663-d47aff228b2d>,
    <urn:uuid:637cfc93-b88b-4bfb-8f7c-2f9e72e27b86>;
  skos:definition "A content delivery network is a fancy caching (plain or reverse) proxy. These networked information services enhance the speed and reliability of websites by putting their hardware physically closer to clients. Requests to the origin (in reverse proxy configuration) or media assets like images or video (in either configuration) are served through the network from the system deemed closest to the client, even if the origin is unavailable."@en;
  skos:hiddenLabel "Content delivery networks"@en,
    "content delivery networks"@en;
  skos:inScheme <urn:uuid:2df6fac6-3122-44dc-9f92-5caab7f9b10b>,
    <urn:uuid:a1a01f1c-7162-439c-94f1-3e28b99ae8ab>,
    <urn:uuid:ddfaaacc-9dcb-451b-afa6-477e6e787a5c>,
    <urn:uuid:797e83d7-a86f-4838-b5c5-0ec20855197d>,
    <urn:uuid:bbe073ad-f449-4b25-91ac-7d919613ca51>,
    <urn:uuid:0c7028f0-8226-47b3-acff-a4e83e6a60fd>,
    <urn:uuid:1b457bed-8a80-4135-92b8-fdea12b4eea3>,
    <urn:uuid:2153d83b-8555-44a3-96e0-821b6663a188>,
    <urn:uuid:4bbcdde6-ed53-4f8d-b3f8-43f800fd05d5>;
  skos:prefLabel "content delivery network"@en;
  skos:related <urn:uuid:be93cce1-f21f-4e85-bd34-e005dea3532f>,
    <urn:uuid:2fd3adcc-1e66-48a5-a375-06992d6fc02b>,
    <urn:uuid:53819af5-c2d0-4edc-9add-ab79829ace96> .

<urn:uuid:117ac161-9f62-4075-8ac5-9a4e7f09fd1d> a skos:Concept;
  dct:created "2022-11-23T23:18:07Z"^^xsd:dateTime;
  dct:creator <urn:uuid:ca637d4b-c11b-4152-be98-bde602e7abd4>;
  skos:altLabel "composable"@en;
  skos:definition "Composability is the ability to connect two functions together to create another function. This necessitates that the output of one function is of the same type as the input of the other, which is implicit in a unified interface."@en;
  skos:inScheme <urn:uuid:1b457bed-8a80-4135-92b8-fdea12b4eea3>,
    <urn:uuid:2153d83b-8555-44a3-96e0-821b6663a188>,
    <urn:uuid:bbe073ad-f449-4b25-91ac-7d919613ca51>,
    <urn:uuid:0c7028f0-8226-47b3-acff-a4e83e6a60fd>,
    <urn:uuid:4bbcdde6-ed53-4f8d-b3f8-43f800fd05d5>;
  skos:prefLabel "composability"@en .

<urn:uuid:132303c5-7f8e-48c0-a680-c282386ba909> a skos:Concept;
  dct:created "2019-03-06T05:49:57Z"^^xsd:dateTime;
  dct:creator <urn:uuid:ca637d4b-c11b-4152-be98-bde602e7abd4>;
  skos:broader <urn:uuid:42747b64-a41c-4321-96cf-c49e711733e6>;
  skos:definition "After a content inventory, the elements are audited for fitness, correctness, relevance, style, etc., and recommendations are made for amendments, replacements, or supplements."@en;
  skos:inScheme <urn:uuid:1b457bed-8a80-4135-92b8-fdea12b4eea3>,
    <urn:uuid:2153d83b-8555-44a3-96e0-821b6663a188>,
    <urn:uuid:bbe073ad-f449-4b25-91ac-7d919613ca51>,
    <urn:uuid:75f35368-e228-47fe-8efd-7251a2bde816>,
    <urn:uuid:2df6fac6-3122-44dc-9f92-5caab7f9b10b>,
    <urn:uuid:4bbcdde6-ed53-4f8d-b3f8-43f800fd05d5>;
  skos:prefLabel "content audit"@en .

<urn:uuid:1417392d-ce8c-4357-8d38-8570258da6a6> a skos:Concept;
  dct:created "2021-12-14T01:15:53Z"^^xsd:dateTime;
  dct:creator <urn:uuid:ca637d4b-c11b-4152-be98-bde602e7abd4>;
  skos:broader <urn:uuid:193a84ec-ef96-44b9-b356-6f6b1c6ec979>;
  skos:definition "A reverse proxy is an intermediary between a client and an origin that has been arranged to operate without explicit attention to its existence. In general the difference between a proxy and a reverse proxy is that the former has been explicitly accessed while the latter is implicit."@en;
  skos:hiddenLabel "reverse proxies"@en,
    "reverse-proxied"@en;
  skos:inScheme <urn:uuid:1b457bed-8a80-4135-92b8-fdea12b4eea3>,
    <urn:uuid:2153d83b-8555-44a3-96e0-821b6663a188>,
    <urn:uuid:2df6fac6-3122-44dc-9f92-5caab7f9b10b>,
    <urn:uuid:0c7028f0-8226-47b3-acff-a4e83e6a60fd>,
    <urn:uuid:797e83d7-a86f-4838-b5c5-0ec20855197d>,
    <urn:uuid:bbe073ad-f449-4b25-91ac-7d919613ca51>,
    <urn:uuid:4bbcdde6-ed53-4f8d-b3f8-43f800fd05d5>;
  skos:narrower <urn:uuid:c38fdbb2-201b-4a88-9273-26fbd0c6fae5>;
  skos:prefLabel "reverse proxy"@en .

<urn:uuid:162516dc-6817-4d47-b4a7-6939c14c0fbb> a skos:Concept;
  dct:created "2017-02-01T23:00:47Z"^^xsd:dateTime;
  dct:creator <urn:uuid:ca637d4b-c11b-4152-be98-bde602e7abd4>;
  dct:modified "2019-02-02T19:07:08Z"^^xsd:dateTime;
  skos:broader <urn:uuid:16d17f33-394d-4d0b-a882-81e8fc3a52fe>;
  skos:definition "Dense hypermedia is a style of hypermedia where the entities are small, and the links that connect them together are numerous. Contrast this with ordinary hypermedia, where entities are large and the links are sparse. A benefit of dense hypermedia is the ability to communicate complex concepts, structures, and the relationships between them."@en,
    """Dense Hypermedia is a style of Hypermedia where the entities are small, and the links that connect them together are numerous.
Contrast this with ordinary Hypermedia, where entities are large and the links are sparse.
A benefit of Dense Hypermedia is the ability to communicate complex concepts, structures, and relationships between concepts and structures."""@en,
    """Dense Hypermedia is a style of Hypermedia where the entities are small, and the links that connect them together are numerous.
Contrast this with ordinary Hypermedia, where entities are large and the links are sparse.
A benefit of Dense Hypermedia is the ability to communicate complex concepts, structures, and relationships between concepts and structures."""@en;
  skos:inScheme <urn:uuid:1b457bed-8a80-4135-92b8-fdea12b4eea3>,
    <urn:uuid:2153d83b-8555-44a3-96e0-821b6663a188>,
    <urn:uuid:49ac68c4-922c-4d9e-88fa-b318fc54d36f>,
    <urn:uuid:bbe073ad-f449-4b25-91ac-7d919613ca51>,
    <urn:uuid:2df6fac6-3122-44dc-9f92-5caab7f9b10b>,
    <urn:uuid:a1a01f1c-7162-439c-94f1-3e28b99ae8ab>,
    <urn:uuid:ddfaaacc-9dcb-451b-afa6-477e6e787a5c>,
    <urn:uuid:4bbcdde6-ed53-4f8d-b3f8-43f800fd05d5>;
  skos:prefLabel "dense hypermedia"@en;
  skos:related <urn:uuid:b801e469-101d-4305-866d-edb0f70979de> .

<urn:uuid:1709ffb5-bbee-40cf-86c3-030f47ff1be7> a skos:Concept;
  dct:created "2022-11-24T00:14:02Z"^^xsd:dateTime;
  dct:creator <urn:uuid:ca637d4b-c11b-4152-be98-bde602e7abd4>;
  skos:altLabel "computability"@en,
    "computable"@en,
    "machine-actionability"@en;
  skos:definition "When a piece of content is machine-actionable (computable), it means that either is or contains formal syntax and semantics that can be directly accessed by a computer program without any additional processing or interpretation."@en;
  skos:inScheme <urn:uuid:1b457bed-8a80-4135-92b8-fdea12b4eea3>,
    <urn:uuid:2153d83b-8555-44a3-96e0-821b6663a188>,
    <urn:uuid:0c7028f0-8226-47b3-acff-a4e83e6a60fd>,
    <urn:uuid:9f98d1d7-745f-47bc-a361-f6b4fe352fbc>,
    <urn:uuid:a1a01f1c-7162-439c-94f1-3e28b99ae8ab>,
    <urn:uuid:ddfaaacc-9dcb-451b-afa6-477e6e787a5c>,
    <urn:uuid:4ec7530b-5536-4fb7-bb5a-45a3f5fddc22>,
    <urn:uuid:bbe073ad-f449-4b25-91ac-7d919613ca51>,
    <urn:uuid:4bbcdde6-ed53-4f8d-b3f8-43f800fd05d5>;
  skos:prefLabel "machine-actionable"@en;
  skos:related <urn:uuid:c757c1ac-1ec6-4bdd-a35d-85f1d85728bb> .

<urn:uuid:1b496cb8-fb39-4b54-ab88-a9663f419bc4> a skos:Concept;
  dct:created "2019-03-04T05:13:41Z"^^xsd:dateTime;
  dct:creator <urn:uuid:ca637d4b-c11b-4152-be98-bde602e7abd4>;
  skos:broader <urn:uuid:33c3211f-322b-4f7a-83f6-63aa617461c3>,
    <urn:uuid:e827d9af-be73-4918-89aa-a296872be199>;
  skos:definition "C++ is an object-oriented extension of C (indeed its own distinct language) by Bjarne Stroustrup. It is said to be like creating an octopus by nailing extra legs on a dog. Popular in game development and with Windows."@en;
  skos:inScheme <urn:uuid:1b457bed-8a80-4135-92b8-fdea12b4eea3>,
    <urn:uuid:2153d83b-8555-44a3-96e0-821b6663a188>,
    <urn:uuid:75f35368-e228-47fe-8efd-7251a2bde816>,
    <urn:uuid:bbe073ad-f449-4b25-91ac-7d919613ca51>,
    <urn:uuid:2df6fac6-3122-44dc-9f92-5caab7f9b10b>,
    <urn:uuid:4bbcdde6-ed53-4f8d-b3f8-43f800fd05d5>;
  skos:prefLabel "C++"@en .

<urn:uuid:1d5cbcc6-63b1-4817-97fa-c979859cf41a> a skos:Concept;
  dct:created "2019-03-03T01:09:50Z"^^xsd:dateTime;
  dct:creator <urn:uuid:ca637d4b-c11b-4152-be98-bde602e7abd4>;
  skos:definition "The Java Virtual Machine can refer to either the specification for, or an implementation of, the virtual machine that runs Java."@en;
  skos:inScheme <urn:uuid:1b457bed-8a80-4135-92b8-fdea12b4eea3>,
    <urn:uuid:2153d83b-8555-44a3-96e0-821b6663a188>,
    <urn:uuid:75f35368-e228-47fe-8efd-7251a2bde816>,
    <urn:uuid:bbe073ad-f449-4b25-91ac-7d919613ca51>,
    <urn:uuid:2df6fac6-3122-44dc-9f92-5caab7f9b10b>,
    <urn:uuid:4bbcdde6-ed53-4f8d-b3f8-43f800fd05d5>;
  skos:prefLabel "JVM"@en;
  skos:related <urn:uuid:855fce21-5560-4ff3-87bf-ef26a28958c4> .

<urn:uuid:1f5fb4c8-4d43-46d6-a205-0339c1b0289e> a skos:Concept;
  dct:created "2019-03-05T23:10:44Z"^^xsd:dateTime;
  dct:creator <urn:uuid:ca637d4b-c11b-4152-be98-bde602e7abd4>;
  skos:broader <urn:uuid:9767147a-1b6a-440c-949f-7f6056e28411>,
    <urn:uuid:bf986385-65ff-424e-8eb1-6c6653cb6b4e>;
  skos:definition "In the general sense, a data structure definition is exactly what it says it is. In the specific sense, it is a particular class in the RDF Data Cube Vocabulary that determines which columns go in a prototypical tabular dataset, and (optionally) in what order."@en;
  skos:inScheme <urn:uuid:1b457bed-8a80-4135-92b8-fdea12b4eea3>,
    <urn:uuid:2153d83b-8555-44a3-96e0-821b6663a188>,
    <urn:uuid:75f35368-e228-47fe-8efd-7251a2bde816>,
    <urn:uuid:bbe073ad-f449-4b25-91ac-7d919613ca51>,
    <urn:uuid:2df6fac6-3122-44dc-9f92-5caab7f9b10b>,
    <urn:uuid:4bbcdde6-ed53-4f8d-b3f8-43f800fd05d5>;
  skos:prefLabel "Data Structure Definition"@en .

<urn:uuid:1f7f1c54-a1d2-453c-87a7-4439a7b6037d> a skos:Concept;
  dct:created "2017-06-08T21:44:44Z"^^xsd:dateTime;
  dct:creator <urn:uuid:ca637d4b-c11b-4152-be98-bde602e7abd4>;
  skos:broader <urn:uuid:4039a99d-c14b-40f2-84d5-4ec72e2217e1>;
  skos:definition "A parametric (information) resource can be thought of as a single logical resource that yields one or more distinct representations based on supplied parameters. In this way it is very much like a (mathematical) function."@en;
  skos:inScheme <urn:uuid:49ac68c4-922c-4d9e-88fa-b318fc54d36f>,
    <urn:uuid:1b457bed-8a80-4135-92b8-fdea12b4eea3>,
    <urn:uuid:2153d83b-8555-44a3-96e0-821b6663a188>,
    <urn:uuid:bbe073ad-f449-4b25-91ac-7d919613ca51>,
    <urn:uuid:2df6fac6-3122-44dc-9f92-5caab7f9b10b>,
    <urn:uuid:4bbcdde6-ed53-4f8d-b3f8-43f800fd05d5>;
  skos:narrower <urn:uuid:fdb190cf-9f79-4c98-b65a-688b00e4f8d3>;
  skos:prefLabel "parametric resource"@en .

<urn:uuid:21d69225-b92a-4440-83a0-62a386451283> a skos:Concept;
  dct:alternative "CSV is the venerable backstop data format for semi-structured data on the Internet, since anything that can be represented in CSV can also be represented in Excel (although not the other way around)."@en;
  dct:created "2017-07-13T18:51:30Z"^^xsd:dateTime;
  dct:creator <urn:uuid:ca637d4b-c11b-4152-be98-bde602e7abd4>;
  dct:description "CSV is the venerable backstop data format for semi-structured data on the Internet, since anything that can be represented in CSV can also be represented in Excel (although not the other way around)."@en;
  dct:modified "2021-12-14T03:22:54Z"^^xsd:dateTime;
  dct:references <https://tools.ietf.org/html/rfc4180>;
  skos:altLabel "CSV"@en;
  skos:broader <urn:uuid:027543f6-04df-4e92-96f4-5b0c8da4b799>,
    <urn:uuid:75b4da00-36b5-467e-bc90-966a7e5256a1>,
    <urn:uuid:8d46494e-5316-43b7-a49e-a625ab716a38>;
  skos:definition "Comma-Separated Values (CSV) is an interchange format for tabular data. It is represented as a text file or network message wherein each line is treated as a record, separated (canonically) by the comma \",\" character. The first record in the file may optionally depict column semantics."@en;
  skos:inScheme <urn:uuid:75f35368-e228-47fe-8efd-7251a2bde816>,
    <urn:uuid:1b457bed-8a80-4135-92b8-fdea12b4eea3>,
    <urn:uuid:2153d83b-8555-44a3-96e0-821b6663a188>,
    <urn:uuid:797e83d7-a86f-4838-b5c5-0ec20855197d>,
    <urn:uuid:bbe073ad-f449-4b25-91ac-7d919613ca51>,
    <urn:uuid:2df6fac6-3122-44dc-9f92-5caab7f9b10b>,
    <urn:uuid:91684d49-7b99-4b2e-9641-ea0b8e22f66c>,
    <urn:uuid:4bbcdde6-ed53-4f8d-b3f8-43f800fd05d5>;
  skos:prefLabel "comma-separated values"@en .

<urn:uuid:23ae24d6-80b8-4f31-8510-562c45871694> a skos:Concept;
  dct:created "2021-12-14T19:12:16Z"^^xsd:dateTime;
  dct:creator <urn:uuid:ca637d4b-c11b-4152-be98-bde602e7abd4>;
  skos:broader <urn:uuid:aa5f9563-e527-4df2-8518-ce325819f1e6>,
    <urn:uuid:fdb43f70-cb11-49dd-aba6-7011b05ad61a>;
  skos:definition "A software framework is a library and set of tools for creating software, generally encodes the opinions of its authors, and tends to be incompatible with other frameworks."@en;
  skos:inScheme <urn:uuid:1b457bed-8a80-4135-92b8-fdea12b4eea3>,
    <urn:uuid:2153d83b-8555-44a3-96e0-821b6663a188>,
    <urn:uuid:bbe073ad-f449-4b25-91ac-7d919613ca51>,
    <urn:uuid:797e83d7-a86f-4838-b5c5-0ec20855197d>,
    <urn:uuid:2df6fac6-3122-44dc-9f92-5caab7f9b10b>,
    <urn:uuid:4bbcdde6-ed53-4f8d-b3f8-43f800fd05d5>;
  skos:prefLabel "framework"@en .

<urn:uuid:262057b5-cdb6-4148-823e-a63fd5d10268> a skos:Concept;
  dct:created "2019-03-03T09:25:26Z"^^xsd:dateTime;
  dct:creator <urn:uuid:ca637d4b-c11b-4152-be98-bde602e7abd4>;
  skos:altLabel "ORM"@en;
  skos:broader <urn:uuid:e840ba8a-4c6d-4be3-a673-dd6620463a39>;
  skos:definition "An object-relational mapper is a software library that abstracts SQL interactions under an object-oriented interface. From the point of view of the programmer it's just another API in the native language, no messing about generating SQL query strings or parsing result sets."@en;
  skos:inScheme <urn:uuid:75f35368-e228-47fe-8efd-7251a2bde816>,
    <urn:uuid:1b457bed-8a80-4135-92b8-fdea12b4eea3>,
    <urn:uuid:2153d83b-8555-44a3-96e0-821b6663a188>,
    <urn:uuid:bbe073ad-f449-4b25-91ac-7d919613ca51>,
    <urn:uuid:2df6fac6-3122-44dc-9f92-5caab7f9b10b>,
    <urn:uuid:4bbcdde6-ed53-4f8d-b3f8-43f800fd05d5>;
  skos:prefLabel "object-relational mapper"@en .

<urn:uuid:27a05aeb-017c-484d-b490-c6949e6eacbc> a skos:Concept;
  dct:created "2021-12-14T23:31:41Z"^^xsd:dateTime;
  dct:creator <urn:uuid:ca637d4b-c11b-4152-be98-bde602e7abd4>;
  skos:altLabel "UUID"@en,
    "Universally Unique Identifier"@en;
  skos:definition "The UUID is a 128-(actually 122, after you remove the control bits)-bit identifier that is particularly useful for naming things when you don't want to spend time coming up with a name for them. By various mechanisms, not the least of which being their size, UUIDs are all but guaranteed to be unique. Hence the name."@en;
  skos:hiddenLabel "universally unique identifier"@en;
  skos:inScheme <urn:uuid:2df6fac6-3122-44dc-9f92-5caab7f9b10b>,
    <urn:uuid:1b457bed-8a80-4135-92b8-fdea12b4eea3>,
    <urn:uuid:2153d83b-8555-44a3-96e0-821b6663a188>,
    <urn:uuid:a1a01f1c-7162-439c-94f1-3e28b99ae8ab>,
    <urn:uuid:ddfaaacc-9dcb-451b-afa6-477e6e787a5c>,
    <urn:uuid:0c7028f0-8226-47b3-acff-a4e83e6a60fd>,
    <urn:uuid:797e83d7-a86f-4838-b5c5-0ec20855197d>,
    <urn:uuid:bbe073ad-f449-4b25-91ac-7d919613ca51>,
    <urn:uuid:4bbcdde6-ed53-4f8d-b3f8-43f800fd05d5>;
  skos:prefLabel "Universally Unique Identifier"@en .

<urn:uuid:295da6bb-7246-431c-b508-196207ab168b> a skos:Concept;
  dct:created "2022-12-07T05:40:04Z"^^xsd:dateTime;
  dct:creator <urn:uuid:ca637d4b-c11b-4152-be98-bde602e7abd4>;
  skos:definition "We haven't forgotten about Chorus."@en;
  skos:hiddenLabel "Chorus"@en;
  skos:inScheme <urn:uuid:0c7028f0-8226-47b3-acff-a4e83e6a60fd>,
    <urn:uuid:bbe073ad-f449-4b25-91ac-7d919613ca51>,
    <urn:uuid:4bbcdde6-ed53-4f8d-b3f8-43f800fd05d5>;
  skos:prefLabel "Chorus (CMS)"@en .

<urn:uuid:29883b00-2202-4684-887d-8077fa0eecc2> a skos:Concept;
  dct:created "2019-03-01T19:50:22Z"^^xsd:dateTime;
  dct:creator <urn:uuid:ca637d4b-c11b-4152-be98-bde602e7abd4>;
  skos:broader <urn:uuid:0bc0aabb-9d9e-4caa-b9c8-553dd8b3ee05>;
  skos:definition "Microdata refers to a set of attributes in HTML 5, distinct from and incompatible with RDFa, that provide some functionality for embedding metadata."@en;
  skos:inScheme <urn:uuid:2df6fac6-3122-44dc-9f92-5caab7f9b10b>,
    <urn:uuid:75f35368-e228-47fe-8efd-7251a2bde816>,
    <urn:uuid:1b457bed-8a80-4135-92b8-fdea12b4eea3>,
    <urn:uuid:2153d83b-8555-44a3-96e0-821b6663a188>,
    <urn:uuid:bbe073ad-f449-4b25-91ac-7d919613ca51>,
    <urn:uuid:4bbcdde6-ed53-4f8d-b3f8-43f800fd05d5>;
  skos:prefLabel "microdata"@en;
  skos:related <urn:uuid:7a81818d-e347-4b40-814d-d1e98a0bc102>,
    <urn:uuid:7b7c4ecf-2544-4c03-ab5f-10de5e1a20d4>,
    <urn:uuid:a91fff32-d160-4cc0-86eb-e78d778a1526>,
    <urn:uuid:f3f67e45-9cdf-4df1-9586-834ba185f63b> .

<urn:uuid:2bd3be3c-a234-4cf5-be07-2f770e08b48b> a skos:Concept;
  dct:created "2022-06-02T02:24:33Z"^^xsd:dateTime;
  dct:creator <urn:uuid:ca637d4b-c11b-4152-be98-bde602e7abd4>;
  skos:definition "\"Pace layers\" is a conceptual framework advanced by the writer Stewart Brand, taking Duffy's concept of shearing layers and applying them to the societal scale."@en;
  skos:inScheme <urn:uuid:abcac1e5-2fe0-4b40-9418-5bc3b62e7d04>,
    <urn:uuid:2df6fac6-3122-44dc-9f92-5caab7f9b10b>,
    <urn:uuid:1b457bed-8a80-4135-92b8-fdea12b4eea3>,
    <urn:uuid:2153d83b-8555-44a3-96e0-821b6663a188>,
    <urn:uuid:bbe073ad-f449-4b25-91ac-7d919613ca51>,
    <urn:uuid:4bbcdde6-ed53-4f8d-b3f8-43f800fd05d5>;
  skos:prefLabel "pace layers"@en;
  skos:related <urn:uuid:561fb472-4c33-400e-bfc4-895b7284fd84> .

<urn:uuid:2d6d3a0f-8888-4d01-8178-bf5bad91a5b6> a skos:Concept;
  dct:created "2019-03-02T05:37:22Z"^^xsd:dateTime;
  dct:creator <urn:uuid:ca637d4b-c11b-4152-be98-bde602e7abd4>;
  skos:definition "Create, Read, Update, Delete are the four basic operations of a database or data-driven application."@en;
  skos:inScheme <urn:uuid:2df6fac6-3122-44dc-9f92-5caab7f9b10b>,
    <urn:uuid:75f35368-e228-47fe-8efd-7251a2bde816>,
    <urn:uuid:bbe073ad-f449-4b25-91ac-7d919613ca51>,
    <urn:uuid:1b457bed-8a80-4135-92b8-fdea12b4eea3>,
    <urn:uuid:2153d83b-8555-44a3-96e0-821b6663a188>,
    <urn:uuid:4bbcdde6-ed53-4f8d-b3f8-43f800fd05d5>;
  skos:prefLabel "CRUD"@en;
  skos:related <urn:uuid:e840ba8a-4c6d-4be3-a673-dd6620463a39> .

<urn:uuid:2dc3da5b-9325-4c28-8609-2b9118ce3028> a skos:Concept;
  dct:created "2019-03-02T00:03:07Z"^^xsd:dateTime;
  dct:creator <urn:uuid:ca637d4b-c11b-4152-be98-bde602e7abd4>;
  skos:broader <urn:uuid:e840ba8a-4c6d-4be3-a673-dd6620463a39>;
  skos:definition "GraphQL is a query language designed at Facebook for remote procedure calls over HTTP."@en;
  skos:inScheme <urn:uuid:2df6fac6-3122-44dc-9f92-5caab7f9b10b>,
    <urn:uuid:75f35368-e228-47fe-8efd-7251a2bde816>,
    <urn:uuid:bbe073ad-f449-4b25-91ac-7d919613ca51>,
    <urn:uuid:1b457bed-8a80-4135-92b8-fdea12b4eea3>,
    <urn:uuid:2153d83b-8555-44a3-96e0-821b6663a188>,
    <urn:uuid:4bbcdde6-ed53-4f8d-b3f8-43f800fd05d5>;
  skos:prefLabel "GraphQL"@en .

<urn:uuid:32092336-fb45-4598-851e-fd3dbffb1dca> a skos:Concept;
  dct:created "2019-03-02T06:49:15Z"^^xsd:dateTime;
  dct:creator <urn:uuid:ca637d4b-c11b-4152-be98-bde602e7abd4>;
  skos:definition "The Shape Constraints Language is a mechanism for expressing integrity constraints in RDF data."@en;
  skos:inScheme <urn:uuid:2df6fac6-3122-44dc-9f92-5caab7f9b10b>,
    <urn:uuid:75f35368-e228-47fe-8efd-7251a2bde816>,
    <urn:uuid:bbe073ad-f449-4b25-91ac-7d919613ca51>,
    <urn:uuid:1b457bed-8a80-4135-92b8-fdea12b4eea3>,
    <urn:uuid:2153d83b-8555-44a3-96e0-821b6663a188>,
    <urn:uuid:a1a01f1c-7162-439c-94f1-3e28b99ae8ab>,
    <urn:uuid:ddfaaacc-9dcb-451b-afa6-477e6e787a5c>,
    <urn:uuid:4bbcdde6-ed53-4f8d-b3f8-43f800fd05d5>;
  skos:prefLabel "SHACL"@en;
  skos:related <urn:uuid:ed4d30d7-d3cf-4b21-bcb4-5f2525027be7> .

<urn:uuid:35ec7a5f-aa2c-4876-bc77-161ebd0a3405> a skos:Concept;
  dct:created "2021-12-14T22:57:20Z"^^xsd:dateTime;
  dct:creator <urn:uuid:ca637d4b-c11b-4152-be98-bde602e7abd4>;
  skos:broader <urn:uuid:da4d162d-c124-43be-a7e7-0ec463f4b32c>;
  skos:definition "In the version control system Git, a submodule is a separate Git repository that is linked to the one in context. Other version control systems exhibit analogous features, though they may go by different names."@en;
  skos:hiddenLabel "Sub-modules"@en,
    "sub-module"@en,
    "submodules"@en;
  skos:inScheme <urn:uuid:2df6fac6-3122-44dc-9f92-5caab7f9b10b>,
    <urn:uuid:797e83d7-a86f-4838-b5c5-0ec20855197d>,
    <urn:uuid:1b457bed-8a80-4135-92b8-fdea12b4eea3>,
    <urn:uuid:2153d83b-8555-44a3-96e0-821b6663a188>,
    <urn:uuid:bbe073ad-f449-4b25-91ac-7d919613ca51>,
    <urn:uuid:4bbcdde6-ed53-4f8d-b3f8-43f800fd05d5>;
  skos:prefLabel "submodule"@en .

<urn:uuid:37810612-aecc-49b8-9df0-bc1255fa214a> a skos:Concept;
  dct:created "2022-12-02T10:12:30Z"^^xsd:dateTime;
  dct:creator <urn:uuid:ca637d4b-c11b-4152-be98-bde602e7abd4>;
  skos:altLabel "canonical representation"@en;
  skos:definition "An information resource may have multiple representations, but the canonical representation is the \"master\" one, and usually the one that you store. Canonicalization can also be the result of a function, where grammars with some play in the representation are brought into one with the same semantic content as the original, but a literal representation (i.e., an exact string of bits) suitable for comparison (as with identifiers), or cryptographic identity (as with larger blobs)."@en;
  skos:hiddenLabel "canonicalize"@en;
  skos:inScheme <urn:uuid:0c7028f0-8226-47b3-acff-a4e83e6a60fd>,
    <urn:uuid:bbe073ad-f449-4b25-91ac-7d919613ca51>,
    <urn:uuid:a1a01f1c-7162-439c-94f1-3e28b99ae8ab>,
    <urn:uuid:ddfaaacc-9dcb-451b-afa6-477e6e787a5c>,
    <urn:uuid:1b457bed-8a80-4135-92b8-fdea12b4eea3>,
    <urn:uuid:2153d83b-8555-44a3-96e0-821b6663a188>,
    <urn:uuid:4bbcdde6-ed53-4f8d-b3f8-43f800fd05d5>;
  skos:prefLabel "canonicalization"@en;
  skos:related <urn:uuid:027543f6-04df-4e92-96f4-5b0c8da4b799>,
    <urn:uuid:6c18acc3-3119-4f0b-8d24-0ca0ea9449d3> .

<urn:uuid:3a978497-8980-4695-a316-cb9c66740c49> a skos:Concept;
  dct:created "2022-11-23T23:05:18Z"^^xsd:dateTime;
  dct:creator <urn:uuid:ca637d4b-c11b-4152-be98-bde602e7abd4>;
  skos:definition "A markup transform differs from an asset transform in that it operates over markup, and often adds information (such as presentation markup) or composes multiple resources together, rather than strictly isomorphic or lossy transformations."@en;
  skos:inScheme <urn:uuid:0c7028f0-8226-47b3-acff-a4e83e6a60fd>,
    <urn:uuid:bbe073ad-f449-4b25-91ac-7d919613ca51>,
    <urn:uuid:1b457bed-8a80-4135-92b8-fdea12b4eea3>,
    <urn:uuid:2153d83b-8555-44a3-96e0-821b6663a188>,
    <urn:uuid:4bbcdde6-ed53-4f8d-b3f8-43f800fd05d5>;
  skos:prefLabel "markup transform"@en;
  skos:related <urn:uuid:453f3a1b-7631-4943-a924-33b1455c3de2> .

<urn:uuid:3e511aba-c593-4b5c-8b10-e60fbd6f3809> a skos:Concept;
  dct:created "2021-12-14T15:47:43Z"^^xsd:dateTime;
  dct:creator <urn:uuid:ca637d4b-c11b-4152-be98-bde602e7abd4>;
  skos:broader <urn:uuid:da4d162d-c124-43be-a7e7-0ec463f4b32c>;
  skos:definition "In software version control, a commit is both an event that represents the advancement of the representational state of the content under management, as well as the record of that state. The changes between one commit and another can be represented as a diff."@en;
  skos:inScheme <urn:uuid:1b457bed-8a80-4135-92b8-fdea12b4eea3>,
    <urn:uuid:2153d83b-8555-44a3-96e0-821b6663a188>,
    <urn:uuid:797e83d7-a86f-4838-b5c5-0ec20855197d>,
    <urn:uuid:2df6fac6-3122-44dc-9f92-5caab7f9b10b>,
    <urn:uuid:bbe073ad-f449-4b25-91ac-7d919613ca51>,
    <urn:uuid:4bbcdde6-ed53-4f8d-b3f8-43f800fd05d5>;
  skos:prefLabel "commit (noun)"@en;
  skos:related <urn:uuid:6e63f013-3c43-49d9-a92e-dbff4aa6550b> .

<urn:uuid:4333e98e-4565-4d4e-b600-d7cc9e95a972> a skos:Concept;
  dct:created "2021-12-14T21:18:40Z"^^xsd:dateTime;
  dct:creator <urn:uuid:ca637d4b-c11b-4152-be98-bde602e7abd4>;
  skos:broader <urn:uuid:aa5f9563-e527-4df2-8518-ce325819f1e6>,
    <urn:uuid:fdb43f70-cb11-49dd-aba6-7011b05ad61a>;
  skos:definition "The other PR is a process pioneered by GitHub (and quickly copied by its competitors) to formalize the process of collaborative software development. The applicant opens a pull request against the maintainer's code repository with their proposed changes, and the latter can review and accept it (or not)."@en;
  skos:inScheme <urn:uuid:1b457bed-8a80-4135-92b8-fdea12b4eea3>,
    <urn:uuid:2153d83b-8555-44a3-96e0-821b6663a188>,
    <urn:uuid:2df6fac6-3122-44dc-9f92-5caab7f9b10b>,
    <urn:uuid:797e83d7-a86f-4838-b5c5-0ec20855197d>,
    <urn:uuid:bbe073ad-f449-4b25-91ac-7d919613ca51>,
    <urn:uuid:4bbcdde6-ed53-4f8d-b3f8-43f800fd05d5>;
  skos:prefLabel "pull request"@en .

<urn:uuid:43649147-ce57-43fe-a960-3b4e71b8686f> a skos:Concept;
  dct:created "2017-02-20T02:57:36Z"^^xsd:dateTime;
  dct:creator <urn:uuid:ca637d4b-c11b-4152-be98-bde602e7abd4>;
  dct:references <https://en.wikipedia.org/wiki/Arithmetic_mean>,
    <https://en.wikipedia.org/wiki/Descriptive_statistics>,
    <https://en.wikipedia.org/wiki/Five-number_summary>,
    <https://en.wikipedia.org/wiki/Standard_deviation>;
  skos:definition "Descriptive statistics are a way to get a sense of the \"shape\" of data which is already quantitative. On this project, we take the term to mean the five-number summary { sample minimum, first quartile, median, third quartile, sample maximum }, plus the average (arithmetic mean) and standard deviation."@en;
  skos:inScheme <urn:uuid:1b457bed-8a80-4135-92b8-fdea12b4eea3>,
    <urn:uuid:2153d83b-8555-44a3-96e0-821b6663a188>,
    <urn:uuid:49ac68c4-922c-4d9e-88fa-b318fc54d36f>,
    <urn:uuid:2df6fac6-3122-44dc-9f92-5caab7f9b10b>,
    <urn:uuid:bbe073ad-f449-4b25-91ac-7d919613ca51>,
    <urn:uuid:4bbcdde6-ed53-4f8d-b3f8-43f800fd05d5>;
  skos:narrower <urn:uuid:7c821c59-a03c-4757-93b8-2a2595e92dbb>;
  skos:prefLabel "descriptive statistics"@en .

<urn:uuid:4a6202a6-b159-4a2b-860a-08efc38e93f1> a skos:Concept;
  dct:created "2019-03-02T06:18:51Z"^^xsd:dateTime;
  dct:creator <urn:uuid:ca637d4b-c11b-4152-be98-bde602e7abd4>;
  skos:broader <urn:uuid:c0e969c3-4528-4968-8418-d5fe609c2a62>;
  skos:definition "WebID is a protocol that weds RDF to X.509, embedding links to the former in client certificates of the latter. A server looking to identify a client can access the link and download profile information, as well as a round-trip verification of the identity of the client."@en;
  skos:inScheme <urn:uuid:bbe073ad-f449-4b25-91ac-7d919613ca51>,
    <urn:uuid:1b457bed-8a80-4135-92b8-fdea12b4eea3>,
    <urn:uuid:2153d83b-8555-44a3-96e0-821b6663a188>,
    <urn:uuid:2df6fac6-3122-44dc-9f92-5caab7f9b10b>,
    <urn:uuid:75f35368-e228-47fe-8efd-7251a2bde816>,
    <urn:uuid:4bbcdde6-ed53-4f8d-b3f8-43f800fd05d5>;
  skos:prefLabel "WebID"@en .

<urn:uuid:4af8a4cc-c12b-47aa-8ab2-d15a74907aa3> a skos:Concept;
  dct:alternative "The Semantic Web refers to the use of (although conceivably not exclusively) RDF to represent structured data on the Web, with user agents performing automated reasoning and inference operations. The vision for the Semantic Web is the decentralization of services currently performed by aggregators such as Google, Facebook, Amazon, etc."@en;
  dct:created "2017-07-12T04:33:53Z"^^xsd:dateTime;
  dct:creator <urn:uuid:ca637d4b-c11b-4152-be98-bde602e7abd4>;
  dct:description "The Semantic Web refers to the use of (although conceivably not exclusively) RDF to represent structured data on the Web, with user agents performing automated reasoning and inference operations. The vision for the Semantic Web is the decentralization of services currently performed by aggregators such as Google, Facebook, Amazon, etc."@en;
  dct:modified "2019-10-13T00:24:20Z"^^xsd:dateTime,
    "2021-12-14T22:35:34Z"^^xsd:dateTime;
  skos:altLabel "Semantic Web"@en;
  skos:definition "The Semantic Web refers to the use of (although conceivably not exclusively) RDF to represent structured data on the Web, with user agents performing automated reasoning and inference operations. The vision for the Semantic Web is the decentralization of services currently performed by aggregators such as Google, Facebook, Amazon, etc."@en,
    "The Semantic Web is an unrealized and likely unrealizable utopia of decentralized linked data systems with smart agents performing inferencing over information they find on the Web. It nevertheless boasts a raft of very useful technologies for everyday practical applications."@en;
  skos:inScheme <urn:uuid:bbe073ad-f449-4b25-91ac-7d919613ca51>,
    <urn:uuid:1b457bed-8a80-4135-92b8-fdea12b4eea3>,
    <urn:uuid:2153d83b-8555-44a3-96e0-821b6663a188>,
    <urn:uuid:2df6fac6-3122-44dc-9f92-5caab7f9b10b>,
    <urn:uuid:75f35368-e228-47fe-8efd-7251a2bde816>,
    <urn:uuid:91684d49-7b99-4b2e-9641-ea0b8e22f66c>,
    <urn:uuid:797e83d7-a86f-4838-b5c5-0ec20855197d>,
    <urn:uuid:4bbcdde6-ed53-4f8d-b3f8-43f800fd05d5>;
  skos:prefLabel "Semantic Web"@en;
  skos:related <urn:uuid:fe500c7a-b458-4d2c-8b3a-efd1bb47d106>,
    <urn:uuid:f3f67e45-9cdf-4df1-9586-834ba185f63b>,
    <urn:uuid:7b7c4ecf-2544-4c03-ab5f-10de5e1a20d4> .

<urn:uuid:4c034864-ee75-4ca7-b93f-119152b11796> a skos:Concept;
  dct:created "2019-02-28T19:03:06Z"^^xsd:dateTime;
  dct:creator <urn:uuid:ca637d4b-c11b-4152-be98-bde602e7abd4>;
  skos:broader <urn:uuid:f352a521-b78e-478e-b01d-3a68638025a4>;
  skos:definition "Atom (RFC 4287) is an XML format for syndication feeds, which supersedes RSS 2.0."@en;
  skos:inScheme <urn:uuid:bbe073ad-f449-4b25-91ac-7d919613ca51>,
    <urn:uuid:1b457bed-8a80-4135-92b8-fdea12b4eea3>,
    <urn:uuid:2153d83b-8555-44a3-96e0-821b6663a188>,
    <urn:uuid:2df6fac6-3122-44dc-9f92-5caab7f9b10b>,
    <urn:uuid:75f35368-e228-47fe-8efd-7251a2bde816>,
    <urn:uuid:4bbcdde6-ed53-4f8d-b3f8-43f800fd05d5>;
  skos:prefLabel "Atom"@en;
  skos:related <urn:uuid:9ed8a948-df9f-4ee3-95d1-47b28174b6a8>,
    <urn:uuid:ba2258e3-efca-4461-82cc-f6ebbf980b36> .

<urn:uuid:4cb1625a-5157-48a4-8140-47fcb14fb8fd> a skos:Concept;
  dct:created "2021-12-14T19:15:22Z"^^xsd:dateTime;
  dct:creator <urn:uuid:ca637d4b-c11b-4152-be98-bde602e7abd4>;
  skos:definition "In software development parlance, the front-end typically refers to the code used to power the user interface. On the Web, this term is synonymous with JavaScript."@en;
  skos:inScheme <urn:uuid:797e83d7-a86f-4838-b5c5-0ec20855197d>,
    <urn:uuid:bbe073ad-f449-4b25-91ac-7d919613ca51>,
    <urn:uuid:1b457bed-8a80-4135-92b8-fdea12b4eea3>,
    <urn:uuid:2153d83b-8555-44a3-96e0-821b6663a188>,
    <urn:uuid:2df6fac6-3122-44dc-9f92-5caab7f9b10b>,
    <urn:uuid:4bbcdde6-ed53-4f8d-b3f8-43f800fd05d5>;
  skos:narrower <urn:uuid:ee2371bb-d9a0-4ee8-a35b-f4e0d9458f02>;
  skos:prefLabel "front-end"@en .

<urn:uuid:4e8865ba-1a0f-4ce4-86fd-b7871c41f259> a skos:Concept;
  dct:created "2022-11-23T23:33:42Z"^^xsd:dateTime;
  dct:creator <urn:uuid:ca637d4b-c11b-4152-be98-bde602e7abd4>;
  skos:definition "Containerization is a strategy for packaging and deploying virtual servers such that they can be rapidly cloned and deployed to utility computing systems (i.e., \"the cloud\")."@en;
  skos:hiddenLabel "containerize"@en,
    "containerized"@en;
  skos:inScheme <urn:uuid:bbe073ad-f449-4b25-91ac-7d919613ca51>,
    <urn:uuid:1b457bed-8a80-4135-92b8-fdea12b4eea3>,
    <urn:uuid:2153d83b-8555-44a3-96e0-821b6663a188>,
    <urn:uuid:0c7028f0-8226-47b3-acff-a4e83e6a60fd>,
    <urn:uuid:4bbcdde6-ed53-4f8d-b3f8-43f800fd05d5>;
  skos:prefLabel "containerization"@en .

<urn:uuid:4ee503d1-1f0d-457a-bcd1-51383d77b068> a skos:Concept;
  dct:created "2019-02-28T06:45:12Z"^^xsd:dateTime;
  dct:creator <urn:uuid:ca637d4b-c11b-4152-be98-bde602e7abd4>;
  skos:definition "XML Schema is the consummately baroque syntax definition specification for XML, intended to replace the senescent DTD, that was resisted tooth and nail until it was supplanted by Relax NG. The only thing that remains of XML Schema with any currency is its second volume, on literal datatypes (which is actually essential)."@en;
  skos:inScheme <urn:uuid:bbe073ad-f449-4b25-91ac-7d919613ca51>,
    <urn:uuid:1b457bed-8a80-4135-92b8-fdea12b4eea3>,
    <urn:uuid:2153d83b-8555-44a3-96e0-821b6663a188>,
    <urn:uuid:2df6fac6-3122-44dc-9f92-5caab7f9b10b>,
    <urn:uuid:75f35368-e228-47fe-8efd-7251a2bde816>,
    <urn:uuid:4bbcdde6-ed53-4f8d-b3f8-43f800fd05d5>;
  skos:prefLabel "XML Schema"@en;
  skos:related <urn:uuid:d3cb15cf-cdad-4b05-ad72-aae158621f42> .

<urn:uuid:5162945a-0397-466c-9cd7-02552f893beb> a skos:Concept;
  dct:created "2018-03-12T19:46:12Z"^^xsd:dateTime;
  dct:creator <urn:uuid:ca637d4b-c11b-4152-be98-bde602e7abd4>;
  dct:references <https://www.w3.org/ns/activitystreams#>;
  skos:inScheme <urn:uuid:bbe073ad-f449-4b25-91ac-7d919613ca51>,
    <urn:uuid:1b457bed-8a80-4135-92b8-fdea12b4eea3>,
    <urn:uuid:2153d83b-8555-44a3-96e0-821b6663a188>,
    <urn:uuid:91684d49-7b99-4b2e-9641-ea0b8e22f66c>,
    <urn:uuid:2df6fac6-3122-44dc-9f92-5caab7f9b10b>,
    <urn:uuid:75f35368-e228-47fe-8efd-7251a2bde816>,
    <urn:uuid:4bbcdde6-ed53-4f8d-b3f8-43f800fd05d5>;
  skos:prefLabel "Activity Streams"@en .

<urn:uuid:525f262f-32e3-4c35-96d4-e9eb11e19370> a skos:Concept;
  dct:created "2021-12-14T23:09:43Z"^^xsd:dateTime;
  dct:creator <urn:uuid:ca637d4b-c11b-4152-be98-bde602e7abd4>;
  dct:description "A transform is a function that relates an input to an at least partially, if not completely isomorphic output. Transforms make very well-defined development targets."@en;
  dct:modified "2022-11-23T23:03:52Z"^^xsd:dateTime;
  skos:altLabel "transform"@en,
    "transformation function"@en;
  skos:broader <urn:uuid:cc74f8e0-34cc-4a69-b9d5-87b990aca6b6>;
  skos:definition "A transform is a pure function that operates over a segment of bytes and returns another segment of bytes. An example would be the gzip and gunzip functions. Not to be confused with the machine learning concept of a transformer."@en;
  skos:hiddenLabel "transforms"@en;
  skos:inScheme <urn:uuid:2df6fac6-3122-44dc-9f92-5caab7f9b10b>,
    <urn:uuid:1b457bed-8a80-4135-92b8-fdea12b4eea3>,
    <urn:uuid:2153d83b-8555-44a3-96e0-821b6663a188>,
    <urn:uuid:797e83d7-a86f-4838-b5c5-0ec20855197d>,
    <urn:uuid:bbe073ad-f449-4b25-91ac-7d919613ca51>,
    <urn:uuid:0c7028f0-8226-47b3-acff-a4e83e6a60fd>,
    <urn:uuid:4bbcdde6-ed53-4f8d-b3f8-43f800fd05d5>;
  skos:narrower <urn:uuid:3a978497-8980-4695-a316-cb9c66740c49>;
  skos:prefLabel "transform (noun)"@en;
  skos:related <urn:uuid:fdb43f70-cb11-49dd-aba6-7011b05ad61a>,
    <urn:uuid:aa5f9563-e527-4df2-8518-ce325819f1e6> .

<urn:uuid:561fb472-4c33-400e-bfc4-895b7284fd84> a skos:Concept;
  dct:created "2022-06-02T02:26:52Z"^^xsd:dateTime;
  dct:creator <urn:uuid:ca637d4b-c11b-4152-be98-bde602e7abd4>;
  skos:broader <urn:uuid:fb8ef397-b65d-4213-8483-4dee04d58eea>;
  skos:definition "Levels of Scale are one of the fifteen fundamental properties and transformations Christopher Alexander described in his magnum opus, The Nature of Order."@en;
  skos:inScheme <urn:uuid:abcac1e5-2fe0-4b40-9418-5bc3b62e7d04>,
    <urn:uuid:bbe073ad-f449-4b25-91ac-7d919613ca51>,
    <urn:uuid:1b457bed-8a80-4135-92b8-fdea12b4eea3>,
    <urn:uuid:2153d83b-8555-44a3-96e0-821b6663a188>,
    <urn:uuid:2df6fac6-3122-44dc-9f92-5caab7f9b10b>,
    <urn:uuid:4bbcdde6-ed53-4f8d-b3f8-43f800fd05d5>;
  skos:prefLabel "Levels of Scale"@en;
  skos:related <urn:uuid:0112333a-e647-4f8a-9b23-2f3861ed079d>,
    <urn:uuid:8d3a484a-17e3-49d3-a5a8-d3cac97c5836> .

<urn:uuid:56742b17-2be3-4fbe-bd6f-a1ff1c884fc4> a skos:Concept;
  dct:created "2019-02-28T21:11:27Z"^^xsd:dateTime;
  dct:creator <urn:uuid:ca637d4b-c11b-4152-be98-bde602e7abd4>;
  skos:broader <urn:uuid:fe500c7a-b458-4d2c-8b3a-efd1bb47d106>;
  skos:definition "Turtle is another terse RDF syntax that is basically N3 minus the inference rules."@en;
  skos:inScheme <urn:uuid:bbe073ad-f449-4b25-91ac-7d919613ca51>,
    <urn:uuid:1b457bed-8a80-4135-92b8-fdea12b4eea3>,
    <urn:uuid:2153d83b-8555-44a3-96e0-821b6663a188>,
    <urn:uuid:2df6fac6-3122-44dc-9f92-5caab7f9b10b>,
    <urn:uuid:75f35368-e228-47fe-8efd-7251a2bde816>,
    <urn:uuid:4bbcdde6-ed53-4f8d-b3f8-43f800fd05d5>;
  skos:prefLabel "Turtle"@en .

<urn:uuid:5dc8e476-6377-429e-865c-562c6454c8a6> a skos:Concept;
  dct:created "2019-03-02T00:06:27Z"^^xsd:dateTime;
  dct:creator <urn:uuid:ca637d4b-c11b-4152-be98-bde602e7abd4>;
  skos:broader <urn:uuid:ca632e87-50d2-4f1d-af83-f3d11e53eca8>;
  skos:definition "JSON Schema is an independent effort to ascribe integrity constraints and hypermedia semantics to JSON. It has a superficial resemblance to JSON-LD, and is about the same age, but is otherwise unrelated."@en;
  skos:inScheme <urn:uuid:75f35368-e228-47fe-8efd-7251a2bde816>,
    <urn:uuid:bbe073ad-f449-4b25-91ac-7d919613ca51>,
    <urn:uuid:1b457bed-8a80-4135-92b8-fdea12b4eea3>,
    <urn:uuid:2153d83b-8555-44a3-96e0-821b6663a188>,
    <urn:uuid:2df6fac6-3122-44dc-9f92-5caab7f9b10b>,
    <urn:uuid:4bbcdde6-ed53-4f8d-b3f8-43f800fd05d5>;
  skos:prefLabel "JSON Schema"@en;
  skos:related <urn:uuid:cda3a7a9-41bc-4de7-ad92-1b9093389c64> .

<urn:uuid:5e6006da-5f7b-4c01-919e-f0708346c727> a skos:Concept;
  dct:created "2019-03-02T06:07:53Z"^^xsd:dateTime;
  dct:creator <urn:uuid:ca637d4b-c11b-4152-be98-bde602e7abd4>;
  skos:broader <urn:uuid:c0e969c3-4528-4968-8418-d5fe609c2a62>,
    <urn:uuid:f0a7ece3-44e6-4f6b-963c-281ab8dff8e6>;
  skos:definition "OpenID Connect is an authentication protocol built on top of OAuth. It provides a standardized mechanism for verifying the identity of the user delegating the token."@en;
  skos:inScheme <urn:uuid:75f35368-e228-47fe-8efd-7251a2bde816>,
    <urn:uuid:bbe073ad-f449-4b25-91ac-7d919613ca51>,
    <urn:uuid:1b457bed-8a80-4135-92b8-fdea12b4eea3>,
    <urn:uuid:2153d83b-8555-44a3-96e0-821b6663a188>,
    <urn:uuid:2df6fac6-3122-44dc-9f92-5caab7f9b10b>,
    <urn:uuid:4bbcdde6-ed53-4f8d-b3f8-43f800fd05d5>;
  skos:prefLabel "OpenID Connect"@en .

<urn:uuid:5effc9c6-6843-4abc-8474-5e4002aa51cf> a skos:Concept;
  dct:created "2019-03-07T01:04:30Z"^^xsd:dateTime,
    "2018-04-26T22:51:11Z"^^xsd:dateTime,
    "2024-02-16T15:24:23Z"^^xsd:dateTime,
    "2022-11-03T14:13:13Z"^^xsd:dateTime;
  dct:creator <urn:uuid:ca637d4b-c11b-4152-be98-bde602e7abd4>;
  skos:inScheme <urn:uuid:75f35368-e228-47fe-8efd-7251a2bde816>,
    <urn:uuid:91684d49-7b99-4b2e-9641-ea0b8e22f66c>,
    <urn:uuid:bbe073ad-f449-4b25-91ac-7d919613ca51>,
    <urn:uuid:1b457bed-8a80-4135-92b8-fdea12b4eea3>,
    <urn:uuid:2153d83b-8555-44a3-96e0-821b6663a188>,
    <urn:uuid:2df6fac6-3122-44dc-9f92-5caab7f9b10b>,
    <urn:uuid:4bbcdde6-ed53-4f8d-b3f8-43f800fd05d5>;
  skos:prefLabel "presentation graphics"@en .

<urn:uuid:615a2418-14be-4a69-b669-14e9f8219e9c> a skos:Concept;
  dct:created "2022-11-03T14:13:13Z"^^xsd:dateTime,
    "2024-07-18T02:03:21Z"^^xsd:dateTime,
    "2024-02-16T15:24:23Z"^^xsd:dateTime,
    "2019-09-23T23:47:53Z"^^xsd:dateTime;
  dct:creator <urn:uuid:ca637d4b-c11b-4152-be98-bde602e7abd4>;
  skos:definition "Automation is the broad technical program that aims reduce the need for directy human attention on any given task. Automation can be understood as the maturation of mechanization, which only reduces physical labor."@en;
  skos:inScheme <urn:uuid:2df6fac6-3122-44dc-9f92-5caab7f9b10b>,
    <urn:uuid:a1a01f1c-7162-439c-94f1-3e28b99ae8ab>,
    <urn:uuid:ddfaaacc-9dcb-451b-afa6-477e6e787a5c>,
    <urn:uuid:bbe073ad-f449-4b25-91ac-7d919613ca51>,
    <urn:uuid:49ac68c4-922c-4d9e-88fa-b318fc54d36f>,
    <urn:uuid:1b457bed-8a80-4135-92b8-fdea12b4eea3>,
    <urn:uuid:2153d83b-8555-44a3-96e0-821b6663a188>,
    <urn:uuid:4bbcdde6-ed53-4f8d-b3f8-43f800fd05d5>;
  skos:prefLabel "automation"@en;
  skos:related <urn:uuid:f5a254ac-4a2b-405e-91be-7de9fbf7174d>,
    <urn:uuid:fdb43f70-cb11-49dd-aba6-7011b05ad61a> .

<urn:uuid:61a28be0-4688-4591-b633-b00ea2053b38> a skos:Concept;
  dct:created "2021-12-14T19:04:56Z"^^xsd:dateTime;
  dct:creator <urn:uuid:ca637d4b-c11b-4152-be98-bde602e7abd4>;
  skos:broader <urn:uuid:fdb43f70-cb11-49dd-aba6-7011b05ad61a>,
    <urn:uuid:aa5f9563-e527-4df2-8518-ce325819f1e6>;
  skos:definition "A format string is a convention in numerous programming languages where static text is interspersed with one or more predefined placeholder symbols, which are then substituted with data from the program."@en;
  skos:hiddenLabel "format strings"@en;
  skos:inScheme <urn:uuid:2df6fac6-3122-44dc-9f92-5caab7f9b10b>,
    <urn:uuid:797e83d7-a86f-4838-b5c5-0ec20855197d>,
    <urn:uuid:bbe073ad-f449-4b25-91ac-7d919613ca51>,
    <urn:uuid:1b457bed-8a80-4135-92b8-fdea12b4eea3>,
    <urn:uuid:2153d83b-8555-44a3-96e0-821b6663a188>,
    <urn:uuid:4bbcdde6-ed53-4f8d-b3f8-43f800fd05d5>;
  skos:prefLabel "format string"@en .

<urn:uuid:63a99f54-a4cf-487b-b217-083384522046> a skos:Concept;
  dct:created "2019-03-01T03:11:19Z"^^xsd:dateTime;
  dct:creator <urn:uuid:ca637d4b-c11b-4152-be98-bde602e7abd4>;
  skos:definition "A search engine is a company (and concomitant website) that helps people find other websites."@en;
  skos:inScheme <urn:uuid:2df6fac6-3122-44dc-9f92-5caab7f9b10b>,
    <urn:uuid:75f35368-e228-47fe-8efd-7251a2bde816>,
    <urn:uuid:bbe073ad-f449-4b25-91ac-7d919613ca51>,
    <urn:uuid:1b457bed-8a80-4135-92b8-fdea12b4eea3>,
    <urn:uuid:2153d83b-8555-44a3-96e0-821b6663a188>,
    <urn:uuid:0c7028f0-8226-47b3-acff-a4e83e6a60fd>,
    <urn:uuid:4bbcdde6-ed53-4f8d-b3f8-43f800fd05d5>;
  skos:prefLabel "search engine"@en .

<urn:uuid:648c3266-e8a9-4d4b-9c3d-25b6611a93b4> a skos:Concept;
  dct:created "2021-12-14T23:53:45Z"^^xsd:dateTime;
  dct:creator <urn:uuid:ca637d4b-c11b-4152-be98-bde602e7abd4>;
  skos:altLabel "white space"@en,
    "white-space"@en;
  skos:definition "In text processing, whitespace refers to the set of codepoints that are interpreted as breaks in the text. In graphic design, whitespace is the literal white (of the paper) space between elements on the page."@en;
  skos:inScheme <urn:uuid:2df6fac6-3122-44dc-9f92-5caab7f9b10b>,
    <urn:uuid:bbe073ad-f449-4b25-91ac-7d919613ca51>,
    <urn:uuid:797e83d7-a86f-4838-b5c5-0ec20855197d>,
    <urn:uuid:1b457bed-8a80-4135-92b8-fdea12b4eea3>,
    <urn:uuid:2153d83b-8555-44a3-96e0-821b6663a188>,
    <urn:uuid:4bbcdde6-ed53-4f8d-b3f8-43f800fd05d5>;
  skos:prefLabel "whitespace"@en;
  skos:related <urn:uuid:02dce02e-d62c-4243-9472-237b53262ac7> .

<urn:uuid:654c0fac-1eb1-4fd2-9139-b4a5f3e6d903> a skos:Concept;
  dct:created "2019-02-28T06:44:07Z"^^xsd:dateTime;
  dct:creator <urn:uuid:ca637d4b-c11b-4152-be98-bde602e7abd4>;
  skos:definition "Relax NG is a schema definition format for XML, which is considerably lighter-weight than XML Schema, and can be expressed using a compact syntax."@en;
  skos:inScheme <urn:uuid:2df6fac6-3122-44dc-9f92-5caab7f9b10b>,
    <urn:uuid:75f35368-e228-47fe-8efd-7251a2bde816>,
    <urn:uuid:bbe073ad-f449-4b25-91ac-7d919613ca51>,
    <urn:uuid:1b457bed-8a80-4135-92b8-fdea12b4eea3>,
    <urn:uuid:2153d83b-8555-44a3-96e0-821b6663a188>,
    <urn:uuid:4bbcdde6-ed53-4f8d-b3f8-43f800fd05d5>;
  skos:prefLabel "Relax NG"@en;
  skos:related <urn:uuid:4ee503d1-1f0d-457a-bcd1-51383d77b068> .

<urn:uuid:696cc8e6-8cc0-4e91-b410-97942abf883c> a skos:Concept;
  dct:created "2021-12-14T20:23:42Z"^^xsd:dateTime;
  dct:creator <urn:uuid:ca637d4b-c11b-4152-be98-bde602e7abd4>;
  skos:broader <urn:uuid:94cd1298-0889-401a-b567-f6181dfefcce>;
  skos:definition "A lambda can be understood as a receptacle and execution environment for a Web hook or microservice that is billed (by Amazon) on a per-use basis."@en;
  skos:hiddenLabel "lambda"@en,
    "lambdas"@en;
  skos:inScheme <urn:uuid:2df6fac6-3122-44dc-9f92-5caab7f9b10b>,
    <urn:uuid:bbe073ad-f449-4b25-91ac-7d919613ca51>,
    <urn:uuid:797e83d7-a86f-4838-b5c5-0ec20855197d>,
    <urn:uuid:1b457bed-8a80-4135-92b8-fdea12b4eea3>,
    <urn:uuid:2153d83b-8555-44a3-96e0-821b6663a188>,
    <urn:uuid:4bbcdde6-ed53-4f8d-b3f8-43f800fd05d5>;
  skos:prefLabel "Lambda (Amazon)"@en .

<urn:uuid:6d154e36-799a-4b7b-8e07-a6d3459d2fd7> a skos:Concept;
  dct:created "2019-03-04T02:36:28Z"^^xsd:dateTime;
  dct:creator <urn:uuid:ca637d4b-c11b-4152-be98-bde602e7abd4>;
  skos:altLabel "b-node"@en,
    "bnode"@en;
  skos:broader <urn:uuid:fe500c7a-b458-4d2c-8b3a-efd1bb47d106>;
  skos:definition "An RDF blank node is an anonymous entity which can only reliably be reached through its topological relationship with non-blank (i.e., URI) nodes."@en;
  skos:inScheme <urn:uuid:1b457bed-8a80-4135-92b8-fdea12b4eea3>,
    <urn:uuid:2153d83b-8555-44a3-96e0-821b6663a188>,
    <urn:uuid:75f35368-e228-47fe-8efd-7251a2bde816>,
    <urn:uuid:2df6fac6-3122-44dc-9f92-5caab7f9b10b>,
    <urn:uuid:bbe073ad-f449-4b25-91ac-7d919613ca51>,
    <urn:uuid:4bbcdde6-ed53-4f8d-b3f8-43f800fd05d5>;
  skos:prefLabel "blank node"@en;
  skos:related <urn:uuid:9e506ca3-8be1-431d-9075-548141d9f8c1>,
    <urn:uuid:de8a5f03-f936-4edb-b5c7-a9dcf00a4678> .

<urn:uuid:6e63f013-3c43-49d9-a92e-dbff4aa6550b> a skos:Concept;
  dct:created "2021-12-14T16:04:55Z"^^xsd:dateTime;
  dct:creator <urn:uuid:ca637d4b-c11b-4152-be98-bde602e7abd4>;
  skos:definition "A diff is an algorithmic attempt to represent the minimum set of changes between two streams of symbols. More colloquially, a diff is a text file containing changes between one or more other text files across time."@en;
  skos:hiddenLabel "diffs"@en;
  skos:inScheme <urn:uuid:1b457bed-8a80-4135-92b8-fdea12b4eea3>,
    <urn:uuid:2153d83b-8555-44a3-96e0-821b6663a188>,
    <urn:uuid:797e83d7-a86f-4838-b5c5-0ec20855197d>,
    <urn:uuid:2df6fac6-3122-44dc-9f92-5caab7f9b10b>,
    <urn:uuid:bbe073ad-f449-4b25-91ac-7d919613ca51>,
    <urn:uuid:4bbcdde6-ed53-4f8d-b3f8-43f800fd05d5>;
  skos:prefLabel "diff"@en .

<urn:uuid:76c47ecd-5507-495d-a14b-14e2f15c0955> a skos:Concept;
  dct:created "2021-12-14T21:32:02Z"^^xsd:dateTime,
    "2019-09-23T23:47:53Z"^^xsd:dateTime;
  dct:creator <urn:uuid:ca637d4b-c11b-4152-be98-bde602e7abd4>;
  skos:altLabel "relational database"@en;
  skos:broader <urn:uuid:4694ebe0-589f-40a7-9ef9-67872edb6214>,
    <urn:uuid:197982df-60a5-4c93-be50-2f8ede43b842>;
  skos:definition "A relational database is just another term for a database built on top of SQL."@en;
  skos:inScheme <urn:uuid:2df6fac6-3122-44dc-9f92-5caab7f9b10b>,
    <urn:uuid:1b457bed-8a80-4135-92b8-fdea12b4eea3>,
    <urn:uuid:2153d83b-8555-44a3-96e0-821b6663a188>,
    <urn:uuid:797e83d7-a86f-4838-b5c5-0ec20855197d>,
    <urn:uuid:49ac68c4-922c-4d9e-88fa-b318fc54d36f>,
    <urn:uuid:bbe073ad-f449-4b25-91ac-7d919613ca51>,
    <urn:uuid:4bbcdde6-ed53-4f8d-b3f8-43f800fd05d5>;
  skos:prefLabel "relational database"@en;
  skos:related <urn:uuid:fdb43f70-cb11-49dd-aba6-7011b05ad61a> .

<urn:uuid:7730f786-d46e-495d-a3bc-79d401599988> a skos:Concept;
  dct:created "2017-02-21T19:55:09Z"^^xsd:dateTime;
  dct:creator <urn:uuid:ca637d4b-c11b-4152-be98-bde602e7abd4>;
  skos:altLabel "user ID"@en,
    "user name"@en,
    "userid"@en;
  skos:broader <urn:uuid:d0d7da4b-4d4d-4262-96a3-a70afbc1a829>;
  skos:definition "A username (user name) is a token or identifier that represents the computer account of a person (or automated software agent)."@en;
  skos:inScheme <urn:uuid:1b457bed-8a80-4135-92b8-fdea12b4eea3>,
    <urn:uuid:2153d83b-8555-44a3-96e0-821b6663a188>,
    <urn:uuid:2df6fac6-3122-44dc-9f92-5caab7f9b10b>,
    <urn:uuid:bbe073ad-f449-4b25-91ac-7d919613ca51>,
    <urn:uuid:49ac68c4-922c-4d9e-88fa-b318fc54d36f>,
    <urn:uuid:4bbcdde6-ed53-4f8d-b3f8-43f800fd05d5>;
  skos:prefLabel "username"@en;
  skos:related <urn:uuid:d85e3c52-cc94-48a4-8dc5-591de86be52f> .

<urn:uuid:775a0b24-a8b3-4e74-989a-ed6f438122d3> a skos:Concept;
  dct:created "2022-11-23T23:43:48Z"^^xsd:dateTime;
  dct:creator <urn:uuid:ca637d4b-c11b-4152-be98-bde602e7abd4>;
  skos:altLabel "situational awareness"@en;
  skos:definition "Situation awareness is the state of being aware of one's surroundings, and the positions and momenta (real or imaginary) of the dynamics of the salient entities within one's environment."@en;
  skos:inScheme <urn:uuid:1b457bed-8a80-4135-92b8-fdea12b4eea3>,
    <urn:uuid:2153d83b-8555-44a3-96e0-821b6663a188>,
    <urn:uuid:bbe073ad-f449-4b25-91ac-7d919613ca51>,
    <urn:uuid:0c7028f0-8226-47b3-acff-a4e83e6a60fd>,
    <urn:uuid:4bbcdde6-ed53-4f8d-b3f8-43f800fd05d5>;
  skos:prefLabel "situation awareness"@en .

<urn:uuid:7a81818d-e347-4b40-814d-d1e98a0bc102> a skos:Concept;
  dct:created "2019-03-01T19:52:43Z"^^xsd:dateTime;
  dct:creator <urn:uuid:ca637d4b-c11b-4152-be98-bde602e7abd4>;
  skos:altLabel "Microformat";
  skos:broader <urn:uuid:0bc0aabb-9d9e-4caa-b9c8-553dd8b3ee05>,
    <urn:uuid:45373ede-a7b0-404f-b797-902298208993>;
  skos:definition "Microformats are an early ad-hoc strategy for embedding structured metadata into HTML, by punning standard elements and attributes. Microformats 2 has expanded and generalized this technique somewhat."@en;
  skos:inScheme <urn:uuid:75f35368-e228-47fe-8efd-7251a2bde816>,
    <urn:uuid:1b457bed-8a80-4135-92b8-fdea12b4eea3>,
    <urn:uuid:2153d83b-8555-44a3-96e0-821b6663a188>,
    <urn:uuid:2df6fac6-3122-44dc-9f92-5caab7f9b10b>,
    <urn:uuid:bbe073ad-f449-4b25-91ac-7d919613ca51>,
    <urn:uuid:4bbcdde6-ed53-4f8d-b3f8-43f800fd05d5>;
  skos:prefLabel "Microformats"@en;
  skos:related <urn:uuid:a91fff32-d160-4cc0-86eb-e78d778a1526> .

<urn:uuid:7c821c59-a03c-4757-93b8-2a2595e92dbb> a skos:Concept;
  dct:created "2017-02-20T02:57:50Z"^^xsd:dateTime;
  dct:creator <urn:uuid:ca637d4b-c11b-4152-be98-bde602e7abd4>;
  dct:references <https://en.wikipedia.org/wiki/Box_plot>;
  skos:broader <urn:uuid:3a2c72e0-4fa5-4477-a51b-d7f073cc1155>;
  skos:definition "A box plot is a way to visualize descriptive statistics."@en;
  skos:inScheme <urn:uuid:49ac68c4-922c-4d9e-88fa-b318fc54d36f>,
    <urn:uuid:1b457bed-8a80-4135-92b8-fdea12b4eea3>,
    <urn:uuid:2153d83b-8555-44a3-96e0-821b6663a188>,
    <urn:uuid:2df6fac6-3122-44dc-9f92-5caab7f9b10b>,
    <urn:uuid:bbe073ad-f449-4b25-91ac-7d919613ca51>,
    <urn:uuid:4bbcdde6-ed53-4f8d-b3f8-43f800fd05d5>;
  skos:prefLabel "box plot"@en .

<urn:uuid:81abc2b5-5ead-4549-bff2-f326c38f535c> a skos:Concept;
  dct:created "2017-02-09T17:40:10Z"^^xsd:dateTime;
  dct:creator <urn:uuid:ca637d4b-c11b-4152-be98-bde602e7abd4>;
  skos:definition "A server is a computer that provides services to multiple clients over a network. Aside from this, and the fact that it is typically made from more expensive parts, it is no different in principle from an ordinary desktop computer."@en;
  skos:inScheme <urn:uuid:49ac68c4-922c-4d9e-88fa-b318fc54d36f>,
    <urn:uuid:1b457bed-8a80-4135-92b8-fdea12b4eea3>,
    <urn:uuid:2153d83b-8555-44a3-96e0-821b6663a188>,
    <urn:uuid:2df6fac6-3122-44dc-9f92-5caab7f9b10b>,
    <urn:uuid:bbe073ad-f449-4b25-91ac-7d919613ca51>,
    <urn:uuid:4bbcdde6-ed53-4f8d-b3f8-43f800fd05d5>;
  skos:prefLabel "server"@en;
  skos:related <urn:uuid:76c47ecd-5507-495d-a14b-14e2f15c0955>,
    <urn:uuid:abadd9b5-844e-4982-8fbe-b6b83d43736d>,
    <urn:uuid:be93cce1-f21f-4e85-bd34-e005dea3532f>,
    <urn:uuid:ad6b1b9b-fec4-4378-b8dd-7bbc07a3d706> .

<urn:uuid:83c1c427-8523-4b51-bcb5-c4fdeb11e859> a skos:Concept;
  dct:created "2021-12-14T18:15:05Z"^^xsd:dateTime;
  dct:creator <urn:uuid:ca637d4b-c11b-4152-be98-bde602e7abd4>;
  skos:definition "A document fragment, colloquially, is what it sounds like, except in XML (and adjacent) parlance it takes on an additional specific meaning. That is, a document fragment consists of one or more nodes like text or markup elements (tags). Thus, a concrete representation (e.g. a file) of a document fragment would itself be valid markup, and not start or end in the middle of a tag. (XML documents go further and require exactly one root element.)"@en;
  skos:hiddenLabel "fragment"@en,
    "document fragments"@en;
  skos:inScheme <urn:uuid:797e83d7-a86f-4838-b5c5-0ec20855197d>,
    <urn:uuid:bbe073ad-f449-4b25-91ac-7d919613ca51>,
    <urn:uuid:1b457bed-8a80-4135-92b8-fdea12b4eea3>,
    <urn:uuid:2153d83b-8555-44a3-96e0-821b6663a188>,
    <urn:uuid:2df6fac6-3122-44dc-9f92-5caab7f9b10b>,
    <urn:uuid:0c7028f0-8226-47b3-acff-a4e83e6a60fd>,
    <urn:uuid:4bbcdde6-ed53-4f8d-b3f8-43f800fd05d5>;
  skos:prefLabel "document fragment"@en .

<urn:uuid:88465aec-782f-4aab-9d50-cc918cceaed5> a skos:Concept;
  dct:created "2021-12-14T17:52:39Z"^^xsd:dateTime;
  dct:creator <urn:uuid:ca637d4b-c11b-4152-be98-bde602e7abd4>;
  skos:definition "A corpus is a term used to refer to the totality of a body of content under consideration. A content inventory, for instance, would describe a corpus. Corpus is just Latin for body, and tends to be useful to disambiguate when there are a number of different bodies around."@en,
    "A corpus is a term used to refer to the totality of a body of content under consideration. A content inventory, for instance, would describe a corpus. Corpus is just Latin for “body”, and tends to be useful to disambiguate when there are a number of different bodies around."@en;
  skos:inScheme <urn:uuid:2df6fac6-3122-44dc-9f92-5caab7f9b10b>,
    <urn:uuid:1b457bed-8a80-4135-92b8-fdea12b4eea3>,
    <urn:uuid:2153d83b-8555-44a3-96e0-821b6663a188>,
    <urn:uuid:797e83d7-a86f-4838-b5c5-0ec20855197d>,
    <urn:uuid:bbe073ad-f449-4b25-91ac-7d919613ca51>,
    <urn:uuid:4bbcdde6-ed53-4f8d-b3f8-43f800fd05d5>;
  skos:prefLabel "corpus"@en;
  skos:related <urn:uuid:01dc6e60-8e23-4c4c-a63d-f149cb104f84> .

<urn:uuid:8d3a484a-17e3-49d3-a5a8-d3cac97c5836> a skos:Concept;
  dct:created "2022-06-02T02:23:37Z"^^xsd:dateTime;
  dct:creator <urn:uuid:ca637d4b-c11b-4152-be98-bde602e7abd4>;
  skos:broader <urn:uuid:2bd3be3c-a234-4cf5-be07-2f770e08b48b>;
  skos:definition "\"Shearing layers\" is a conceptual framework coined by the architect Frank Duffy to refer to aspects of a building which vary by orders of magnitude in their sensitivity to time."@en;
  skos:inScheme <urn:uuid:abcac1e5-2fe0-4b40-9418-5bc3b62e7d04>,
    <urn:uuid:bbe073ad-f449-4b25-91ac-7d919613ca51>,
    <urn:uuid:1b457bed-8a80-4135-92b8-fdea12b4eea3>,
    <urn:uuid:2153d83b-8555-44a3-96e0-821b6663a188>,
    <urn:uuid:2df6fac6-3122-44dc-9f92-5caab7f9b10b>,
    <urn:uuid:4bbcdde6-ed53-4f8d-b3f8-43f800fd05d5>;
  skos:prefLabel "Shearing Layers"@en .

<urn:uuid:919d84fb-a760-45da-bbed-cdf2b3b40a5f> a skos:Concept;
  dct:created "2019-03-04T05:47:23Z"^^xsd:dateTime;
  dct:creator <urn:uuid:ca637d4b-c11b-4152-be98-bde602e7abd4>;
  skos:broader <urn:uuid:33c3211f-322b-4f7a-83f6-63aa617461c3>;
  skos:definition "Perl is a general-purpose interpreted programming language designed by Larry Wall. It was the lingua franca of server-side programming for at least the first decade of the Web."@en;
  skos:inScheme <urn:uuid:2df6fac6-3122-44dc-9f92-5caab7f9b10b>,
    <urn:uuid:75f35368-e228-47fe-8efd-7251a2bde816>,
    <urn:uuid:bbe073ad-f449-4b25-91ac-7d919613ca51>,
    <urn:uuid:1b457bed-8a80-4135-92b8-fdea12b4eea3>,
    <urn:uuid:2153d83b-8555-44a3-96e0-821b6663a188>,
    <urn:uuid:4bbcdde6-ed53-4f8d-b3f8-43f800fd05d5>;
  skos:prefLabel "Perl"@en;
  skos:related <urn:uuid:3e3aa9b0-efaf-4dc5-83fb-4456e24f021d>,
    <urn:uuid:e081bcbf-c245-4345-b797-13f9934c6bda> .

<urn:uuid:91d3f305-8c2c-4922-ac6d-fee77af3e4eb> a skos:Concept;
  dct:created "2017-02-02T22:41:09Z"^^xsd:dateTime;
  dct:creator <urn:uuid:ca637d4b-c11b-4152-be98-bde602e7abd4>;
  skos:definition """A snapshot, when referring to data, captures the state of a set of entities at one particular instant.
Unlike a log, which is cumulative, a snapshot replaces the contents of any snapshot that comes before it."""@en;
  skos:inScheme <urn:uuid:1b457bed-8a80-4135-92b8-fdea12b4eea3>,
    <urn:uuid:2153d83b-8555-44a3-96e0-821b6663a188>,
    <urn:uuid:2df6fac6-3122-44dc-9f92-5caab7f9b10b>,
    <urn:uuid:bbe073ad-f449-4b25-91ac-7d919613ca51>,
    <urn:uuid:49ac68c4-922c-4d9e-88fa-b318fc54d36f>,
    <urn:uuid:4bbcdde6-ed53-4f8d-b3f8-43f800fd05d5>;
  skos:prefLabel "snapshot"@en;
  skos:related <urn:uuid:2575586a-6ce1-4527-bb67-7ed7c11f52f7>,
    <urn:uuid:5964a9f9-5a6b-4491-8236-2d27e16218ec> .

<urn:uuid:92b60601-4c7e-4a44-b42f-9648fefc11d4> a skos:Concept;
  dct:created "2019-03-04T05:59:24Z"^^xsd:dateTime;
  dct:creator <urn:uuid:ca637d4b-c11b-4152-be98-bde602e7abd4>;
  skos:broader <urn:uuid:33c3211f-322b-4f7a-83f6-63aa617461c3>;
  skos:definition "R is both a language and programming environment designed for statistical computing."@en;
  skos:inScheme <urn:uuid:1b457bed-8a80-4135-92b8-fdea12b4eea3>,
    <urn:uuid:2153d83b-8555-44a3-96e0-821b6663a188>,
    <urn:uuid:2df6fac6-3122-44dc-9f92-5caab7f9b10b>,
    <urn:uuid:75f35368-e228-47fe-8efd-7251a2bde816>,
    <urn:uuid:bbe073ad-f449-4b25-91ac-7d919613ca51>,
    <urn:uuid:4bbcdde6-ed53-4f8d-b3f8-43f800fd05d5>;
  skos:prefLabel "R"@en .

<urn:uuid:94cd1298-0889-401a-b567-f6181dfefcce> a skos:Concept;
  dct:created "2021-12-14T20:29:22Z"^^xsd:dateTime;
  dct:creator <urn:uuid:ca637d4b-c11b-4152-be98-bde602e7abd4>;
  skos:altLabel "AWS"@en;
  skos:broader <urn:uuid:7ddb6eed-d37d-4412-9c10-eff42447eddf>;
  skos:definition "AWS is a sprawling set of software-as-a-service products from Amazon that began as their own infrastructure."@en;
  skos:hiddenLabel "amazon web services"@en,
    "aws"@en;
  skos:inScheme <urn:uuid:2df6fac6-3122-44dc-9f92-5caab7f9b10b>,
    <urn:uuid:1b457bed-8a80-4135-92b8-fdea12b4eea3>,
    <urn:uuid:2153d83b-8555-44a3-96e0-821b6663a188>,
    <urn:uuid:bbe073ad-f449-4b25-91ac-7d919613ca51>,
    <urn:uuid:797e83d7-a86f-4838-b5c5-0ec20855197d>,
    <urn:uuid:4bbcdde6-ed53-4f8d-b3f8-43f800fd05d5>;
  skos:prefLabel "Amazon Web Services"@en .

<urn:uuid:9763e3fc-30bc-4547-a8e6-6747088f914b> a skos:Concept;
  dct:created "2019-03-04T06:10:36Z"^^xsd:dateTime;
  dct:creator <urn:uuid:ca637d4b-c11b-4152-be98-bde602e7abd4>;
  skos:broader <urn:uuid:33c3211f-322b-4f7a-83f6-63aa617461c3>;
  skos:definition "Rust is a new programming language which aims to be a modern replacement for C. The goal is the speed of C with a level of program safety (i.e., from undefined behaviour and concomitant attacks) completely unattainable by C. Many of the developers of Rust also work on WebAssembly, a target to which Rust can compile."@en;
  skos:inScheme <urn:uuid:2df6fac6-3122-44dc-9f92-5caab7f9b10b>,
    <urn:uuid:1b457bed-8a80-4135-92b8-fdea12b4eea3>,
    <urn:uuid:2153d83b-8555-44a3-96e0-821b6663a188>,
    <urn:uuid:75f35368-e228-47fe-8efd-7251a2bde816>,
    <urn:uuid:bbe073ad-f449-4b25-91ac-7d919613ca51>,
    <urn:uuid:4bbcdde6-ed53-4f8d-b3f8-43f800fd05d5>;
  skos:prefLabel "Rust"@en;
  skos:related <urn:uuid:447cbc26-1fb8-4ffe-95f4-1f83b3bc3d21>,
    <urn:uuid:a718d483-af90-4eaf-a59f-31d8897d6e8e>,
    <urn:uuid:c7066ab9-ad6b-4a19-b682-d919827eec71> .

<urn:uuid:97fb551f-c68a-43bb-8153-9c88f916e70b> a skos:Concept;
  dct:created "2021-12-14T18:46:59Z"^^xsd:dateTime;
  dct:creator <urn:uuid:ca637d4b-c11b-4152-be98-bde602e7abd4>;
  skos:definition "A DNS subdomain is precisely that delegated symbolic namespace, the delegate in delegate.principal.top. In effect, all (available) domain names are technically subdomains."@en;
  skos:hiddenLabel "sub-domain"@en,
    "sub-domains"@en,
    "subdomains"@en;
  skos:inScheme <urn:uuid:2df6fac6-3122-44dc-9f92-5caab7f9b10b>,
    <urn:uuid:1b457bed-8a80-4135-92b8-fdea12b4eea3>,
    <urn:uuid:2153d83b-8555-44a3-96e0-821b6663a188>,
    <urn:uuid:bbe073ad-f449-4b25-91ac-7d919613ca51>,
    <urn:uuid:797e83d7-a86f-4838-b5c5-0ec20855197d>,
    <urn:uuid:4bbcdde6-ed53-4f8d-b3f8-43f800fd05d5>;
  skos:prefLabel "subdomain"@en .

<urn:uuid:9ad22902-84a2-488b-92ea-360182357ed1> a skos:Concept;
  dct:alternative "The user interface of a piece of software or product is its control and reporting surface; the part that comes in contact with humans."@en,
    "The user interface is the subset of an artifact that comes in (approximately) direct contact with human beings. This is a term coined for software but is by no means exclusive to it."@en;
  dct:created "2017-02-09T16:57:24Z"^^xsd:dateTime;
  dct:creator <urn:uuid:ca637d4b-c11b-4152-be98-bde602e7abd4>;
  dct:description "The user interface is the subset of an artifact that comes in (approximately) direct contact with human beings. This is a term coined for software but is by no means exclusive to it."@en,
    "The user interface of a piece of software or product is its control and reporting surface; the part that comes in contact with humans."@en;
  dct:modified "2019-03-04T06:48:45Z"^^xsd:dateTime,
    "2021-12-14T23:43:55Z"^^xsd:dateTime;
  skos:altLabel "UI"@en,
    "user interface"@en;
  skos:broader <urn:uuid:055e91e4-5edf-46fd-9bad-9847dbf57a72>,
    <urn:uuid:d2089ee2-d605-43ac-af18-ffbb7151a32d>,
    <urn:uuid:fdb43f70-cb11-49dd-aba6-7011b05ad61a>;
  skos:definition "A user interface is an interface that comes in direct contact with a human."@en;
  skos:hiddenLabel "ui"@en;
  skos:inScheme <urn:uuid:2df6fac6-3122-44dc-9f92-5caab7f9b10b>,
    <urn:uuid:1b457bed-8a80-4135-92b8-fdea12b4eea3>,
    <urn:uuid:2153d83b-8555-44a3-96e0-821b6663a188>,
    <urn:uuid:bbe073ad-f449-4b25-91ac-7d919613ca51>,
    <urn:uuid:a1a01f1c-7162-439c-94f1-3e28b99ae8ab>,
    <urn:uuid:ddfaaacc-9dcb-451b-afa6-477e6e787a5c>,
    <urn:uuid:49ac68c4-922c-4d9e-88fa-b318fc54d36f>,
    <urn:uuid:797e83d7-a86f-4838-b5c5-0ec20855197d>,
    <urn:uuid:4bbcdde6-ed53-4f8d-b3f8-43f800fd05d5>;
  skos:prefLabel "user interface"@en;
  skos:related <urn:uuid:4cb1625a-5157-48a4-8140-47fcb14fb8fd> .

<urn:uuid:9b56c5ee-7c41-4dc3-920f-f8d11ca869cf> a skos:Concept;
  dct:created "2021-12-14T16:40:24Z"^^xsd:dateTime;
  dct:creator <urn:uuid:ca637d4b-c11b-4152-be98-bde602e7abd4>;
  skos:definition "The content-type of a file or network message is a specific mapping between identifiers and data serialization (file) formats. The identifiers, which are registered with IANA, are used in operating systems and network protocols like e-mail and HTTP to determine what type of file or message is being accessed. This term is also used by content strategists to refer to categories (genres, formats) of documents."@en;
  skos:inScheme <urn:uuid:797e83d7-a86f-4838-b5c5-0ec20855197d>,
    <urn:uuid:2df6fac6-3122-44dc-9f92-5caab7f9b10b>,
    <urn:uuid:1b457bed-8a80-4135-92b8-fdea12b4eea3>,
    <urn:uuid:2153d83b-8555-44a3-96e0-821b6663a188>,
    <urn:uuid:bbe073ad-f449-4b25-91ac-7d919613ca51>,
    <urn:uuid:4bbcdde6-ed53-4f8d-b3f8-43f800fd05d5>;
  skos:prefLabel "content type"@en;
  skos:related <urn:uuid:68e38d88-1afd-4443-a1a4-f28abd9dc77d> .

<urn:uuid:9b7d80f4-7cdb-44a0-8ca8-c0b5606fb05a> a skos:Concept;
  dct:created "2017-02-20T02:16:19Z"^^xsd:dateTime;
  dct:creator <urn:uuid:ca637d4b-c11b-4152-be98-bde602e7abd4>;
  skos:definition "A time series is any data set where one of the dimensions is time."@en;
  skos:inScheme <urn:uuid:49ac68c4-922c-4d9e-88fa-b318fc54d36f>,
    <urn:uuid:2df6fac6-3122-44dc-9f92-5caab7f9b10b>,
    <urn:uuid:1b457bed-8a80-4135-92b8-fdea12b4eea3>,
    <urn:uuid:2153d83b-8555-44a3-96e0-821b6663a188>,
    <urn:uuid:bbe073ad-f449-4b25-91ac-7d919613ca51>,
    <urn:uuid:4bbcdde6-ed53-4f8d-b3f8-43f800fd05d5>;
  skos:prefLabel "time series"@en;
  skos:related <urn:uuid:b8565dd1-8c4d-4699-a240-56898fc32ac8> .

<urn:uuid:9d01c1e5-77f4-481f-bcf9-d9a3ad4b57c8> a skos:Concept;
  dct:created "2017-02-21T20:05:52Z"^^xsd:dateTime;
  dct:creator <urn:uuid:ca637d4b-c11b-4152-be98-bde602e7abd4>;
  skos:broader <urn:uuid:c0e969c3-4528-4968-8418-d5fe609c2a62>;
  skos:definition "Authorization is the process of judging whether a person (or automated agent), or rather their account, is allowed to access a particular resource, after they have been authenticated."@en;
  skos:inScheme <urn:uuid:bbe073ad-f449-4b25-91ac-7d919613ca51>,
    <urn:uuid:2df6fac6-3122-44dc-9f92-5caab7f9b10b>,
    <urn:uuid:1b457bed-8a80-4135-92b8-fdea12b4eea3>,
    <urn:uuid:2153d83b-8555-44a3-96e0-821b6663a188>,
    <urn:uuid:49ac68c4-922c-4d9e-88fa-b318fc54d36f>,
    <urn:uuid:4bbcdde6-ed53-4f8d-b3f8-43f800fd05d5>;
  skos:prefLabel "authorization"@en;
  skos:related <urn:uuid:8a0718ec-7bfc-48ee-bfa6-5e0edc285565>,
    <urn:uuid:abadd9b5-844e-4982-8fbe-b6b83d43736d>,
    <urn:uuid:d0d7da4b-4d4d-4262-96a3-a70afbc1a829>,
    <urn:uuid:d85e3c52-cc94-48a4-8dc5-591de86be52f> .

<urn:uuid:a20b533d-6723-457b-aec0-570076760d32> a skos:Concept;
  dct:created "2022-11-23T21:40:00Z"^^xsd:dateTime;
  dct:creator <urn:uuid:ca637d4b-c11b-4152-be98-bde602e7abd4>;
  skos:altLabel "HTTPS"@en;
  skos:definition "HTTPS is HTTP which has been wrapped in Transport Layer Security (TLS) encryption."@en;
  skos:inScheme <urn:uuid:0c7028f0-8226-47b3-acff-a4e83e6a60fd>,
    <urn:uuid:a1a01f1c-7162-439c-94f1-3e28b99ae8ab>,
    <urn:uuid:ddfaaacc-9dcb-451b-afa6-477e6e787a5c>,
    <urn:uuid:bbe073ad-f449-4b25-91ac-7d919613ca51>,
    <urn:uuid:1b457bed-8a80-4135-92b8-fdea12b4eea3>,
    <urn:uuid:2153d83b-8555-44a3-96e0-821b6663a188>,
    <urn:uuid:4bbcdde6-ed53-4f8d-b3f8-43f800fd05d5>;
  skos:prefLabel "Hypertext Transfer Protocol (Secure)"@en .

<urn:uuid:a30dc8ed-a356-4a20-9085-a0d40e75f0e9> a skos:Concept;
  dct:created "2021-12-14T22:11:31Z"^^xsd:dateTime;
  dct:creator <urn:uuid:ca637d4b-c11b-4152-be98-bde602e7abd4>;
  skos:broader <urn:uuid:288e85ab-887f-437c-9caa-c109cb9d478d>;
  skos:definition "The Hypermedia Constraint (erstwhile known as HATEOAS) is a feature of REST whereby, when treating a complying system as a state machine, subsequent states (or rather their identifiers) are embedded in the representation of the current hypermedia resource. A website that shows a page with links nominally qualifies, with the user clicking on the links in the role of the state transition function."@en;
  skos:inScheme <urn:uuid:bbe073ad-f449-4b25-91ac-7d919613ca51>,
    <urn:uuid:2df6fac6-3122-44dc-9f92-5caab7f9b10b>,
    <urn:uuid:1b457bed-8a80-4135-92b8-fdea12b4eea3>,
    <urn:uuid:2153d83b-8555-44a3-96e0-821b6663a188>,
    <urn:uuid:797e83d7-a86f-4838-b5c5-0ec20855197d>,
    <urn:uuid:4bbcdde6-ed53-4f8d-b3f8-43f800fd05d5>;
  skos:prefLabel "The Hypermedia Constraint"@en .

<urn:uuid:a4a25c35-91ab-4c8e-9bea-ee877ad0e18b> a skos:Concept;
  dct:created "2019-03-02T05:06:16Z"^^xsd:dateTime;
  dct:creator <urn:uuid:ca637d4b-c11b-4152-be98-bde602e7abd4>;
  skos:definition "Friend-of-a-Friend is a vocabulary for expressing social networks."@en;
  skos:inScheme <urn:uuid:2df6fac6-3122-44dc-9f92-5caab7f9b10b>,
    <urn:uuid:bbe073ad-f449-4b25-91ac-7d919613ca51>,
    <urn:uuid:1b457bed-8a80-4135-92b8-fdea12b4eea3>,
    <urn:uuid:75f35368-e228-47fe-8efd-7251a2bde816>,
    <urn:uuid:2153d83b-8555-44a3-96e0-821b6663a188>,
    <urn:uuid:4bbcdde6-ed53-4f8d-b3f8-43f800fd05d5>;
  skos:prefLabel "FOAF"@en .

<urn:uuid:a94728e6-4a3f-4694-9e9e-c1c949ed66c2> a skos:Concept;
  dct:created "2017-07-12T02:28:09Z"^^xsd:dateTime;
  dct:creator <urn:uuid:ca637d4b-c11b-4152-be98-bde602e7abd4>;
  dct:references <http://sioc-project.org/>;
  skos:definition "SIOC (Semantically-Interlinked Online Communities; pronounced \"shock\") is an OWL ontology for representing metadata related to blogs, CMSes and social media websites."@en;
  skos:inScheme <urn:uuid:2df6fac6-3122-44dc-9f92-5caab7f9b10b>,
    <urn:uuid:75f35368-e228-47fe-8efd-7251a2bde816>,
    <urn:uuid:bbe073ad-f449-4b25-91ac-7d919613ca51>,
    <urn:uuid:1b457bed-8a80-4135-92b8-fdea12b4eea3>,
    <urn:uuid:2153d83b-8555-44a3-96e0-821b6663a188>,
    <urn:uuid:91684d49-7b99-4b2e-9641-ea0b8e22f66c>,
    <urn:uuid:4bbcdde6-ed53-4f8d-b3f8-43f800fd05d5>;
  skos:prefLabel "SIOC"@en;
  skos:related <urn:uuid:ed4d30d7-d3cf-4b21-bcb4-5f2525027be7> .

<urn:uuid:ab11cb80-b052-4a74-bbb7-bd19dc120437> a skos:Concept;
  dct:created "2019-02-28T19:34:04Z"^^xsd:dateTime;
  dct:creator <urn:uuid:ca637d4b-c11b-4152-be98-bde602e7abd4>;
  skos:definition "XUL is an XML vocabulary, developed by Mozilla, for describing graphical user interfaces."@en;
  skos:inScheme <urn:uuid:75f35368-e228-47fe-8efd-7251a2bde816>,
    <urn:uuid:2df6fac6-3122-44dc-9f92-5caab7f9b10b>,
    <urn:uuid:bbe073ad-f449-4b25-91ac-7d919613ca51>,
    <urn:uuid:1b457bed-8a80-4135-92b8-fdea12b4eea3>,
    <urn:uuid:2153d83b-8555-44a3-96e0-821b6663a188>,
    <urn:uuid:4bbcdde6-ed53-4f8d-b3f8-43f800fd05d5>;
  skos:prefLabel "XUL"@en .

<urn:uuid:abdd08b5-9728-41b8-b56a-b53ce1ff1137> a skos:Concept;
  dct:created "2019-03-02T06:04:13Z"^^xsd:dateTime;
  dct:creator <urn:uuid:ca637d4b-c11b-4152-be98-bde602e7abd4>;
  skos:broader <urn:uuid:c0e969c3-4528-4968-8418-d5fe609c2a62>,
    <urn:uuid:f0a7ece3-44e6-4f6b-963c-281ab8dff8e6>;
  skos:definition "OAuth (Open Authorization) is a token-passing protocol that enables users to delegate to a bearer (e.g. an application or website) their access rights to a different website."@en;
  skos:inScheme <urn:uuid:bbe073ad-f449-4b25-91ac-7d919613ca51>,
    <urn:uuid:2df6fac6-3122-44dc-9f92-5caab7f9b10b>,
    <urn:uuid:75f35368-e228-47fe-8efd-7251a2bde816>,
    <urn:uuid:1b457bed-8a80-4135-92b8-fdea12b4eea3>,
    <urn:uuid:2153d83b-8555-44a3-96e0-821b6663a188>,
    <urn:uuid:4bbcdde6-ed53-4f8d-b3f8-43f800fd05d5>;
  skos:narrower <urn:uuid:5e6006da-5f7b-4c01-919e-f0708346c727>;
  skos:prefLabel "OAuth"@en .

<urn:uuid:afb9bfa2-d565-460b-855a-69331787ff1b> a skos:Concept;
  dct:created "2019-03-01T03:04:23Z"^^xsd:dateTime;
  dct:creator <urn:uuid:ca637d4b-c11b-4152-be98-bde602e7abd4>;
  skos:definition "An upper ontology is intended to tie together domain-specific \"lower\" ontologies into a unified frame."@en;
  skos:inScheme <urn:uuid:a1a01f1c-7162-439c-94f1-3e28b99ae8ab>,
    <urn:uuid:ddfaaacc-9dcb-451b-afa6-477e6e787a5c>,
    <urn:uuid:2df6fac6-3122-44dc-9f92-5caab7f9b10b>,
    <urn:uuid:75f35368-e228-47fe-8efd-7251a2bde816>,
    <urn:uuid:bbe073ad-f449-4b25-91ac-7d919613ca51>,
    <urn:uuid:1b457bed-8a80-4135-92b8-fdea12b4eea3>,
    <urn:uuid:2153d83b-8555-44a3-96e0-821b6663a188>,
    <urn:uuid:4bbcdde6-ed53-4f8d-b3f8-43f800fd05d5>;
  skos:prefLabel "upper ontology"@en .

<urn:uuid:b43684d3-ac8c-4804-b490-8e29a582cfc7> a skos:Concept;
  dct:alternative "A blob (binary large object) is a segment of arbitrary bytes. A blob with a name (and some other rudimentary metadata, like modification time) is a file."@en;
  dct:created "2021-12-14T00:58:37Z"^^xsd:dateTime;
  dct:creator <urn:uuid:ca637d4b-c11b-4152-be98-bde602e7abd4>;
  dct:description "A blob (binary large object) is a segment of arbitrary bytes. A blob with a name (and some other rudimentary metadata, like modification time) is a file."@en;
  dct:modified "2022-10-06T11:23:55Z"^^xsd:dateTime;
  skos:altLabel "blob"@en,
    "Blob"@en;
  skos:definition "A binary large object is a backronym for a segment of bytes treated as opaque by the information system."@en;
  skos:hiddenLabel "blobs"@en;
  skos:inScheme <urn:uuid:bbe073ad-f449-4b25-91ac-7d919613ca51>,
    <urn:uuid:797e83d7-a86f-4838-b5c5-0ec20855197d>,
    <urn:uuid:2df6fac6-3122-44dc-9f92-5caab7f9b10b>,
    <urn:uuid:1b457bed-8a80-4135-92b8-fdea12b4eea3>,
    <urn:uuid:2153d83b-8555-44a3-96e0-821b6663a188>,
    <urn:uuid:4bbcdde6-ed53-4f8d-b3f8-43f800fd05d5>;
  skos:narrower <urn:uuid:4f4aa0ac-c1b4-4a15-a6f3-518419d5b771>;
  skos:prefLabel "blob"@en;
  skos:related <urn:uuid:332a68b3-06d6-4ac2-8897-4212ba0f3a94>,
    <urn:uuid:9adc8b42-bbd1-4065-bb57-9a789253c4e4>,
    <urn:uuid:c9038f6c-67a7-4a26-9e68-19a6c54bf1bb> .

<urn:uuid:b7bb05a0-86af-4d5d-9d59-0d1691cc766d> a skos:Concept;
  dct:created "2019-02-28T21:44:45Z"^^xsd:dateTime;
  dct:creator <urn:uuid:ca637d4b-c11b-4152-be98-bde602e7abd4>;
  skos:broader <urn:uuid:fe500c7a-b458-4d2c-8b3a-efd1bb47d106>;
  skos:definition "The SPARQL query language is an analogue of SQL for RDF data."@en;
  skos:inScheme <urn:uuid:2df6fac6-3122-44dc-9f92-5caab7f9b10b>,
    <urn:uuid:bbe073ad-f449-4b25-91ac-7d919613ca51>,
    <urn:uuid:1b457bed-8a80-4135-92b8-fdea12b4eea3>,
    <urn:uuid:2153d83b-8555-44a3-96e0-821b6663a188>,
    <urn:uuid:75f35368-e228-47fe-8efd-7251a2bde816>,
    <urn:uuid:4bbcdde6-ed53-4f8d-b3f8-43f800fd05d5>;
  skos:prefLabel "SPARQL"@en;
  skos:related <urn:uuid:2dc3da5b-9325-4c28-8609-2b9118ce3028> .

<urn:uuid:c0d27ab7-6727-4df0-8231-805b201e4663> a skos:Concept;
  dct:created "2022-11-23T21:26:10Z"^^xsd:dateTime;
  dct:creator <urn:uuid:ca637d4b-c11b-4152-be98-bde602e7abd4>;
  skos:definition "In REST parlance, a layered system is when there are multiple waypoints (such as reverse proxies) between an origin server and a client."@en;
  skos:hiddenLabel "layer system"@en;
  skos:inScheme <urn:uuid:bbe073ad-f449-4b25-91ac-7d919613ca51>,
    <urn:uuid:1b457bed-8a80-4135-92b8-fdea12b4eea3>,
    <urn:uuid:2153d83b-8555-44a3-96e0-821b6663a188>,
    <urn:uuid:a1a01f1c-7162-439c-94f1-3e28b99ae8ab>,
    <urn:uuid:ddfaaacc-9dcb-451b-afa6-477e6e787a5c>,
    <urn:uuid:0c7028f0-8226-47b3-acff-a4e83e6a60fd>,
    <urn:uuid:4bbcdde6-ed53-4f8d-b3f8-43f800fd05d5>;
  skos:prefLabel "layered system"@en;
  skos:related <urn:uuid:770bfd11-d9d3-4e5a-8285-13fcff030de6> .

<urn:uuid:c8f8c1d9-7fe5-484e-86ee-8388c2e3b83b> a skos:Concept;
  dct:created "2022-06-15T20:10:02Z"^^xsd:dateTime;
  dct:creator <urn:uuid:ca637d4b-c11b-4152-be98-bde602e7abd4>;
  skos:broader <urn:uuid:826fb218-7346-4a9b-8597-4c30807e21ff>,
    <urn:uuid:51a7c4b2-ef0c-4dc1-a538-553622131f09>;
  skos:inScheme <urn:uuid:abcac1e5-2fe0-4b40-9418-5bc3b62e7d04>,
    <urn:uuid:bbe073ad-f449-4b25-91ac-7d919613ca51>,
    <urn:uuid:2df6fac6-3122-44dc-9f92-5caab7f9b10b>,
    <urn:uuid:1b457bed-8a80-4135-92b8-fdea12b4eea3>,
    <urn:uuid:2153d83b-8555-44a3-96e0-821b6663a188>,
    <urn:uuid:4bbcdde6-ed53-4f8d-b3f8-43f800fd05d5>;
  skos:prefLabel "typology"@en;
  skos:related <urn:uuid:5a29cf77-ddb2-4ad8-ae08-9d43da245166>,
    <urn:uuid:0f872daf-97f4-445e-b5d9-0de0087dd129>,
    <urn:uuid:45b6c768-da32-4e5f-9c87-a18d5ec94635> .

<urn:uuid:cd9605ea-abe2-425e-904a-5dd35acdec8f> a skos:Concept;
  dct:created "2021-12-14T19:03:12Z"^^xsd:dateTime;
  dct:creator <urn:uuid:ca637d4b-c11b-4152-be98-bde602e7abd4>;
  skos:altLabel "directory"@en;
  skos:definition "A folder (directory) is a virtual container in, and the mechanism that creates the hierarchy of, a hierarchical file system."@en;
  skos:hiddenLabel "folders"@en;
  skos:inScheme <urn:uuid:797e83d7-a86f-4838-b5c5-0ec20855197d>,
    <urn:uuid:bbe073ad-f449-4b25-91ac-7d919613ca51>,
    <urn:uuid:1b457bed-8a80-4135-92b8-fdea12b4eea3>,
    <urn:uuid:2df6fac6-3122-44dc-9f92-5caab7f9b10b>,
    <urn:uuid:2153d83b-8555-44a3-96e0-821b6663a188>,
    <urn:uuid:4bbcdde6-ed53-4f8d-b3f8-43f800fd05d5>;
  skos:prefLabel "folder"@en .

<urn:uuid:d3cb15cf-cdad-4b05-ad72-aae158621f42> a skos:Concept;
  dct:created "2019-02-28T06:41:59Z"^^xsd:dateTime;
  dct:creator <urn:uuid:ca637d4b-c11b-4152-be98-bde602e7abd4>;
  skos:definition "DTD is the legacy XML schema definition format inherited from HTML via SGML. It has been supplanted by XML Schema and Relax NG."@en;
  skos:inScheme <urn:uuid:75f35368-e228-47fe-8efd-7251a2bde816>,
    <urn:uuid:bbe073ad-f449-4b25-91ac-7d919613ca51>,
    <urn:uuid:1b457bed-8a80-4135-92b8-fdea12b4eea3>,
    <urn:uuid:2df6fac6-3122-44dc-9f92-5caab7f9b10b>,
    <urn:uuid:2153d83b-8555-44a3-96e0-821b6663a188>,
    <urn:uuid:4bbcdde6-ed53-4f8d-b3f8-43f800fd05d5>;
  skos:prefLabel "Document Type Definition"@en;
  skos:related <urn:uuid:45373ede-a7b0-404f-b797-902298208993>,
    <urn:uuid:0bc0aabb-9d9e-4caa-b9c8-553dd8b3ee05>,
    <urn:uuid:654c0fac-1eb1-4fd2-9139-b4a5f3e6d903>,
    <urn:uuid:f352a521-b78e-478e-b01d-3a68638025a4> .

<urn:uuid:d3e380b6-59b0-4ddf-b932-de8d7683594e> a skos:Concept;
  dct:created "2021-12-14T23:14:44Z"^^xsd:dateTime;
  dct:creator <urn:uuid:ca637d4b-c11b-4152-be98-bde602e7abd4>;
  skos:altLabel "UTF-8"@en;
  skos:definition "UTF-8 is the ubiquitous encoding format that represents Unicode codepoints as variable sequences of one to seven bytes."@en;
  skos:hiddenLabel "unicode transfer format (8-bit)"@en,
    "utf-8"@en;
  skos:inScheme <urn:uuid:bbe073ad-f449-4b25-91ac-7d919613ca51>,
    <urn:uuid:797e83d7-a86f-4838-b5c5-0ec20855197d>,
    <urn:uuid:1b457bed-8a80-4135-92b8-fdea12b4eea3>,
    <urn:uuid:2df6fac6-3122-44dc-9f92-5caab7f9b10b>,
    <urn:uuid:2153d83b-8555-44a3-96e0-821b6663a188>,
    <urn:uuid:4bbcdde6-ed53-4f8d-b3f8-43f800fd05d5>;
  skos:prefLabel "Unicode Transfer Format (8-Bit)"@en;
  skos:related <urn:uuid:02dce02e-d62c-4243-9472-237b53262ac7> .

<urn:uuid:d5b402b1-92b0-47c2-9063-3b0358b616ee> a skos:Concept;
  dct:created "2022-11-23T23:27:07Z"^^xsd:dateTime;
  dct:creator <urn:uuid:ca637d4b-c11b-4152-be98-bde602e7abd4>;
  skos:definition "A bastion host is a server whose duties have been partitioned to handle only relatively low-sensitivity information. Bastion hosts are part of a security strategy such that an attacker would have to compromise the ultimately disposable bastion host first before proceeding to more sensitive targets. Without any persistent data of its own, a bastion host can be wiped and reinstalled if it is ever compromised, making them particularly suitable to containerization."@en;
  skos:inScheme <urn:uuid:0c7028f0-8226-47b3-acff-a4e83e6a60fd>,
    <urn:uuid:bbe073ad-f449-4b25-91ac-7d919613ca51>,
    <urn:uuid:1b457bed-8a80-4135-92b8-fdea12b4eea3>,
    <urn:uuid:2153d83b-8555-44a3-96e0-821b6663a188>,
    <urn:uuid:4bbcdde6-ed53-4f8d-b3f8-43f800fd05d5>;
  skos:prefLabel "bastion host"@en;
  skos:related <urn:uuid:4e8865ba-1a0f-4ce4-86fd-b7871c41f259> .

<urn:uuid:d5cb742c-9f75-42a4-967f-70b1fda5f0be> a skos:Concept;
  dct:created "2019-03-02T06:38:59Z"^^xsd:dateTime;
  dct:creator <urn:uuid:ca637d4b-c11b-4152-be98-bde602e7abd4>;
  skos:broader <urn:uuid:f0e4c33f-8930-454a-9a7e-dd2b6cc79dce>,
    <urn:uuid:4694ebe0-589f-40a7-9ef9-67872edb6214>;
  skos:definition "MySQL is a popular open-source database product. Its main competitors are PostgreSQL or SQLite (depending on the application)."@en;
  skos:inScheme <urn:uuid:75f35368-e228-47fe-8efd-7251a2bde816>,
    <urn:uuid:bbe073ad-f449-4b25-91ac-7d919613ca51>,
    <urn:uuid:2df6fac6-3122-44dc-9f92-5caab7f9b10b>,
    <urn:uuid:1b457bed-8a80-4135-92b8-fdea12b4eea3>,
    <urn:uuid:2153d83b-8555-44a3-96e0-821b6663a188>,
    <urn:uuid:4bbcdde6-ed53-4f8d-b3f8-43f800fd05d5>;
  skos:prefLabel "MySQL"@en .

<urn:uuid:da6f9f27-38f3-47e9-8b16-03728bea9f5e> a skos:Concept;
  dct:created "2017-02-21T19:59:04Z"^^xsd:dateTime;
  dct:creator <urn:uuid:ca637d4b-c11b-4152-be98-bde602e7abd4>;
  skos:broader <urn:uuid:197982df-60a5-4c93-be50-2f8ede43b842>,
    <urn:uuid:4694ebe0-589f-40a7-9ef9-67872edb6214>;
  skos:definition "A record is typically represented as a single row in a database or spreadsheet. It corresponds to one entity."@en;
  skos:inScheme <urn:uuid:bbe073ad-f449-4b25-91ac-7d919613ca51>,
    <urn:uuid:49ac68c4-922c-4d9e-88fa-b318fc54d36f>,
    <urn:uuid:2df6fac6-3122-44dc-9f92-5caab7f9b10b>,
    <urn:uuid:1b457bed-8a80-4135-92b8-fdea12b4eea3>,
    <urn:uuid:2153d83b-8555-44a3-96e0-821b6663a188>,
    <urn:uuid:4bbcdde6-ed53-4f8d-b3f8-43f800fd05d5>;
  skos:prefLabel "record"@en .

<urn:uuid:dabce9e1-eb5b-4db3-82fd-15558aa40e88> a skos:Concept;
  dct:created "2019-03-04T05:57:39Z"^^xsd:dateTime;
  dct:creator <urn:uuid:ca637d4b-c11b-4152-be98-bde602e7abd4>;
  skos:broader <urn:uuid:33c3211f-322b-4f7a-83f6-63aa617461c3>;
  skos:definition "TeX is a quasi-declarative macro processing language designed by Donald Knuth in the 1970s for the purpose of typesetting (in particular mathematical) documents."@en;
  skos:inScheme <urn:uuid:75f35368-e228-47fe-8efd-7251a2bde816>,
    <urn:uuid:bbe073ad-f449-4b25-91ac-7d919613ca51>,
    <urn:uuid:2df6fac6-3122-44dc-9f92-5caab7f9b10b>,
    <urn:uuid:1b457bed-8a80-4135-92b8-fdea12b4eea3>,
    <urn:uuid:2153d83b-8555-44a3-96e0-821b6663a188>,
    <urn:uuid:4bbcdde6-ed53-4f8d-b3f8-43f800fd05d5>;
  skos:prefLabel "TeX"@en .

<urn:uuid:db972323-c096-4ddf-80ce-0e98f6b7c7c7> a skos:Concept;
  dct:created "2021-12-13T23:15:59Z"^^xsd:dateTime;
  dct:creator <urn:uuid:ca637d4b-c11b-4152-be98-bde602e7abd4>;
  skos:broader <urn:uuid:e840ba8a-4c6d-4be3-a673-dd6620463a39>;
  skos:definition "An API adapter is typically considered in the context of Web-based APIs, where an organization's system connects to a remote networked information service to send or receive data."@en;
  skos:hiddenLabel "api adapter"@en,
    "api adapters"@en;
  skos:inScheme <urn:uuid:bbe073ad-f449-4b25-91ac-7d919613ca51>,
    <urn:uuid:2df6fac6-3122-44dc-9f92-5caab7f9b10b>,
    <urn:uuid:797e83d7-a86f-4838-b5c5-0ec20855197d>,
    <urn:uuid:1b457bed-8a80-4135-92b8-fdea12b4eea3>,
    <urn:uuid:2153d83b-8555-44a3-96e0-821b6663a188>,
    <urn:uuid:4bbcdde6-ed53-4f8d-b3f8-43f800fd05d5>;
  skos:prefLabel "API adapter"@en;
  skos:related <urn:uuid:3cdd469a-195b-4040-8d74-fd27bc71f12d> .

<urn:uuid:dbadda22-ff04-4508-8b6f-591b364de982> a skos:Concept;
  dct:created "2019-03-02T06:30:27Z"^^xsd:dateTime;
  dct:creator <urn:uuid:ca637d4b-c11b-4152-be98-bde602e7abd4>;
  dct:modified "2021-12-14T21:05:06Z"^^xsd:dateTime;
  skos:altLabel "PHP"@en;
  skos:broader <urn:uuid:33c3211f-322b-4f7a-83f6-63aa617461c3>,
    <urn:uuid:fdb43f70-cb11-49dd-aba6-7011b05ad61a>;
  skos:definition "PHP is a popular interpreted programming language for making web pages."@en;
  skos:hiddenLabel "PHP's"@en,
    "php"@en;
  skos:inScheme <urn:uuid:75f35368-e228-47fe-8efd-7251a2bde816>,
    <urn:uuid:bbe073ad-f449-4b25-91ac-7d919613ca51>,
    <urn:uuid:2df6fac6-3122-44dc-9f92-5caab7f9b10b>,
    <urn:uuid:1b457bed-8a80-4135-92b8-fdea12b4eea3>,
    <urn:uuid:2153d83b-8555-44a3-96e0-821b6663a188>,
    <urn:uuid:797e83d7-a86f-4838-b5c5-0ec20855197d>,
    <urn:uuid:4bbcdde6-ed53-4f8d-b3f8-43f800fd05d5>;
  skos:prefLabel "PHP"@en .

<urn:uuid:de8a5f03-f936-4edb-b5c7-a9dcf00a4678> a skos:Concept;
  dct:created "2019-03-04T02:39:24Z"^^xsd:dateTime;
  dct:creator <urn:uuid:ca637d4b-c11b-4152-be98-bde602e7abd4>;
  skos:definition "In mathematical logic, skolemization is the removal of existential quantifiers from a formal statement. In RDF, it means turning a blank node into an isomorphic (and potentially dereferenceable) URI node."@en;
  skos:inScheme <urn:uuid:1b457bed-8a80-4135-92b8-fdea12b4eea3>,
    <urn:uuid:2153d83b-8555-44a3-96e0-821b6663a188>,
    <urn:uuid:75f35368-e228-47fe-8efd-7251a2bde816>,
    <urn:uuid:bbe073ad-f449-4b25-91ac-7d919613ca51>,
    <urn:uuid:2df6fac6-3122-44dc-9f92-5caab7f9b10b>,
    <urn:uuid:4bbcdde6-ed53-4f8d-b3f8-43f800fd05d5>;
  skos:prefLabel "skolemization"@en .

<urn:uuid:dfddf2a2-9648-4237-a922-6295c151eff4> a skos:Concept;
  dct:created "2019-02-28T21:22:19Z"^^xsd:dateTime;
  dct:creator <urn:uuid:ca637d4b-c11b-4152-be98-bde602e7abd4>;
  skos:definition "A JSON-LD context is a piece of metadata that enables the decoupling of JSON-LD terms from RDF terms, enabling JSON-LD to do double-duty as vanilla JSON."@en;
  skos:inScheme <urn:uuid:2df6fac6-3122-44dc-9f92-5caab7f9b10b>,
    <urn:uuid:1b457bed-8a80-4135-92b8-fdea12b4eea3>,
    <urn:uuid:2153d83b-8555-44a3-96e0-821b6663a188>,
    <urn:uuid:bbe073ad-f449-4b25-91ac-7d919613ca51>,
    <urn:uuid:75f35368-e228-47fe-8efd-7251a2bde816>,
    <urn:uuid:4bbcdde6-ed53-4f8d-b3f8-43f800fd05d5>;
  skos:prefLabel "JSON-LD context"@en .

<urn:uuid:e081bcbf-c245-4345-b797-13f9934c6bda> a skos:Concept;
  dct:created "2019-03-04T05:50:14Z"^^xsd:dateTime;
  dct:creator <urn:uuid:ca637d4b-c11b-4152-be98-bde602e7abd4>;
  skos:broader <urn:uuid:33c3211f-322b-4f7a-83f6-63aa617461c3>,
    <urn:uuid:e827d9af-be73-4918-89aa-a296872be199>;
  skos:definition "Python is an object-oriented programming language by Guido van Rossum, initially designed for teaching programming. It is very similar in performance and capabilities to (albeit with some notable improvements), and slightly younger than Perl. Python is currently (2019) gaining attention in data science and machine learning applications."@en;
  skos:inScheme <urn:uuid:2df6fac6-3122-44dc-9f92-5caab7f9b10b>,
    <urn:uuid:1b457bed-8a80-4135-92b8-fdea12b4eea3>,
    <urn:uuid:2153d83b-8555-44a3-96e0-821b6663a188>,
    <urn:uuid:75f35368-e228-47fe-8efd-7251a2bde816>,
    <urn:uuid:bbe073ad-f449-4b25-91ac-7d919613ca51>,
    <urn:uuid:4bbcdde6-ed53-4f8d-b3f8-43f800fd05d5>;
  skos:prefLabel "Python"@en;
  skos:related <urn:uuid:3e3aa9b0-efaf-4dc5-83fb-4456e24f021d> .

<urn:uuid:e5394a0c-c64a-4ded-a37b-55c1507dc24c> a skos:Concept;
  dct:created "2024-02-16T15:24:23Z"^^xsd:dateTime,
    "2024-07-18T17:03:17Z"^^xsd:dateTime;
  dct:creator <urn:uuid:ca637d4b-c11b-4152-be98-bde602e7abd4>;
  rdfs:seeAlso <https://data.org/resources/the-fair-data-principles/>,
    <https://www.go-fair.org/fair-principles/>;
  skos:altLabel "FAIR"@en,
    "FAIR data"@en,
    "FAIR principles"@en;
  skos:definition "Data which is Findable, Accessible, Interoperable and Reusable. FAIR began as an initiative in the scientific community to improve the hygiene around experimental data."@en;
  skos:inScheme <urn:uuid:1b457bed-8a80-4135-92b8-fdea12b4eea3>,
    <urn:uuid:2153d83b-8555-44a3-96e0-821b6663a188>,
    <urn:uuid:bbe073ad-f449-4b25-91ac-7d919613ca51>,
    <urn:uuid:a1a01f1c-7162-439c-94f1-3e28b99ae8ab>,
    <urn:uuid:ddfaaacc-9dcb-451b-afa6-477e6e787a5c>,
    <urn:uuid:4bbcdde6-ed53-4f8d-b3f8-43f800fd05d5>;
  skos:prefLabel "FAIR data principles"@en;
  skos:related <urn:uuid:c757c1ac-1ec6-4bdd-a35d-85f1d85728bb>,
    <urn:uuid:637cfc93-b88b-4bfb-8f7c-2f9e72e27b86> .

<urn:uuid:ea81d3fd-8cd6-4321-81c0-c4c5299f5844> a skos:Concept;
  dct:created "2021-12-14T22:55:19Z"^^xsd:dateTime;
  dct:creator <urn:uuid:ca637d4b-c11b-4152-be98-bde602e7abd4>;
  skos:broader <urn:uuid:fdb43f70-cb11-49dd-aba6-7011b05ad61a>;
  skos:definition "In programming, a string literal is a constant that contains a string of text."@en;
  skos:hiddenLabel "string literals"@en;
  skos:inScheme <urn:uuid:2df6fac6-3122-44dc-9f92-5caab7f9b10b>,
    <urn:uuid:1b457bed-8a80-4135-92b8-fdea12b4eea3>,
    <urn:uuid:2153d83b-8555-44a3-96e0-821b6663a188>,
    <urn:uuid:bbe073ad-f449-4b25-91ac-7d919613ca51>,
    <urn:uuid:797e83d7-a86f-4838-b5c5-0ec20855197d>,
    <urn:uuid:4bbcdde6-ed53-4f8d-b3f8-43f800fd05d5>;
  skos:prefLabel "string literal"@en .

<urn:uuid:eb45112f-3c6a-47be-a547-e3462fb853e4> a skos:Concept;
  dct:created "2019-02-19T21:35:56Z"^^xsd:dateTime;
  dct:creator <urn:uuid:ca637d4b-c11b-4152-be98-bde602e7abd4>;
  dct:modified "2021-12-14T19:01:37Z"^^xsd:dateTime;
  skos:altLabel "XHTML"@en;
  skos:broader <urn:uuid:45373ede-a7b0-404f-b797-902298208993>,
    <urn:uuid:0bc0aabb-9d9e-4caa-b9c8-553dd8b3ee05>,
    <urn:uuid:8d46494e-5316-43b7-a49e-a625ab716a38>,
    <urn:uuid:f352a521-b78e-478e-b01d-3a68638025a4>;
  skos:definition "XHTML is a dialect of HTML implemented in XML. With the exception of a namespace URI and some very minor differences in the syntax, it is otherwise identical to HTML."@en;
  skos:hiddenLabel "xhtml"@en;
  skos:inScheme <urn:uuid:75f35368-e228-47fe-8efd-7251a2bde816>,
    <urn:uuid:2df6fac6-3122-44dc-9f92-5caab7f9b10b>,
    <urn:uuid:1b457bed-8a80-4135-92b8-fdea12b4eea3>,
    <urn:uuid:2153d83b-8555-44a3-96e0-821b6663a188>,
    <urn:uuid:797e83d7-a86f-4838-b5c5-0ec20855197d>,
    <urn:uuid:bbe073ad-f449-4b25-91ac-7d919613ca51>,
    <urn:uuid:4bbcdde6-ed53-4f8d-b3f8-43f800fd05d5>;
  skos:prefLabel "Extensible Hypertext Markup Language"@en .

<urn:uuid:f477beaf-1b44-42dd-88b6-69857070627d> a skos:Concept;
  dct:created "2022-06-02T02:07:31Z"^^xsd:dateTime;
  dct:creator <urn:uuid:ca637d4b-c11b-4152-be98-bde602e7abd4>;
  skos:broader <urn:uuid:a43e33d9-1788-4514-8fbd-1b4982535f73>;
  skos:definition "A business ecosystem is a model that situates an organization in the centre of a set of relationships with the entities with which it interacts. Entities like customers may be represented as archetypal classes, whereas certain competitors, important shareholders, or regulatory bodies might be modeled as themselves."@en;
  skos:inScheme <urn:uuid:abcac1e5-2fe0-4b40-9418-5bc3b62e7d04>,
    <urn:uuid:2df6fac6-3122-44dc-9f92-5caab7f9b10b>,
    <urn:uuid:1b457bed-8a80-4135-92b8-fdea12b4eea3>,
    <urn:uuid:2153d83b-8555-44a3-96e0-821b6663a188>,
    <urn:uuid:bbe073ad-f449-4b25-91ac-7d919613ca51>,
    <urn:uuid:4bbcdde6-ed53-4f8d-b3f8-43f800fd05d5>;
  skos:prefLabel "business ecosystem"@en .

<urn:uuid:f70f6095-f27b-4485-b245-3431f77a6e17> a skos:Concept;
  dct:created "2019-03-04T06:01:10Z"^^xsd:dateTime;
  dct:creator <urn:uuid:ca637d4b-c11b-4152-be98-bde602e7abd4>;
  skos:broader <urn:uuid:33c3211f-322b-4f7a-83f6-63aa617461c3>;
  skos:definition "Haskell is a functional programming language with the unique characteristic that all programs are pure functions with no side effects (such as input/output). Side effects, and indeed a great many other aspects of programming in Haskell, are handled through a creative use of monads."@en;
  skos:inScheme <urn:uuid:75f35368-e228-47fe-8efd-7251a2bde816>,
    <urn:uuid:2df6fac6-3122-44dc-9f92-5caab7f9b10b>,
    <urn:uuid:1b457bed-8a80-4135-92b8-fdea12b4eea3>,
    <urn:uuid:2153d83b-8555-44a3-96e0-821b6663a188>,
    <urn:uuid:bbe073ad-f449-4b25-91ac-7d919613ca51>,
    <urn:uuid:4bbcdde6-ed53-4f8d-b3f8-43f800fd05d5>;
  skos:prefLabel "Haskell"@en;
  skos:related <urn:uuid:00ae5130-bb3f-478b-b97a-e868c8bb17d8> .

<urn:uuid:f8d5f1b1-ca7f-4610-9026-20b68c04783d> a skos:Concept;
  dct:created "2021-12-14T19:25:36Z"^^xsd:dateTime;
  dct:creator <urn:uuid:ca637d4b-c11b-4152-be98-bde602e7abd4>;
  skos:broader <urn:uuid:db2fb779-83e8-407b-a538-5fe9a86271de>;
  skos:definition "In object-oriented programming, a method is the term for a subroutine bound to an object (or its class), and therefore has access to the object's state."@en;
  skos:inScheme <urn:uuid:2df6fac6-3122-44dc-9f92-5caab7f9b10b>,
    <urn:uuid:797e83d7-a86f-4838-b5c5-0ec20855197d>,
    <urn:uuid:1b457bed-8a80-4135-92b8-fdea12b4eea3>,
    <urn:uuid:2153d83b-8555-44a3-96e0-821b6663a188>,
    <urn:uuid:bbe073ad-f449-4b25-91ac-7d919613ca51>,
    <urn:uuid:4bbcdde6-ed53-4f8d-b3f8-43f800fd05d5>;
  skos:prefLabel "method"@en .

<urn:uuid:f99b9a38-43c5-4219-8ca8-166c49b80ac1> a skos:Concept;
  dct:created "2019-03-04T04:11:54Z"^^xsd:dateTime;
  dct:creator <urn:uuid:ca637d4b-c11b-4152-be98-bde602e7abd4>;
  skos:definition "A reasoner is an important piece of software (usually manifested as either a library or a service) that performs inferences over RDF data: it uses inference rules generated from RDF Schema, OWL, or some other mechanism, to supplement an RDF graph with inferred statements based on asserted statements."@en;
  skos:inScheme <urn:uuid:a1a01f1c-7162-439c-94f1-3e28b99ae8ab>,
    <urn:uuid:ddfaaacc-9dcb-451b-afa6-477e6e787a5c>,
    <urn:uuid:75f35368-e228-47fe-8efd-7251a2bde816>,
    <urn:uuid:2df6fac6-3122-44dc-9f92-5caab7f9b10b>,
    <urn:uuid:1b457bed-8a80-4135-92b8-fdea12b4eea3>,
    <urn:uuid:2153d83b-8555-44a3-96e0-821b6663a188>,
    <urn:uuid:bbe073ad-f449-4b25-91ac-7d919613ca51>,
    <urn:uuid:4bbcdde6-ed53-4f8d-b3f8-43f800fd05d5>;
  skos:prefLabel "Reasoner"@en;
  skos:related <urn:uuid:ed4d30d7-d3cf-4b21-bcb4-5f2525027be7> .

<urn:uuid:f9decec4-c869-4d17-aaa0-3a44ea18e6df> a skos:Concept;
  dct:alternative "A composite document is one assembled from two or more distinct resources via transclusion."@en;
  dct:created "2019-02-22T01:26:57Z"^^xsd:dateTime;
  dct:creator <urn:uuid:ca637d4b-c11b-4152-be98-bde602e7abd4>;
  dct:description "A composite document is one assembled from two or more distinct resources via transclusion."@en;
  dct:modified "2021-12-14T03:11:35Z"^^xsd:dateTime;
  skos:altLabel "composite document"@en;
  skos:broader <urn:uuid:0bb63dd9-2d87-4e26-af1d-ebe272d45b1c>;
  skos:definition "A composite document is one assembled from two or more distinct resources via transclusion."@en,
    "A composite document is made up of more than one reusable fragments, merged together through transclusion, generally agglomerated into a shell or umbrella-like structure."@en;
  skos:inScheme <urn:uuid:bbe073ad-f449-4b25-91ac-7d919613ca51>,
    <urn:uuid:75f35368-e228-47fe-8efd-7251a2bde816>,
    <urn:uuid:797e83d7-a86f-4838-b5c5-0ec20855197d>,
    <urn:uuid:1b457bed-8a80-4135-92b8-fdea12b4eea3>,
    <urn:uuid:2153d83b-8555-44a3-96e0-821b6663a188>,
    <urn:uuid:2df6fac6-3122-44dc-9f92-5caab7f9b10b>,
    <urn:uuid:4bbcdde6-ed53-4f8d-b3f8-43f800fd05d5>;
  skos:prefLabel "composite document"@en;
  skos:related <urn:uuid:0bb63dd9-2d87-4e26-af1d-ebe272d45b1c>,
    <urn:uuid:61c0c9c3-4d91-4509-902a-db09c4188ae5>,
    <urn:uuid:83c1c427-8523-4b51-bcb5-c4fdeb11e859>,
    <urn:uuid:cbc4f4d6-96a1-44fc-8f07-e3282626fe3f> .

<urn:uuid:f9df502b-051e-441d-811f-ea1661254373> a skos:Concept;
  dct:created "2019-03-04T05:11:02Z"^^xsd:dateTime;
  dct:creator <urn:uuid:ca637d4b-c11b-4152-be98-bde602e7abd4>;
  skos:broader <urn:uuid:33c3211f-322b-4f7a-83f6-63aa617461c3>;
  skos:definition "C is a general-purpose programming language designed by Dennis Ritchie in the early 1970s, which is basically the backbone for everything else."@en;
  skos:inScheme <urn:uuid:bbe073ad-f449-4b25-91ac-7d919613ca51>,
    <urn:uuid:75f35368-e228-47fe-8efd-7251a2bde816>,
    <urn:uuid:2df6fac6-3122-44dc-9f92-5caab7f9b10b>,
    <urn:uuid:1b457bed-8a80-4135-92b8-fdea12b4eea3>,
    <urn:uuid:2153d83b-8555-44a3-96e0-821b6663a188>,
    <urn:uuid:4bbcdde6-ed53-4f8d-b3f8-43f800fd05d5>;
  skos:prefLabel "C"@en;
  skos:related <urn:uuid:1b496cb8-fb39-4b54-ab88-a9663f419bc4> .

<urn:uuid:fb8ef397-b65d-4213-8483-4dee04d58eea> a skos:Concept;
  dct:created "2022-06-02T03:08:17Z"^^xsd:dateTime;
  dct:creator <urn:uuid:ca637d4b-c11b-4152-be98-bde602e7abd4>;
  skos:altLabel "15 fundamental geometric properties",
    "15 fundamental properties",
    "15 geometric properties",
    "15 properties",
    "fifteen fundamental geometric properties",
    "fifteen fundamental properties",
    "fifteen geometric properties";
  skos:definition "The Fifteen Fundamental Properties/Transformations are a conceptual framework invented by Christopher Alexander and described at length in The Nature of Order. They describe certain empirically observable geometric properties in (built) space that are associated with Alexander's conceptualizations of \"wholeness\" and \"life\". They also represent structure-preserving transformations that take a region of space from a state of the given geometric property being weakly-expressed to being expressed more strongly."@en;
  skos:inScheme <urn:uuid:abcac1e5-2fe0-4b40-9418-5bc3b62e7d04>,
    <urn:uuid:2df6fac6-3122-44dc-9f92-5caab7f9b10b>,
    <urn:uuid:1b457bed-8a80-4135-92b8-fdea12b4eea3>,
    <urn:uuid:2153d83b-8555-44a3-96e0-821b6663a188>,
    <urn:uuid:bbe073ad-f449-4b25-91ac-7d919613ca51>,
    <urn:uuid:4bbcdde6-ed53-4f8d-b3f8-43f800fd05d5>;
  skos:prefLabel "Fifteen Properties"@en .

<urn:uuid:fd1478d3-a6ba-430b-bdb2-2d47a4e7caf9> a skos:Concept;
  dct:created "2019-03-02T00:33:52Z"^^xsd:dateTime;
  dct:creator <urn:uuid:ca637d4b-c11b-4152-be98-bde602e7abd4>;
  skos:broader <urn:uuid:33c3211f-322b-4f7a-83f6-63aa617461c3>;
  skos:definition "JavaScript is the de facto scripting language embedded in Web browsers to provide interactive functionality to websites, and since about 2008, has been gaining momentum as a general-purpose programming language. JavaScript is so named to capitalize on the momentum of Java in the 1990s, which, while the syntax is superficially similar, is otherwise unrelated."@en;
  skos:inScheme <urn:uuid:bbe073ad-f449-4b25-91ac-7d919613ca51>,
    <urn:uuid:2df6fac6-3122-44dc-9f92-5caab7f9b10b>,
    <urn:uuid:1b457bed-8a80-4135-92b8-fdea12b4eea3>,
    <urn:uuid:2153d83b-8555-44a3-96e0-821b6663a188>,
    <urn:uuid:4bbcdde6-ed53-4f8d-b3f8-43f800fd05d5>;
  skos:prefLabel "JavaScript"@en;
  skos:related <urn:uuid:855fce21-5560-4ff3-87bf-ef26a28958c4>,
    <urn:uuid:ca632e87-50d2-4f1d-af83-f3d11e53eca8> .

<urn:uuid:fdb190cf-9f79-4c98-b65a-688b00e4f8d3> a skos:Concept;
  dct:created "2017-06-08T21:40:45Z"^^xsd:dateTime;
  dct:creator <urn:uuid:ca637d4b-c11b-4152-be98-bde602e7abd4>;
  skos:broader <urn:uuid:bdb1ca1d-7f9d-4e26-8fd6-639b9a3348d9>;
  skos:definition "The matrix resource, in the context of this project, is a program which generates a tabular grid representing (usually) 2-dimensional data, based on a set of input parameters. Instantiations of the matrix resource provide the data for visualizations in this project."@en;
  skos:inScheme <urn:uuid:49ac68c4-922c-4d9e-88fa-b318fc54d36f>,
    <urn:uuid:2df6fac6-3122-44dc-9f92-5caab7f9b10b>,
    <urn:uuid:1b457bed-8a80-4135-92b8-fdea12b4eea3>,
    <urn:uuid:2153d83b-8555-44a3-96e0-821b6663a188>,
    <urn:uuid:bbe073ad-f449-4b25-91ac-7d919613ca51>,
    <urn:uuid:4bbcdde6-ed53-4f8d-b3f8-43f800fd05d5>;
  skos:prefLabel "matrix resource"@en .

<urn:uuid:fe14fe9c-8794-440a-86ad-0e245c3cbb7b> a skos:Concept;
  dct:created "2017-07-12T03:18:06Z"^^xsd:dateTime;
  dct:creator <urn:uuid:ca637d4b-c11b-4152-be98-bde602e7abd4>;
  skos:broader <urn:uuid:0f872daf-97f4-445e-b5d9-0de0087dd129>;
  skos:definition "A thesaurus is a specific kind of concept scheme, insofar as it organizes terms (words and phrases), rather than concepts which need not necessarily be labeled."@en;
  skos:inScheme <urn:uuid:91684d49-7b99-4b2e-9641-ea0b8e22f66c>,
    <urn:uuid:75f35368-e228-47fe-8efd-7251a2bde816>,
    <urn:uuid:2df6fac6-3122-44dc-9f92-5caab7f9b10b>,
    <urn:uuid:1b457bed-8a80-4135-92b8-fdea12b4eea3>,
    <urn:uuid:2153d83b-8555-44a3-96e0-821b6663a188>,
    <urn:uuid:bbe073ad-f449-4b25-91ac-7d919613ca51>,
    <urn:uuid:4bbcdde6-ed53-4f8d-b3f8-43f800fd05d5>;
  skos:prefLabel "Thesaurus"@en .

<urn:uuid:02dce02e-d62c-4243-9472-237b53262ac7> a skos:Concept;
  dct:created "2021-12-14T03:17:37Z"^^xsd:dateTime;
  dct:creator <urn:uuid:ca637d4b-c11b-4152-be98-bde602e7abd4>;
  skos:altLabel "code point"@en;
  skos:definition "An individual codepoint is generally understood to be the virtual index of a given Unicode character. As such, the concrete representation of a codepoint may occupy a range of bytes within a particular encoding scheme. UTF-8, for example, represents individual Unicode codepoints within a specially-crafted representation that can span one to seven bytes per codepoint."@en;
  skos:hiddenLabel "code-point"@en;
  skos:inScheme <urn:uuid:bbe073ad-f449-4b25-91ac-7d919613ca51>,
    <urn:uuid:2df6fac6-3122-44dc-9f92-5caab7f9b10b>,
    <urn:uuid:1b457bed-8a80-4135-92b8-fdea12b4eea3>,
    <urn:uuid:2153d83b-8555-44a3-96e0-821b6663a188>,
    <urn:uuid:797e83d7-a86f-4838-b5c5-0ec20855197d>,
    <urn:uuid:4bbcdde6-ed53-4f8d-b3f8-43f800fd05d5>;
  skos:prefLabel "codepoint"@en;
  skos:related <urn:uuid:d3e380b6-59b0-4ddf-b932-de8d7683594e> .

<urn:uuid:06f86a10-1b5f-4711-b2fc-3bb5ce14a26e> a skos:Concept;
  dct:created "2022-12-14T11:16:10Z"^^xsd:dateTime;
  dct:creator <urn:uuid:ca637d4b-c11b-4152-be98-bde602e7abd4>;
  skos:broader <urn:uuid:0cf51602-4fc1-4a38-9663-d47aff228b2d>;
  skos:definition "Content infrastructure can be understood as the superset of all content management and related systems within an organization."@en;
  skos:inScheme <urn:uuid:bbe073ad-f449-4b25-91ac-7d919613ca51>,
    <urn:uuid:a1a01f1c-7162-439c-94f1-3e28b99ae8ab>,
    <urn:uuid:ddfaaacc-9dcb-451b-afa6-477e6e787a5c>,
    <urn:uuid:0c7028f0-8226-47b3-acff-a4e83e6a60fd>,
    <urn:uuid:1b457bed-8a80-4135-92b8-fdea12b4eea3>,
    <urn:uuid:2153d83b-8555-44a3-96e0-821b6663a188>,
    <urn:uuid:4bbcdde6-ed53-4f8d-b3f8-43f800fd05d5>;
  skos:narrower <urn:uuid:61c0c9c3-4d91-4509-902a-db09c4188ae5>;
  skos:prefLabel "content infrastructure"@en .

<urn:uuid:0bb63dd9-2d87-4e26-af1d-ebe272d45b1c> a skos:Concept;
  dct:alternative "Transclusion, a term coined by Ted Nelson in the early 1960s, is the seamless weaving of one document (or document fragment) into another. This document set makes heavy use of transclusion."@en;
  dct:created "2019-02-22T01:27:40Z"^^xsd:dateTime;
  dct:creator <urn:uuid:ca637d4b-c11b-4152-be98-bde602e7abd4>;
  dct:description "Transclusion, a term coined by Ted Nelson in the early 1960s, is the seamless weaving of one document (or document fragment) into another. This document set makes heavy use of transclusion."@en;
  dct:modified "2021-12-14T23:06:58Z"^^xsd:dateTime;
  skos:altLabel "transclusion"@en;
  skos:definition "Transclusion is the seamless embedding of one segment of content inside another."@en;
  skos:hiddenLabel "transclude"@en;
  skos:inScheme <urn:uuid:bbe073ad-f449-4b25-91ac-7d919613ca51>,
    <urn:uuid:797e83d7-a86f-4838-b5c5-0ec20855197d>,
    <urn:uuid:75f35368-e228-47fe-8efd-7251a2bde816>,
    <urn:uuid:2df6fac6-3122-44dc-9f92-5caab7f9b10b>,
    <urn:uuid:1b457bed-8a80-4135-92b8-fdea12b4eea3>,
    <urn:uuid:2153d83b-8555-44a3-96e0-821b6663a188>,
    <urn:uuid:4bbcdde6-ed53-4f8d-b3f8-43f800fd05d5>;
  skos:prefLabel "transclusion"@en .

<urn:uuid:13385ea1-1f87-4612-b86b-27bc4e339be6> a skos:Concept;
  dct:created "2022-11-23T23:08:41Z"^^xsd:dateTime;
  dct:creator <urn:uuid:ca637d4b-c11b-4152-be98-bde602e7abd4>;
  skos:broader <urn:uuid:0cf51602-4fc1-4a38-9663-d47aff228b2d>;
  skos:definition "An asset is any information resource that is subsidiary to some main piece of content, such as an image, sound file, video, or script."@en;
  skos:hiddenLabel "assets"@en;
  skos:inScheme <urn:uuid:1b457bed-8a80-4135-92b8-fdea12b4eea3>,
    <urn:uuid:2153d83b-8555-44a3-96e0-821b6663a188>,
    <urn:uuid:0c7028f0-8226-47b3-acff-a4e83e6a60fd>,
    <urn:uuid:bbe073ad-f449-4b25-91ac-7d919613ca51>,
    <urn:uuid:4bbcdde6-ed53-4f8d-b3f8-43f800fd05d5>;
  skos:prefLabel "asset (content)"@en;
  skos:related <urn:uuid:755dd3a1-cffc-4d65-9446-435552bac541> .

<urn:uuid:193a84ec-ef96-44b9-b356-6f6b1c6ec979> a skos:Concept;
  dct:created "2021-12-14T01:16:25Z"^^xsd:dateTime;
  dct:creator <urn:uuid:ca637d4b-c11b-4152-be98-bde602e7abd4>;
  skos:definition "A proxy, in information system parlance, is an intermediary between a client and an origin. Proxies may simply convey information without changing it, or they may perform additional operations on the information in transit."@en;
  skos:inScheme <urn:uuid:797e83d7-a86f-4838-b5c5-0ec20855197d>,
    <urn:uuid:bbe073ad-f449-4b25-91ac-7d919613ca51>,
    <urn:uuid:1b457bed-8a80-4135-92b8-fdea12b4eea3>,
    <urn:uuid:2153d83b-8555-44a3-96e0-821b6663a188>,
    <urn:uuid:a1a01f1c-7162-439c-94f1-3e28b99ae8ab>,
    <urn:uuid:ddfaaacc-9dcb-451b-afa6-477e6e787a5c>,
    <urn:uuid:2df6fac6-3122-44dc-9f92-5caab7f9b10b>,
    <urn:uuid:0c7028f0-8226-47b3-acff-a4e83e6a60fd>,
    <urn:uuid:4bbcdde6-ed53-4f8d-b3f8-43f800fd05d5>;
  skos:narrower <urn:uuid:53819af5-c2d0-4edc-9add-ab79829ace96>;
  skos:prefLabel "proxy"@en;
  skos:related <urn:uuid:770bfd11-d9d3-4e5a-8285-13fcff030de6> .

<urn:uuid:1b004393-fdea-438b-a0d8-1919184d4bd1> a skos:Concept;
  dct:created "2022-11-23T21:25:18Z"^^xsd:dateTime;
  dct:creator <urn:uuid:ca637d4b-c11b-4152-be98-bde602e7abd4>;
  skos:altLabel "homogeneity"@en,
    "homogeneous"@en;
  skos:definition "An information system is homogeneous when it is entirely made using a single platform."@en;
  skos:inScheme <urn:uuid:a1a01f1c-7162-439c-94f1-3e28b99ae8ab>,
    <urn:uuid:ddfaaacc-9dcb-451b-afa6-477e6e787a5c>,
    <urn:uuid:1b457bed-8a80-4135-92b8-fdea12b4eea3>,
    <urn:uuid:2153d83b-8555-44a3-96e0-821b6663a188>,
    <urn:uuid:bbe073ad-f449-4b25-91ac-7d919613ca51>,
    <urn:uuid:0c7028f0-8226-47b3-acff-a4e83e6a60fd>,
    <urn:uuid:4bbcdde6-ed53-4f8d-b3f8-43f800fd05d5>;
  skos:prefLabel "homogeneity (information systems)"@en .

<urn:uuid:1ba688e9-6a85-4596-be01-379d90b8a5c6> a skos:Concept;
  dct:created "2022-11-23T21:28:01Z"^^xsd:dateTime;
  dct:creator <urn:uuid:ca637d4b-c11b-4152-be98-bde602e7abd4>;
  skos:broader <urn:uuid:055e91e4-5edf-46fd-9bad-9847dbf57a72>;
  skos:definition "In REST parlance, a unified interface is exactly what it sounds like: all parts of the system speak the same language."@en;
  skos:inScheme <urn:uuid:1b457bed-8a80-4135-92b8-fdea12b4eea3>,
    <urn:uuid:2153d83b-8555-44a3-96e0-821b6663a188>,
    <urn:uuid:bbe073ad-f449-4b25-91ac-7d919613ca51>,
    <urn:uuid:a1a01f1c-7162-439c-94f1-3e28b99ae8ab>,
    <urn:uuid:ddfaaacc-9dcb-451b-afa6-477e6e787a5c>,
    <urn:uuid:0c7028f0-8226-47b3-acff-a4e83e6a60fd>,
    <urn:uuid:4bbcdde6-ed53-4f8d-b3f8-43f800fd05d5>;
  skos:prefLabel "unified interface"@en .

<urn:uuid:22c5c553-d574-4bf7-9a4d-13e70afa7f1c> a skos:Concept;
  dct:created "2022-11-24T01:04:45Z"^^xsd:dateTime;
  dct:creator <urn:uuid:ca637d4b-c11b-4152-be98-bde602e7abd4>;
  skos:altLabel "operations team"@en,
    "ops"@en,
    "ops team"@en;
  skos:definition "The ops team is responsible for running the software written by the dev team. Sometimes this is the same team (DevOps). Ops is also typically responsible for information security and SRE."@en;
  skos:inScheme <urn:uuid:0c7028f0-8226-47b3-acff-a4e83e6a60fd>,
    <urn:uuid:1b457bed-8a80-4135-92b8-fdea12b4eea3>,
    <urn:uuid:2153d83b-8555-44a3-96e0-821b6663a188>,
    <urn:uuid:bbe073ad-f449-4b25-91ac-7d919613ca51>,
    <urn:uuid:4bbcdde6-ed53-4f8d-b3f8-43f800fd05d5>;
  skos:prefLabel "(system) operations team"@en;
  skos:related <urn:uuid:a718d483-af90-4eaf-a59f-31d8897d6e8e> .

<urn:uuid:2575586a-6ce1-4527-bb67-7ed7c11f52f7> a skos:Concept;
  dct:created "2017-02-02T22:49:55Z"^^xsd:dateTime;
  dct:creator <urn:uuid:ca637d4b-c11b-4152-be98-bde602e7abd4>;
  skos:altLabel "log"@en,
    "Log"@en;
  skos:definition "A log, when referring to data, is a list of entities that accumulate over time."@en;
  skos:inScheme <urn:uuid:bbe073ad-f449-4b25-91ac-7d919613ca51>,
    <urn:uuid:1b457bed-8a80-4135-92b8-fdea12b4eea3>,
    <urn:uuid:2153d83b-8555-44a3-96e0-821b6663a188>,
    <urn:uuid:2df6fac6-3122-44dc-9f92-5caab7f9b10b>,
    <urn:uuid:4bbcdde6-ed53-4f8d-b3f8-43f800fd05d5>;
  skos:prefLabel "logging"@en .

<urn:uuid:2f6700a6-9ecb-47af-8106-a652b4c852e5> a skos:Concept;
  dct:created "2019-02-19T04:38:12Z"^^xsd:dateTime;
  dct:creator <urn:uuid:ca637d4b-c11b-4152-be98-bde602e7abd4>;
  skos:broader <urn:uuid:33c3211f-322b-4f7a-83f6-63aa617461c3>,
    <urn:uuid:f352a521-b78e-478e-b01d-3a68638025a4>;
  skos:inScheme <urn:uuid:75f35368-e228-47fe-8efd-7251a2bde816>,
    <urn:uuid:bbe073ad-f449-4b25-91ac-7d919613ca51>,
    <urn:uuid:1b457bed-8a80-4135-92b8-fdea12b4eea3>,
    <urn:uuid:2153d83b-8555-44a3-96e0-821b6663a188>,
    <urn:uuid:2df6fac6-3122-44dc-9f92-5caab7f9b10b>,
    <urn:uuid:4bbcdde6-ed53-4f8d-b3f8-43f800fd05d5>;
  skos:prefLabel "XSLT"@en .

<urn:uuid:332a68b3-06d6-4ac2-8897-4212ba0f3a94> a skos:Concept;
  dct:created "2024-11-26T23:40:53Z"^^xsd:dateTime,
    "2021-12-14T20:52:05Z"^^xsd:dateTime,
    "2022-11-03T14:13:13Z"^^xsd:dateTime;
  dct:creator <urn:uuid:ca637d4b-c11b-4152-be98-bde602e7abd4>;
  skos:altLabel "opaque resource"@en;
  skos:broader <urn:uuid:79d6fcde-90b7-4f59-b4a9-937b09973432>,
    <urn:uuid:4039a99d-c14b-40f2-84d5-4ec72e2217e1>;
  skos:definition "We can say an information resource is opaque when the information system that surrounds it either cannot or does not inspect its contents. Opaque resources are typically stored, retrieved, and conveyed by the system as-is, and have a canonical literal representation from which all other representations are derived."@en;
  skos:inScheme <urn:uuid:0c7028f0-8226-47b3-acff-a4e83e6a60fd>,
    <urn:uuid:797e83d7-a86f-4838-b5c5-0ec20855197d>,
    <urn:uuid:bbe073ad-f449-4b25-91ac-7d919613ca51>,
    <urn:uuid:1b457bed-8a80-4135-92b8-fdea12b4eea3>,
    <urn:uuid:2153d83b-8555-44a3-96e0-821b6663a188>,
    <urn:uuid:2df6fac6-3122-44dc-9f92-5caab7f9b10b>,
    <urn:uuid:4bbcdde6-ed53-4f8d-b3f8-43f800fd05d5>;
  skos:prefLabel "opaque"@en;
  skos:related <urn:uuid:5bdd2fb7-d84d-4583-998b-7d3f2803307e>,
    <urn:uuid:5e2780c6-58f7-4ef9-8b1f-91fdcf4f8a6a> .

<urn:uuid:384f764c-9d71-46a3-9865-0af7068c0703> a skos:Concept;
  dct:created "2017-07-12T02:40:25Z"^^xsd:dateTime;
  dct:creator <urn:uuid:ca637d4b-c11b-4152-be98-bde602e7abd4>;
  dct:references <https://en.wikipedia.org/wiki/RDF_Schema>,
    <https://www.w3.org/TR/rdf-schema/>;
  skos:broader <urn:uuid:fe500c7a-b458-4d2c-8b3a-efd1bb47d106>;
  skos:definition "RDF Schema is an RDF vocabulary for expressing RDF vocabularies. Compared to its superset, OWL, RDF Schema is bare-bones, only specifying classes, properties, subclass and subproperty relations, and relations denoting the domains and ranges of properties."@en;
  skos:inScheme <urn:uuid:bbe073ad-f449-4b25-91ac-7d919613ca51>,
    <urn:uuid:75f35368-e228-47fe-8efd-7251a2bde816>,
    <urn:uuid:2df6fac6-3122-44dc-9f92-5caab7f9b10b>,
    <urn:uuid:91684d49-7b99-4b2e-9641-ea0b8e22f66c>,
    <urn:uuid:1b457bed-8a80-4135-92b8-fdea12b4eea3>,
    <urn:uuid:2153d83b-8555-44a3-96e0-821b6663a188>,
    <urn:uuid:a1a01f1c-7162-439c-94f1-3e28b99ae8ab>,
    <urn:uuid:ddfaaacc-9dcb-451b-afa6-477e6e787a5c>,
    <urn:uuid:4bbcdde6-ed53-4f8d-b3f8-43f800fd05d5>;
  skos:narrower <urn:uuid:ed4d30d7-d3cf-4b21-bcb4-5f2525027be7>;
  skos:prefLabel "RDF Schema"@en;
  skos:related <urn:uuid:f99b9a38-43c5-4219-8ca8-166c49b80ac1> .

<urn:uuid:3cdd469a-195b-4040-8d74-fd27bc71f12d> a skos:Concept;
  dct:created "2024-02-16T15:24:23Z"^^xsd:dateTime,
    "2024-11-26T23:40:53Z"^^xsd:dateTime,
    "2022-11-03T14:13:13Z"^^xsd:dateTime;
  dct:creator <urn:uuid:ca637d4b-c11b-4152-be98-bde602e7abd4>;
  skos:definition "An adapter bus is a bus (in computer science parlance, a trunking mechanism) for adapters. Assuming a set of adapters have relatively common behavior, that common behavior could be taken over by the bus, to which the adapters would act as plug-ins."@en;
  skos:inScheme <urn:uuid:797e83d7-a86f-4838-b5c5-0ec20855197d>,
    <urn:uuid:bbe073ad-f449-4b25-91ac-7d919613ca51>,
    <urn:uuid:2df6fac6-3122-44dc-9f92-5caab7f9b10b>,
    <urn:uuid:1b457bed-8a80-4135-92b8-fdea12b4eea3>,
    <urn:uuid:2153d83b-8555-44a3-96e0-821b6663a188>,
    <urn:uuid:4bbcdde6-ed53-4f8d-b3f8-43f800fd05d5>;
  skos:prefLabel "adapter bus"@en .

<urn:uuid:453f3a1b-7631-4943-a924-33b1455c3de2> a skos:Concept;
  dct:created "2022-11-23T21:45:36Z"^^xsd:dateTime;
  dct:creator <urn:uuid:ca637d4b-c11b-4152-be98-bde602e7abd4>;
  skos:definition "Markup is a general strategy for data representation (particularly but not necessarily text) where data structure and semantics are embedded into the content, as opposed to overlaid onto it."@en;
  skos:inScheme <urn:uuid:1b457bed-8a80-4135-92b8-fdea12b4eea3>,
    <urn:uuid:2153d83b-8555-44a3-96e0-821b6663a188>,
    <urn:uuid:bbe073ad-f449-4b25-91ac-7d919613ca51>,
    <urn:uuid:0c7028f0-8226-47b3-acff-a4e83e6a60fd>,
    <urn:uuid:4bbcdde6-ed53-4f8d-b3f8-43f800fd05d5>;
  skos:narrower <urn:uuid:df3de73d-3cb1-4b82-8773-415f1f16cbda>;
  skos:prefLabel "markup"@en .

<urn:uuid:4e296fcb-0a17-4397-970b-11e8813f7883> a skos:Concept;
  dct:created "2019-03-02T00:16:58Z"^^xsd:dateTime;
  dct:creator <urn:uuid:ca637d4b-c11b-4152-be98-bde602e7abd4>;
  skos:altLabel "Turing complete",
    "Turing completeness",
    "Turing-complete";
  skos:definition "A programming language is Turing-complete, roughly, if it is capable of self-reference, and thus capable of redefining its own behaviour. Such programs are mathematically impossible to determine whether or not they will carry out some particular (e.g., malicious) process at some point in the future or under what conditions, and thus can never be considered completely safe."@en;
  skos:inScheme <urn:uuid:bbe073ad-f449-4b25-91ac-7d919613ca51>,
    <urn:uuid:1b457bed-8a80-4135-92b8-fdea12b4eea3>,
    <urn:uuid:2153d83b-8555-44a3-96e0-821b6663a188>,
    <urn:uuid:75f35368-e228-47fe-8efd-7251a2bde816>,
    <urn:uuid:2df6fac6-3122-44dc-9f92-5caab7f9b10b>,
    <urn:uuid:4bbcdde6-ed53-4f8d-b3f8-43f800fd05d5>;
  skos:prefLabel "Turing-completeness"@en;
  skos:related <urn:uuid:33c3211f-322b-4f7a-83f6-63aa617461c3>,
    <urn:uuid:5abd5284-7197-4eed-895d-6daefa019de8> .

<urn:uuid:5b30faaa-7c8b-4c57-8dc5-26bd63047d3f> a skos:Concept;
  dct:created "2018-03-06T21:48:41Z"^^xsd:dateTime;
  dct:creator <urn:uuid:ca637d4b-c11b-4152-be98-bde602e7abd4>;
  dct:references <http://bibliontology.com/>;
  skos:definition "The bibliographic ontology offers numerous extensions of foaf:Document for use in bibliographic citations."@en;
  skos:inScheme <urn:uuid:75f35368-e228-47fe-8efd-7251a2bde816>,
    <urn:uuid:91684d49-7b99-4b2e-9641-ea0b8e22f66c>,
    <urn:uuid:bbe073ad-f449-4b25-91ac-7d919613ca51>,
    <urn:uuid:1b457bed-8a80-4135-92b8-fdea12b4eea3>,
    <urn:uuid:2153d83b-8555-44a3-96e0-821b6663a188>,
    <urn:uuid:2df6fac6-3122-44dc-9f92-5caab7f9b10b>,
    <urn:uuid:4bbcdde6-ed53-4f8d-b3f8-43f800fd05d5>;
  skos:prefLabel "Bibliographic Ontology"@en .

<urn:uuid:5e2780c6-58f7-4ef9-8b1f-91fdcf4f8a6a> a skos:Concept;
  dct:created "2021-09-24T13:14:38Z"^^xsd:dateTime;
  dct:creator <urn:uuid:ca637d4b-c11b-4152-be98-bde602e7abd4>;
  dct:modified "2021-12-14T23:12:28Z"^^xsd:dateTime;
  skos:altLabel "transparent resource"@en;
  skos:broader <urn:uuid:4039a99d-c14b-40f2-84d5-4ec72e2217e1>,
    <urn:uuid:79d6fcde-90b7-4f59-b4a9-937b09973432>;
  skos:definition "An information resource can be said to be transparent if the information system surrounding it can, or indeed must, inspect its contents in order to address them. Transparent resources typically do not have canonical representations as all (lossless) representations are equivalent. Contrast with opaque resources."@en;
  skos:inScheme <urn:uuid:797e83d7-a86f-4838-b5c5-0ec20855197d>,
    <urn:uuid:bbe073ad-f449-4b25-91ac-7d919613ca51>,
    <urn:uuid:2df6fac6-3122-44dc-9f92-5caab7f9b10b>,
    <urn:uuid:1b457bed-8a80-4135-92b8-fdea12b4eea3>,
    <urn:uuid:2153d83b-8555-44a3-96e0-821b6663a188>,
    <urn:uuid:0c7028f0-8226-47b3-acff-a4e83e6a60fd>,
    <urn:uuid:4bbcdde6-ed53-4f8d-b3f8-43f800fd05d5>;
  skos:prefLabel "transparent"@en .

<urn:uuid:68e38d88-1afd-4443-a1a4-f28abd9dc77d> a skos:Concept;
  dct:alternative "Content negotiation is the act of superimposing multiple representations of a the same resource onto the same location. The HTTP protocol supports five dimensions (e.g. file type,  written language, character set...) of content negotiation, and thus every URL can potentially locate the Cartesian product of concrete representations for a given abstract resource."@en;
  dct:created "2019-03-02T03:11:38Z"^^xsd:dateTime;
  dct:creator <urn:uuid:ca637d4b-c11b-4152-be98-bde602e7abd4>;
  dct:description "Content negotiation is the act of superimposing multiple representations of a the same resource onto the same location. The HTTP protocol supports five dimensions (e.g. file type,  written language, character set...) of content negotiation, and thus every URL can potentially locate the Cartesian product of concrete representations for a given abstract resource."@en;
  dct:modified "2021-12-14T16:38:12Z"^^xsd:dateTime;
  skos:altLabel "content negotiation"@en,
    "conneg"@en;
  skos:definition "Content negotiation is the act of superimposing multiple representations of a the same resource onto the same location. The HTTP protocol supports five dimensions (e.g. file type,  written language, character set...) of content negotiation, and thus every URL can potentially locate the Cartesian product of concrete representations for a given abstract resource."@en,
    "Content negotiation is a long-standing feature of HTTP that affords the varying of representations of a resource at a given URI along a number of different dimensions. Two dimensions of particular interest are content type and natural language."@en;
  skos:hiddenLabel "conneg"@en,
    "con-neg"@en;
  skos:inScheme <urn:uuid:2df6fac6-3122-44dc-9f92-5caab7f9b10b>,
    <urn:uuid:0c7028f0-8226-47b3-acff-a4e83e6a60fd>,
    <urn:uuid:797e83d7-a86f-4838-b5c5-0ec20855197d>,
    <urn:uuid:bbe073ad-f449-4b25-91ac-7d919613ca51>,
    <urn:uuid:75f35368-e228-47fe-8efd-7251a2bde816>,
    <urn:uuid:1b457bed-8a80-4135-92b8-fdea12b4eea3>,
    <urn:uuid:2153d83b-8555-44a3-96e0-821b6663a188>,
    <urn:uuid:4bbcdde6-ed53-4f8d-b3f8-43f800fd05d5>;
  skos:prefLabel "content negotiation"@en;
  skos:related <urn:uuid:9b56c5ee-7c41-4dc3-920f-f8d11ca869cf>,
    <urn:uuid:027543f6-04df-4e92-96f4-5b0c8da4b799>,
    <urn:uuid:02b3d282-d134-487b-8226-80141b5a4338>,
    <urn:uuid:4039a99d-c14b-40f2-84d5-4ec72e2217e1>,
    <urn:uuid:5bdd2fb7-d84d-4583-998b-7d3f2803307e>,
    <urn:uuid:9e506ca3-8be1-431d-9075-548141d9f8c1>,
    <urn:uuid:e162d03b-bfec-4f01-ab7e-56da309550f6> .

<urn:uuid:770bfd11-d9d3-4e5a-8285-13fcff030de6> a skos:Concept;
  dct:created "2021-12-14T20:56:28Z"^^xsd:dateTime;
  dct:creator <urn:uuid:ca637d4b-c11b-4152-be98-bde602e7abd4>;
  dct:description "In Web (or in general networked information system) parlance, an origin (as opposed to a proxy) is the authoritative source of information."@en;
  dct:modified "2022-11-24T01:16:07Z"^^xsd:dateTime;
  skos:altLabel "origin server"@en;
  skos:definition "In a layered system, and in particular with Web systems, an origin server is one that is an authoritative source for content. This is in contrast to something like a (reverse) proxy, which only acts as an intermediary and houses no content of its own."@en;
  skos:inScheme <urn:uuid:1b457bed-8a80-4135-92b8-fdea12b4eea3>,
    <urn:uuid:2153d83b-8555-44a3-96e0-821b6663a188>,
    <urn:uuid:a1a01f1c-7162-439c-94f1-3e28b99ae8ab>,
    <urn:uuid:ddfaaacc-9dcb-451b-afa6-477e6e787a5c>,
    <urn:uuid:2df6fac6-3122-44dc-9f92-5caab7f9b10b>,
    <urn:uuid:0c7028f0-8226-47b3-acff-a4e83e6a60fd>,
    <urn:uuid:797e83d7-a86f-4838-b5c5-0ec20855197d>,
    <urn:uuid:bbe073ad-f449-4b25-91ac-7d919613ca51>,
    <urn:uuid:4bbcdde6-ed53-4f8d-b3f8-43f800fd05d5>;
  skos:prefLabel "origin"@en .

<urn:uuid:7ddb6eed-d37d-4412-9c10-eff42447eddf> a skos:Concept;
  dct:created "2021-12-14T22:48:02Z"^^xsd:dateTime;
  dct:creator <urn:uuid:ca637d4b-c11b-4152-be98-bde602e7abd4>;
  skos:altLabel "SaaS"@en,
    "cloud"@en;
  skos:definition "SaaS is a special, albeit common, case of utility (cloud) computing, in which access to some particular functionality—often but not exclusively user-facing application software—is what is being rented, rather than just the raw computing resources. Examples of SaaS are services like GMail, Twilio, or Salesforce."@en;
  skos:hiddenLabel "saas"@en;
  skos:inScheme <urn:uuid:2df6fac6-3122-44dc-9f92-5caab7f9b10b>,
    <urn:uuid:797e83d7-a86f-4838-b5c5-0ec20855197d>,
    <urn:uuid:a1a01f1c-7162-439c-94f1-3e28b99ae8ab>,
    <urn:uuid:ddfaaacc-9dcb-451b-afa6-477e6e787a5c>,
    <urn:uuid:1b457bed-8a80-4135-92b8-fdea12b4eea3>,
    <urn:uuid:2153d83b-8555-44a3-96e0-821b6663a188>,
    <urn:uuid:bbe073ad-f449-4b25-91ac-7d919613ca51>,
    <urn:uuid:4bbcdde6-ed53-4f8d-b3f8-43f800fd05d5>;
  skos:prefLabel "software-as-a-service"@en .

<urn:uuid:87cc031a-dab5-41cb-8c86-5225565a0534> a skos:Concept;
  dct:created "2017-06-07T20:31:49Z"^^xsd:dateTime;
  dct:creator <urn:uuid:ca637d4b-c11b-4152-be98-bde602e7abd4>;
  skos:altLabel "DSL"@en;
  skos:broader <urn:uuid:33c3211f-322b-4f7a-83f6-63aa617461c3>;
  skos:definition "A domain-specific language is a programming language optimized for, or indeed only capable of, some particular category of application. Contrast with a general-purpose language, which can typically be used for anything."@en;
  skos:inScheme <urn:uuid:49ac68c4-922c-4d9e-88fa-b318fc54d36f>,
    <urn:uuid:0c7028f0-8226-47b3-acff-a4e83e6a60fd>,
    <urn:uuid:1b457bed-8a80-4135-92b8-fdea12b4eea3>,
    <urn:uuid:2153d83b-8555-44a3-96e0-821b6663a188>,
    <urn:uuid:2df6fac6-3122-44dc-9f92-5caab7f9b10b>,
    <urn:uuid:bbe073ad-f449-4b25-91ac-7d919613ca51>,
    <urn:uuid:4bbcdde6-ed53-4f8d-b3f8-43f800fd05d5>;
  skos:prefLabel "domain-specific language"@en .

<urn:uuid:8cb5c042-8ce4-4d8d-a4c0-dd47d90e4bf5> a skos:Concept;
  dct:created "2021-12-14T01:51:36Z"^^xsd:dateTime;
  dct:creator <urn:uuid:ca637d4b-c11b-4152-be98-bde602e7abd4>;
  skos:altLabel "AST"@en;
  skos:definition "An abstract syntax tree is a representation of software code which has been tokenized and parsed, and is typically the penultimate step before the code's semantics are interpreted. It is a convenient representation for navigating the different structural elements of the code."@en;
  skos:inScheme <urn:uuid:2df6fac6-3122-44dc-9f92-5caab7f9b10b>,
    <urn:uuid:797e83d7-a86f-4838-b5c5-0ec20855197d>,
    <urn:uuid:bbe073ad-f449-4b25-91ac-7d919613ca51>,
    <urn:uuid:1b457bed-8a80-4135-92b8-fdea12b4eea3>,
    <urn:uuid:2153d83b-8555-44a3-96e0-821b6663a188>,
    <urn:uuid:4bbcdde6-ed53-4f8d-b3f8-43f800fd05d5>;
  skos:prefLabel "abstract syntax tree"@en .

<urn:uuid:91bffd8d-1f18-4604-844e-6a5557947a67> a skos:Concept;
  dct:created "2021-12-14T20:45:01Z"^^xsd:dateTime;
  dct:creator <urn:uuid:ca637d4b-c11b-4152-be98-bde602e7abd4>;
  skos:broader <urn:uuid:42a48e75-a413-4b91-8787-a8c2dc1a65ed>,
    <urn:uuid:935ab72b-b74c-4204-9c00-f1f8f83f105e>;
  skos:definition "A web API is an API that has been implemented over HTTP. Web APIs often use JSON to transfer payloads and give a passing nod to REST."@en;
  skos:inScheme <urn:uuid:1b457bed-8a80-4135-92b8-fdea12b4eea3>,
    <urn:uuid:2153d83b-8555-44a3-96e0-821b6663a188>,
    <urn:uuid:2df6fac6-3122-44dc-9f92-5caab7f9b10b>,
    <urn:uuid:797e83d7-a86f-4838-b5c5-0ec20855197d>,
    <urn:uuid:a1a01f1c-7162-439c-94f1-3e28b99ae8ab>,
    <urn:uuid:ddfaaacc-9dcb-451b-afa6-477e6e787a5c>,
    <urn:uuid:bbe073ad-f449-4b25-91ac-7d919613ca51>,
    <urn:uuid:4bbcdde6-ed53-4f8d-b3f8-43f800fd05d5>;
  skos:prefLabel "Web API"@en;
  skos:related <urn:uuid:02b3d282-d134-487b-8226-80141b5a4338>,
    <urn:uuid:288e85ab-887f-437c-9caa-c109cb9d478d>,
    <urn:uuid:ca632e87-50d2-4f1d-af83-f3d11e53eca8> .

<urn:uuid:9283f8a5-c02f-4f5d-af14-3a9648e5639f> a skos:Concept;
  dct:created "2022-11-23T23:45:40Z"^^xsd:dateTime;
  dct:creator <urn:uuid:ca637d4b-c11b-4152-be98-bde602e7abd4>;
  skos:definition "Content governance is the practice of managing the life cycle of content within an organization, and setting policies for content strategy and information architecture."@en;
  skos:inScheme <urn:uuid:1b457bed-8a80-4135-92b8-fdea12b4eea3>,
    <urn:uuid:2153d83b-8555-44a3-96e0-821b6663a188>,
    <urn:uuid:a1a01f1c-7162-439c-94f1-3e28b99ae8ab>,
    <urn:uuid:ddfaaacc-9dcb-451b-afa6-477e6e787a5c>,
    <urn:uuid:bbe073ad-f449-4b25-91ac-7d919613ca51>,
    <urn:uuid:0c7028f0-8226-47b3-acff-a4e83e6a60fd>,
    <urn:uuid:4bbcdde6-ed53-4f8d-b3f8-43f800fd05d5>;
  skos:prefLabel "content governance"@en .

<urn:uuid:96a2b1d2-732d-45a1-addb-a8cbb9868480> a skos:Concept;
  dct:created "2017-02-21T20:00:54Z"^^xsd:dateTime;
  dct:creator <urn:uuid:ca637d4b-c11b-4152-be98-bde602e7abd4>;
  skos:broader <urn:uuid:d0d7da4b-4d4d-4262-96a3-a70afbc1a829>;
  skos:definition "A password is a secret intended to be known only by the person (or people) who are authorized to access an account."@en;
  skos:inScheme <urn:uuid:49ac68c4-922c-4d9e-88fa-b318fc54d36f>,
    <urn:uuid:1b457bed-8a80-4135-92b8-fdea12b4eea3>,
    <urn:uuid:2153d83b-8555-44a3-96e0-821b6663a188>,
    <urn:uuid:2df6fac6-3122-44dc-9f92-5caab7f9b10b>,
    <urn:uuid:bbe073ad-f449-4b25-91ac-7d919613ca51>,
    <urn:uuid:4bbcdde6-ed53-4f8d-b3f8-43f800fd05d5>;
  skos:prefLabel "password"@en .

<urn:uuid:9adc8b42-bbd1-4065-bb57-9a789253c4e4> a skos:Concept;
  dct:created "2021-12-14T16:10:23Z"^^xsd:dateTime;
  dct:creator <urn:uuid:ca637d4b-c11b-4152-be98-bde602e7abd4>;
  skos:definition "A content-addressable store is a form of opaque blob storage where the method of indexing and retrieval is derived from the content itself. This derivation is almost always one or more cryptographic digests from a chosen set of algorithms."@en;
  skos:hiddenLabel "content-addressable storage"@en;
  skos:inScheme <urn:uuid:2df6fac6-3122-44dc-9f92-5caab7f9b10b>,
    <urn:uuid:1b457bed-8a80-4135-92b8-fdea12b4eea3>,
    <urn:uuid:2153d83b-8555-44a3-96e0-821b6663a188>,
    <urn:uuid:0c7028f0-8226-47b3-acff-a4e83e6a60fd>,
    <urn:uuid:797e83d7-a86f-4838-b5c5-0ec20855197d>,
    <urn:uuid:bbe073ad-f449-4b25-91ac-7d919613ca51>,
    <urn:uuid:4bbcdde6-ed53-4f8d-b3f8-43f800fd05d5>;
  skos:prefLabel "content-addressable store"@en;
  skos:related <urn:uuid:b43684d3-ac8c-4804-b490-8e29a582cfc7> .

<urn:uuid:9ed8a948-df9f-4ee3-95d1-47b28174b6a8> a skos:Concept;
  dct:created "2019-02-28T19:00:46Z"^^xsd:dateTime;
  dct:creator <urn:uuid:ca637d4b-c11b-4152-be98-bde602e7abd4>;
  skos:broader <urn:uuid:f352a521-b78e-478e-b01d-3a68638025a4>;
  skos:definition "Really Simple Syndication (2.0) is an XML vocabulary designed by Dave Winer to compete with RSS 1.0. It has no genealogical relation to RSS 1.0."@en;
  skos:inScheme <urn:uuid:75f35368-e228-47fe-8efd-7251a2bde816>,
    <urn:uuid:2df6fac6-3122-44dc-9f92-5caab7f9b10b>,
    <urn:uuid:1b457bed-8a80-4135-92b8-fdea12b4eea3>,
    <urn:uuid:2153d83b-8555-44a3-96e0-821b6663a188>,
    <urn:uuid:bbe073ad-f449-4b25-91ac-7d919613ca51>,
    <urn:uuid:4bbcdde6-ed53-4f8d-b3f8-43f800fd05d5>;
  skos:prefLabel "RSS 2.0"@en;
  skos:related <urn:uuid:ba2258e3-efca-4461-82cc-f6ebbf980b36> .

<urn:uuid:a43e33d9-1788-4514-8fbd-1b4982535f73> a skos:Concept;
  dct:alternative "A knowledge graph is a hypermedia system where the resources represent objects rather than documents."@en;
  dct:created "2021-12-14T20:19:08Z"^^xsd:dateTime;
  dct:creator <urn:uuid:ca637d4b-c11b-4152-be98-bde602e7abd4>;
  dct:description "A knowledge graph is a hypermedia system where the resources represent objects rather than documents."@en;
  dct:modified "2022-06-02T01:59:39Z"^^xsd:dateTime;
  skos:altLabel "Knowledge Graph"@en;
  skos:broader <urn:uuid:c6ab3854-e8a7-4cd8-8ca3-3928d926f224>;
  skos:definition "A knowledge graph is a buzzphrase for a database structured as a directed graph, giving it the unique ability to make arbitrary connections between heterogeneous entities within the database. Knowledge graphs may or may not be created on top of RDF. This set of documents is an RDF knowledge graph."@en;
  skos:inScheme <urn:uuid:2df6fac6-3122-44dc-9f92-5caab7f9b10b>,
    <urn:uuid:0c7028f0-8226-47b3-acff-a4e83e6a60fd>,
    <urn:uuid:a1a01f1c-7162-439c-94f1-3e28b99ae8ab>,
    <urn:uuid:ddfaaacc-9dcb-451b-afa6-477e6e787a5c>,
    <urn:uuid:2153d83b-8555-44a3-96e0-821b6663a188>,
    <urn:uuid:1b457bed-8a80-4135-92b8-fdea12b4eea3>,
    <urn:uuid:797e83d7-a86f-4838-b5c5-0ec20855197d>,
    <urn:uuid:bbe073ad-f449-4b25-91ac-7d919613ca51>,
    <urn:uuid:4bbcdde6-ed53-4f8d-b3f8-43f800fd05d5>;
  skos:narrower <urn:uuid:f477beaf-1b44-42dd-88b6-69857070627d>,
    <urn:uuid:0f872daf-97f4-445e-b5d9-0de0087dd129>;
  skos:prefLabel "knowledge graph"@en;
  skos:related <urn:uuid:fe500c7a-b458-4d2c-8b3a-efd1bb47d106> .

<urn:uuid:b097ff77-48cb-4b65-a433-a4aac8abe2ee> a skos:Concept;
  dct:created "2024-07-03T21:27:51Z"^^xsd:dateTime,
    "2022-11-03T14:13:13Z"^^xsd:dateTime,
    "2024-07-25T15:19:18Z"^^xsd:dateTime,
    "2020-04-26T15:10:48Z"^^xsd:dateTime,
    "2024-02-16T15:24:23Z"^^xsd:dateTime;
  dct:creator <urn:uuid:ca637d4b-c11b-4152-be98-bde602e7abd4>;
  rdfs:seeAlso <https://en.wikipedia.org/wiki/Wicked_problem>;
  skos:definition "Wicked problems, a term coined by Horst Rittel, refer to a category of problems which are complex, dynamic, with multiple stakeholders, and often involve considerable trade-offs. The quintessential wicked problem is climate change."@en;
  skos:inScheme <urn:uuid:0c7028f0-8226-47b3-acff-a4e83e6a60fd>,
    <urn:uuid:bbe073ad-f449-4b25-91ac-7d919613ca51>,
    <urn:uuid:2df6fac6-3122-44dc-9f92-5caab7f9b10b>,
    <urn:uuid:a1a01f1c-7162-439c-94f1-3e28b99ae8ab>,
    <urn:uuid:ddfaaacc-9dcb-451b-afa6-477e6e787a5c>,
    <urn:uuid:1b457bed-8a80-4135-92b8-fdea12b4eea3>,
    <urn:uuid:2153d83b-8555-44a3-96e0-821b6663a188>,
    <urn:uuid:d4317ece-d4aa-40cb-9df1-1b058cbc24d8>,
    <urn:uuid:4bbcdde6-ed53-4f8d-b3f8-43f800fd05d5>;
  skos:prefLabel "wicked problem"@en .

<urn:uuid:b20221c0-4949-471a-adb1-45dfccfbdf1c> a skos:Concept;
  dct:created "2017-02-16T23:23:12Z"^^xsd:dateTime;
  dct:creator <urn:uuid:ca637d4b-c11b-4152-be98-bde602e7abd4>;
  skos:broader <urn:uuid:ad6b1b9b-fec4-4378-b8dd-7bbc07a3d706>,
    <urn:uuid:10bafb58-6eb8-4d99-9b7d-9840842d3947>,
    <urn:uuid:759d2f68-3d16-4122-9758-c84f7760d691>,
    <urn:uuid:935ab72b-b74c-4204-9c00-f1f8f83f105e>,
    <urn:uuid:be93cce1-f21f-4e85-bd34-e005dea3532f>;
  skos:definition "An Intranet is a synonym for a local (e.g. office) computer network. Colloquially, it refers to an internal website or Web application."@en;
  skos:inScheme <urn:uuid:49ac68c4-922c-4d9e-88fa-b318fc54d36f>,
    <urn:uuid:2df6fac6-3122-44dc-9f92-5caab7f9b10b>,
    <urn:uuid:a1a01f1c-7162-439c-94f1-3e28b99ae8ab>,
    <urn:uuid:ddfaaacc-9dcb-451b-afa6-477e6e787a5c>,
    <urn:uuid:bbe073ad-f449-4b25-91ac-7d919613ca51>,
    <urn:uuid:1b457bed-8a80-4135-92b8-fdea12b4eea3>,
    <urn:uuid:2153d83b-8555-44a3-96e0-821b6663a188>,
    <urn:uuid:4bbcdde6-ed53-4f8d-b3f8-43f800fd05d5>;
  skos:prefLabel "intranet"@en .

<urn:uuid:b801e469-101d-4305-866d-edb0f70979de> a skos:Concept;
  dct:created "2017-02-01T23:38:28Z"^^xsd:dateTime;
  dct:creator <urn:uuid:ca637d4b-c11b-4152-be98-bde602e7abd4>;
  rdfs:seeAlso <urn:isbn:9780801855795>,
    <https://www.press.jhu.edu/books/title/1398/cybertext>;
  skos:definition "Cybertext is a generalization of the concept of hypertext to include non-deterministic processes."@en;
  skos:inScheme <urn:uuid:bbe073ad-f449-4b25-91ac-7d919613ca51>,
    <urn:uuid:1b457bed-8a80-4135-92b8-fdea12b4eea3>,
    <urn:uuid:2153d83b-8555-44a3-96e0-821b6663a188>,
    <urn:uuid:49ac68c4-922c-4d9e-88fa-b318fc54d36f>,
    <urn:uuid:2df6fac6-3122-44dc-9f92-5caab7f9b10b>,
    <urn:uuid:a1a01f1c-7162-439c-94f1-3e28b99ae8ab>,
    <urn:uuid:ddfaaacc-9dcb-451b-afa6-477e6e787a5c>,
    <urn:uuid:4bbcdde6-ed53-4f8d-b3f8-43f800fd05d5>;
  skos:narrower <urn:uuid:9fc41de2-b16c-4170-8818-893302baa77d>;
  skos:prefLabel "cybertext"@en .

<urn:uuid:b8565dd1-8c4d-4699-a240-56898fc32ac8> a skos:Concept;
  dct:created "2017-02-20T01:10:15Z"^^xsd:dateTime;
  dct:creator <urn:uuid:ca637d4b-c11b-4152-be98-bde602e7abd4>;
  skos:definition "A (data) dimension is the same thing as a \"column\" in Excel, at least when each column is being treated as a separate field, or distinct kind of thing. In this usage, each row is a record with possibly many dimensions. If the spreadsheet is being treated as a grid instead, then there are only two dimensions: all columns and all rows."@en;
  skos:inScheme <urn:uuid:1b457bed-8a80-4135-92b8-fdea12b4eea3>,
    <urn:uuid:2153d83b-8555-44a3-96e0-821b6663a188>,
    <urn:uuid:2df6fac6-3122-44dc-9f92-5caab7f9b10b>,
    <urn:uuid:49ac68c4-922c-4d9e-88fa-b318fc54d36f>,
    <urn:uuid:bbe073ad-f449-4b25-91ac-7d919613ca51>,
    <urn:uuid:4bbcdde6-ed53-4f8d-b3f8-43f800fd05d5>;
  skos:prefLabel "dimension"@en;
  skos:related <urn:uuid:9767147a-1b6a-440c-949f-7f6056e28411> .

<urn:uuid:b95d0656-3b14-4e38-8fe2-75401ff7ee31> a skos:Concept;
  dct:created "2020-04-26T14:19:02Z"^^xsd:dateTime;
  dct:creator <urn:uuid:ca637d4b-c11b-4152-be98-bde602e7abd4>;
  rdfs:seeAlso <https://en.wikipedia.org/wiki/Issue-based_information_system>,
    <https://en.wikipedia.org/wiki/Horst_Rittel>;
  skos:altLabel "IBIS"@en;
  skos:definition "Issue-Based Information System refers to a particular methodology for structured argumentation invented by Horst Rittel and collaborators in the late 1960s, intended to provide design rationale and support for solving wicked problems. The system was originally implemented using index cards, though digital versions have existed since the 1980s."@en;
  skos:inScheme <urn:uuid:1b457bed-8a80-4135-92b8-fdea12b4eea3>,
    <urn:uuid:bbe073ad-f449-4b25-91ac-7d919613ca51>,
    <urn:uuid:2df6fac6-3122-44dc-9f92-5caab7f9b10b>,
    <urn:uuid:2153d83b-8555-44a3-96e0-821b6663a188>,
    <urn:uuid:0c7028f0-8226-47b3-acff-a4e83e6a60fd>,
    <urn:uuid:a1a01f1c-7162-439c-94f1-3e28b99ae8ab>,
    <urn:uuid:ddfaaacc-9dcb-451b-afa6-477e6e787a5c>,
    <urn:uuid:4bbcdde6-ed53-4f8d-b3f8-43f800fd05d5>;
  skos:prefLabel "Issue-Based Information System"@en;
  skos:related <urn:uuid:b097ff77-48cb-4b65-a433-a4aac8abe2ee> .

<urn:uuid:b99ffccd-0042-4e5a-a4ce-b58cbdcf3ef9> a skos:Concept;
  dct:created "2022-11-23T21:53:54Z"^^xsd:dateTime;
  dct:creator <urn:uuid:ca637d4b-c11b-4152-be98-bde602e7abd4>;
  skos:broader <urn:uuid:453f3a1b-7631-4943-a924-33b1455c3de2>;
  skos:definition "Presentation markup is the subset of markup that forms the basis for (e.g.) a document's presentation. In contrast to structural markup, presentation markup can be removed from the document without changing the meaning of the content."@en;
  skos:inScheme <urn:uuid:bbe073ad-f449-4b25-91ac-7d919613ca51>,
    <urn:uuid:1b457bed-8a80-4135-92b8-fdea12b4eea3>,
    <urn:uuid:2153d83b-8555-44a3-96e0-821b6663a188>,
    <urn:uuid:0c7028f0-8226-47b3-acff-a4e83e6a60fd>,
    <urn:uuid:4bbcdde6-ed53-4f8d-b3f8-43f800fd05d5>;
  skos:prefLabel "presentation markup"@en .

<urn:uuid:bf986385-65ff-424e-8eb1-6c6653cb6b4e> a skos:Concept;
  dct:created "2019-03-07T01:04:30Z"^^xsd:dateTime,
    "2022-11-03T14:13:13Z"^^xsd:dateTime,
    "2018-04-26T22:51:11Z"^^xsd:dateTime,
    "2024-02-16T15:24:23Z"^^xsd:dateTime;
  dct:creator <urn:uuid:ca637d4b-c11b-4152-be98-bde602e7abd4>;
  skos:inScheme <urn:uuid:75f35368-e228-47fe-8efd-7251a2bde816>,
    <urn:uuid:1b457bed-8a80-4135-92b8-fdea12b4eea3>,
    <urn:uuid:2153d83b-8555-44a3-96e0-821b6663a188>,
    <urn:uuid:2df6fac6-3122-44dc-9f92-5caab7f9b10b>,
    <urn:uuid:91684d49-7b99-4b2e-9641-ea0b8e22f66c>,
    <urn:uuid:bbe073ad-f449-4b25-91ac-7d919613ca51>,
    <urn:uuid:4bbcdde6-ed53-4f8d-b3f8-43f800fd05d5>;
  skos:prefLabel "RDF Data Cube Vocabulary"@en .

<urn:uuid:c38fdbb2-201b-4a88-9273-26fbd0c6fae5> a skos:Concept;
  dct:created "2021-12-14T01:10:58Z"^^xsd:dateTime;
  dct:creator <urn:uuid:ca637d4b-c11b-4152-be98-bde602e7abd4>;
  skos:definition "A caching reverse proxy is a reverse proxy with the addition of a cache."@en;
  skos:hiddenLabel "caching reverse proxy"@en;
  skos:inScheme <urn:uuid:0c7028f0-8226-47b3-acff-a4e83e6a60fd>,
    <urn:uuid:2df6fac6-3122-44dc-9f92-5caab7f9b10b>,
    <urn:uuid:1b457bed-8a80-4135-92b8-fdea12b4eea3>,
    <urn:uuid:2153d83b-8555-44a3-96e0-821b6663a188>,
    <urn:uuid:797e83d7-a86f-4838-b5c5-0ec20855197d>,
    <urn:uuid:bbe073ad-f449-4b25-91ac-7d919613ca51>,
    <urn:uuid:a1a01f1c-7162-439c-94f1-3e28b99ae8ab>,
    <urn:uuid:ddfaaacc-9dcb-451b-afa6-477e6e787a5c>,
    <urn:uuid:4bbcdde6-ed53-4f8d-b3f8-43f800fd05d5>;
  skos:narrower <urn:uuid:1417392d-ce8c-4357-8d38-8570258da6a6>;
  skos:prefLabel "caching reverse proxy"@en .

<urn:uuid:c6ab3854-e8a7-4cd8-8ca3-3928d926f224> a skos:Concept;
  dct:created "2021-12-14T18:10:14Z"^^xsd:dateTime;
  dct:creator <urn:uuid:ca637d4b-c11b-4152-be98-bde602e7abd4>;
  skos:definition "A directed graph is a mathematical object consisting of a set of nodes and a set of ordered pairs that connect the nodes together. Directed graphs are absolutely everywhere in computing."@en;
  skos:hiddenLabel "directed graph"@en;
  skos:inScheme <urn:uuid:0c7028f0-8226-47b3-acff-a4e83e6a60fd>,
    <urn:uuid:2df6fac6-3122-44dc-9f92-5caab7f9b10b>,
    <urn:uuid:1b457bed-8a80-4135-92b8-fdea12b4eea3>,
    <urn:uuid:2153d83b-8555-44a3-96e0-821b6663a188>,
    <urn:uuid:797e83d7-a86f-4838-b5c5-0ec20855197d>,
    <urn:uuid:bbe073ad-f449-4b25-91ac-7d919613ca51>,
    <urn:uuid:4bbcdde6-ed53-4f8d-b3f8-43f800fd05d5>;
  skos:narrower <urn:uuid:5495f814-fd98-4b43-aba3-9e63a2063fd5>;
  skos:prefLabel "directed graph"@en .

<urn:uuid:c7066ab9-ad6b-4a19-b682-d919827eec71> a skos:Concept;
  dct:created "2019-03-02T01:41:39Z"^^xsd:dateTime;
  dct:creator <urn:uuid:ca637d4b-c11b-4152-be98-bde602e7abd4>;
  skos:broader <urn:uuid:33c3211f-322b-4f7a-83f6-63aa617461c3>;
  skos:definition "WebAssembly is an assembly language for virtual machines such as those found in a Web browser. Being an assembly language, it is a compilation target for any ahead-of-time compiled programming language. The net effect of WebAssembly is that a Web browser is now a general-purpose computing environment that can run arbitrary programs."@en;
  skos:inScheme <urn:uuid:75f35368-e228-47fe-8efd-7251a2bde816>,
    <urn:uuid:bbe073ad-f449-4b25-91ac-7d919613ca51>,
    <urn:uuid:2df6fac6-3122-44dc-9f92-5caab7f9b10b>,
    <urn:uuid:1b457bed-8a80-4135-92b8-fdea12b4eea3>,
    <urn:uuid:2153d83b-8555-44a3-96e0-821b6663a188>,
    <urn:uuid:4bbcdde6-ed53-4f8d-b3f8-43f800fd05d5>;
  skos:prefLabel "WebAssembly"@en .

<urn:uuid:cbc4f4d6-96a1-44fc-8f07-e3282626fe3f> a skos:Concept;
  dct:created "2019-02-28T06:33:16Z"^^xsd:dateTime;
  dct:creator <urn:uuid:ca637d4b-c11b-4152-be98-bde602e7abd4>;
  skos:inScheme <urn:uuid:75f35368-e228-47fe-8efd-7251a2bde816>,
    <urn:uuid:bbe073ad-f449-4b25-91ac-7d919613ca51>,
    <urn:uuid:2df6fac6-3122-44dc-9f92-5caab7f9b10b>,
    <urn:uuid:1b457bed-8a80-4135-92b8-fdea12b4eea3>,
    <urn:uuid:2153d83b-8555-44a3-96e0-821b6663a188>,
    <urn:uuid:4bbcdde6-ed53-4f8d-b3f8-43f800fd05d5>;
  skos:prefLabel "content/presentation separation"@en;
  skos:related <urn:uuid:123bcb4d-b7e1-4715-b95b-73161516e789>,
    <urn:uuid:2f6700a6-9ecb-47af-8106-a652b4c852e5>,
    <urn:uuid:f352a521-b78e-478e-b01d-3a68638025a4> .

<urn:uuid:cc74f8e0-34cc-4a69-b9d5-87b990aca6b6> a skos:Concept;
  dct:created "2021-12-14T19:21:54Z"^^xsd:dateTime;
  dct:creator <urn:uuid:ca637d4b-c11b-4152-be98-bde602e7abd4>;
  dct:description "In many programming languages, a function is synonymous with a subroutine. In some, however, it carries the additional constraint that it does not produce side effects, thus making it conceptually closer to the word's meaning in mathematics."@en;
  dct:modified "2022-11-23T23:13:05Z"^^xsd:dateTime;
  skos:altLabel "function"@en, "pure function"@en;
  skos:broader <urn:uuid:db2fb779-83e8-407b-a538-5fe9a86271de>;
  skos:definition "A pure function—a necessary distinction in computing, as in mathematics, a function is just a relation, and inherently “pure”—is a procedure that takes an input and returns a value without causing any side effects. This makes them very predictable and well-behaved development targets. Pure functions, like their mathematical counterparts, are therefore composable."@en,
    "In many programming languages, a function is synonymous with a subroutine. In some, however, it carries the additional constraint that it does not produce side effects, thus making it conceptually closer to the word's meaning in mathematics."@en;
  skos:inScheme <urn:uuid:797e83d7-a86f-4838-b5c5-0ec20855197d>,
    <urn:uuid:bbe073ad-f449-4b25-91ac-7d919613ca51>,
    <urn:uuid:1b457bed-8a80-4135-92b8-fdea12b4eea3>,
    <urn:uuid:2153d83b-8555-44a3-96e0-821b6663a188>,
    <urn:uuid:2df6fac6-3122-44dc-9f92-5caab7f9b10b>,
    <urn:uuid:0c7028f0-8226-47b3-acff-a4e83e6a60fd>,
    <urn:uuid:4bbcdde6-ed53-4f8d-b3f8-43f800fd05d5>;
  skos:prefLabel "(pure) function"@en;
  skos:related <urn:uuid:117ac161-9f62-4075-8ac5-9a4e7f09fd1d>,
    <urn:uuid:1ba688e9-6a85-4596-be01-379d90b8a5c6> .

<urn:uuid:da4d162d-c124-43be-a7e7-0ec463f4b32c> a skos:Concept;
  dct:created "2021-12-14T22:58:04Z"^^xsd:dateTime;
  dct:creator <urn:uuid:ca637d4b-c11b-4152-be98-bde602e7abd4>;
  skos:broader <urn:uuid:fdb43f70-cb11-49dd-aba6-7011b05ad61a>;
  skos:definition "In software development, version control is the process of, and attendant tooling for, preserving the changes to a set of files over time."@en;
  skos:inScheme <urn:uuid:0c7028f0-8226-47b3-acff-a4e83e6a60fd>,
    <urn:uuid:2df6fac6-3122-44dc-9f92-5caab7f9b10b>,
    <urn:uuid:797e83d7-a86f-4838-b5c5-0ec20855197d>,
    <urn:uuid:bbe073ad-f449-4b25-91ac-7d919613ca51>,
    <urn:uuid:1b457bed-8a80-4135-92b8-fdea12b4eea3>,
    <urn:uuid:2153d83b-8555-44a3-96e0-821b6663a188>,
    <urn:uuid:4bbcdde6-ed53-4f8d-b3f8-43f800fd05d5>;
  skos:narrower <urn:uuid:3e511aba-c593-4b5c-8b10-e60fbd6f3809>,
    <urn:uuid:35ec7a5f-aa2c-4876-bc77-161ebd0a3405>;
  skos:prefLabel "version control"@en .

<urn:uuid:db2fb779-83e8-407b-a538-5fe9a86271de> a skos:Concept;
  dct:created "2021-12-14T19:23:57Z"^^xsd:dateTime;
  dct:creator <urn:uuid:ca637d4b-c11b-4152-be98-bde602e7abd4>;
  skos:broader <urn:uuid:fdb43f70-cb11-49dd-aba6-7011b05ad61a>;
  skos:definition "In programming, a subroutine is a procedure that has been demarcated from the rest of the program somehow, often (but not exclusively) by giving it a name."@en;
  skos:inScheme <urn:uuid:0c7028f0-8226-47b3-acff-a4e83e6a60fd>,
    <urn:uuid:2df6fac6-3122-44dc-9f92-5caab7f9b10b>,
    <urn:uuid:797e83d7-a86f-4838-b5c5-0ec20855197d>,
    <urn:uuid:bbe073ad-f449-4b25-91ac-7d919613ca51>,
    <urn:uuid:1b457bed-8a80-4135-92b8-fdea12b4eea3>,
    <urn:uuid:2153d83b-8555-44a3-96e0-821b6663a188>,
    <urn:uuid:4bbcdde6-ed53-4f8d-b3f8-43f800fd05d5>;
  skos:narrower <urn:uuid:f8d5f1b1-ca7f-4610-9026-20b68c04783d>;
  skos:prefLabel "subroutine"@en .

<urn:uuid:df3de73d-3cb1-4b82-8773-415f1f16cbda> a skos:Concept;
  dct:created "2022-11-23T21:51:22Z"^^xsd:dateTime;
  dct:creator <urn:uuid:ca637d4b-c11b-4152-be98-bde602e7abd4>;
  skos:definition "Structural markup can be understood as the subset of markup which exclusively describes the topological structure of (e.g.) a document and its semantics, i.e. all the parts and what they all mean. This is in contrast to presentation markup."@en;
  skos:inScheme <urn:uuid:1b457bed-8a80-4135-92b8-fdea12b4eea3>,
    <urn:uuid:2153d83b-8555-44a3-96e0-821b6663a188>,
    <urn:uuid:bbe073ad-f449-4b25-91ac-7d919613ca51>,
    <urn:uuid:0c7028f0-8226-47b3-acff-a4e83e6a60fd>,
    <urn:uuid:4bbcdde6-ed53-4f8d-b3f8-43f800fd05d5>;
  skos:prefLabel "structural markup"@en;
  skos:related <urn:uuid:b99ffccd-0042-4e5a-a4ce-b58cbdcf3ef9>,
    <urn:uuid:c757c1ac-1ec6-4bdd-a35d-85f1d85728bb> .

<urn:uuid:e7ccb716-f967-439f-9682-dad225efc0b6> a skos:Concept;
  dct:created "2022-11-23T21:23:25Z"^^xsd:dateTime;
  dct:creator <urn:uuid:ca637d4b-c11b-4152-be98-bde602e7abd4>;
  skos:altLabel "heterogeneous"@en;
  skos:definition "Heterogeneity in an information system is when the system is made of different technologies, vendors, and platforms."@en;
  skos:hiddenLabel "heterogeneity"@en;
  skos:inScheme <urn:uuid:1b457bed-8a80-4135-92b8-fdea12b4eea3>,
    <urn:uuid:2153d83b-8555-44a3-96e0-821b6663a188>,
    <urn:uuid:bbe073ad-f449-4b25-91ac-7d919613ca51>,
    <urn:uuid:0c7028f0-8226-47b3-acff-a4e83e6a60fd>,
    <urn:uuid:a1a01f1c-7162-439c-94f1-3e28b99ae8ab>,
    <urn:uuid:ddfaaacc-9dcb-451b-afa6-477e6e787a5c>,
    <urn:uuid:4bbcdde6-ed53-4f8d-b3f8-43f800fd05d5>;
  skos:prefLabel "heterogeneity (information systems)"@en;
  skos:related <urn:uuid:1b004393-fdea-438b-a0d8-1919184d4bd1> .

<urn:uuid:ecf5fe36-229a-4eea-8b2d-24686da80aba> a skos:Concept;
  dct:created "2018-02-03T13:30:46Z"^^xsd:dateTime;
  dct:creator <urn:uuid:ca637d4b-c11b-4152-be98-bde602e7abd4>;
  skos:broader <urn:uuid:9e506ca3-8be1-431d-9075-548141d9f8c1>;
  skos:definition "A uniform resource name is a kind of URI which occupies the \"urn:\" scheme, and is used to refer to resources whose dereferencing mechanisms are well-known, unspecified (e.g. urn:isbn:9780262691918), or do not exist at all. Contrast with URLs, which encode both how (by scheme) and where (by network address) to obtain the resource."@en;
  skos:inScheme <urn:uuid:75f35368-e228-47fe-8efd-7251a2bde816>,
    <urn:uuid:1b457bed-8a80-4135-92b8-fdea12b4eea3>,
    <urn:uuid:2153d83b-8555-44a3-96e0-821b6663a188>,
    <urn:uuid:2df6fac6-3122-44dc-9f92-5caab7f9b10b>,
    <urn:uuid:91684d49-7b99-4b2e-9641-ea0b8e22f66c>,
    <urn:uuid:bbe073ad-f449-4b25-91ac-7d919613ca51>,
    <urn:uuid:4bbcdde6-ed53-4f8d-b3f8-43f800fd05d5>;
  skos:prefLabel "Uniform Resource Name"@en;
  skos:related <urn:uuid:e162d03b-bfec-4f01-ab7e-56da309550f6> .

<urn:uuid:ee2371bb-d9a0-4ee8-a35b-f4e0d9458f02> a skos:Concept;
  dct:created "2021-12-14T03:03:32Z"^^xsd:dateTime;
  dct:creator <urn:uuid:ca637d4b-c11b-4152-be98-bde602e7abd4>;
  skos:definition "A client-side script is procedural code executed on the site of a client in a client-server model of networked information services."@en;
  skos:hiddenLabel "client-side scripting"@en;
  skos:inScheme <urn:uuid:1b457bed-8a80-4135-92b8-fdea12b4eea3>,
    <urn:uuid:2153d83b-8555-44a3-96e0-821b6663a188>,
    <urn:uuid:0c7028f0-8226-47b3-acff-a4e83e6a60fd>,
    <urn:uuid:2df6fac6-3122-44dc-9f92-5caab7f9b10b>,
    <urn:uuid:797e83d7-a86f-4838-b5c5-0ec20855197d>,
    <urn:uuid:bbe073ad-f449-4b25-91ac-7d919613ca51>,
    <urn:uuid:4bbcdde6-ed53-4f8d-b3f8-43f800fd05d5>;
  skos:prefLabel "client-side script"@en .

<urn:uuid:01dc6e60-8e23-4c4c-a63d-f149cb104f84> a skos:Concept;
  dct:alternative "A content inventory is both the process and result of enumerating and recording the totality of the content on one or more Web properties. It is one of the essential work products of content strategists."@en;
  dct:created "2019-03-06T05:47:22Z"^^xsd:dateTime;
  dct:creator <urn:uuid:ca637d4b-c11b-4152-be98-bde602e7abd4>;
  dct:description "A content inventory is both the process and result of enumerating and recording the totality of the content on one or more Web properties. It is one of the essential work products of content strategists."@en;
  dct:modified "2021-12-14T16:35:22Z"^^xsd:dateTime;
  skos:altLabel "content inventory"@en;
  skos:broader <urn:uuid:42747b64-a41c-4321-96cf-c49e711733e6>;
  skos:definition "A content inventory is an exhaustive account of all information resources e.g. on a website, or indeed within an entire organization. The results are typically delivered on one or more spreadsheets, with e.g. a URI or other identifier in the first column, the title in the second, author, date, etc."@en;
  skos:hiddenLabel "content inventories"@en;
  skos:inScheme <urn:uuid:bbe073ad-f449-4b25-91ac-7d919613ca51>,
    <urn:uuid:797e83d7-a86f-4838-b5c5-0ec20855197d>,
    <urn:uuid:1b457bed-8a80-4135-92b8-fdea12b4eea3>,
    <urn:uuid:2153d83b-8555-44a3-96e0-821b6663a188>,
    <urn:uuid:2df6fac6-3122-44dc-9f92-5caab7f9b10b>,
    <urn:uuid:75f35368-e228-47fe-8efd-7251a2bde816>,
    <urn:uuid:4bbcdde6-ed53-4f8d-b3f8-43f800fd05d5>;
  skos:prefLabel "content inventory"@en;
  skos:related <urn:uuid:123bcb4d-b7e1-4715-b95b-73161516e789>,
    <urn:uuid:132303c5-7f8e-48c0-a680-c282386ba909>,
    <urn:uuid:88465aec-782f-4aab-9d50-cc918cceaed5> .

<urn:uuid:055e91e4-5edf-46fd-9bad-9847dbf57a72> a skos:Concept;
  dct:alternative "An interface is a substructure in a system where two (or more) parts come together."@en;
  dct:created "2017-02-09T16:55:48Z"^^xsd:dateTime;
  dct:creator <urn:uuid:ca637d4b-c11b-4152-be98-bde602e7abd4>;
  dct:description "An interface is a substructure in a system where two (or more) parts come together."@en;
  dct:modified "2019-03-04T06:57:16Z"^^xsd:dateTime;
  skos:definition "An interface is a substructure in a system where two (or more) parts come together."@en,
    "An interface can be understood as a junction between two or more systems or media. Interfaces are closely related to protocols, with a possible distinction that an interface is biased toward space, while a protocol is biased toward time."@en;
  skos:inScheme <urn:uuid:bbe073ad-f449-4b25-91ac-7d919613ca51>,
    <urn:uuid:49ac68c4-922c-4d9e-88fa-b318fc54d36f>,
    <urn:uuid:2df6fac6-3122-44dc-9f92-5caab7f9b10b>,
    <urn:uuid:1b457bed-8a80-4135-92b8-fdea12b4eea3>,
    <urn:uuid:2153d83b-8555-44a3-96e0-821b6663a188>,
    <urn:uuid:a1a01f1c-7162-439c-94f1-3e28b99ae8ab>,
    <urn:uuid:ddfaaacc-9dcb-451b-afa6-477e6e787a5c>,
    <urn:uuid:4bbcdde6-ed53-4f8d-b3f8-43f800fd05d5>;
  skos:prefLabel "interface"@en .

<urn:uuid:10bafb58-6eb8-4d99-9b7d-9840842d3947> a skos:Concept;
  dct:created "2017-02-08T06:40:47Z"^^xsd:dateTime;
  dct:creator <urn:uuid:ca637d4b-c11b-4152-be98-bde602e7abd4>;
  dct:modified "2019-05-30T20:56:58Z"^^xsd:dateTime;
  skos:broader <urn:uuid:b39c1f53-b8ed-49fb-ba57-24dfe7dc2d9f>;
  skos:definition "Information infrastructure is that which helps a person or organization manage and organize its stocks and flows of information."@en,
    "Information infrastructure is the information system that helps a person or organization manage and organize its stocks and flows of information. As with any information system, the information is more significant than whatever technology is used to manipulate it."@en;
  skos:inScheme <urn:uuid:0c7028f0-8226-47b3-acff-a4e83e6a60fd>,
    <urn:uuid:a1a01f1c-7162-439c-94f1-3e28b99ae8ab>,
    <urn:uuid:ddfaaacc-9dcb-451b-afa6-477e6e787a5c>,
    <urn:uuid:2df6fac6-3122-44dc-9f92-5caab7f9b10b>,
    <urn:uuid:bbe073ad-f449-4b25-91ac-7d919613ca51>,
    <urn:uuid:49ac68c4-922c-4d9e-88fa-b318fc54d36f>,
    <urn:uuid:1b457bed-8a80-4135-92b8-fdea12b4eea3>,
    <urn:uuid:2153d83b-8555-44a3-96e0-821b6663a188>,
    <urn:uuid:4bbcdde6-ed53-4f8d-b3f8-43f800fd05d5>;
  skos:narrower <urn:uuid:4694ebe0-589f-40a7-9ef9-67872edb6214>,
    <urn:uuid:06f86a10-1b5f-4711-b2fc-3bb5ce14a26e>,
    <urn:uuid:abadd9b5-844e-4982-8fbe-b6b83d43736d>,
    <urn:uuid:197982df-60a5-4c93-be50-2f8ede43b842>,
    <urn:uuid:b20221c0-4949-471a-adb1-45dfccfbdf1c>;
  skos:prefLabel "information infrastructure"@en;
  skos:related <urn:uuid:16d17f33-394d-4d0b-a882-81e8fc3a52fe> .

<urn:uuid:123bcb4d-b7e1-4715-b95b-73161516e789> a skos:Concept;
  dct:created "2019-03-06T05:32:37Z"^^xsd:dateTime;
  dct:creator <urn:uuid:ca637d4b-c11b-4152-be98-bde602e7abd4>;
  skos:broader <urn:uuid:42747b64-a41c-4321-96cf-c49e711733e6>;
  skos:definition "Content management is the art and science of dealing with the mass of (usually digital) stuffâusually textâwithin an organization."@en,
    "Content management is the art and science of dealing with the mass of (usually digital) stuff—usually text—within an organization."@en;
  skos:inScheme <urn:uuid:1b457bed-8a80-4135-92b8-fdea12b4eea3>,
    <urn:uuid:2153d83b-8555-44a3-96e0-821b6663a188>,
    <urn:uuid:75f35368-e228-47fe-8efd-7251a2bde816>,
    <urn:uuid:a1a01f1c-7162-439c-94f1-3e28b99ae8ab>,
    <urn:uuid:ddfaaacc-9dcb-451b-afa6-477e6e787a5c>,
    <urn:uuid:2df6fac6-3122-44dc-9f92-5caab7f9b10b>,
    <urn:uuid:0c7028f0-8226-47b3-acff-a4e83e6a60fd>,
    <urn:uuid:bbe073ad-f449-4b25-91ac-7d919613ca51>,
    <urn:uuid:4bbcdde6-ed53-4f8d-b3f8-43f800fd05d5>;
  skos:prefLabel "content management"@en;
  skos:related <urn:uuid:cbc4f4d6-96a1-44fc-8f07-e3282626fe3f>,
    <urn:uuid:7284c136-288b-49aa-b129-a56e2be938d2> .

<urn:uuid:2717d0b5-cb79-4d1a-82c0-69cdc1e590a1> a skos:Concept;
  dct:created "2019-02-28T21:46:13Z"^^xsd:dateTime;
  dct:creator <urn:uuid:ca637d4b-c11b-4152-be98-bde602e7abd4>;
  skos:broader <urn:uuid:e827d9af-be73-4918-89aa-a296872be199>,
    <urn:uuid:33c3211f-322b-4f7a-83f6-63aa617461c3>;
  skos:definition "Structured Query Language is a standardized fourth-generation programming language for accessing and manipulating relational databases."@en;
  skos:inScheme <urn:uuid:bbe073ad-f449-4b25-91ac-7d919613ca51>,
    <urn:uuid:1b457bed-8a80-4135-92b8-fdea12b4eea3>,
    <urn:uuid:2153d83b-8555-44a3-96e0-821b6663a188>,
    <urn:uuid:2df6fac6-3122-44dc-9f92-5caab7f9b10b>,
    <urn:uuid:75f35368-e228-47fe-8efd-7251a2bde816>,
    <urn:uuid:4bbcdde6-ed53-4f8d-b3f8-43f800fd05d5>;
  skos:narrower <urn:uuid:d5cb742c-9f75-42a4-967f-70b1fda5f0be>;
  skos:prefLabel "SQL"@en;
  skos:related <urn:uuid:0aabcb14-9aee-4b16-835e-02530dcb0c23>,
    <urn:uuid:262057b5-cdb6-4148-823e-a63fd5d10268>,
    <urn:uuid:9767147a-1b6a-440c-949f-7f6056e28411>,
    <urn:uuid:b7bb05a0-86af-4d5d-9d59-0d1691cc766d> .

<urn:uuid:3e3aa9b0-efaf-4dc5-83fb-4456e24f021d> a skos:Concept;
  dct:created "2019-03-04T05:54:05Z"^^xsd:dateTime,
    "2018-04-26T22:51:11Z"^^xsd:dateTime;
  dct:creator <urn:uuid:ca637d4b-c11b-4152-be98-bde602e7abd4>;
  skos:broader <urn:uuid:33c3211f-322b-4f7a-83f6-63aa617461c3>;
  skos:definition "Ruby is an object-oriented interpreted programming language by Yukihiro Matsumoto. It is very similar in capabilities and performance to both Perl and Python (and the youngest of the three). Ruby is a popular server-side programming language for Web applications."@en;
  skos:inScheme <urn:uuid:bbe073ad-f449-4b25-91ac-7d919613ca51>,
    <urn:uuid:75f35368-e228-47fe-8efd-7251a2bde816>,
    <urn:uuid:91684d49-7b99-4b2e-9641-ea0b8e22f66c>,
    <urn:uuid:2df6fac6-3122-44dc-9f92-5caab7f9b10b>,
    <urn:uuid:1b457bed-8a80-4135-92b8-fdea12b4eea3>,
    <urn:uuid:2153d83b-8555-44a3-96e0-821b6663a188>,
    <urn:uuid:4bbcdde6-ed53-4f8d-b3f8-43f800fd05d5>;
  skos:prefLabel "Ruby"@en .

<urn:uuid:42a48e75-a413-4b91-8787-a8c2dc1a65ed> a skos:Concept;
  dct:created "2021-12-14T20:42:10Z"^^xsd:dateTime;
  dct:creator <urn:uuid:ca637d4b-c11b-4152-be98-bde602e7abd4>;
  skos:broader <urn:uuid:759d2f68-3d16-4122-9758-c84f7760d691>,
    <urn:uuid:637cfc93-b88b-4bfb-8f7c-2f9e72e27b86>;
  skos:definition "A Web property is another, smaller umbrella term for networked information services that operate exclusively over the Web, such as ordinary websites, and Web APIs."@en;
  skos:inScheme <urn:uuid:1b457bed-8a80-4135-92b8-fdea12b4eea3>,
    <urn:uuid:2153d83b-8555-44a3-96e0-821b6663a188>,
    <urn:uuid:a1a01f1c-7162-439c-94f1-3e28b99ae8ab>,
    <urn:uuid:ddfaaacc-9dcb-451b-afa6-477e6e787a5c>,
    <urn:uuid:797e83d7-a86f-4838-b5c5-0ec20855197d>,
    <urn:uuid:2df6fac6-3122-44dc-9f92-5caab7f9b10b>,
    <urn:uuid:bbe073ad-f449-4b25-91ac-7d919613ca51>,
    <urn:uuid:4bbcdde6-ed53-4f8d-b3f8-43f800fd05d5>;
  skos:narrower <urn:uuid:be93cce1-f21f-4e85-bd34-e005dea3532f>,
    <urn:uuid:2fd3adcc-1e66-48a5-a375-06992d6fc02b>;
  skos:prefLabel "Web property"@en;
  skos:related <urn:uuid:61c0c9c3-4d91-4509-902a-db09c4188ae5> .

<urn:uuid:440e5d73-d654-4051-b482-2a960835306b> a skos:Concept;
  dct:created "2017-07-09T22:09:15Z"^^xsd:dateTime;
  dct:creator <urn:uuid:ca637d4b-c11b-4152-be98-bde602e7abd4>;
  skos:broader <urn:uuid:0aabcb14-9aee-4b16-835e-02530dcb0c23>,
    <urn:uuid:9767147a-1b6a-440c-949f-7f6056e28411>;
  skos:definition "Website navigation, as a noun, refers to the data structure that encodes the hierarchical groupings of pages on a website."@en;
  skos:inScheme <urn:uuid:bbe073ad-f449-4b25-91ac-7d919613ca51>,
    <urn:uuid:1b457bed-8a80-4135-92b8-fdea12b4eea3>,
    <urn:uuid:2153d83b-8555-44a3-96e0-821b6663a188>,
    <urn:uuid:91684d49-7b99-4b2e-9641-ea0b8e22f66c>,
    <urn:uuid:75f35368-e228-47fe-8efd-7251a2bde816>,
    <urn:uuid:2df6fac6-3122-44dc-9f92-5caab7f9b10b>,
    <urn:uuid:4bbcdde6-ed53-4f8d-b3f8-43f800fd05d5>;
  skos:prefLabel "website navigation"@en;
  skos:related <urn:uuid:65a4359d-9ef6-44a3-9317-875495517b3c>,
    <urn:uuid:7284c136-288b-49aa-b129-a56e2be938d2>,
    <urn:uuid:85a069f9-1a66-4462-b0e2-d042db345919> .

<urn:uuid:4f4aa0ac-c1b4-4a15-a6f3-518419d5b771> a skos:Concept;
  dct:created "2008-07-17T17:17:44+00:00"^^xsd:dateTime,
    "2022-10-06T03:15:59Z"^^xsd:dateTime;
  dct:creator <urn:uuid:ca637d4b-c11b-4152-be98-bde602e7abd4>;
  dct:modified "2008-07-18T18:59:52+00:00"^^xsd:dateTime,
    "2008-07-19T02:49:48+00:00"^^xsd:dateTime,
    "2008-07-19T02:57:06+00:00"^^xsd:dateTime,
    "2008-07-24T20:51:04+00:00"^^xsd:dateTime,
    "2008-09-01T04:55:33+00:00"^^xsd:dateTime,
    "2008-10-09T02:02:01+00:00"^^xsd:dateTime,
    "2008-10-10T16:02:45+00:00"^^xsd:dateTime,
    "2008-10-10T21:28:23+00:00"^^xsd:dateTime,
    "2009-03-04T00:43:00+00:00"^^xsd:dateTime,
    "2022-05-31T04:18:52+00:00"^^xsd:dateTime,
    "2022-10-06T03:15:59Z"^^xsd:dateTime;
  skos:definition "A file is an opaque blob—a segment of bytes—with a name."@en;
  skos:inScheme <urn:uuid:4ec7530b-5536-4fb7-bb5a-45a3f5fddc22>,
    <urn:uuid:1b457bed-8a80-4135-92b8-fdea12b4eea3>,
    <urn:uuid:2153d83b-8555-44a3-96e0-821b6663a188>,
    <urn:uuid:bbe073ad-f449-4b25-91ac-7d919613ca51>,
    <urn:uuid:2df6fac6-3122-44dc-9f92-5caab7f9b10b>,
    <urn:uuid:4bbcdde6-ed53-4f8d-b3f8-43f800fd05d5>;
  skos:prefLabel "file"@en .

<urn:uuid:53819af5-c2d0-4edc-9add-ab79829ace96> a skos:Concept;
  dct:created "2021-12-14T01:10:41Z"^^xsd:dateTime;
  dct:creator <urn:uuid:ca637d4b-c11b-4152-be98-bde602e7abd4>;
  skos:definition "A caching proxy is a proxy with a cache attached."@en;
  skos:hiddenLabel "caching proxies"@en;
  skos:inScheme <urn:uuid:a1a01f1c-7162-439c-94f1-3e28b99ae8ab>,
    <urn:uuid:ddfaaacc-9dcb-451b-afa6-477e6e787a5c>,
    <urn:uuid:1b457bed-8a80-4135-92b8-fdea12b4eea3>,
    <urn:uuid:2153d83b-8555-44a3-96e0-821b6663a188>,
    <urn:uuid:0c7028f0-8226-47b3-acff-a4e83e6a60fd>,
    <urn:uuid:797e83d7-a86f-4838-b5c5-0ec20855197d>,
    <urn:uuid:bbe073ad-f449-4b25-91ac-7d919613ca51>,
    <urn:uuid:2df6fac6-3122-44dc-9f92-5caab7f9b10b>,
    <urn:uuid:4bbcdde6-ed53-4f8d-b3f8-43f800fd05d5>;
  skos:narrower <urn:uuid:c38fdbb2-201b-4a88-9273-26fbd0c6fae5>;
  skos:prefLabel "caching proxy"@en .

<urn:uuid:5495f814-fd98-4b43-aba3-9e63a2063fd5> a skos:Concept;
  dct:created "2021-12-14T01:59:47Z"^^xsd:dateTime;
  dct:creator <urn:uuid:ca637d4b-c11b-4152-be98-bde602e7abd4>;
  skos:broader <urn:uuid:c6ab3854-e8a7-4cd8-8ca3-3928d926f224>;
  skos:definition "A call graph is a statistical representation of code as it is being executed, useful for determining the code's actual behavior. A call graph generally makes use of AST to produce meaningful results."@en;
  skos:inScheme <urn:uuid:bbe073ad-f449-4b25-91ac-7d919613ca51>,
    <urn:uuid:1b457bed-8a80-4135-92b8-fdea12b4eea3>,
    <urn:uuid:2153d83b-8555-44a3-96e0-821b6663a188>,
    <urn:uuid:797e83d7-a86f-4838-b5c5-0ec20855197d>,
    <urn:uuid:2df6fac6-3122-44dc-9f92-5caab7f9b10b>,
    <urn:uuid:4bbcdde6-ed53-4f8d-b3f8-43f800fd05d5>;
  skos:prefLabel "call graph"@en;
  skos:related <urn:uuid:8cb5c042-8ce4-4d8d-a4c0-dd47d90e4bf5> .

<urn:uuid:5abd5284-7197-4eed-895d-6daefa019de8> a skos:Concept;
  dct:created "2019-03-02T00:13:41Z"^^xsd:dateTime;
  dct:creator <urn:uuid:ca637d4b-c11b-4152-be98-bde602e7abd4>;
  skos:broader <urn:uuid:33c3211f-322b-4f7a-83f6-63aa617461c3>;
  skos:definition "A safe language is a data format or programming language whose entire range of possible behaviour can be deduced through static analysis. Safe languages are therefore not Turing-complete. Sandboxing is a popular, though not completely reliable strategy for dealing with unsafe languages."@en;
  skos:inScheme <urn:uuid:75f35368-e228-47fe-8efd-7251a2bde816>,
    <urn:uuid:bbe073ad-f449-4b25-91ac-7d919613ca51>,
    <urn:uuid:1b457bed-8a80-4135-92b8-fdea12b4eea3>,
    <urn:uuid:2153d83b-8555-44a3-96e0-821b6663a188>,
    <urn:uuid:2df6fac6-3122-44dc-9f92-5caab7f9b10b>,
    <urn:uuid:4bbcdde6-ed53-4f8d-b3f8-43f800fd05d5>;
  skos:prefLabel "safe language"@en;
  skos:related <urn:uuid:45373ede-a7b0-404f-b797-902298208993>,
    <urn:uuid:06f69b4c-ce8b-42ea-b0cb-7f52f233b592>,
    <urn:uuid:0bc0aabb-9d9e-4caa-b9c8-553dd8b3ee05>,
    <urn:uuid:755dd3a1-cffc-4d65-9446-435552bac541> .

<urn:uuid:65a4359d-9ef6-44a3-9317-875495517b3c> a skos:Concept;
  dct:alternative "Search engine optimization is the practice of altering a website's content and structure to improve its ranking in search engine results. SEO is the ostensible major motivator for publishing metadata."@en;
  dct:created "2019-03-01T03:06:10Z"^^xsd:dateTime,
    "2024-11-26T23:40:53Z"^^xsd:dateTime;
  dct:creator <urn:uuid:ca637d4b-c11b-4152-be98-bde602e7abd4>;
  dct:description "Search engine optimization is the practice of altering a website's content and structure to improve its ranking in search engine results. SEO is the ostensible major motivator for publishing metadata."@en;
  skos:altLabel "Search engine optimization"@en,
    "SEO"@en;
  skos:broader <urn:uuid:63a99f54-a4cf-487b-b217-083384522046>;
  skos:definition "SEO is the sacred cow of internet marketing. Nothing bad is to be said about SEO."@en;
  skos:hiddenLabel "seo"@en;
  skos:inScheme <urn:uuid:2df6fac6-3122-44dc-9f92-5caab7f9b10b>,
    <urn:uuid:797e83d7-a86f-4838-b5c5-0ec20855197d>,
    <urn:uuid:bbe073ad-f449-4b25-91ac-7d919613ca51>,
    <urn:uuid:1b457bed-8a80-4135-92b8-fdea12b4eea3>,
    <urn:uuid:2153d83b-8555-44a3-96e0-821b6663a188>,
    <urn:uuid:0c7028f0-8226-47b3-acff-a4e83e6a60fd>,
    <urn:uuid:4bbcdde6-ed53-4f8d-b3f8-43f800fd05d5>;
  skos:prefLabel "search engine optimization"@en;
  skos:related <urn:uuid:440e5d73-d654-4051-b482-2a960835306b>,
    <urn:uuid:cda3a7a9-41bc-4de7-ad92-1b9093389c64>,
    <urn:uuid:7284c136-288b-49aa-b129-a56e2be938d2>,
    <urn:uuid:a91fff32-d160-4cc0-86eb-e78d778a1526>,
    <urn:uuid:e162d03b-bfec-4f01-ab7e-56da309550f6> .

<urn:uuid:855fce21-5560-4ff3-87bf-ef26a28958c4> a skos:Concept;
  dct:created "2019-03-02T01:28:54Z"^^xsd:dateTime;
  dct:creator <urn:uuid:ca637d4b-c11b-4152-be98-bde602e7abd4>;
  skos:broader <urn:uuid:33c3211f-322b-4f7a-83f6-63aa617461c3>,
    <urn:uuid:e827d9af-be73-4918-89aa-a296872be199>;
  skos:definition "Java is a programming language and virtual machine designed for \"write once, run anywhere\" cross-platform targeting, initially developed by Sun Microsystems in the 1990s, which was subsequently acquired by Oracle. Java appears to be the language of choice for academics and large corporations, which may account for its strong representation in RDF tools."@en;
  skos:inScheme <urn:uuid:2df6fac6-3122-44dc-9f92-5caab7f9b10b>,
    <urn:uuid:bbe073ad-f449-4b25-91ac-7d919613ca51>,
    <urn:uuid:75f35368-e228-47fe-8efd-7251a2bde816>,
    <urn:uuid:1b457bed-8a80-4135-92b8-fdea12b4eea3>,
    <urn:uuid:2153d83b-8555-44a3-96e0-821b6663a188>,
    <urn:uuid:4bbcdde6-ed53-4f8d-b3f8-43f800fd05d5>;
  skos:prefLabel "Java"@en .

<urn:uuid:935ab72b-b74c-4204-9c00-f1f8f83f105e> a skos:Concept;
  dct:created "2017-02-09T21:53:01Z"^^xsd:dateTime;
  dct:creator <urn:uuid:ca637d4b-c11b-4152-be98-bde602e7abd4>;
  skos:broader <urn:uuid:bdb1ca1d-7f9d-4e26-8fd6-639b9a3348d9>;
  skos:definition "A Web application is a software application which uses the World-Wide Web as a user interface. A Web application can be an entire website, or a cluster of Web resources embedded within a website, or even a single Web resource."@en;
  skos:inScheme <urn:uuid:1b457bed-8a80-4135-92b8-fdea12b4eea3>,
    <urn:uuid:2153d83b-8555-44a3-96e0-821b6663a188>,
    <urn:uuid:2df6fac6-3122-44dc-9f92-5caab7f9b10b>,
    <urn:uuid:a1a01f1c-7162-439c-94f1-3e28b99ae8ab>,
    <urn:uuid:ddfaaacc-9dcb-451b-afa6-477e6e787a5c>,
    <urn:uuid:bbe073ad-f449-4b25-91ac-7d919613ca51>,
    <urn:uuid:49ac68c4-922c-4d9e-88fa-b318fc54d36f>,
    <urn:uuid:4bbcdde6-ed53-4f8d-b3f8-43f800fd05d5>;
  skos:prefLabel "Web Application"@en,
    "Web application"@en;
  skos:related <urn:uuid:bdb1ca1d-7f9d-4e26-8fd6-639b9a3348d9>,
    <urn:uuid:9ad22902-84a2-488b-92ea-360182357ed1> .

<urn:uuid:a91fff32-d160-4cc0-86eb-e78d778a1526> a skos:Concept;
  dct:created "2019-02-21T22:15:02Z"^^xsd:dateTime;
  dct:creator <urn:uuid:ca637d4b-c11b-4152-be98-bde602e7abd4>;
  skos:broader <urn:uuid:fe500c7a-b458-4d2c-8b3a-efd1bb47d106>;
  skos:definition "RDFa (RDF in Attributes) describes a set of markup attributes that carry RDF data, which can be embedded in HTML or an XML host language. This enables the semantic data to piggyback on the markup structure and often reuse the same content."@en;
  skos:inScheme <urn:uuid:bbe073ad-f449-4b25-91ac-7d919613ca51>,
    <urn:uuid:2df6fac6-3122-44dc-9f92-5caab7f9b10b>,
    <urn:uuid:0c7028f0-8226-47b3-acff-a4e83e6a60fd>,
    <urn:uuid:75f35368-e228-47fe-8efd-7251a2bde816>,
    <urn:uuid:1b457bed-8a80-4135-92b8-fdea12b4eea3>,
    <urn:uuid:2153d83b-8555-44a3-96e0-821b6663a188>,
    <urn:uuid:4bbcdde6-ed53-4f8d-b3f8-43f800fd05d5>;
  skos:prefLabel "RDFa"@en .

<urn:uuid:ba2258e3-efca-4461-82cc-f6ebbf980b36> a skos:Concept;
  dct:created "2019-02-28T18:58:27Z"^^xsd:dateTime;
  dct:creator <urn:uuid:ca637d4b-c11b-4152-be98-bde602e7abd4>;
  skos:broader <urn:uuid:fe500c7a-b458-4d2c-8b3a-efd1bb47d106>;
  skos:definition "RDF Site Summary 1.0 is a feed definition format based on RDF."@en;
  skos:inScheme <urn:uuid:1b457bed-8a80-4135-92b8-fdea12b4eea3>,
    <urn:uuid:2153d83b-8555-44a3-96e0-821b6663a188>,
    <urn:uuid:2df6fac6-3122-44dc-9f92-5caab7f9b10b>,
    <urn:uuid:bbe073ad-f449-4b25-91ac-7d919613ca51>,
    <urn:uuid:75f35368-e228-47fe-8efd-7251a2bde816>,
    <urn:uuid:4bbcdde6-ed53-4f8d-b3f8-43f800fd05d5>;
  skos:prefLabel "RSS 1.0"@en .

<urn:uuid:bdb1ca1d-7f9d-4e26-8fd6-639b9a3348d9> a skos:Concept;
  dct:created "2017-02-09T21:55:53Z"^^xsd:dateTime;
  dct:creator <urn:uuid:ca637d4b-c11b-4152-be98-bde602e7abd4>;
  skos:broader <urn:uuid:4039a99d-c14b-40f2-84d5-4ec72e2217e1>,
    <urn:uuid:759d2f68-3d16-4122-9758-c84f7760d691>;
  skos:definition "A Web Resource is any information on the World-Wide Web which is distinctly identifiable by an address, or Uniform Resource Identifier. A Web resource can take a variety of forms, including a conventional document file, a document fragment, or an interface to a software program."@en;
  skos:inScheme <urn:uuid:1b457bed-8a80-4135-92b8-fdea12b4eea3>,
    <urn:uuid:2153d83b-8555-44a3-96e0-821b6663a188>,
    <urn:uuid:49ac68c4-922c-4d9e-88fa-b318fc54d36f>,
    <urn:uuid:2df6fac6-3122-44dc-9f92-5caab7f9b10b>,
    <urn:uuid:a1a01f1c-7162-439c-94f1-3e28b99ae8ab>,
    <urn:uuid:ddfaaacc-9dcb-451b-afa6-477e6e787a5c>,
    <urn:uuid:bbe073ad-f449-4b25-91ac-7d919613ca51>,
    <urn:uuid:4bbcdde6-ed53-4f8d-b3f8-43f800fd05d5>;
  skos:prefLabel "Web resource"@en,
    "Web Resource"@en .

<urn:uuid:cda3a7a9-41bc-4de7-ad92-1b9093389c64> a skos:Concept;
  dct:created "2017-07-13T18:47:10Z"^^xsd:dateTime;
  dct:creator <urn:uuid:ca637d4b-c11b-4152-be98-bde602e7abd4>;
  skos:broader <urn:uuid:f3f67e45-9cdf-4df1-9586-834ba185f63b>,
    <urn:uuid:7b7c4ecf-2544-4c03-ab5f-10de5e1a20d4>,
    <urn:uuid:ca632e87-50d2-4f1d-af83-f3d11e53eca8>,
    <urn:uuid:fe500c7a-b458-4d2c-8b3a-efd1bb47d106>;
  skos:definition "JSON-LD is a particular configuration of JSON (i.e., it is a serialization syntax) that enables the encoding of Linked Data (RDF)."@en;
  skos:inScheme <urn:uuid:2df6fac6-3122-44dc-9f92-5caab7f9b10b>,
    <urn:uuid:75f35368-e228-47fe-8efd-7251a2bde816>,
    <urn:uuid:bbe073ad-f449-4b25-91ac-7d919613ca51>,
    <urn:uuid:1b457bed-8a80-4135-92b8-fdea12b4eea3>,
    <urn:uuid:2153d83b-8555-44a3-96e0-821b6663a188>,
    <urn:uuid:91684d49-7b99-4b2e-9641-ea0b8e22f66c>,
    <urn:uuid:4bbcdde6-ed53-4f8d-b3f8-43f800fd05d5>;
  skos:narrower <urn:uuid:dfddf2a2-9648-4237-a922-6295c151eff4>;
  skos:prefLabel "JSON-LD"@en;
  skos:related <urn:uuid:65a4359d-9ef6-44a3-9317-875495517b3c> .

<urn:uuid:d2089ee2-d605-43ac-af18-ffbb7151a32d> a skos:Concept;
  dct:created "2021-12-14T17:38:51Z"^^xsd:dateTime;
  dct:creator <urn:uuid:ca637d4b-c11b-4152-be98-bde602e7abd4>;
  skos:definition "UX design, erstwhile called interaction design, is the strategic discipline of crafting the process of using a (often but not exclusively software) product. It is closely related to information architecture and content strategy."@en;
  skos:inScheme <urn:uuid:bbe073ad-f449-4b25-91ac-7d919613ca51>,
    <urn:uuid:2df6fac6-3122-44dc-9f92-5caab7f9b10b>,
    <urn:uuid:797e83d7-a86f-4838-b5c5-0ec20855197d>,
    <urn:uuid:1b457bed-8a80-4135-92b8-fdea12b4eea3>,
    <urn:uuid:2153d83b-8555-44a3-96e0-821b6663a188>,
    <urn:uuid:a1a01f1c-7162-439c-94f1-3e28b99ae8ab>,
    <urn:uuid:ddfaaacc-9dcb-451b-afa6-477e6e787a5c>,
    <urn:uuid:4bbcdde6-ed53-4f8d-b3f8-43f800fd05d5>;
  skos:prefLabel "user experience design"@en;
  skos:related <urn:uuid:42747b64-a41c-4321-96cf-c49e711733e6>,
    <urn:uuid:7284c136-288b-49aa-b129-a56e2be938d2> .

<urn:uuid:f0a7ece3-44e6-4f6b-963c-281ab8dff8e6> a skos:Concept;
  dct:created "2019-02-22T01:31:28Z"^^xsd:dateTime;
  dct:creator <urn:uuid:ca637d4b-c11b-4152-be98-bde602e7abd4>;
  skos:altLabel "protocol"@en;
  skos:broader <urn:uuid:75b4da00-36b5-467e-bc90-966a7e5256a1>;
  skos:definition "This refers to the formal grammar and semantics of communication over (in our case) a digital network. We can think of a network protocol as an analogous design problem to a file format, in that it's some definite representation of data, albeit with an emphasis on transporting it rather than storing it. Network protocols also tend to (but not always) model some kind of conversational state between two or more systems, and are therefore potentially more complex to specify than a data format."@en;
  skos:inScheme <urn:uuid:bbe073ad-f449-4b25-91ac-7d919613ca51>,
    <urn:uuid:75f35368-e228-47fe-8efd-7251a2bde816>,
    <urn:uuid:1b457bed-8a80-4135-92b8-fdea12b4eea3>,
    <urn:uuid:2153d83b-8555-44a3-96e0-821b6663a188>,
    <urn:uuid:0c7028f0-8226-47b3-acff-a4e83e6a60fd>,
    <urn:uuid:2df6fac6-3122-44dc-9f92-5caab7f9b10b>,
    <urn:uuid:a1a01f1c-7162-439c-94f1-3e28b99ae8ab>,
    <urn:uuid:ddfaaacc-9dcb-451b-afa6-477e6e787a5c>,
    <urn:uuid:4bbcdde6-ed53-4f8d-b3f8-43f800fd05d5>;
  skos:narrower <urn:uuid:abdd08b5-9728-41b8-b56a-b53ce1ff1137>;
  skos:prefLabel "network protocol"@en;
  skos:related <urn:uuid:027543f6-04df-4e92-96f4-5b0c8da4b799> .

<urn:uuid:f5a254ac-4a2b-405e-91be-7de9fbf7174d> a skos:Concept;
  dct:created "2019-03-02T02:45:36Z"^^xsd:dateTime;
  dct:creator <urn:uuid:ca637d4b-c11b-4152-be98-bde602e7abd4>;
  skos:altLabel "AI"@en;
  skos:definition "Artificial intelligence can be understood as an umbrella term for computers behaving in (adaptive) ways they were not explicitly programmed to behave. Machine learning is one particular subfield of (and strategy for) artificial intelligence."@en;
  skos:inScheme <urn:uuid:75f35368-e228-47fe-8efd-7251a2bde816>,
    <urn:uuid:2df6fac6-3122-44dc-9f92-5caab7f9b10b>,
    <urn:uuid:4ec7530b-5536-4fb7-bb5a-45a3f5fddc22>,
    <urn:uuid:1b457bed-8a80-4135-92b8-fdea12b4eea3>,
    <urn:uuid:2153d83b-8555-44a3-96e0-821b6663a188>,
    <urn:uuid:a1a01f1c-7162-439c-94f1-3e28b99ae8ab>,
    <urn:uuid:ddfaaacc-9dcb-451b-afa6-477e6e787a5c>,
    <urn:uuid:bbe073ad-f449-4b25-91ac-7d919613ca51>,
    <urn:uuid:4bbcdde6-ed53-4f8d-b3f8-43f800fd05d5>;
  skos:prefLabel "artificial intelligence"@en .

<urn:uuid:288e85ab-887f-437c-9caa-c109cb9d478d> a skos:Concept;
  dct:alternative "REST is an architectural style for networked information systems centered around information resources and their representations. To wit: the representational state of a hypermedia resource is transferred between client and server. These states are identified by URLs, and therefore subsequent representational states in the process are embedded in the current state (a concept abstrusely known as HATEOAS).  This architectural style can be implemented on the Web but is not exclusively bound to it."@en;
  dct:created "2017-07-12T04:43:58Z"^^xsd:dateTime;
  dct:creator <urn:uuid:ca637d4b-c11b-4152-be98-bde602e7abd4>;
  dct:description "REST is an architectural style for networked information systems centered around information resources and their representations. To wit: the representational state of a hypermedia resource is transferred between client and server. These states are identified by URLs, and therefore subsequent representational states in the process are embedded in the current state (a concept abstrusely known as HATEOAS).  This architectural style can be implemented on the Web but is not exclusively bound to it."@en;
  dct:modified "2021-12-14T21:36:53Z"^^xsd:dateTime;
  dct:references <http://www.ics.uci.edu/~fielding/pubs/dissertation/top.htm>;
  rdfs:seeAlso <https://ics.uci.edu/~fielding/pubs/dissertation/top.htm>;
  skos:altLabel "REST"@en;
  skos:definition """REST (Representational State Transfer) is an architectural style of (originally but not necessarily confined to Web) software, wherein a resource (identified, e.g., by a URI) is considered to be a state in a state machine, and its representation (content) contains the list of subsequent states (i.e., links to other URIs).
REST has a considerable amount in common with Linked Data."""@en;
  skos:hiddenLabel "representational state transfer"@en;
  skos:inScheme <urn:uuid:797e83d7-a86f-4838-b5c5-0ec20855197d>,
    <urn:uuid:bbe073ad-f449-4b25-91ac-7d919613ca51>,
    <urn:uuid:75f35368-e228-47fe-8efd-7251a2bde816>,
    <urn:uuid:1b457bed-8a80-4135-92b8-fdea12b4eea3>,
    <urn:uuid:2153d83b-8555-44a3-96e0-821b6663a188>,
    <urn:uuid:a1a01f1c-7162-439c-94f1-3e28b99ae8ab>,
    <urn:uuid:ddfaaacc-9dcb-451b-afa6-477e6e787a5c>,
    <urn:uuid:91684d49-7b99-4b2e-9641-ea0b8e22f66c>,
    <urn:uuid:0c7028f0-8226-47b3-acff-a4e83e6a60fd>,
    <urn:uuid:2df6fac6-3122-44dc-9f92-5caab7f9b10b>,
    <urn:uuid:4bbcdde6-ed53-4f8d-b3f8-43f800fd05d5>;
  skos:narrower <urn:uuid:1ba688e9-6a85-4596-be01-379d90b8a5c6>,
    <urn:uuid:c0d27ab7-6727-4df0-8231-805b201e4663>,
    <urn:uuid:a30dc8ed-a356-4a20-9085-a0d40e75f0e9>;
  skos:prefLabel "Representational State Transfer"@en,
    "REST"@en;
  skos:related <urn:uuid:4039a99d-c14b-40f2-84d5-4ec72e2217e1>,
    <urn:uuid:5bdd2fb7-d84d-4583-998b-7d3f2803307e>,
    <urn:uuid:637cfc93-b88b-4bfb-8f7c-2f9e72e27b86> .

<urn:uuid:637cfc93-b88b-4bfb-8f7c-2f9e72e27b86> a skos:Concept;
  dct:created "2021-12-14T20:41:30Z"^^xsd:dateTime;
  dct:creator <urn:uuid:ca637d4b-c11b-4152-be98-bde602e7abd4>;
  skos:broader <urn:uuid:b39c1f53-b8ed-49fb-ba57-24dfe7dc2d9f>;
  skos:definition "A networked information service is an umbrella term for systems where computation, to the extent that there is any, happens at the site of the service's operator, and only the resulting information is conveyed over the network."@en;
  skos:hiddenLabel "networked information services"@en;
  skos:inScheme <urn:uuid:2df6fac6-3122-44dc-9f92-5caab7f9b10b>,
    <urn:uuid:a1a01f1c-7162-439c-94f1-3e28b99ae8ab>,
    <urn:uuid:ddfaaacc-9dcb-451b-afa6-477e6e787a5c>,
    <urn:uuid:797e83d7-a86f-4838-b5c5-0ec20855197d>,
    <urn:uuid:bbe073ad-f449-4b25-91ac-7d919613ca51>,
    <urn:uuid:1b457bed-8a80-4135-92b8-fdea12b4eea3>,
    <urn:uuid:2153d83b-8555-44a3-96e0-821b6663a188>,
    <urn:uuid:0c7028f0-8226-47b3-acff-a4e83e6a60fd>,
    <urn:uuid:4bbcdde6-ed53-4f8d-b3f8-43f800fd05d5>;
  skos:narrower <urn:uuid:193a84ec-ef96-44b9-b356-6f6b1c6ec979>,
    <urn:uuid:42a48e75-a413-4b91-8787-a8c2dc1a65ed>;
  skos:prefLabel "networked information service"@en .

<urn:uuid:6c18acc3-3119-4f0b-8d24-0ca0ea9449d3> a skos:Concept;
  dct:created "2021-12-14T19:40:13Z"^^xsd:dateTime;
  dct:creator <urn:uuid:ca637d4b-c11b-4152-be98-bde602e7abd4>;
  skos:altLabel "ID"@en;
  skos:definition "In information systems, an identifier is a symbol, word, or token that is associated with an information resource, that (ideally) uniquely identifies it."@en;
  skos:hiddenLabel "IDs"@en;
  skos:inScheme <urn:uuid:2df6fac6-3122-44dc-9f92-5caab7f9b10b>,
    <urn:uuid:1b457bed-8a80-4135-92b8-fdea12b4eea3>,
    <urn:uuid:2153d83b-8555-44a3-96e0-821b6663a188>,
    <urn:uuid:797e83d7-a86f-4838-b5c5-0ec20855197d>,
    <urn:uuid:bbe073ad-f449-4b25-91ac-7d919613ca51>,
    <urn:uuid:a1a01f1c-7162-439c-94f1-3e28b99ae8ab>,
    <urn:uuid:ddfaaacc-9dcb-451b-afa6-477e6e787a5c>,
    <urn:uuid:0c7028f0-8226-47b3-acff-a4e83e6a60fd>,
    <urn:uuid:4bbcdde6-ed53-4f8d-b3f8-43f800fd05d5>;
  skos:narrower <urn:uuid:27a05aeb-017c-484d-b490-c6949e6eacbc>,
    <urn:uuid:9e506ca3-8be1-431d-9075-548141d9f8c1>,
    <urn:uuid:349633ba-03b8-4126-8e55-1ed9a7c7e4ec>,
    <urn:uuid:32453ea5-50cb-4ee1-a1f9-c03c0693fdda>;
  skos:prefLabel "identifier"@en .

<urn:uuid:755dd3a1-cffc-4d65-9446-435552bac541> a skos:Concept;
  dct:alternative "CSS is an open data standard promulgated by the W3C. It is a configuration language for communicating mainly but not necessarily visual and geometric representations of HTML and XML documents."@en;
  dct:created "2019-03-02T00:28:55Z"^^xsd:dateTime;
  dct:creator <urn:uuid:ca637d4b-c11b-4152-be98-bde602e7abd4>;
  dct:description "CSS is an open data standard promulgated by the W3C. It is a configuration language for communicating mainly but not necessarily visual and geometric representations of HTML and XML documents."@en;
  dct:modified "2021-12-14T03:01:01Z"^^xsd:dateTime;
  skos:altLabel "CSS"@en,
    "stylesheet"@en,
    "Cascading Style Sheets"@en;
  skos:definition "CSS is a standardized, declarative, rule-based language for applying styling information to HTML and XML content."@en;
  skos:hiddenLabel "Cascading Style Sheet"@en,
    "Cascading Stylesheet"@en,
    "style sheet"@en,
    "cascading style sheets"@en,
    "css"@en;
  skos:inScheme <urn:uuid:a1a01f1c-7162-439c-94f1-3e28b99ae8ab>,
    <urn:uuid:ddfaaacc-9dcb-451b-afa6-477e6e787a5c>,
    <urn:uuid:75f35368-e228-47fe-8efd-7251a2bde816>,
    <urn:uuid:1b457bed-8a80-4135-92b8-fdea12b4eea3>,
    <urn:uuid:2153d83b-8555-44a3-96e0-821b6663a188>,
    <urn:uuid:797e83d7-a86f-4838-b5c5-0ec20855197d>,
    <urn:uuid:bbe073ad-f449-4b25-91ac-7d919613ca51>,
    <urn:uuid:2df6fac6-3122-44dc-9f92-5caab7f9b10b>,
    <urn:uuid:0c7028f0-8226-47b3-acff-a4e83e6a60fd>,
    <urn:uuid:4bbcdde6-ed53-4f8d-b3f8-43f800fd05d5>;
  skos:prefLabel "Cascading Style Sheets"@en;
  skos:related <urn:uuid:45373ede-a7b0-404f-b797-902298208993>,
    <urn:uuid:5abd5284-7197-4eed-895d-6daefa019de8>,
    <urn:uuid:f352a521-b78e-478e-b01d-3a68638025a4>,
    <urn:uuid:0bc0aabb-9d9e-4caa-b9c8-553dd8b3ee05> .

<urn:uuid:75b4da00-36b5-467e-bc90-966a7e5256a1> a skos:Concept;
  dct:created "2017-07-13T18:41:57Z"^^xsd:dateTime;
  dct:creator <urn:uuid:ca637d4b-c11b-4152-be98-bde602e7abd4>;
  skos:definition "Data interchange is the transmission of data across information system boundaries in a manner that keeps the meaning of the data intact."@en;
  skos:inScheme <urn:uuid:2df6fac6-3122-44dc-9f92-5caab7f9b10b>,
    <urn:uuid:75f35368-e228-47fe-8efd-7251a2bde816>,
    <urn:uuid:1b457bed-8a80-4135-92b8-fdea12b4eea3>,
    <urn:uuid:2153d83b-8555-44a3-96e0-821b6663a188>,
    <urn:uuid:a1a01f1c-7162-439c-94f1-3e28b99ae8ab>,
    <urn:uuid:ddfaaacc-9dcb-451b-afa6-477e6e787a5c>,
    <urn:uuid:bbe073ad-f449-4b25-91ac-7d919613ca51>,
    <urn:uuid:91684d49-7b99-4b2e-9641-ea0b8e22f66c>,
    <urn:uuid:0c7028f0-8226-47b3-acff-a4e83e6a60fd>,
    <urn:uuid:4bbcdde6-ed53-4f8d-b3f8-43f800fd05d5>;
  skos:narrower <urn:uuid:027543f6-04df-4e92-96f4-5b0c8da4b799>,
    <urn:uuid:fe500c7a-b458-4d2c-8b3a-efd1bb47d106>;
  skos:prefLabel "data interchange"@en;
  skos:related <urn:uuid:7b7c4ecf-2544-4c03-ab5f-10de5e1a20d4>,
    <urn:uuid:f3f67e45-9cdf-4df1-9586-834ba185f63b>,
    <urn:uuid:0aabcb14-9aee-4b16-835e-02530dcb0c23>,
    <urn:uuid:9767147a-1b6a-440c-949f-7f6056e28411> .

<urn:uuid:9fc41de2-b16c-4170-8818-893302baa77d> a skos:Concept;
  dct:created "2017-02-01T23:11:59Z"^^xsd:dateTime;
  dct:creator <urn:uuid:ca637d4b-c11b-4152-be98-bde602e7abd4>;
  skos:broader <urn:uuid:b801e469-101d-4305-866d-edb0f70979de>,
    <urn:uuid:16d17f33-394d-4d0b-a882-81e8fc3a52fe>;
  skos:definition "Hypertext is a style of text where segments of content are connected together by links."@en;
  skos:inScheme <urn:uuid:0c7028f0-8226-47b3-acff-a4e83e6a60fd>,
    <urn:uuid:2df6fac6-3122-44dc-9f92-5caab7f9b10b>,
    <urn:uuid:bbe073ad-f449-4b25-91ac-7d919613ca51>,
    <urn:uuid:1b457bed-8a80-4135-92b8-fdea12b4eea3>,
    <urn:uuid:2153d83b-8555-44a3-96e0-821b6663a188>,
    <urn:uuid:a1a01f1c-7162-439c-94f1-3e28b99ae8ab>,
    <urn:uuid:ddfaaacc-9dcb-451b-afa6-477e6e787a5c>,
    <urn:uuid:4bbcdde6-ed53-4f8d-b3f8-43f800fd05d5>;
  skos:prefLabel "hypertext"@en .

<urn:uuid:abadd9b5-844e-4982-8fbe-b6b83d43736d> a skos:Concept;
  dct:created "2017-02-05T04:09:28Z"^^xsd:dateTime;
  dct:creator <urn:uuid:ca637d4b-c11b-4152-be98-bde602e7abd4>;
  skos:broader <urn:uuid:10bafb58-6eb8-4d99-9b7d-9840842d3947>;
  skos:inScheme <urn:uuid:49ac68c4-922c-4d9e-88fa-b318fc54d36f>,
    <urn:uuid:2df6fac6-3122-44dc-9f92-5caab7f9b10b>,
    <urn:uuid:bbe073ad-f449-4b25-91ac-7d919613ca51>,
    <urn:uuid:1b457bed-8a80-4135-92b8-fdea12b4eea3>,
    <urn:uuid:2153d83b-8555-44a3-96e0-821b6663a188>,
    <urn:uuid:4bbcdde6-ed53-4f8d-b3f8-43f800fd05d5>;
  skos:prefLabel "active directory"@en .

<urn:uuid:b39c1f53-b8ed-49fb-ba57-24dfe7dc2d9f> a skos:Concept;
  dct:created "2022-12-14T01:22:53Z"^^xsd:dateTime;
  dct:creator <urn:uuid:ca637d4b-c11b-4152-be98-bde602e7abd4>;
  skos:definition "An information system can be understood as a system (a whole made of mutually-interacting parts) for storing, operating over, and moving information. While specific information technologies may influence the behavior of the system, how the information system does what it does is secondary to what it does."@en;
  skos:inScheme <urn:uuid:0c7028f0-8226-47b3-acff-a4e83e6a60fd>,
    <urn:uuid:a1a01f1c-7162-439c-94f1-3e28b99ae8ab>,
    <urn:uuid:ddfaaacc-9dcb-451b-afa6-477e6e787a5c>,
    <urn:uuid:bbe073ad-f449-4b25-91ac-7d919613ca51>,
    <urn:uuid:1b457bed-8a80-4135-92b8-fdea12b4eea3>,
    <urn:uuid:2153d83b-8555-44a3-96e0-821b6663a188>,
    <urn:uuid:4bbcdde6-ed53-4f8d-b3f8-43f800fd05d5>;
  skos:narrower <urn:uuid:b95d0656-3b14-4e38-8fe2-75401ff7ee31>,
    <urn:uuid:1b004393-fdea-438b-a0d8-1919184d4bd1>,
    <urn:uuid:e7ccb716-f967-439f-9682-dad225efc0b6>;
  skos:prefLabel "information system"@en;
  skos:related <urn:uuid:7284c136-288b-49aa-b129-a56e2be938d2> .

<urn:uuid:c9f9e746-371c-4d67-a962-e3906c86a5c3> a skos:Concept;
  dct:alternative "An ontology is a type of controlled vocabulary that formally defines, not only what kinds of thing exist in a particular domain of discourse, but how those things can relate to one another."@en;
  dct:created "2017-07-12T03:23:57Z"^^xsd:dateTime;
  dct:creator <urn:uuid:ca637d4b-c11b-4152-be98-bde602e7abd4>;
  dct:description "An ontology is a type of controlled vocabulary that formally defines, not only what kinds of thing exist in a particular domain of discourse, but how those things can relate to one another."@en;
  dct:modified "2022-06-15T18:23:14Z"^^xsd:dateTime;
  skos:broader <urn:uuid:51a7c4b2-ef0c-4dc1-a538-553622131f09>;
  skos:definition """An ontology (in the sense of computing and information science) differs from a taxonomy, in that a taxonomy organizes categories through a fixed set of (often hierarchical) semantic relations, whereas an ontology also affords the definition and meta-relation of semantic relations themselves.
(this definition is bad; make a better one someday)"""@en;
  skos:inScheme <urn:uuid:2df6fac6-3122-44dc-9f92-5caab7f9b10b>,
    <urn:uuid:bbe073ad-f449-4b25-91ac-7d919613ca51>,
    <urn:uuid:1b457bed-8a80-4135-92b8-fdea12b4eea3>,
    <urn:uuid:2153d83b-8555-44a3-96e0-821b6663a188>,
    <urn:uuid:91684d49-7b99-4b2e-9641-ea0b8e22f66c>,
    <urn:uuid:a1a01f1c-7162-439c-94f1-3e28b99ae8ab>,
    <urn:uuid:ddfaaacc-9dcb-451b-afa6-477e6e787a5c>,
    <urn:uuid:75f35368-e228-47fe-8efd-7251a2bde816>,
    <urn:uuid:4bbcdde6-ed53-4f8d-b3f8-43f800fd05d5>;
  skos:narrower <urn:uuid:afb9bfa2-d565-460b-855a-69331787ff1b>,
    <urn:uuid:ed4d30d7-d3cf-4b21-bcb4-5f2525027be7>;
  skos:prefLabel "ontology"@en;
  skos:related <urn:uuid:45b6c768-da32-4e5f-9c87-a18d5ec94635>,
    <urn:uuid:7284c136-288b-49aa-b129-a56e2be938d2>,
    <urn:uuid:85a069f9-1a66-4462-b0e2-d042db345919> .

<urn:uuid:d85e3c52-cc94-48a4-8dc5-591de86be52f> a skos:Concept;
  dct:created "2017-02-21T19:56:34Z"^^xsd:dateTime;
  dct:creator <urn:uuid:ca637d4b-c11b-4152-be98-bde602e7abd4>;
  skos:altLabel "account"@en;
  skos:broader <urn:uuid:a718d483-af90-4eaf-a59f-31d8897d6e8e>,
    <urn:uuid:da6f9f27-38f3-47e9-8b16-03728bea9f5e>;
  skos:definition "An account is a record in a database that stores information about a person (or automated software agent), including their username and password (or cryptographic keys)."@en;
  skos:inScheme <urn:uuid:2df6fac6-3122-44dc-9f92-5caab7f9b10b>,
    <urn:uuid:49ac68c4-922c-4d9e-88fa-b318fc54d36f>,
    <urn:uuid:bbe073ad-f449-4b25-91ac-7d919613ca51>,
    <urn:uuid:1b457bed-8a80-4135-92b8-fdea12b4eea3>,
    <urn:uuid:2153d83b-8555-44a3-96e0-821b6663a188>,
    <urn:uuid:4bbcdde6-ed53-4f8d-b3f8-43f800fd05d5>;
  skos:narrower <urn:uuid:96a2b1d2-732d-45a1-addb-a8cbb9868480>;
  skos:prefLabel "account (user)"@en;
  skos:related <urn:uuid:d0d7da4b-4d4d-4262-96a3-a70afbc1a829> .

<urn:uuid:0cf51602-4fc1-4a38-9663-d47aff228b2d> a skos:Concept;
  dct:created "2022-11-23T21:38:05Z"^^xsd:dateTime;
  dct:creator <urn:uuid:ca637d4b-c11b-4152-be98-bde602e7abd4>;
  skos:definition "Content is the information that the user of an information system uses the system for."@en;
  skos:inScheme <urn:uuid:bbe073ad-f449-4b25-91ac-7d919613ca51>,
    <urn:uuid:a1a01f1c-7162-439c-94f1-3e28b99ae8ab>,
    <urn:uuid:ddfaaacc-9dcb-451b-afa6-477e6e787a5c>,
    <urn:uuid:1b457bed-8a80-4135-92b8-fdea12b4eea3>,
    <urn:uuid:2153d83b-8555-44a3-96e0-821b6663a188>,
    <urn:uuid:0c7028f0-8226-47b3-acff-a4e83e6a60fd>,
    <urn:uuid:4bbcdde6-ed53-4f8d-b3f8-43f800fd05d5>;
  skos:narrower <urn:uuid:9283f8a5-c02f-4f5d-af14-3a9648e5639f>;
  skos:prefLabel "content"@en;
  skos:related <urn:uuid:b39c1f53-b8ed-49fb-ba57-24dfe7dc2d9f> .

<urn:uuid:16d17f33-394d-4d0b-a882-81e8fc3a52fe> a skos:Concept;
  dct:created "2017-02-01T04:45:22Z"^^xsd:dateTime;
  dct:creator <urn:uuid:ca637d4b-c11b-4152-be98-bde602e7abd4>;
  dct:modified "2019-02-02T19:07:37Z"^^xsd:dateTime;
  skos:definition "Hypermedia is a generalization of the concept of hypertext, to include audiovisual content."@en;
  skos:inScheme <urn:uuid:49ac68c4-922c-4d9e-88fa-b318fc54d36f>,
    <urn:uuid:bbe073ad-f449-4b25-91ac-7d919613ca51>,
    <urn:uuid:1b457bed-8a80-4135-92b8-fdea12b4eea3>,
    <urn:uuid:2153d83b-8555-44a3-96e0-821b6663a188>,
    <urn:uuid:2df6fac6-3122-44dc-9f92-5caab7f9b10b>,
    <urn:uuid:a1a01f1c-7162-439c-94f1-3e28b99ae8ab>,
    <urn:uuid:ddfaaacc-9dcb-451b-afa6-477e6e787a5c>,
    <urn:uuid:0c7028f0-8226-47b3-acff-a4e83e6a60fd>,
    <urn:uuid:4bbcdde6-ed53-4f8d-b3f8-43f800fd05d5>;
  skos:narrower <urn:uuid:03e66b30-1bba-4663-bdcb-facd7b8dc7a7>,
    <urn:uuid:9fc41de2-b16c-4170-8818-893302baa77d>,
    <urn:uuid:162516dc-6817-4d47-b4a7-6939c14c0fbb>;
  skos:prefLabel "hypermedia"@en .

<urn:uuid:3a2c72e0-4fa5-4477-a51b-d7f073cc1155> a skos:Concept;
  dct:created "2017-02-20T02:45:20Z"^^xsd:dateTime;
  dct:creator <urn:uuid:ca637d4b-c11b-4152-be98-bde602e7abd4>;
  dct:modified "2017-07-09T22:51:11Z"^^xsd:dateTime,
    "2019-05-30T19:12:56Z"^^xsd:dateTime,
    "2020-06-01T20:59:14Z"^^xsd:dateTime;
  skos:definition "A data visualization is a graphical representation of a data structure or set of data structures. Data visualizations can either be quantitative, where the geometry is driven by numerical values, or qualitative, where the geometry is driven by semantic relations between structures."@en;
  skos:inScheme <urn:uuid:bbe073ad-f449-4b25-91ac-7d919613ca51>,
    <urn:uuid:49ac68c4-922c-4d9e-88fa-b318fc54d36f>,
    <urn:uuid:2df6fac6-3122-44dc-9f92-5caab7f9b10b>,
    <urn:uuid:1b457bed-8a80-4135-92b8-fdea12b4eea3>,
    <urn:uuid:2153d83b-8555-44a3-96e0-821b6663a188>,
    <urn:uuid:4bbcdde6-ed53-4f8d-b3f8-43f800fd05d5>;
  skos:prefLabel "data visualization"@en;
  skos:related <urn:uuid:3a2c72e0-4fa5-4477-a51b-d7f073cc1155>,
    <urn:uuid:5effc9c6-6843-4abc-8474-5e4002aa51cf>,
    <urn:uuid:91d3f305-8c2c-4922-ac6d-fee77af3e4eb>,
    <urn:uuid:9b7d80f4-7cdb-44a0-8ca8-c0b5606fb05a>,
    <urn:uuid:be93cce1-f21f-4e85-bd34-e005dea3532f> .

<urn:uuid:61c0c9c3-4d91-4509-902a-db09c4188ae5> a skos:Concept;
  dct:alternative "A content management system (CMS) is a piece of infrastructure software for organizing (usually) websites."@en;
  dct:created "2017-07-10T00:34:13Z"^^xsd:dateTime;
  dct:creator <urn:uuid:ca637d4b-c11b-4152-be98-bde602e7abd4>;
  dct:description "A content management system (CMS) is a piece of infrastructure software for organizing (usually) websites."@en;
  dct:modified "2021-12-15T03:09:38Z"^^xsd:dateTime;
  skos:altLabel "content management system"@en,
    "CMS"@en;
  skos:broader <urn:uuid:123bcb4d-b7e1-4715-b95b-73161516e789>;
  skos:definition "A CMS is a piece of software for organizing and operating over one or more Web properties. Functions include things like applying visual design templates and composing pages, as well as organizing linked files and embedded audiovisual media."@en;
  skos:hiddenLabel "cms"@en,
    "CMSes"@en;
  skos:inScheme <urn:uuid:2df6fac6-3122-44dc-9f92-5caab7f9b10b>,
    <urn:uuid:a1a01f1c-7162-439c-94f1-3e28b99ae8ab>,
    <urn:uuid:ddfaaacc-9dcb-451b-afa6-477e6e787a5c>,
    <urn:uuid:797e83d7-a86f-4838-b5c5-0ec20855197d>,
    <urn:uuid:bbe073ad-f449-4b25-91ac-7d919613ca51>,
    <urn:uuid:1b457bed-8a80-4135-92b8-fdea12b4eea3>,
    <urn:uuid:2153d83b-8555-44a3-96e0-821b6663a188>,
    <urn:uuid:0c7028f0-8226-47b3-acff-a4e83e6a60fd>,
    <urn:uuid:4bbcdde6-ed53-4f8d-b3f8-43f800fd05d5>;
  skos:narrower <urn:uuid:295da6bb-7246-431c-b508-196207ab168b>;
  skos:prefLabel "content management system"@en;
  skos:related <urn:uuid:f9decec4-c869-4d17-aaa0-3a44ea18e6df>,
    <urn:uuid:42a48e75-a413-4b91-8787-a8c2dc1a65ed> .

<urn:uuid:759d2f68-3d16-4122-9758-c84f7760d691> a skos:Concept;
  dct:created "2017-02-09T21:50:06Z"^^xsd:dateTime;
  dct:creator <urn:uuid:ca637d4b-c11b-4152-be98-bde602e7abd4>;
  dct:references <https://en.wikipedia.org/wiki/World_Wide_Web>;
  skos:definition "The World-Wide Web is a particular implementation of Hypermedia, which runs on top of the internet."@en;
  skos:inScheme <urn:uuid:1b457bed-8a80-4135-92b8-fdea12b4eea3>,
    <urn:uuid:2153d83b-8555-44a3-96e0-821b6663a188>,
    <urn:uuid:2df6fac6-3122-44dc-9f92-5caab7f9b10b>,
    <urn:uuid:bbe073ad-f449-4b25-91ac-7d919613ca51>,
    <urn:uuid:49ac68c4-922c-4d9e-88fa-b318fc54d36f>,
    <urn:uuid:a1a01f1c-7162-439c-94f1-3e28b99ae8ab>,
    <urn:uuid:ddfaaacc-9dcb-451b-afa6-477e6e787a5c>,
    <urn:uuid:0c7028f0-8226-47b3-acff-a4e83e6a60fd>,
    <urn:uuid:4bbcdde6-ed53-4f8d-b3f8-43f800fd05d5>;
  skos:narrower <urn:uuid:0bc0aabb-9d9e-4caa-b9c8-553dd8b3ee05>,
    <urn:uuid:e162d03b-bfec-4f01-ab7e-56da309550f6>,
    <urn:uuid:02b3d282-d134-487b-8226-80141b5a4338>;
  skos:prefLabel "World-Wide Web"@en;
  skos:related <urn:uuid:16d17f33-394d-4d0b-a882-81e8fc3a52fe> .

<urn:uuid:7b7c4ecf-2544-4c03-ab5f-10de5e1a20d4> a skos:Concept;
  dct:alternative "Linked Data is the use (embedding) of metadata in Web resources (ideally but not exclusively RDF) as a way to provision structured data objects across the internet. The concept is very closely related to REST."@en;
  dct:created "2017-07-12T04:40:19Z"^^xsd:dateTime;
  dct:creator <urn:uuid:ca637d4b-c11b-4152-be98-bde602e7abd4>;
  dct:description "Linked Data is the use (embedding) of metadata  in Web resources (ideally but not exclusively RDF) as a way to provision structured data objects across the internet. The concept is very closely related to REST."@en;
  dct:modified "2021-12-14T22:30:37Z"^^xsd:dateTime;
  dct:references <http://linkeddata.org/>,
    <https://en.wikipedia.org/wiki/Linked_data>;
  skos:altLabel "linked data"@en;
  skos:definition "Linked data is an architectural style with considerable overlap with REST, involving making hypermedia resources that contain machine-readable structured data with discernible semantics, in contrast with opaque documents with no machine-readable semantics. A rudimentary form of linked data is in use in SEO circles with JSON-LD."@en;
  skos:inScheme <urn:uuid:797e83d7-a86f-4838-b5c5-0ec20855197d>,
    <urn:uuid:1b457bed-8a80-4135-92b8-fdea12b4eea3>,
    <urn:uuid:2153d83b-8555-44a3-96e0-821b6663a188>,
    <urn:uuid:bbe073ad-f449-4b25-91ac-7d919613ca51>,
    <urn:uuid:2df6fac6-3122-44dc-9f92-5caab7f9b10b>,
    <urn:uuid:4bbcdde6-ed53-4f8d-b3f8-43f800fd05d5>;
  skos:narrower <urn:uuid:5162945a-0397-466c-9cd7-02552f893beb>;
  skos:prefLabel "Linked Data"@en;
  skos:related <urn:uuid:288e85ab-887f-437c-9caa-c109cb9d478d>,
    <urn:uuid:5e2780c6-58f7-4ef9-8b1f-91fdcf4f8a6a>,
    <urn:uuid:65a4359d-9ef6-44a3-9317-875495517b3c>,
    <urn:uuid:75b4da00-36b5-467e-bc90-966a7e5256a1>,
    <urn:uuid:ca632e87-50d2-4f1d-af83-f3d11e53eca8>,
    <urn:uuid:fe500c7a-b458-4d2c-8b3a-efd1bb47d106>,
    <urn:uuid:e903395d-2497-4394-8067-d77daf60f198> .

<urn:uuid:85a069f9-1a66-4462-b0e2-d042db345919> a skos:Concept;
  dct:created "2017-07-26T20:47:31Z"^^xsd:dateTime;
  dct:creator <urn:uuid:ca637d4b-c11b-4152-be98-bde602e7abd4>;
  rdfs:seeAlso <https://doriantaylor.com/the-symbol-management-problem>;
  skos:definition "The symbol management problem is roughly that of having too many symbols to manage: object keys, enumerated values, variables, class names, method names, URL path segments and query parameters, CSS selectors, etc."@en;
  skos:inScheme <urn:uuid:2df6fac6-3122-44dc-9f92-5caab7f9b10b>,
    <urn:uuid:a1a01f1c-7162-439c-94f1-3e28b99ae8ab>,
    <urn:uuid:ddfaaacc-9dcb-451b-afa6-477e6e787a5c>,
    <urn:uuid:91684d49-7b99-4b2e-9641-ea0b8e22f66c>,
    <urn:uuid:bbe073ad-f449-4b25-91ac-7d919613ca51>,
    <urn:uuid:0c7028f0-8226-47b3-acff-a4e83e6a60fd>,
    <urn:uuid:1b457bed-8a80-4135-92b8-fdea12b4eea3>,
    <urn:uuid:2153d83b-8555-44a3-96e0-821b6663a188>,
    <urn:uuid:75f35368-e228-47fe-8efd-7251a2bde816>,
    <urn:uuid:4bbcdde6-ed53-4f8d-b3f8-43f800fd05d5>;
  skos:prefLabel "symbol management problem"@en;
  skos:related <urn:uuid:0f872daf-97f4-445e-b5d9-0de0087dd129>,
    <urn:uuid:45b6c768-da32-4e5f-9c87-a18d5ec94635>,
    <urn:uuid:51a7c4b2-ef0c-4dc1-a538-553622131f09>,
    <urn:uuid:755dd3a1-cffc-4d65-9446-435552bac541>,
    <urn:uuid:440e5d73-d654-4051-b482-2a960835306b>,
    <urn:uuid:c9f9e746-371c-4d67-a962-e3906c86a5c3>,
    <urn:uuid:2c534735-69b5-4d54-bd9f-dd47b4a5e678>,
    <urn:uuid:e840ba8a-4c6d-4be3-a673-dd6620463a39> .

<urn:uuid:c757c1ac-1ec6-4bdd-a35d-85f1d85728bb> a skos:Concept;
  dct:created "2022-11-24T00:10:11Z"^^xsd:dateTime;
  dct:creator <urn:uuid:ca637d4b-c11b-4152-be98-bde602e7abd4>;
  skos:altLabel "data object"@en,
    "structured data object"@en;
  skos:definition "Structured data (in contrast to unstructured data) is a representation of information such that its content is machine-actionable by a deterministic process, i.e. it does not require interpretation by a human or by statistical means (i.e., artificial intelligence). The structure represented by a structured data object is of course a data structure (which would have a different representation inside a running program). An example of structured data (assuming some kind of schema to communicate the semantics) would be JSON."@en;
  skos:inScheme <urn:uuid:1b457bed-8a80-4135-92b8-fdea12b4eea3>,
    <urn:uuid:2153d83b-8555-44a3-96e0-821b6663a188>,
    <urn:uuid:9f98d1d7-745f-47bc-a361-f6b4fe352fbc>,
    <urn:uuid:a1a01f1c-7162-439c-94f1-3e28b99ae8ab>,
    <urn:uuid:ddfaaacc-9dcb-451b-afa6-477e6e787a5c>,
    <urn:uuid:bbe073ad-f449-4b25-91ac-7d919613ca51>,
    <urn:uuid:0c7028f0-8226-47b3-acff-a4e83e6a60fd>,
    <urn:uuid:4bbcdde6-ed53-4f8d-b3f8-43f800fd05d5>;
  skos:narrower <urn:uuid:9767147a-1b6a-440c-949f-7f6056e28411>;
  skos:prefLabel "structured data"@en;
  skos:related <urn:uuid:f5a254ac-4a2b-405e-91be-7de9fbf7174d>,
    <urn:uuid:8d46494e-5316-43b7-a49e-a625ab716a38> .

<urn:uuid:d0d7da4b-4d4d-4262-96a3-a70afbc1a829> a skos:Concept;
  dct:alternative "Authentication is the part of access control concerned with verifying that a person is who they say they are. A conventional way to authenticate is with a system of accounts, each with a username and password."@en;
  dct:created "2017-02-21T19:54:05Z"^^xsd:dateTime;
  dct:creator <urn:uuid:ca637d4b-c11b-4152-be98-bde602e7abd4>;
  dct:description "Authentication is the part of access control concerned with verifying that a person is who they say they are. A conventional way to authenticate is with a system of accounts, each with a username and password."@en;
  dct:modified "2019-03-06T16:23:17Z"^^xsd:dateTime;
  skos:broader <urn:uuid:c0e969c3-4528-4968-8418-d5fe609c2a62>;
  skos:definition "Authentication is the part of access control concerned with verifying that a person is who they say they are. A conventional way to authenticate is with a system of accounts, each with a username and password."@en,
    "Authentication is the aspect of access control concerned with figuring out who a principal (usually a person) is, or otherwise proving who they claim they are, should they be making such a claim."@en;
  skos:inScheme <urn:uuid:2df6fac6-3122-44dc-9f92-5caab7f9b10b>,
    <urn:uuid:bbe073ad-f449-4b25-91ac-7d919613ca51>,
    <urn:uuid:0c7028f0-8226-47b3-acff-a4e83e6a60fd>,
    <urn:uuid:49ac68c4-922c-4d9e-88fa-b318fc54d36f>,
    <urn:uuid:1b457bed-8a80-4135-92b8-fdea12b4eea3>,
    <urn:uuid:2153d83b-8555-44a3-96e0-821b6663a188>,
    <urn:uuid:4bbcdde6-ed53-4f8d-b3f8-43f800fd05d5>;
  skos:narrower <urn:uuid:96a2b1d2-732d-45a1-addb-a8cbb9868480>,
    <urn:uuid:7730f786-d46e-495d-a3bc-79d401599988>;
  skos:prefLabel "authentication"@en;
  skos:related <urn:uuid:d85e3c52-cc94-48a4-8dc5-591de86be52f> .

<urn:uuid:42747b64-a41c-4321-96cf-c49e711733e6> a skos:Concept;
  dct:alternative "Content strategy is a strategic design discipline that concerns itself with the management and organizing of mainly, but not necessarily exclusively, written text. Practitioners of the discipline, which is closely related to information architecture and user experience design, can range in capabilities along a spectrum of editorial to technical concerns."@en;
  dct:created "2019-03-06T05:44:08Z"^^xsd:dateTime;
  dct:creator <urn:uuid:ca637d4b-c11b-4152-be98-bde602e7abd4>;
  dct:description "Content strategy is a strategic design discipline that concerns itself with the management and organizing of mainly, but not necessarily exclusively, written text. Practitioners of the discipline, which is closely related to information architecture and user experience design, can range in capabilities along a spectrum of editorial to technical concerns."@en;
  dct:modified "2021-12-14T17:29:43Z"^^xsd:dateTime;
  skos:altLabel "content strategy"@en;
  skos:broader <urn:uuid:0cf51602-4fc1-4a38-9663-d47aff228b2d>;
  skos:definition "Content strategy is a broader concept than content management, because it entails more than merely \"managing\" content, but also concerns the governance, life cycle, technical minutiae, as well as things like style guides for the voice and tone of (usually textual) content."@en;
  skos:inScheme <urn:uuid:1b457bed-8a80-4135-92b8-fdea12b4eea3>,
    <urn:uuid:2153d83b-8555-44a3-96e0-821b6663a188>,
    <urn:uuid:a1a01f1c-7162-439c-94f1-3e28b99ae8ab>,
    <urn:uuid:ddfaaacc-9dcb-451b-afa6-477e6e787a5c>,
    <urn:uuid:797e83d7-a86f-4838-b5c5-0ec20855197d>,
    <urn:uuid:bbe073ad-f449-4b25-91ac-7d919613ca51>,
    <urn:uuid:2df6fac6-3122-44dc-9f92-5caab7f9b10b>,
    <urn:uuid:75f35368-e228-47fe-8efd-7251a2bde816>,
    <urn:uuid:0c7028f0-8226-47b3-acff-a4e83e6a60fd>,
    <urn:uuid:4bbcdde6-ed53-4f8d-b3f8-43f800fd05d5>;
  skos:narrower <urn:uuid:9283f8a5-c02f-4f5d-af14-3a9648e5639f>,
    <urn:uuid:01dc6e60-8e23-4c4c-a63d-f149cb104f84>;
  skos:prefLabel "content strategy"@en;
  skos:related <urn:uuid:7284c136-288b-49aa-b129-a56e2be938d2>,
    <urn:uuid:d2089ee2-d605-43ac-af18-ffbb7151a32d> .

<urn:uuid:4694ebe0-589f-40a7-9ef9-67872edb6214> a skos:Concept;
  dct:created "2019-05-30T20:56:58Z"^^xsd:dateTime,
    "2017-02-05T04:09:02Z"^^xsd:dateTime;
  dct:creator <urn:uuid:ca637d4b-c11b-4152-be98-bde602e7abd4>;
  dct:modified "2019-03-02T05:24:24Z"^^xsd:dateTime;
  skos:broader <urn:uuid:11227a90-60be-4845-a675-b88b599ac79b>,
    <urn:uuid:10bafb58-6eb8-4d99-9b7d-9840842d3947>;
  skos:definition "A database is any persistent storage facility for digital information. Databases can be embedded in applications, or be stand-alone online resources accessed over a network. File systems are a form of database, as are relational (SQL) databases and (RDF or otherwise) graph stores."@en;
  skos:inScheme <urn:uuid:1b457bed-8a80-4135-92b8-fdea12b4eea3>,
    <urn:uuid:2153d83b-8555-44a3-96e0-821b6663a188>,
    <urn:uuid:86eb4d1a-12f8-44ec-be89-ca588c2ee1d4>,
    <urn:uuid:2df6fac6-3122-44dc-9f92-5caab7f9b10b>,
    <urn:uuid:bbe073ad-f449-4b25-91ac-7d919613ca51>,
    <urn:uuid:4bbcdde6-ed53-4f8d-b3f8-43f800fd05d5>;
  skos:narrower <urn:uuid:2717d0b5-cb79-4d1a-82c0-69cdc1e590a1>,
    <urn:uuid:abadd9b5-844e-4982-8fbe-b6b83d43736d>;
  skos:prefLabel "database"@en;
  skos:related <urn:uuid:2d6d3a0f-8888-4d01-8178-bf5bad91a5b6>,
    <urn:uuid:9767147a-1b6a-440c-949f-7f6056e28411> .

<urn:uuid:5bdd2fb7-d84d-4583-998b-7d3f2803307e> a skos:Concept;
  dct:alternative "In REST parlance, a representation refers to the literal sequence of bits needed to convey the content of an information resource. An information resource can have multiple representations."@en;
  dct:created "2019-03-06T23:10:18Z"^^xsd:dateTime,
    "2008-06-14T04:30:27+00:00"^^xsd:dateTime;
  dct:creator <urn:uuid:ca637d4b-c11b-4152-be98-bde602e7abd4>;
  dct:description "In REST parlance, a representation refers to the literal sequence of bits needed to convey the content of an information resource. An information resource can have multiple representations."@en;
  dct:modified "2008-10-09T02:02:01+00:00"^^xsd:dateTime,
    "2008-10-10T16:02:45+00:00"^^xsd:dateTime,
    "2008-10-10T21:28:23+00:00"^^xsd:dateTime,
    "2009-03-04T00:43:00+00:00"^^xsd:dateTime,
    "2019-03-06T23:10:18Z"^^xsd:dateTime,
    "2021-12-14T21:34:55Z"^^xsd:dateTime,
    "2022-05-31T04:18:52+00:00"^^xsd:dateTime,
    "2008-06-14T06:38:36+00:00"^^xsd:dateTime,
    "2008-07-18T18:59:52+00:00"^^xsd:dateTime;
  skos:altLabel "representation"@en;
  skos:definition "A representation (of a Web resource) refers to the literal sequence of bits that comes out of an HTTP response. It could be a file, or it could be the output of a program. A resource can have multiple representations that vary along a number of dimensions (e.g. language, content type). The process of choosing a representation of a resource is called content negotiation."@en;
  skos:hiddenLabel "representations"@en;
  skos:inScheme <urn:uuid:75f35368-e228-47fe-8efd-7251a2bde816>,
    <urn:uuid:4ec7530b-5536-4fb7-bb5a-45a3f5fddc22>,
    <urn:uuid:797e83d7-a86f-4838-b5c5-0ec20855197d>,
    <urn:uuid:bbe073ad-f449-4b25-91ac-7d919613ca51>,
    <urn:uuid:a1a01f1c-7162-439c-94f1-3e28b99ae8ab>,
    <urn:uuid:ddfaaacc-9dcb-451b-afa6-477e6e787a5c>,
    <urn:uuid:1b457bed-8a80-4135-92b8-fdea12b4eea3>,
    <urn:uuid:2153d83b-8555-44a3-96e0-821b6663a188>,
    <urn:uuid:2df6fac6-3122-44dc-9f92-5caab7f9b10b>,
    <urn:uuid:0c7028f0-8226-47b3-acff-a4e83e6a60fd>,
    <urn:uuid:4bbcdde6-ed53-4f8d-b3f8-43f800fd05d5>;
  skos:narrower <urn:uuid:37810612-aecc-49b8-9df0-bc1255fa214a>;
  skos:prefLabel "representation"@en;
  skos:related <urn:uuid:02b3d282-d134-487b-8226-80141b5a4338>,
    <urn:uuid:c0e969c3-4528-4968-8418-d5fe609c2a62> .

<urn:uuid:86c65d14-2d23-4350-8004-233b2f3e873f> a skos:Concept;
  dct:alternative "An RDF vocabulary is an umbrella concept for an information resource that describes a set of RDF classes and properties, their usage, and their semantics. A vocabulary could be expressed in RDF Schema, OWL, SHACL, or a mix of all three."@en;
  dct:created "2017-07-12T02:32:21Z"^^xsd:dateTime;
  dct:creator <urn:uuid:ca637d4b-c11b-4152-be98-bde602e7abd4>;
  dct:description "An RDF vocabulary is an umbrella concept for an information resource that describes a set of RDF classes and properties, their usage, and their semantics. A vocabulary could be expressed in RDF Schema, OWL, SHACL, or a mix of all three."@en;
  dct:modified "2021-12-14T18:03:21Z"^^xsd:dateTime;
  skos:altLabel "RDF vocabulary"@en;
  skos:broader <urn:uuid:51a7c4b2-ef0c-4dc1-a538-553622131f09>,
    <urn:uuid:8d46494e-5316-43b7-a49e-a625ab716a38>,
    <urn:uuid:fe500c7a-b458-4d2c-8b3a-efd1bb47d106>;
  skos:definition "An RDF vocabulary is a set of terms specifying classes of resources, properties those resources exhibit, and value ranges for those properties. An RDF vocabulary can either be represented in RDF Schema or OWL (Web Ontology Language), which has additional features."@en;
  skos:inScheme <urn:uuid:2df6fac6-3122-44dc-9f92-5caab7f9b10b>,
    <urn:uuid:1b457bed-8a80-4135-92b8-fdea12b4eea3>,
    <urn:uuid:2153d83b-8555-44a3-96e0-821b6663a188>,
    <urn:uuid:797e83d7-a86f-4838-b5c5-0ec20855197d>,
    <urn:uuid:bbe073ad-f449-4b25-91ac-7d919613ca51>,
    <urn:uuid:4bbcdde6-ed53-4f8d-b3f8-43f800fd05d5>;
  skos:narrower <urn:uuid:32092336-fb45-4598-851e-fd3dbffb1dca>,
    <urn:uuid:384f764c-9d71-46a3-9865-0af7068c0703>,
    <urn:uuid:5b30faaa-7c8b-4c57-8dc5-26bd63047d3f>,
    <urn:uuid:a4a25c35-91ab-4c8e-9bea-ee877ad0e18b>,
    <urn:uuid:a94728e6-4a3f-4694-9e9e-c1c949ed66c2>,
    <urn:uuid:bf986385-65ff-424e-8eb1-6c6653cb6b4e>,
    <urn:uuid:ed4d30d7-d3cf-4b21-bcb4-5f2525027be7>;
  skos:prefLabel "RDF Vocabulary"@en .

<urn:uuid:8d46494e-5316-43b7-a49e-a625ab716a38> a skos:Concept;
  dct:created "2021-12-14T20:10:33Z"^^xsd:dateTime;
  dct:creator <urn:uuid:ca637d4b-c11b-4152-be98-bde602e7abd4>;
  skos:definition "An open data standard is a specification for a content type or network protocol that has the principal characteristic that you don't have to pay to use or even see it. Specificatons for open data standards are therefore freely available and almost always online."@en;
  skos:hiddenLabel "open data standards"@en,
    "open standard"@en;
  skos:inScheme <urn:uuid:2df6fac6-3122-44dc-9f92-5caab7f9b10b>,
    <urn:uuid:797e83d7-a86f-4838-b5c5-0ec20855197d>,
    <urn:uuid:bbe073ad-f449-4b25-91ac-7d919613ca51>,
    <urn:uuid:0c7028f0-8226-47b3-acff-a4e83e6a60fd>,
    <urn:uuid:1b457bed-8a80-4135-92b8-fdea12b4eea3>,
    <urn:uuid:2153d83b-8555-44a3-96e0-821b6663a188>,
    <urn:uuid:a1a01f1c-7162-439c-94f1-3e28b99ae8ab>,
    <urn:uuid:ddfaaacc-9dcb-451b-afa6-477e6e787a5c>,
    <urn:uuid:4bbcdde6-ed53-4f8d-b3f8-43f800fd05d5>;
  skos:narrower <urn:uuid:86c65d14-2d23-4350-8004-233b2f3e873f>,
    <urn:uuid:f352a521-b78e-478e-b01d-3a68638025a4>,
    <urn:uuid:eb45112f-3c6a-47be-a547-e3462fb853e4>,
    <urn:uuid:0bc0aabb-9d9e-4caa-b9c8-553dd8b3ee05>,
    <urn:uuid:fe500c7a-b458-4d2c-8b3a-efd1bb47d106>;
  skos:prefLabel "open data standard"@en;
  skos:related <urn:uuid:fe500c7a-b458-4d2c-8b3a-efd1bb47d106>,
    <urn:uuid:e5394a0c-c64a-4ded-a37b-55c1507dc24c> .

<urn:uuid:a718d483-af90-4eaf-a59f-31d8897d6e8e> a skos:Concept;
  dct:created "2017-02-21T19:53:28Z"^^xsd:dateTime;
  dct:creator <urn:uuid:ca637d4b-c11b-4152-be98-bde602e7abd4>;
  dct:description "(Information) security refers to the practice of protecting information from being stolen or damaged."@en;
  dct:modified "2020-06-01T21:09:22Z"^^xsd:dateTime,
    "2018-02-03T14:09:09Z"^^xsd:dateTime,
    "2022-11-23T23:26:53Z"^^xsd:dateTime;
  skos:altLabel "Security"@en,
    "cybersecurity",
    "security"@en,
    "security (information)"@en;
  skos:definition "(Information) security refers to the practice of protecting information from being stolen or damaged."@en,
    "Information security is the discipline and practice of ensuring that only the people who are allowed to access a given set of information, are the ones who can access it."@en;
  skos:hiddenLabel "security (information)";
  skos:inScheme <urn:uuid:49ac68c4-922c-4d9e-88fa-b318fc54d36f>,
    <urn:uuid:2df6fac6-3122-44dc-9f92-5caab7f9b10b>,
    <urn:uuid:a1a01f1c-7162-439c-94f1-3e28b99ae8ab>,
    <urn:uuid:ddfaaacc-9dcb-451b-afa6-477e6e787a5c>,
    <urn:uuid:1b457bed-8a80-4135-92b8-fdea12b4eea3>,
    <urn:uuid:2153d83b-8555-44a3-96e0-821b6663a188>,
    <urn:uuid:0c7028f0-8226-47b3-acff-a4e83e6a60fd>,
    <urn:uuid:bbe073ad-f449-4b25-91ac-7d919613ca51>,
    <urn:uuid:4bbcdde6-ed53-4f8d-b3f8-43f800fd05d5>;
  skos:narrower <urn:uuid:c0e969c3-4528-4968-8418-d5fe609c2a62>;
  skos:prefLabel "information security"@en .

<urn:uuid:ca632e87-50d2-4f1d-af83-f3d11e53eca8> a skos:Concept;
  dct:alternative "JSON is an enterprising appropriation of the primitive data types in JavaScript as a general-purpose serialization format to represent structured data. It has since evolved into its own open data standard."@en;
  dct:created "2017-07-13T18:46:35Z"^^xsd:dateTime;
  dct:creator <urn:uuid:ca637d4b-c11b-4152-be98-bde602e7abd4>;
  dct:description "JSON is an enterprising appropriation of the primitive data types in JavaScript as a general-purpose serialization format to represent structured data. It has since evolved into its own open data standard."@en;
  dct:modified "2021-12-14T20:09:32Z"^^xsd:dateTime;
  dct:references <https://tools.ietf.org/html/rfc7159>;
  rdfs:seeAlso <https://tools.ietf.org/html/rfc7159>,
    <https://datatracker.ietf.org/doc/html/rfc7159>;
  skos:altLabel "JSON"@en;
  skos:broader <urn:uuid:75b4da00-36b5-467e-bc90-966a7e5256a1>,
    <urn:uuid:8d46494e-5316-43b7-a49e-a625ab716a38>,
    <urn:uuid:9767147a-1b6a-440c-949f-7f6056e28411>,
    <urn:uuid:0aabcb14-9aee-4b16-835e-02530dcb0c23>;
  skos:definition "JSON (JavaScript Object Notation) is a popular data interchange (serialization) format (syntax) for structured data."@en,
    "JSON (JavaScript Object Notation) is a data interchange (serialization) format  (syntax) for structured data."@en;
  skos:hiddenLabel "javascript object notation"@en,
    "json"@en;
  skos:inScheme <urn:uuid:797e83d7-a86f-4838-b5c5-0ec20855197d>,
    <urn:uuid:bbe073ad-f449-4b25-91ac-7d919613ca51>,
    <urn:uuid:2df6fac6-3122-44dc-9f92-5caab7f9b10b>,
    <urn:uuid:0c7028f0-8226-47b3-acff-a4e83e6a60fd>,
    <urn:uuid:91684d49-7b99-4b2e-9641-ea0b8e22f66c>,
    <urn:uuid:1b457bed-8a80-4135-92b8-fdea12b4eea3>,
    <urn:uuid:2153d83b-8555-44a3-96e0-821b6663a188>,
    <urn:uuid:a1a01f1c-7162-439c-94f1-3e28b99ae8ab>,
    <urn:uuid:ddfaaacc-9dcb-451b-afa6-477e6e787a5c>,
    <urn:uuid:75f35368-e228-47fe-8efd-7251a2bde816>,
    <urn:uuid:4bbcdde6-ed53-4f8d-b3f8-43f800fd05d5>;
  skos:narrower <urn:uuid:5dc8e476-6377-429e-865c-562c6454c8a6>,
    <urn:uuid:cda3a7a9-41bc-4de7-ad92-1b9093389c64>;
  skos:prefLabel "JavaScript Object Notation"@en,
    "JSON"@en .

<urn:uuid:e840ba8a-4c6d-4be3-a673-dd6620463a39> a skos:Concept;
  dct:created "2017-07-10T00:49:29Z"^^xsd:dateTime;
  dct:creator <urn:uuid:ca637d4b-c11b-4152-be98-bde602e7abd4>;
  dct:modified "2021-12-13T23:24:25Z"^^xsd:dateTime;
  skos:altLabel "application programming interface"@en,
    "API"@en;
  skos:broader <urn:uuid:73cc630b-2000-46d7-8777-b0fe17e5e901>,
    <urn:uuid:055e91e4-5edf-46fd-9bad-9847dbf57a72>,
    <urn:uuid:51a7c4b2-ef0c-4dc1-a538-553622131f09>;
  skos:definition "An API is, in the most generic sense, a published commitment on the part of a person or business entity to expose certain functionality, behavior, or semantics of an information system under their control. In the sense in which we are more accustomed, an API refers to a specific class of software that implements this functionality on the Web."@en;
  skos:hiddenLabel "API's"@en,
    "APIs"@en,
    "api"@en,
    "application programming interfaces"@en;
  skos:inScheme <urn:uuid:91684d49-7b99-4b2e-9641-ea0b8e22f66c>,
    <urn:uuid:bbe073ad-f449-4b25-91ac-7d919613ca51>,
    <urn:uuid:a1a01f1c-7162-439c-94f1-3e28b99ae8ab>,
    <urn:uuid:ddfaaacc-9dcb-451b-afa6-477e6e787a5c>,
    <urn:uuid:1b457bed-8a80-4135-92b8-fdea12b4eea3>,
    <urn:uuid:2153d83b-8555-44a3-96e0-821b6663a188>,
    <urn:uuid:75f35368-e228-47fe-8efd-7251a2bde816>,
    <urn:uuid:4ec7530b-5536-4fb7-bb5a-45a3f5fddc22>,
    <urn:uuid:797e83d7-a86f-4838-b5c5-0ec20855197d>,
    <urn:uuid:2df6fac6-3122-44dc-9f92-5caab7f9b10b>,
    <urn:uuid:4bbcdde6-ed53-4f8d-b3f8-43f800fd05d5>;
  skos:narrower <urn:uuid:91bffd8d-1f18-4604-844e-6a5557947a67>;
  skos:prefLabel "application programming interface"@en;
  skos:related <urn:uuid:6edac7a8-c4ae-4304-a511-ac1d971f4552>,
    <urn:uuid:615a2418-14be-4a69-b669-14e9f8219e9c>,
    <urn:uuid:85a069f9-1a66-4462-b0e2-d042db345919> .

<urn:uuid:027543f6-04df-4e92-96f4-5b0c8da4b799> a skos:Concept;
  dct:created "2019-02-22T01:32:35Z"^^xsd:dateTime;
  dct:creator <urn:uuid:ca637d4b-c11b-4152-be98-bde602e7abd4>;
  skos:altLabel "content type"@en,
    "media type"@en;
  skos:definition "A data (or file format, or serialization format) is a set of rules for turning a data structure into a sequence of bytes which can be stored or transported. The term is also used when speaking about instances of such serializations."@en;
  skos:inScheme <urn:uuid:a1a01f1c-7162-439c-94f1-3e28b99ae8ab>,
    <urn:uuid:ddfaaacc-9dcb-451b-afa6-477e6e787a5c>,
    <urn:uuid:75f35368-e228-47fe-8efd-7251a2bde816>,
    <urn:uuid:bbe073ad-f449-4b25-91ac-7d919613ca51>,
    <urn:uuid:1b457bed-8a80-4135-92b8-fdea12b4eea3>,
    <urn:uuid:2153d83b-8555-44a3-96e0-821b6663a188>,
    <urn:uuid:2df6fac6-3122-44dc-9f92-5caab7f9b10b>,
    <urn:uuid:0c7028f0-8226-47b3-acff-a4e83e6a60fd>,
    <urn:uuid:4bbcdde6-ed53-4f8d-b3f8-43f800fd05d5>;
  skos:narrower <urn:uuid:21d69225-b92a-4440-83a0-62a386451283>,
    <urn:uuid:45373ede-a7b0-404f-b797-902298208993>,
    <urn:uuid:f352a521-b78e-478e-b01d-3a68638025a4>,
    <urn:uuid:0bc0aabb-9d9e-4caa-b9c8-553dd8b3ee05>,
    <urn:uuid:ca632e87-50d2-4f1d-af83-f3d11e53eca8>;
  skos:prefLabel "data format"@en;
  skos:related <urn:uuid:0aabcb14-9aee-4b16-835e-02530dcb0c23>,
    <urn:uuid:85a069f9-1a66-4462-b0e2-d042db345919>,
    <urn:uuid:9767147a-1b6a-440c-949f-7f6056e28411> .

<urn:uuid:02b3d282-d134-487b-8226-80141b5a4338> a skos:Concept;
  dct:created "2019-03-07T01:04:30Z"^^xsd:dateTime,
    "2021-12-14T19:39:46Z"^^xsd:dateTime;
  dct:creator <urn:uuid:ca637d4b-c11b-4152-be98-bde602e7abd4>;
  skos:altLabel "Hypertext Transfer Protocol"@en,
    "HTTP"@en;
  skos:broader <urn:uuid:9fc41de2-b16c-4170-8818-893302baa77d>,
    <urn:uuid:f0a7ece3-44e6-4f6b-963c-281ab8dff8e6>;
  skos:definition "HTTP is the protocol that carries the World-Wide Web."@en;
  skos:hiddenLabel "hypertext transfer protocol"@en,
    "http"@en;
  skos:inScheme <urn:uuid:2df6fac6-3122-44dc-9f92-5caab7f9b10b>,
    <urn:uuid:75f35368-e228-47fe-8efd-7251a2bde816>,
    <urn:uuid:797e83d7-a86f-4838-b5c5-0ec20855197d>,
    <urn:uuid:bbe073ad-f449-4b25-91ac-7d919613ca51>,
    <urn:uuid:1b457bed-8a80-4135-92b8-fdea12b4eea3>,
    <urn:uuid:2153d83b-8555-44a3-96e0-821b6663a188>,
    <urn:uuid:a1a01f1c-7162-439c-94f1-3e28b99ae8ab>,
    <urn:uuid:ddfaaacc-9dcb-451b-afa6-477e6e787a5c>,
    <urn:uuid:0c7028f0-8226-47b3-acff-a4e83e6a60fd>,
    <urn:uuid:4bbcdde6-ed53-4f8d-b3f8-43f800fd05d5>;
  skos:narrower <urn:uuid:a20b533d-6723-457b-aec0-570076760d32>;
  skos:prefLabel "HTTP"@en,
    "Hypertext Transfer Protocol"@en .

<urn:uuid:be93cce1-f21f-4e85-bd34-e005dea3532f> a skos:Concept;
  dct:alternative "A website is the kind of Web property we are most familiar with."@en;
  dct:created "2019-05-30T20:56:58Z"^^xsd:dateTime,
    "2017-02-09T17:50:13Z"^^xsd:dateTime;
  dct:creator <urn:uuid:ca637d4b-c11b-4152-be98-bde602e7abd4>;
  dct:description "A website is the kind of Web property we are most familiar with."@en;
  dct:modified "2021-12-14T23:52:24Z"^^xsd:dateTime;
  skos:altLabel "Web site"@en,
    "website"@en;
  skos:definition "A website can be understood in one aspect as a service, which runs on a server. In another aspect, it is an authoritative location—one of many locations on the World-Wide Web—for information resources, such as web pages and interfaces to software applications."@en,
    "A website can be understood in one aspect as a service, which runs on a server. In another aspect, it is an authoritative locationâone of many locations on the World-Wide Webâfor information resources, such as web pages and interfaces to software applications."@en;
  skos:inScheme <urn:uuid:86eb4d1a-12f8-44ec-be89-ca588c2ee1d4>,
    <urn:uuid:bbe073ad-f449-4b25-91ac-7d919613ca51>,
    <urn:uuid:797e83d7-a86f-4838-b5c5-0ec20855197d>,
    <urn:uuid:1b457bed-8a80-4135-92b8-fdea12b4eea3>,
    <urn:uuid:2153d83b-8555-44a3-96e0-821b6663a188>,
    <urn:uuid:a1a01f1c-7162-439c-94f1-3e28b99ae8ab>,
    <urn:uuid:ddfaaacc-9dcb-451b-afa6-477e6e787a5c>,
    <urn:uuid:2df6fac6-3122-44dc-9f92-5caab7f9b10b>,
    <urn:uuid:4bbcdde6-ed53-4f8d-b3f8-43f800fd05d5>;
  skos:narrower <urn:uuid:935ab72b-b74c-4204-9c00-f1f8f83f105e>;
  skos:prefLabel "website"@en;
  skos:related <urn:uuid:0f6e28e8-8a36-49f8-94d4-c681609d448f>,
    <urn:uuid:4039a99d-c14b-40f2-84d5-4ec72e2217e1>,
    <urn:uuid:759d2f68-3d16-4122-9758-c84f7760d691> .

<urn:uuid:45b6c768-da32-4e5f-9c87-a18d5ec94635> a skos:Concept;
  dct:created "2017-07-12T03:04:30Z"^^xsd:dateTime;
  dct:creator <urn:uuid:ca637d4b-c11b-4152-be98-bde602e7abd4>;
  dct:modified "2022-06-15T20:09:56Z"^^xsd:dateTime;
  dct:references <https://en.wikipedia.org/wiki/Dewey_Decimal_Classification>,
    <https://en.wikipedia.org/wiki/Linnaean_taxonomy>,
    <https://en.wikipedia.org/wiki/North_American_Industry_Classification_System>;
  skos:definition "A taxonomy is a flat, hierarchical (i.e., tree), set-theoretic, or graph-theoretic structure relating a set of categories to one another. Examples: the Linnaean Taxonomy relates categories of life form, NAICS relates categories of industry, and the Dewey Decimal System relates categories of books."@en;
  skos:inScheme <urn:uuid:1b457bed-8a80-4135-92b8-fdea12b4eea3>,
    <urn:uuid:2153d83b-8555-44a3-96e0-821b6663a188>,
    <urn:uuid:a1a01f1c-7162-439c-94f1-3e28b99ae8ab>,
    <urn:uuid:ddfaaacc-9dcb-451b-afa6-477e6e787a5c>,
    <urn:uuid:2df6fac6-3122-44dc-9f92-5caab7f9b10b>,
    <urn:uuid:0c7028f0-8226-47b3-acff-a4e83e6a60fd>,
    <urn:uuid:bbe073ad-f449-4b25-91ac-7d919613ca51>,
    <urn:uuid:75f35368-e228-47fe-8efd-7251a2bde816>,
    <urn:uuid:91684d49-7b99-4b2e-9641-ea0b8e22f66c>,
    <urn:uuid:4bbcdde6-ed53-4f8d-b3f8-43f800fd05d5>;
  skos:narrower <urn:uuid:0f872daf-97f4-445e-b5d9-0de0087dd129>;
  skos:prefLabel "taxonomy"@en;
  skos:related <urn:uuid:c8f8c1d9-7fe5-484e-86ee-8388c2e3b83b>,
    <urn:uuid:0f872daf-97f4-445e-b5d9-0de0087dd129>,
    <urn:uuid:c9f9e746-371c-4d67-a962-e3906c86a5c3>,
    <urn:uuid:03618f78-d09e-44d1-9149-c6cbebadd9b2> .

<urn:uuid:51a7c4b2-ef0c-4dc1-a538-553622131f09> a skos:Concept;
  dct:alternative "A controlled vocabulary is any deliberately-designed set of terms, which constitutes some official subset of some domain-specific language. A controlled vocabulary can operate in the human sphere, such as with a thesaurus or jargon lexicon, in the computer realm with APIs and database schemas, or straddling the two with taxonomies and ontologies."@en;
  dct:created "2019-05-30T20:56:58Z"^^xsd:dateTime,
    "2019-03-02T03:03:03Z"^^xsd:dateTime;
  dct:creator <urn:uuid:ca637d4b-c11b-4152-be98-bde602e7abd4>;
  dct:description "A controlled vocabulary is any deliberately-designed set of terms, which constitutes some official subset of some domain-specific language. A controlled vocabulary can operate in the human sphere, such as with a thesaurus or jargon lexicon, in the computer realm with APIs and database schemas, or straddling the two with taxonomies and ontologies."@en;
  dct:modified "2022-06-15T19:03:59Z"^^xsd:dateTime;
  skos:definition "A controlled vocabulary can be understood as both a document and a database of valid terms for a particular information domain."@en;
  skos:inScheme <urn:uuid:a1a01f1c-7162-439c-94f1-3e28b99ae8ab>,
    <urn:uuid:ddfaaacc-9dcb-451b-afa6-477e6e787a5c>,
    <urn:uuid:1b457bed-8a80-4135-92b8-fdea12b4eea3>,
    <urn:uuid:2153d83b-8555-44a3-96e0-821b6663a188>,
    <urn:uuid:86eb4d1a-12f8-44ec-be89-ca588c2ee1d4>,
    <urn:uuid:bbe073ad-f449-4b25-91ac-7d919613ca51>,
    <urn:uuid:0c7028f0-8226-47b3-acff-a4e83e6a60fd>,
    <urn:uuid:2df6fac6-3122-44dc-9f92-5caab7f9b10b>,
    <urn:uuid:4bbcdde6-ed53-4f8d-b3f8-43f800fd05d5>;
  skos:narrower <urn:uuid:0f872daf-97f4-445e-b5d9-0de0087dd129>,
    <urn:uuid:45b6c768-da32-4e5f-9c87-a18d5ec94635>,
    <urn:uuid:c9f9e746-371c-4d67-a962-e3906c86a5c3>,
    <urn:uuid:e840ba8a-4c6d-4be3-a673-dd6620463a39>;
  skos:prefLabel "controlled vocabulary"@en;
  skos:related <urn:uuid:0f872daf-97f4-445e-b5d9-0de0087dd129> .

<urn:uuid:7284c136-288b-49aa-b129-a56e2be938d2> a skos:Concept;
  dct:alternative "Information architecture is the discipline of structuring information systems to enable people to comprehend and orient themselves within those systems, and help them find the information they are looking for. It is closely related to content strategy and user experience design."@en;
  dct:created "2019-03-01T03:23:51Z"^^xsd:dateTime;
  dct:creator <urn:uuid:ca637d4b-c11b-4152-be98-bde602e7abd4>;
  dct:description "Information architecture is the discipline of structuring information systems to enable people to comprehend and orient themselves within those systems, and help them find the information they are looking for. It is closely related to content strategy and user experience design."@en;
  dct:modified "2021-12-14T17:38:23Z"^^xsd:dateTime;
  skos:altLabel "information architecture"@en;
  skos:definition "Information architecture is the design of both the topological structure and the semantic content of information systems. The goal of information architecture is to help people situate themselves, understand their surroundings, find the things they're looking for, and even arrange for valuable serendipitous discoveries."@en;
  skos:inScheme <urn:uuid:1b457bed-8a80-4135-92b8-fdea12b4eea3>,
    <urn:uuid:2153d83b-8555-44a3-96e0-821b6663a188>,
    <urn:uuid:797e83d7-a86f-4838-b5c5-0ec20855197d>,
    <urn:uuid:bbe073ad-f449-4b25-91ac-7d919613ca51>,
    <urn:uuid:a1a01f1c-7162-439c-94f1-3e28b99ae8ab>,
    <urn:uuid:ddfaaacc-9dcb-451b-afa6-477e6e787a5c>,
    <urn:uuid:2df6fac6-3122-44dc-9f92-5caab7f9b10b>,
    <urn:uuid:0c7028f0-8226-47b3-acff-a4e83e6a60fd>,
    <urn:uuid:75f35368-e228-47fe-8efd-7251a2bde816>,
    <urn:uuid:4bbcdde6-ed53-4f8d-b3f8-43f800fd05d5>;
  skos:prefLabel "information architecture"@en;
  skos:related <urn:uuid:0f872daf-97f4-445e-b5d9-0de0087dd129>,
    <urn:uuid:45b6c768-da32-4e5f-9c87-a18d5ec94635>,
    <urn:uuid:51a7c4b2-ef0c-4dc1-a538-553622131f09>,
    <urn:uuid:440e5d73-d654-4051-b482-2a960835306b>,
    <urn:uuid:c9f9e746-371c-4d67-a962-e3906c86a5c3>,
    <urn:uuid:2c534735-69b5-4d54-bd9f-dd47b4a5e678> .

<urn:uuid:c0e969c3-4528-4968-8418-d5fe609c2a62> a skos:Concept;
  dct:created "2019-03-07T01:04:30Z"^^xsd:dateTime,
    "2017-02-21T19:52:53Z"^^xsd:dateTime,
    "2018-04-26T22:51:11Z"^^xsd:dateTime;
  dct:creator <urn:uuid:ca637d4b-c11b-4152-be98-bde602e7abd4>;
  skos:broader <urn:uuid:a718d483-af90-4eaf-a59f-31d8897d6e8e>;
  skos:definition "Access is the part of a security policy that concerns the assignment of privileges: who is allowed to see or change an information resource. It is usually discussed in terms of authentication and authorization."@en;
  skos:inScheme <urn:uuid:75f35368-e228-47fe-8efd-7251a2bde816>,
    <urn:uuid:1b457bed-8a80-4135-92b8-fdea12b4eea3>,
    <urn:uuid:2153d83b-8555-44a3-96e0-821b6663a188>,
    <urn:uuid:bbe073ad-f449-4b25-91ac-7d919613ca51>,
    <urn:uuid:91684d49-7b99-4b2e-9641-ea0b8e22f66c>,
    <urn:uuid:a1a01f1c-7162-439c-94f1-3e28b99ae8ab>,
    <urn:uuid:ddfaaacc-9dcb-451b-afa6-477e6e787a5c>,
    <urn:uuid:2df6fac6-3122-44dc-9f92-5caab7f9b10b>,
    <urn:uuid:0c7028f0-8226-47b3-acff-a4e83e6a60fd>,
    <urn:uuid:4bbcdde6-ed53-4f8d-b3f8-43f800fd05d5>;
  skos:narrower <urn:uuid:4a6202a6-b159-4a2b-860a-08efc38e93f1>,
    <urn:uuid:fae79c9e-2e3b-43de-8233-0dbdb4463791>,
    <urn:uuid:9d01c1e5-77f4-481f-bcf9-d9a3ad4b57c8>,
    <urn:uuid:d0d7da4b-4d4d-4262-96a3-a70afbc1a829>;
  skos:prefLabel "access control"@en .

<urn:uuid:ed4d30d7-d3cf-4b21-bcb4-5f2525027be7> a skos:Concept;
  dct:created "2017-07-12T02:44:55Z"^^xsd:dateTime;
  dct:creator <urn:uuid:ca637d4b-c11b-4152-be98-bde602e7abd4>;
  dct:references <https://en.wikipedia.org/wiki/Web_Ontology_Language>,
    <https://www.w3.org/TR/owl2-overview/>;
  skos:altLabel "Web Ontology Language"@en;
  skos:definition "OWL (Web Ontology Language) is a framework for expressing ontologies for automated reasoning applications. While not strictly subordinate to RDF, OWL has an incarnation as an RDF vocabulary, which is a superset of RDF Schema. In this form, OWL ontologies make it possible to express stipulations of cardinality on properties, term reconciliation and equivalencies between classes and properties, and a number of other desirable capabilities."@en;
  skos:inScheme <urn:uuid:75f35368-e228-47fe-8efd-7251a2bde816>,
    <urn:uuid:a1a01f1c-7162-439c-94f1-3e28b99ae8ab>,
    <urn:uuid:ddfaaacc-9dcb-451b-afa6-477e6e787a5c>,
    <urn:uuid:bbe073ad-f449-4b25-91ac-7d919613ca51>,
    <urn:uuid:1b457bed-8a80-4135-92b8-fdea12b4eea3>,
    <urn:uuid:2153d83b-8555-44a3-96e0-821b6663a188>,
    <urn:uuid:91684d49-7b99-4b2e-9641-ea0b8e22f66c>,
    <urn:uuid:2df6fac6-3122-44dc-9f92-5caab7f9b10b>,
    <urn:uuid:4bbcdde6-ed53-4f8d-b3f8-43f800fd05d5>;
  skos:prefLabel "OWL"@en;
  skos:related <urn:uuid:5b30faaa-7c8b-4c57-8dc5-26bd63047d3f> .

<urn:uuid:0bc0aabb-9d9e-4caa-b9c8-553dd8b3ee05> a skos:Concept;
  dct:alternative "Hypertext Markup Language"@en;
  dct:created "2019-02-19T21:36:05Z"^^xsd:dateTime,
    "2024-11-26T23:40:53Z"^^xsd:dateTime;
  dct:creator <urn:uuid:ca637d4b-c11b-4152-be98-bde602e7abd4>;
  skos:altLabel "HTML"@en;
  skos:broader <urn:uuid:9fc41de2-b16c-4170-8818-893302baa77d>;
  skos:definition "HTML is, of course, the lingua franca of the Web."@en;
  skos:hiddenLabel "html"@en,
    "hypertext markup language"@en;
  skos:inScheme <urn:uuid:a1a01f1c-7162-439c-94f1-3e28b99ae8ab>,
    <urn:uuid:ddfaaacc-9dcb-451b-afa6-477e6e787a5c>,
    <urn:uuid:797e83d7-a86f-4838-b5c5-0ec20855197d>,
    <urn:uuid:bbe073ad-f449-4b25-91ac-7d919613ca51>,
    <urn:uuid:2df6fac6-3122-44dc-9f92-5caab7f9b10b>,
    <urn:uuid:1b457bed-8a80-4135-92b8-fdea12b4eea3>,
    <urn:uuid:2153d83b-8555-44a3-96e0-821b6663a188>,
    <urn:uuid:0c7028f0-8226-47b3-acff-a4e83e6a60fd>,
    <urn:uuid:4bbcdde6-ed53-4f8d-b3f8-43f800fd05d5>;
  skos:narrower <urn:uuid:29883b00-2202-4684-887d-8077fa0eecc2>;
  skos:prefLabel "Hypertext Markup Language"@en .

<urn:uuid:9e506ca3-8be1-431d-9075-548141d9f8c1> a skos:Concept;
  dct:alternative "A URI is a superset of the URL, intended to identify information resources that are not necessarily amenable to being located, or otherwise for which location mechanisms are implicit. The URI framework affords URIs of various schemes (registered with IANA) to express their own semantics for identifying and resolving information resources."@en,
    "The Uniform Resource Identifier (URI) is a kind of normalized, machine-readable identifier for picking out information resources."@en;
  dct:created "2018-02-03T13:30:27Z"^^xsd:dateTime,
    "2008-06-14T04:30:27+00:00"^^xsd:dateTime;
  dct:creator <urn:uuid:ca637d4b-c11b-4152-be98-bde602e7abd4>;
  dct:description "A URI is a superset of the URL, intended to identify information resources that are not necessarily amenable to being located, or otherwise for which location mechanisms are implicit. The URI framework affords URIs of various schemes (registered with IANA) to express their own semantics for identifying and resolving information resources."@en,
    "The Uniform Resource Identifier (URI) is a kind of normalized, machine-readable identifier for picking out information resources."@en;
  dct:modified "2008-06-14T06:38:36+00:00"^^xsd:dateTime,
    "2008-06-15T06:44:20+00:00"^^xsd:dateTime,
    "2008-10-09T02:02:01+00:00"^^xsd:dateTime,
    "2008-10-10T16:02:45+00:00"^^xsd:dateTime,
    "2008-10-10T21:28:23+00:00"^^xsd:dateTime,
    "2009-03-04T00:43:00+00:00"^^xsd:dateTime,
    "2018-02-03T13:30:27Z"^^xsd:dateTime,
    "2019-10-13T00:22:54Z"^^xsd:dateTime,
    "2021-12-14T23:17:19Z"^^xsd:dateTime,
    "2022-05-31T04:18:52+00:00"^^xsd:dateTime;
  dct:references <https://tools.ietf.org/html/rfc3986>;
  skos:altLabel "URI"@en,
    "Uniform Resource Identifier"@en;
  skos:definition "A uniform resource identifier is exactly what the name says: an identifier (text symbol) for (information, chiefly) resources which is (syntactically) uniform."@en;
  skos:hiddenLabel "URIs"@en,
    "uniform resource identifier"@en,
    "uri"@en;
  skos:inScheme <urn:uuid:75f35368-e228-47fe-8efd-7251a2bde816>,
    <urn:uuid:a1a01f1c-7162-439c-94f1-3e28b99ae8ab>,
    <urn:uuid:ddfaaacc-9dcb-451b-afa6-477e6e787a5c>,
    <urn:uuid:4ec7530b-5536-4fb7-bb5a-45a3f5fddc22>,
    <urn:uuid:797e83d7-a86f-4838-b5c5-0ec20855197d>,
    <urn:uuid:bbe073ad-f449-4b25-91ac-7d919613ca51>,
    <urn:uuid:91684d49-7b99-4b2e-9641-ea0b8e22f66c>,
    <urn:uuid:1b457bed-8a80-4135-92b8-fdea12b4eea3>,
    <urn:uuid:2153d83b-8555-44a3-96e0-821b6663a188>,
    <urn:uuid:0c7028f0-8226-47b3-acff-a4e83e6a60fd>,
    <urn:uuid:2df6fac6-3122-44dc-9f92-5caab7f9b10b>,
    <urn:uuid:4bbcdde6-ed53-4f8d-b3f8-43f800fd05d5>;
  skos:narrower <urn:uuid:ecf5fe36-229a-4eea-8b2d-24686da80aba>,
    <urn:uuid:e162d03b-bfec-4f01-ab7e-56da309550f6>;
  skos:prefLabel "Uniform Resource Identifier"@en;
  skos:related <urn:uuid:4039a99d-c14b-40f2-84d5-4ec72e2217e1> .

<urn:uuid:e162d03b-bfec-4f01-ab7e-56da309550f6> a skos:Concept;
  dct:alternative "A URL is the original identifier designed by Tim Berners-Lee which is intended to normalize the representation of (in the original case) the location of Web resources. The pattern was subsequently expanded to the more generic URI."@en;
  dct:created "2018-02-03T13:30:58Z"^^xsd:dateTime;
  dct:creator <urn:uuid:ca637d4b-c11b-4152-be98-bde602e7abd4>;
  dct:description "A URL is the original identifier designed by Tim Berners-Lee which is intended to normalize the representation of (in the original case) the location of Web resources. The pattern was subsequently expanded to the more generic URI."@en;
  dct:modified "2021-12-14T18:40:25Z"^^xsd:dateTime;
  skos:altLabel "URL"@en,
    "Uniform Resource Locator"@en;
  skos:broader <urn:uuid:9e506ca3-8be1-431d-9075-548141d9f8c1>;
  skos:definition "A uniform resource locator is a subset of URI which specifies a protocol-specific network resource which can be de-referenced, that is to say accessed."@en;
  skos:hiddenLabel "URLs"@en,
    "uniform resource locators"@en,
    "url"@en;
  skos:inScheme <urn:uuid:1b457bed-8a80-4135-92b8-fdea12b4eea3>,
    <urn:uuid:2153d83b-8555-44a3-96e0-821b6663a188>,
    <urn:uuid:797e83d7-a86f-4838-b5c5-0ec20855197d>,
    <urn:uuid:bbe073ad-f449-4b25-91ac-7d919613ca51>,
    <urn:uuid:a1a01f1c-7162-439c-94f1-3e28b99ae8ab>,
    <urn:uuid:ddfaaacc-9dcb-451b-afa6-477e6e787a5c>,
    <urn:uuid:2df6fac6-3122-44dc-9f92-5caab7f9b10b>,
    <urn:uuid:75f35368-e228-47fe-8efd-7251a2bde816>,
    <urn:uuid:0c7028f0-8226-47b3-acff-a4e83e6a60fd>,
    <urn:uuid:91684d49-7b99-4b2e-9641-ea0b8e22f66c>,
    <urn:uuid:4bbcdde6-ed53-4f8d-b3f8-43f800fd05d5>;
  skos:prefLabel "Uniform Resource Locator"@en;
  skos:related <urn:uuid:ecf5fe36-229a-4eea-8b2d-24686da80aba> .

<urn:uuid:0f872daf-97f4-445e-b5d9-0de0087dd129> a skos:Concept;
  dct:alternative "Concept scheme is an umbrella term for typologies, taxonomies, dictionaries and glossaries, thesauri, et cetera."@en;
  dct:created "2017-07-12T03:05:30Z"^^xsd:dateTime;
  dct:creator <urn:uuid:ca637d4b-c11b-4152-be98-bde602e7abd4>;
  dct:description "A concept scheme is a taxonomy—that is, a structure—of concepts."@en;
  dct:modified "2022-06-02T02:14:52Z"^^xsd:dateTime;
  skos:altLabel "concept taxonomy"@en;
  skos:definition "Concept scheme is an umbrella term for typologies, taxonomies, dictionaries and glossaries, thesauri, et cetera. A concept scheme typically not only lists a set of concepts and their definitions, but also the (hierarchical or set-theoretic) relationships between them."@en,
    "Concept scheme is an umbrella term for typologies, taxonomies, dictionaries and glossaries, thesauri, et cetera. A concept scheme typically not only lists a set of concepts and their definitions, but also the (hierarchical, but not always) relationships between them."@en,
    "A concept scheme is simply a taxonomy of concepts."@en;
  skos:inScheme <urn:uuid:a1a01f1c-7162-439c-94f1-3e28b99ae8ab>,
    <urn:uuid:ddfaaacc-9dcb-451b-afa6-477e6e787a5c>,
    <urn:uuid:75f35368-e228-47fe-8efd-7251a2bde816>,
    <urn:uuid:bbe073ad-f449-4b25-91ac-7d919613ca51>,
    <urn:uuid:91684d49-7b99-4b2e-9641-ea0b8e22f66c>,
    <urn:uuid:0c7028f0-8226-47b3-acff-a4e83e6a60fd>,
    <urn:uuid:1b457bed-8a80-4135-92b8-fdea12b4eea3>,
    <urn:uuid:2153d83b-8555-44a3-96e0-821b6663a188>,
    <urn:uuid:2df6fac6-3122-44dc-9f92-5caab7f9b10b>,
    <urn:uuid:4bbcdde6-ed53-4f8d-b3f8-43f800fd05d5>;
  skos:narrower <urn:uuid:45b6c768-da32-4e5f-9c87-a18d5ec94635>;
  skos:prefLabel "concept scheme"@en;
  skos:related <urn:uuid:51a7c4b2-ef0c-4dc1-a538-553622131f09>,
    <urn:uuid:a43e33d9-1788-4514-8fbd-1b4982535f73> .

<urn:uuid:9767147a-1b6a-440c-949f-7f6056e28411> a skos:Concept;
  dct:alternative "A data structure refers to both the abstract denotation of relations between entities and values, as well as their concrete representation in computer memory or serialized to storage formats and/or network messages."@en;
  dct:created "2017-02-20T01:11:48Z"^^xsd:dateTime;
  dct:creator <urn:uuid:ca637d4b-c11b-4152-be98-bde602e7abd4>;
  dct:description "A data structure refers to both the abstract denotation of relations between entities and values, as well as their concrete representation in computer memory or serialized to storage formats and/or network messages."@en;
  dct:modified "2017-07-09T22:09:45Z"^^xsd:dateTime;
  skos:definition "A data structure is an object that associates together a set of slots (properties, fields, dimensions, columns), where each slot has a meaning, and can hold a value, which can possibly be another data structure."@en;
  skos:inScheme <urn:uuid:49ac68c4-922c-4d9e-88fa-b318fc54d36f>,
    <urn:uuid:1b457bed-8a80-4135-92b8-fdea12b4eea3>,
    <urn:uuid:2153d83b-8555-44a3-96e0-821b6663a188>,
    <urn:uuid:a1a01f1c-7162-439c-94f1-3e28b99ae8ab>,
    <urn:uuid:ddfaaacc-9dcb-451b-afa6-477e6e787a5c>,
    <urn:uuid:0c7028f0-8226-47b3-acff-a4e83e6a60fd>,
    <urn:uuid:bbe073ad-f449-4b25-91ac-7d919613ca51>,
    <urn:uuid:2df6fac6-3122-44dc-9f92-5caab7f9b10b>,
    <urn:uuid:4bbcdde6-ed53-4f8d-b3f8-43f800fd05d5>;
  skos:narrower <urn:uuid:1f5fb4c8-4d43-46d6-a205-0339c1b0289e>;
  skos:prefLabel "data structure"@en;
  skos:related <urn:uuid:197982df-60a5-4c93-be50-2f8ede43b842>,
    <urn:uuid:4694ebe0-589f-40a7-9ef9-67872edb6214>,
    <urn:uuid:527ab630-b325-4a7a-8cb7-ec448a90db62> .

<urn:uuid:4039a99d-c14b-40f2-84d5-4ec72e2217e1> a skos:Concept;
  dct:alternative "An information resource is any identifiable artifact that contains information. This can range from a book, to a film, to a library, to a database, to a Post-It note."@en,
    "A (Web) resource can be understood as a relation between one or more URIs and one or more representations."@en,
    "An information resource is an abstract relation between a set of identifiers (usually URIs) and a set of representations."@en;
  dct:created "2008-06-14T04:30:27+00:00"^^xsd:dateTime,
    "2017-02-09T21:59:51Z"^^xsd:dateTime;
  dct:creator <urn:uuid:ca637d4b-c11b-4152-be98-bde602e7abd4>;
  dct:description "A (Web) resource can be understood as a relation between one or more URIs and one or more representations."@en,
    "An information resource is an abstract relation between a set of identifiers (usually URIs) and a set of representations."@en,
    "An information resource is any identifiable artifact that contains information. This can range from a book, to a film, to a library, to a database, to a Post-It note."@en;
  dct:modified "2008-06-14T06:38:36+00:00"^^xsd:dateTime,
    "2008-07-18T18:59:52+00:00"^^xsd:dateTime,
    "2008-10-09T02:02:01+00:00"^^xsd:dateTime,
    "2008-10-10T16:02:45+00:00"^^xsd:dateTime,
    "2008-10-10T21:28:23+00:00"^^xsd:dateTime,
    "2009-03-04T00:43:00+00:00"^^xsd:dateTime,
    "2017-02-09T21:59:51Z"^^xsd:dateTime,
    "2017-02-20T01:32:04Z"^^xsd:dateTime,
    "2019-03-06T23:09:18Z"^^xsd:dateTime,
    "2021-09-24T13:14:28Z"^^xsd:dateTime,
    "2021-12-15T05:57:13Z"^^xsd:dateTime,
    "2022-05-31T04:18:52+00:00"^^xsd:dateTime;
  skos:altLabel "resource"@en,
    "Resource"@en,
    "information resource"@en;
  skos:broader <urn:uuid:16d17f33-394d-4d0b-a882-81e8fc3a52fe>,
    <urn:uuid:759d2f68-3d16-4122-9758-c84f7760d691>;
  skos:definition "An information resource is any identifiable artifact that contains information. This can range from a book, to a film, to a library, to a database, to a Post-It note."@en,
    "An information resource is a distinct, identifiable object that carries information. On a website, a resource is uniquely identifiable by a URI, aka Web address. On our project, the resource is the basic unit of visible progress. Pages are resources, so are images, videos, etc. Resources can also be the interfaces to programs, take parameters, and process input."@en,
    "A (Hypermedia) resource is a distinct object that carries information. On a website, a resource is uniquely identifiable by a URI, aka Web address. On our project, the resource is the basic unit of visible progress. Pages are resources, so are images, videos, etc. Resources can also be the interfaces to programs, take parameters, and process input."@en;
  skos:hiddenLabel "resources"@en,
    "information resources"@en;
  skos:inScheme <urn:uuid:1b457bed-8a80-4135-92b8-fdea12b4eea3>,
    <urn:uuid:2153d83b-8555-44a3-96e0-821b6663a188>,
    <urn:uuid:49ac68c4-922c-4d9e-88fa-b318fc54d36f>,
    <urn:uuid:4ec7530b-5536-4fb7-bb5a-45a3f5fddc22>,
    <urn:uuid:797e83d7-a86f-4838-b5c5-0ec20855197d>,
    <urn:uuid:bbe073ad-f449-4b25-91ac-7d919613ca51>,
    <urn:uuid:a1a01f1c-7162-439c-94f1-3e28b99ae8ab>,
    <urn:uuid:ddfaaacc-9dcb-451b-afa6-477e6e787a5c>,
    <urn:uuid:2df6fac6-3122-44dc-9f92-5caab7f9b10b>,
    <urn:uuid:0c7028f0-8226-47b3-acff-a4e83e6a60fd>,
    <urn:uuid:4bbcdde6-ed53-4f8d-b3f8-43f800fd05d5>;
  skos:narrower <urn:uuid:1f7f1c54-a1d2-453c-87a7-4439a7b6037d>,
    <urn:uuid:e3f7b71e-1366-4f1e-aaf8-fd15a37e7f61>;
  skos:prefLabel "information resource"@en;
  skos:related <urn:uuid:5bdd2fb7-d84d-4583-998b-7d3f2803307e>,
    <urn:uuid:9e506ca3-8be1-431d-9075-548141d9f8c1>,
    <urn:uuid:be93cce1-f21f-4e85-bd34-e005dea3532f> .

<urn:uuid:f352a521-b78e-478e-b01d-3a68638025a4> a skos:Concept;
  dct:created "2021-12-15T06:07:52Z"^^xsd:dateTime,
    "2019-03-07T01:04:30Z"^^xsd:dateTime;
  dct:creator <urn:uuid:ca637d4b-c11b-4152-be98-bde602e7abd4>;
  skos:altLabel "XML"@en;
  skos:broader <urn:uuid:027543f6-04df-4e92-96f4-5b0c8da4b799>,
    <urn:uuid:8d46494e-5316-43b7-a49e-a625ab716a38>;
  skos:definition "XML, while scorned and vilified by contemporary Web developers, is still a usable standard framework for expressing ordered-tree data structures."@en;
  skos:hiddenLabel "xml"@en;
  skos:inScheme <urn:uuid:2df6fac6-3122-44dc-9f92-5caab7f9b10b>,
    <urn:uuid:797e83d7-a86f-4838-b5c5-0ec20855197d>,
    <urn:uuid:bbe073ad-f449-4b25-91ac-7d919613ca51>,
    <urn:uuid:75f35368-e228-47fe-8efd-7251a2bde816>,
    <urn:uuid:1b457bed-8a80-4135-92b8-fdea12b4eea3>,
    <urn:uuid:2153d83b-8555-44a3-96e0-821b6663a188>,
    <urn:uuid:4bbcdde6-ed53-4f8d-b3f8-43f800fd05d5>;
  skos:narrower <urn:uuid:0b356e36-b115-4c86-890b-8b05850a125b>,
    <urn:uuid:ab11cb80-b052-4a74-bbb7-bd19dc120437>;
  skos:prefLabel "Extensible Markup Language"@en,
    "XML"@en;
  skos:related <urn:uuid:755dd3a1-cffc-4d65-9446-435552bac541> .

<urn:uuid:fe500c7a-b458-4d2c-8b3a-efd1bb47d106> a skos:Concept;
  dct:alternative "The W3C Resource Description Framework (RDF) is a standard for representing labeled, directed graphs, where the labels are URIs."@en,
    "The W3C Resource Description Framework is an open data standard for expressing edge-labeled directed graphs where the nodes and edge labels are URIs. RDF proper only spells out these constraints and requires a number of other specifications for serialization syntaxes, schemata, inferences, and so on. RDF is one (but not the only) technology underpinning linked data, as well as the technology behind the Semantic Web."@en;
  dct:created "2017-07-12T02:27:51Z"^^xsd:dateTime;
  dct:creator <urn:uuid:ca637d4b-c11b-4152-be98-bde602e7abd4>;
  dct:description "The W3C Resource Description Framework (RDF) is a standard for representing labeled, directed graphs, where the labels are URIs."@en,
    "The W3C Resource Description Framework is an open data standard for expressing edge-labeled directed graphs where the nodes and edge labels are URIs. RDF proper only spells out these constraints and requires a number of other specifications for serialization syntaxes, schemata, inferences, and so on. RDF is one (but not the only) technology underpinning linked data, as well as the technology behind the Semantic Web."@en;
  dct:modified "2019-10-13T00:22:23Z"^^xsd:dateTime,
    "2021-12-14T22:24:24Z"^^xsd:dateTime;
  dct:references <https://www.w3.org/TR/rdf11-primer/>,
    <https://en.wikipedia.org/wiki/Resource_Description_Framework>,
    <https://www.w3.org/RDF/>;
  rdfs:seeAlso <https://en.wikipedia.org/wiki/Resource_Description_Framework>,
    <https://www.w3.org/RDF/>,
    <https://www.w3.org/TR/rdf11-primer/>;
  skos:altLabel "Resource Description Framework"@en,
    "RDF"@en;
  skos:definition "RDF is a W3C open standard framework for the encoding of data semantics. RDF uses URIs to uniquely identify information resources and the semantic relations between them. It is important to understand that RDF is not a syntax; there are many syntaxes available that will encode RDF."@en;
  skos:hiddenLabel "resource description framework"@en,
    "rdf"@en;
  skos:inScheme <urn:uuid:2df6fac6-3122-44dc-9f92-5caab7f9b10b>,
    <urn:uuid:a1a01f1c-7162-439c-94f1-3e28b99ae8ab>,
    <urn:uuid:ddfaaacc-9dcb-451b-afa6-477e6e787a5c>,
    <urn:uuid:75f35368-e228-47fe-8efd-7251a2bde816>,
    <urn:uuid:1b457bed-8a80-4135-92b8-fdea12b4eea3>,
    <urn:uuid:2153d83b-8555-44a3-96e0-821b6663a188>,
    <urn:uuid:91684d49-7b99-4b2e-9641-ea0b8e22f66c>,
    <urn:uuid:797e83d7-a86f-4838-b5c5-0ec20855197d>,
    <urn:uuid:bbe073ad-f449-4b25-91ac-7d919613ca51>,
    <urn:uuid:0c7028f0-8226-47b3-acff-a4e83e6a60fd>,
    <urn:uuid:4bbcdde6-ed53-4f8d-b3f8-43f800fd05d5>;
  skos:narrower <urn:uuid:86c65d14-2d23-4350-8004-233b2f3e873f>,
    <urn:uuid:6d154e36-799a-4b7b-8e07-a6d3459d2fd7>,
    <urn:uuid:4eab5a63-adc6-4efd-b49e-402131b519fa>;
  skos:prefLabel "Resource Description Framework"@en;
  skos:related <urn:uuid:4af8a4cc-c12b-47aa-8ab2-d15a74907aa3>,
    <urn:uuid:7b7c4ecf-2544-4c03-ab5f-10de5e1a20d4>,
    <urn:uuid:4039a99d-c14b-40f2-84d5-4ec72e2217e1>,
    <urn:uuid:9e506ca3-8be1-431d-9075-548141d9f8c1> .

<urn:uuid:33c3211f-322b-4f7a-83f6-63aa617461c3> a skos:Concept;
  dct:alternative "We will define a programming language as any (mathematically) formal language capable of causing a computer to execute potentially non-deterministic behaviour. This is in contrast to (indeed a subset of) a data format, which may not necessarily possess the adequate semantics to express non-deterministic behaviour."@en;
  dct:created "2017-06-07T20:51:08Z"^^xsd:dateTime;
  dct:creator <urn:uuid:ca637d4b-c11b-4152-be98-bde602e7abd4>;
  dct:description "We will define a programming language as any (mathematically) formal language capable of causing a computer to execute potentially non-deterministic behaviour. This is in contrast to (indeed a subset of) a data format, which may not necessarily possess the adequate semantics to express non-deterministic behaviour."@en;
  dct:modified "2019-02-28T21:51:13Z"^^xsd:dateTime;
  skos:broader <urn:uuid:027543f6-04df-4e92-96f4-5b0c8da4b799>;
  skos:definition "A programming language is a formal language in which software is written."@en;
  skos:inScheme <urn:uuid:0c7028f0-8226-47b3-acff-a4e83e6a60fd>,
    <urn:uuid:49ac68c4-922c-4d9e-88fa-b318fc54d36f>,
    <urn:uuid:2df6fac6-3122-44dc-9f92-5caab7f9b10b>,
    <urn:uuid:bbe073ad-f449-4b25-91ac-7d919613ca51>,
    <urn:uuid:1b457bed-8a80-4135-92b8-fdea12b4eea3>,
    <urn:uuid:2153d83b-8555-44a3-96e0-821b6663a188>,
    <urn:uuid:4bbcdde6-ed53-4f8d-b3f8-43f800fd05d5>;
  skos:narrower <urn:uuid:dbadda22-ff04-4508-8b6f-591b364de982>,
    <urn:uuid:2f6700a6-9ecb-47af-8106-a652b4c852e5>,
    <urn:uuid:92b60601-4c7e-4a44-b42f-9648fefc11d4>,
    <urn:uuid:f9df502b-051e-441d-811f-ea1661254373>,
    <urn:uuid:5abd5284-7197-4eed-895d-6daefa019de8>,
    <urn:uuid:fd1478d3-a6ba-430b-bdb2-2d47a4e7caf9>,
    <urn:uuid:f70f6095-f27b-4485-b245-3431f77a6e17>,
    <urn:uuid:dabce9e1-eb5b-4db3-82fd-15558aa40e88>,
    <urn:uuid:c7066ab9-ad6b-4a19-b682-d919827eec71>,
    <urn:uuid:919d84fb-a760-45da-bbed-cdf2b3b40a5f>,
    <urn:uuid:9763e3fc-30bc-4547-a8e6-6747088f914b>,
    <urn:uuid:3e3aa9b0-efaf-4dc5-83fb-4456e24f021d>;
  skos:prefLabel "programming language"@en;
  skos:related <urn:uuid:4e296fcb-0a17-4397-970b-11e8813f7883>,
    <urn:uuid:85a069f9-1a66-4462-b0e2-d042db345919> .

<urn:uuid:fdb43f70-cb11-49dd-aba6-7011b05ad61a> a skos:Concept;
  dct:created "2020-04-26T15:10:48Z"^^xsd:dateTime,
    "2021-12-14T17:28:40Z"^^xsd:dateTime;
  dct:creator <urn:uuid:ca637d4b-c11b-4152-be98-bde602e7abd4>;
  skos:altLabel "software development"@en;
  skos:definition "The making of software, which I trust the audience is familiar with."@en;
  skos:hiddenLabel "development"@en,
    "development (software)"@en;
  skos:inScheme <urn:uuid:a1a01f1c-7162-439c-94f1-3e28b99ae8ab>,
    <urn:uuid:ddfaaacc-9dcb-451b-afa6-477e6e787a5c>,
    <urn:uuid:2df6fac6-3122-44dc-9f92-5caab7f9b10b>,
    <urn:uuid:d4317ece-d4aa-40cb-9df1-1b058cbc24d8>,
    <urn:uuid:1b457bed-8a80-4135-92b8-fdea12b4eea3>,
    <urn:uuid:2153d83b-8555-44a3-96e0-821b6663a188>,
    <urn:uuid:797e83d7-a86f-4838-b5c5-0ec20855197d>,
    <urn:uuid:bbe073ad-f449-4b25-91ac-7d919613ca51>,
    <urn:uuid:0c7028f0-8226-47b3-acff-a4e83e6a60fd>,
    <urn:uuid:4bbcdde6-ed53-4f8d-b3f8-43f800fd05d5>;
  skos:prefLabel "software development"@en .
